@prefix : <http://inspire.ec.europa.eu/ont#> .
@prefix lr: <http://www.roadotl.eu/iso19148/def/> .
@prefix sf: <http://www.opengis.net/ont/sf#> .
@prefix gsp: <http://www.opengis.net/ont/geosparql#> .
@prefix owl: <http://www.w3.org/2002/07/owl#> .
@prefix rdf: <http://www.w3.org/1999/02/22-rdf-syntax-ns#> .
@prefix xml: <http://www.w3.org/XML/1998/namespace> .
@prefix xsd: <http://www.w3.org/2001/XMLSchema#> .
@prefix rdfs: <http://www.w3.org/2000/01/rdf-schema#> .
@prefix skos: <http://www.w3.org/2004/02/skos/core#> .
@prefix dc: <http://purl.org/dc/terms/> .
@base <http://inspire.ec.europa.eu/isotc211> .

<http://inspire.ec.europa.eu/ont> a owl:Ontology ;
	owl:imports <http://www.w3.org/2004/02/skos/core> ;
	owl:imports gsp: ;
	owl:imports <http://inspire.ec.europa.eu/isotc211> ;

	### GeoSPARQL rdf file: http://schemas.opengis.net/geosparql/1.0/geosparql_vocab_all.rdf
	### ISO 19148 ttl file: https://ontologi.atlas.vegvesen.no/nvdb/core/iso-19148.ttl
	### ISO 19115 rdf file: http://def.isotc211.org/iso19115/-1/2014/MetadataInformation.rdf

	dc:creator "INSPIRE" ;
	dc:date "31.08.2022" ;
	dc:description "Ontology for INSPIRE Road Transport Network Complete, derived from the UML model"@en ;
	dc:title "INSPIRE Road Transport Network Complete"@en ;
	dc:description "Ontology for INSPIRE Road Transport Network Complete, derived from the UML model"@en .

### http://inspire.ec.europa.eu/ont#itnr
:itnr a owl:Class ;
         owl:disjointUnionOf ( :itnrFeature :itnrCodeList :itnrEnumeration :itnrDataType ) ;
         rdfs:label "INSPIRE Root"@en .
### http://inspire.ec.europa.eu/ont#Feature
:itnrFeature a owl:Class ;
         rdfs:subClassOf <http://def.isotc211.org/iso19109/2015/GeneralFeatureModel#AnyFeature> ,
                          :itnr ,
                       gsp:Feature ;
         rdfs:label "INSPIRE Feature"@en .
### http://inspire.ec.europa.eu/ont#CodeList
:itnrCodeList a owl:Class ;
         rdfs:subClassOf :itnr, skos:Concept ;
         rdfs:label "INSPIRE Code value"@en .
### http://inspire.ec.europa.eu/ont#Enumeration
:itnrEnumeration a owl:Class ;
         rdfs:subClassOf :itnr, skos:Concept ;
         rdfs:label "INSPIRE Enumeration value"@en .
### http://inspire.ec.europa.eu/ont#DataType
:itnrDataType a owl:Class ;
         rdfs:subClassOf :itnr ;
         rdfs:label "INSPIRE Data type"@en .



### http://inspire.ec.europa.eu/ont:Identifier
:Identifier a owl:Class ;
       rdfs:subClassOf :itnrDataType ;
         skos:definition "-- Definition -- External unique object identifier published by the responsible body, which may be used by external applications to reference the spatial object.  -- Description -- NOTE1 External object identifiers are distinct from thematic object identifiers.  NOTE 2 The voidable version identifier attribute is not part of the unique identifier of a spatial object and may be used to distinguish two versions of the same spatial object.  NOTE 3 The unique identifier will not change during the life-time of a spatial object. "@en ;
       rdfs:label "Identifier"@en .

### http://inspire.ec.europa.eu/ont#localId
:localId rdf:type owl:DatatypeProperty ;
         skos:definition "-- Definition -- A local identifier, assigned by the data provider. The local identifier is unique within the namespace, that is no other spatial object carries the same unique identifier.  -- Description -- NOTE It is the responsibility of the data provider to guarantee uniqueness of the local identifier within the namespace. "@en ;
         rdfs:domain :Identifier;
         rdfs:range xsd:string;
         rdf:type owl:FunctionalProperty;
         rdfs:label "localId"@en .
:Identifier rdfs:subClassOf [ rdf:type owl:Restriction ;
         owl:onProperty :localId;
         owl:onDataRange xsd:string;
       owl:qualifiedCardinality "1"^^xsd:nonNegativeInteger ;
         ] .
:Identifier rdfs:subClassOf [ rdf:type owl:Restriction ;
         owl:onProperty :localId;
         owl:allValuesFrom xsd:string;
         ] .


### http://inspire.ec.europa.eu/ont#namespace
:namespace rdf:type owl:DatatypeProperty ;
         skos:definition "-- Definition -- Namespace uniquely identifying the data source of the spatial object.  -- Description -- NOTE The namespace value will be owned by the data provider of the spatial object and will be registered in the INSPIRE External Object Identifier Namespaces Register. "@en ;
         rdfs:domain :Identifier;
         rdfs:range xsd:string;
         rdf:type owl:FunctionalProperty;
         rdfs:label "namespace"@en .
:Identifier rdfs:subClassOf [ rdf:type owl:Restriction ;
         owl:onProperty :namespace;
         owl:onDataRange xsd:string;
       owl:qualifiedCardinality "1"^^xsd:nonNegativeInteger ;
         ] .
:Identifier rdfs:subClassOf [ rdf:type owl:Restriction ;
         owl:onProperty :namespace;
         owl:allValuesFrom xsd:string;
         ] .


### http://inspire.ec.europa.eu/ont#versionId
:versionId rdf:type owl:DatatypeProperty ;
         skos:definition "-- Definition -- The identifier of the particular version of the spatial object, with a maximum length of 25 characters. If the specification of a spatial object type with an external object identifier includes life-cycle information, the version identifier is used to distinguish between the different versions of a spatial object. Within the set of all versions of a spatial object, the version identifier is unique.   -- Description -- NOTE The maximum length has been selected to allow for time stamps based on ISO 8601, for example, \"2007-02-12T12:12:12+05:30\" as the version identifier.  NOTE 2 The property is void, if the spatial data set does not distinguish between different versions of the spatial object. It is missing, if the spatial object type does not support any life-cycle information. "@en ;
         rdfs:domain :Identifier;
         rdfs:range xsd:string;
         rdfs:label "versionId"@en .
:Identifier rdfs:subClassOf [ rdf:type owl:Restriction ;
         owl:onProperty :versionId;
         owl:onDataRange xsd:string;
       owl:maxQualifiedCardinality "1"^^xsd:nonNegativeInteger ;
         ] .
:Identifier rdfs:subClassOf [ rdf:type owl:Restriction ;
         owl:onProperty :versionId;
         owl:allValuesFrom xsd:string;
         ] .


### http://inspire.ec.europa.eu/ont:ConditionOfFacilityValue
:ConditionOfFacilityValue a owl:Class ;
       rdfs:subClassOf :itnrCodeList ;
          rdfs:isDefinedBy  <https://inspire.ec.europa.eu/codelist/ConditionOfFacilityValue>;
         skos:definition "-- Definition -- The status of a facility with regards to its completion and use."@en ;
       rdfs:label "ConditionOfFacilityValue"@en .

### http://inspire.ec.europa.eu/ont:ConditionOfFacilityValueCode
:ConditionOfFacilityValueCode a skos:ConceptScheme ;
         skos:definition "-- Definition -- The status of a facility with regards to its completion and use."@en ;
          owl:sameAs  <https://inspire.ec.europa.eu/codelist/ConditionOfFacilityValue>;
       dc:isFormatOf :ConditionOfFacilityValue .

### http://inspire.ec.europa.eu/ont:ConditionOfFacilityValue.disused
:ConditionOfFacilityValue.disused a :ConditionOfFacilityValue,skos:Concept ;
         skos:inScheme :ConditionOfFacilityValueCode ;
         skos:definition "-- Name -- disused  -- Definition -- The facility is no longer used, but is not being or has not been decommissioned."@en ;
          owl:sameAs  <https://inspire.ec.europa.eu/codelist/ConditionOfFacilityValue/disused>;
          rdfs:isDefinedBy  <https://inspire.ec.europa.eu/codelist/ConditionOfFacilityValue/disused>;
         rdfs:label "disused"@no .

### http://inspire.ec.europa.eu/ont:ConditionOfFacilityValue.functional
:ConditionOfFacilityValue.functional a :ConditionOfFacilityValue,skos:Concept ;
         skos:inScheme :ConditionOfFacilityValueCode ;
         skos:definition "-- Name -- functional  -- Definition -- The facility is functional."@en ;
          owl:sameAs  <https://inspire.ec.europa.eu/codelist/ConditionOfFacilityValue/functional>;
          rdfs:isDefinedBy  <https://inspire.ec.europa.eu/codelist/ConditionOfFacilityValue/functional>;
         rdfs:label "functional"@no .

### http://inspire.ec.europa.eu/ont:ConditionOfFacilityValue.projected
:ConditionOfFacilityValue.projected a :ConditionOfFacilityValue,skos:Concept ;
         skos:inScheme :ConditionOfFacilityValueCode ;
         skos:definition "-- Name -- projected  -- Definition -- The facility is being designed. Construction has not yet started."@en ;
          owl:sameAs  <https://inspire.ec.europa.eu/codelist/ConditionOfFacilityValue/projected>;
          rdfs:isDefinedBy  <https://inspire.ec.europa.eu/codelist/ConditionOfFacilityValue/projected>;
         rdfs:label "projected"@no .

### http://inspire.ec.europa.eu/ont:ConditionOfFacilityValue.underConstruction
:ConditionOfFacilityValue.underConstruction a :ConditionOfFacilityValue,skos:Concept ;
         skos:inScheme :ConditionOfFacilityValueCode ;
         skos:definition "-- Name -- under construction  -- Definition -- The facility is under construction and not yet functional. This applies only to the initial construction of the facility and not to maintenance work."@en ;
          owl:sameAs  <https://inspire.ec.europa.eu/codelist/ConditionOfFacilityValue/underConstruction>;
          rdfs:isDefinedBy  <https://inspire.ec.europa.eu/codelist/ConditionOfFacilityValue/underConstruction>;
         rdfs:label "underConstruction"@no .

### http://inspire.ec.europa.eu/ont:ConditionOfFacilityValue.decommissioned
:ConditionOfFacilityValue.decommissioned a :ConditionOfFacilityValue,skos:Concept ;
         skos:inScheme :ConditionOfFacilityValueCode ;
         skos:definition "-- Name -- decommissioned  -- Definition -- The facility is no longer used and is being or has been decommissioned."@en ;
          owl:sameAs  <https://inspire.ec.europa.eu/codelist/ConditionOfFacilityValue/decommissioned>;
          rdfs:isDefinedBy  <https://inspire.ec.europa.eu/codelist/ConditionOfFacilityValue/decommissioned>;
         rdfs:label "decommissioned"@no .

### http://inspire.ec.europa.eu/ont:VerticalPositionValue
:VerticalPositionValue a owl:Class ;
       rdfs:subClassOf :itnrEnumeration ;
          rdfs:isDefinedBy  <https://inspire.ec.europa.eu/enumeration/VerticalPositionValue>;
         skos:definition "-- Definition -- The relative vertical position of a spatial object.  "@en ;
       rdfs:label "VerticalPositionValue"@en .

### http://inspire.ec.europa.eu/ont:VerticalPositionValueCode
:VerticalPositionValueCode a skos:ConceptScheme ;
         skos:definition "-- Definition -- The relative vertical position of a spatial object.  "@en ;
          owl:sameAs  <https://inspire.ec.europa.eu/enumeration/VerticalPositionValue>;
       dc:isFormatOf :VerticalPositionValue .

### http://inspire.ec.europa.eu/ont:VerticalPositionValue.onGroundSurface
:VerticalPositionValue.onGroundSurface a :VerticalPositionValue,skos:Concept ;
         skos:inScheme :VerticalPositionValueCode ;
         skos:definition "-- Definition -- The spatial object is on ground level. "@en ;
          owl:sameAs  <https://inspire.ec.europa.eu/enumeration/VerticalPositionValue/onGroundSurface>;
          rdfs:isDefinedBy  <https://inspire.ec.europa.eu/enumeration/VerticalPositionValue/onGroundSurface>;
         rdfs:label "onGroundSurface"@no .

### http://inspire.ec.europa.eu/ont:VerticalPositionValue.suspendedOrElevated
:VerticalPositionValue.suspendedOrElevated a :VerticalPositionValue,skos:Concept ;
         skos:inScheme :VerticalPositionValueCode ;
         skos:definition "-- Definition -- The spatial object is suspended or elevated. "@en ;
          owl:sameAs  <https://inspire.ec.europa.eu/enumeration/VerticalPositionValue/suspendedOrElevated>;
          rdfs:isDefinedBy  <https://inspire.ec.europa.eu/enumeration/VerticalPositionValue/suspendedOrElevated>;
         rdfs:label "suspendedOrElevated"@no .

### http://inspire.ec.europa.eu/ont:VerticalPositionValue.underground
:VerticalPositionValue.underground a :VerticalPositionValue,skos:Concept ;
         skos:inScheme :VerticalPositionValueCode ;
         skos:definition "-- Definition -- The spatial object is underground. "@en ;
          owl:sameAs  <https://inspire.ec.europa.eu/enumeration/VerticalPositionValue/underground>;
          rdfs:isDefinedBy  <https://inspire.ec.europa.eu/enumeration/VerticalPositionValue/underground>;
         rdfs:label "underground"@no .
:VerticalPositionValue owl:oneOf ( :VerticalPositionValue.onGroundSurface :VerticalPositionValue.suspendedOrElevated :VerticalPositionValue.underground  ) ; .


### http://inspire.ec.europa.eu/ont:AddressComponent
:AddressComponent a owl:Class ;
       rdfs:subClassOf :itnrFeature ;
          rdfs:isDefinedBy  <http://inspire.ec.europa.eu/featureconcept/AddressComponent>;
         skos:definition "-- Definition -- Identifier or geographic name of a specific geographic area, location, or other spatial object which defines the scope of an address.  -- Description -- NOTE 1 Four different subclasses of address components are defined:  o    Administrative unit name, which may include name of country, name of municipality, name of district o    Address area name like e.g. name of village or settlement  o    Thoroughfare name, most often road name   o    Postal descriptor  In order to construct an address, these subclasses are often structured hierarchically.  NOTE 2 It is the combination of the address locator and the address components, which makes a specific address spatial object readable and unambiguous for the human user.   EXAMPLE The combination of the locator \"13\" and the address components \"Calle Mayor\" (thoroughfare name), \"Cortijo del Marqués\" (address area name), \"41037\" (postal descriptor), \"Écija\", \"Sevilla\" and \"España\" (administrative unit names) makes this specific address spatial object readable and unambiguous."@en ;
       rdfs:label "AddressComponent"@en .

### http://inspire.ec.europa.eu/ont#situatedWithin
:situatedWithin rdf:type owl:ObjectProperty ;
         skos:definition "-- Definition -- Another address component within which the geographic feature represented by this address component is situated.  -- Description -- NOTE 1 The association enables the application schema to express that the subtypes of address components in the dataset form a hierarchy e.g. like: thoroughfare name within municipality within region within country   NOTE 2 The representation of the hierarchy facilitates queries e.g. for a specific thoroughfare name within a given municipality or postcode. It is also necessary where the application schema is used to create or update, for example , a gazetteer which is based on the hierarchical structure of the address components.   NOTE 3 The multiplicity of the association allows it to express that a thoroughfare name is situated in a certain municipality and in a certain postcode. It is also possible to express, for example, that some thoroughfare names cross borders between municipalities and thus is situated within more than one municipality.  EXAMPLE 1 In Spain many spatial objects of the thoroughfare name \"Calle Santiago\" exist. The association can express that one of the spatial objects is situated within in the municipality of Albacete. From the same example the municipality name \"Albacete\" is situated within the administrative name (region) of \"Castilla La Mancha\".  EXAMPLE 2 In Denmark, several address area names entitled \"Strandby\" exists. In order to identify a specific spatial object it is necessary to know that the relevant spatial object is situated e.g. in the municipality of \"Frederikshavn\"."@en ;
         rdfs:domain :AddressComponent;
         rdfs:range :AddressComponent;
         rdfs:label "situatedWithin"@en .
:AddressComponent rdfs:subClassOf [ rdf:type owl:Restriction ;
         owl:onProperty :situatedWithin;
         owl:allValuesFrom :AddressComponent;
         ] .


### http://inspire.ec.europa.eu/ont#inspireId
:inspireId rdf:type owl:ObjectProperty ;
         skos:definition "-- Definition -- External object identifier of the spatial object.  -- Description -- NOTE 1 An external object identifier is a unique object identifier published by the responsible body, which may be used by external applications to reference the spatial object. The identifier is an identifier of the spatial object, not an identifier of the real-world phenomenon.   NOTE 2 The primary purpose of this identifier is to enable links between various sources and the address components.  EXAMPLE An address component spatial object from Denmark could carry this identifier:  Namespace: DK_ADR Local identifier: 0A3F507B2AB032B8E0440003BA298018 Version identifier: 12-02-2008T10:05:01+01:00"@en ;
         rdfs:range :Identifier;
         rdfs:label "inspireId"@en .
:AddressComponent rdfs:subClassOf [ rdf:type owl:Restriction ;
         owl:onProperty :inspireId;
         owl:onClass :Identifier;
       owl:maxQualifiedCardinality "1"^^xsd:nonNegativeInteger ;
         ] .
:AddressComponent rdfs:subClassOf [ rdf:type owl:Restriction ;
         owl:onProperty :inspireId;
         owl:allValuesFrom :Identifier;
         ] .


### http://inspire.ec.europa.eu/ont#alternativeIdentifier
:alternativeIdentifier rdf:type owl:DatatypeProperty ;
         skos:definition "-- Definition -- External, thematic identifier of the address component spatial object, which enables interoperability with existing legacy systems or applications.   -- Description -- NOTE Compared with a proper identifier of the address component, the alternative identifier is not necessarily persistent in the lifetime of the component spatial object. Likewise it is usually not globally unique and in general does include information on the version of the spatial object.   EXAMPLE 1 National or regional sector-specific identifiers (like e.g. a number- or letter code) for administrative units, address areas (localities, villages, sub-divisions) or thoroughfare names, which are used by a number of existing legacy systems.   EXAMPLE 2 In Denmark the four character municipal \"road name code\" (0001-9899) is only unique within the present municipality, thus if two municipalities merge, it is necessary to assign new road name codes."@en ;
         rdfs:domain :AddressComponent;
         rdfs:range xsd:string;
         rdfs:label "alternativeIdentifier"@en .
:AddressComponent rdfs:subClassOf [ rdf:type owl:Restriction ;
         owl:onProperty :alternativeIdentifier;
         owl:onDataRange xsd:string;
       owl:maxQualifiedCardinality "1"^^xsd:nonNegativeInteger ;
         ] .
:AddressComponent rdfs:subClassOf [ rdf:type owl:Restriction ;
         owl:onProperty :alternativeIdentifier;
         owl:allValuesFrom xsd:string;
         ] .


### http://inspire.ec.europa.eu/ont#beginLifespanVersion
:beginLifespanVersion rdf:type owl:DatatypeProperty ;
         skos:definition "-- Definition -- Date and time at which this version of the spatial object was inserted or changed in the spatial data set.   -- Description -- NOTE This date is recorded to enable the generation of change only update files. "@en ;
         rdfs:range xsd:dateTime;
         rdfs:label "beginLifespanVersion"@en .
:AddressComponent rdfs:subClassOf [ rdf:type owl:Restriction ;
         owl:onProperty :beginLifespanVersion;
         owl:onDataRange xsd:dateTime;
       owl:qualifiedCardinality "1"^^xsd:nonNegativeInteger ;
         ] .
:AddressComponent rdfs:subClassOf [ rdf:type owl:Restriction ;
         owl:onProperty :beginLifespanVersion;
         owl:allValuesFrom xsd:dateTime;
         ] .


### http://inspire.ec.europa.eu/ont#endLifespanVersion
:endLifespanVersion rdf:type owl:DatatypeProperty ;
         skos:definition "-- Definition -- Date and time at which this version of the spatial object was superseded or retired in the spatial data set.  -- Description -- NOTE This date is recorded primarily for those systems which \"close\" an entry in the spatial data set in the event of an attribute change."@en ;
         rdfs:range xsd:dateTime;
         rdfs:label "endLifespanVersion"@en .
:AddressComponent rdfs:subClassOf [ rdf:type owl:Restriction ;
         owl:onProperty :endLifespanVersion;
         owl:onDataRange xsd:dateTime;
       owl:maxQualifiedCardinality "1"^^xsd:nonNegativeInteger ;
         ] .
:AddressComponent rdfs:subClassOf [ rdf:type owl:Restriction ;
         owl:onProperty :endLifespanVersion;
         owl:allValuesFrom xsd:dateTime;
         ] .


### http://inspire.ec.europa.eu/ont#status
:status rdf:type owl:ObjectProperty ;
         skos:definition "-- Definition -- Validity of the address component within the life-cycle (version) of the address component spatial object.   -- Description -- NOTE This status relates to the address component and is not a property of the object to which the address is assigned (the addressable object)."@en ;
         rdfs:domain :AddressComponent;
         rdfs:range :StatusValue;
         rdfs:label "status"@en .
:AddressComponent rdfs:subClassOf [ rdf:type owl:Restriction ;
         owl:onProperty :status;
         owl:onClass :StatusValue;
       owl:maxQualifiedCardinality "1"^^xsd:nonNegativeInteger ;
         ] .
:AddressComponent rdfs:subClassOf [ rdf:type owl:Restriction ;
         owl:onProperty :status;
         owl:allValuesFrom :StatusValue;
         ] .


### http://inspire.ec.europa.eu/ont#validFrom
:validFrom rdf:type owl:DatatypeProperty ;
         skos:definition "-- Definition -- Date and time of which this version of the spatial object was or will be valid in the real world.   -- Description -- NOTE This date and time can be set in the future for situations where an spatial object or a version of spatial object has been decided by the appropriate authority to take effect for a future date."@en ;
         rdfs:range xsd:dateTime;
         rdfs:label "validFrom"@en .
:AddressComponent rdfs:subClassOf [ rdf:type owl:Restriction ;
         owl:onProperty :validFrom;
         owl:onDataRange xsd:dateTime;
       owl:qualifiedCardinality "1"^^xsd:nonNegativeInteger ;
         ] .
:AddressComponent rdfs:subClassOf [ rdf:type owl:Restriction ;
         owl:onProperty :validFrom;
         owl:allValuesFrom xsd:dateTime;
         ] .


### http://inspire.ec.europa.eu/ont#validTo
:validTo rdf:type owl:DatatypeProperty ;
         skos:definition "-- Definition -- Date and time at which the spatial object ceased or will cease to exist in the real world."@en ;
         rdfs:range xsd:dateTime;
         rdfs:label "validTo"@en .
:AddressComponent rdfs:subClassOf [ rdf:type owl:Restriction ;
         owl:onProperty :validTo;
         owl:onDataRange xsd:dateTime;
       owl:maxQualifiedCardinality "1"^^xsd:nonNegativeInteger ;
         ] .
:AddressComponent rdfs:subClassOf [ rdf:type owl:Restriction ;
         owl:onProperty :validTo;
         owl:allValuesFrom xsd:dateTime;
         ] .

:AddressComponent owl:disjointUnionOf ( :ThoroughfareName  ) ; .

### http://inspire.ec.europa.eu/ont:PartOfName
:PartOfName a owl:Class ;
       rdfs:subClassOf :itnrDataType ;
         skos:definition "-- Definition -- A part of the full name resulting from the subdivision of the thoroughfare name into separate, semantic parts, using the same language and script as the full thoroughfare name.  -- Description -- NOTE Each part of the name must be qualified by using the type attribute."@en ;
       rdfs:label "PartOfName"@en .

### http://inspire.ec.europa.eu/ont#part
:part rdf:type owl:DatatypeProperty ;
         skos:definition "-- Definition -- The character string that expresses the separate part of the name using the same language and script as the full thoroughfare name."@en ;
         rdfs:domain :PartOfName;
         rdfs:range xsd:string;
         rdf:type owl:FunctionalProperty;
         rdfs:label "part"@en .
:PartOfName rdfs:subClassOf [ rdf:type owl:Restriction ;
         owl:onProperty :part;
         owl:onDataRange xsd:string;
       owl:qualifiedCardinality "1"^^xsd:nonNegativeInteger ;
         ] .
:PartOfName rdfs:subClassOf [ rdf:type owl:Restriction ;
         owl:onProperty :part;
         owl:allValuesFrom xsd:string;
         ] .


### http://inspire.ec.europa.eu/ont#PartOfName.type
:PartOfName.type rdf:type owl:ObjectProperty ;
         skos:definition "-- Definition -- A classification of the part of name according to its semantics (meaning) in the complete thoroughfare name. "@en ;
         rdfs:domain :PartOfName;
         rdfs:range :PartTypeValue;
         rdf:type owl:FunctionalProperty;
         rdfs:label "PartOfName.type"@en .
:PartOfName rdfs:subClassOf [ rdf:type owl:Restriction ;
         owl:onProperty :PartOfName.type;
         owl:onClass :PartTypeValue;
       owl:qualifiedCardinality "1"^^xsd:nonNegativeInteger ;
         ] .
:PartOfName rdfs:subClassOf [ rdf:type owl:Restriction ;
         owl:onProperty :PartOfName.type;
         owl:allValuesFrom :PartTypeValue;
         ] .


### http://inspire.ec.europa.eu/ont:PartTypeValue
:PartTypeValue a owl:Class ;
       rdfs:subClassOf :itnrCodeList ;
          rdfs:isDefinedBy  <https://inspire.ec.europa.eu/codelist/PartTypeValue>;
         skos:definition "-- Definition -- A classification of the part of name according to its semantics in the complete thoroughfare name."@en ;
       rdfs:label "PartTypeValue"@en .

### http://inspire.ec.europa.eu/ont:PartTypeValueCode
:PartTypeValueCode a skos:ConceptScheme ;
         skos:definition "-- Definition -- A classification of the part of name according to its semantics in the complete thoroughfare name."@en ;
          owl:sameAs  <https://inspire.ec.europa.eu/codelist/PartTypeValue>;
       dc:isFormatOf :PartTypeValue .

### http://inspire.ec.europa.eu/ont:PartTypeValue.name
:PartTypeValue.name a :PartTypeValue,skos:Concept ;
         skos:inScheme :PartTypeValueCode ;
         skos:definition "-- Definition -- The part of name constitutes the core or root of the thoroughfare name.   -- Description -- EXAMPLE \"Abelheira\" in Rua da Abelheira (Caçém, Portugal), \"Madeleine\" in Place de la Madeleine (Paris, France), \"Christo Canneregio\" in Calle del Christo Canneregio (Venezia, Italy), \"Quai\" in Unterer Quai (Biel/Bienne, Switzerland) and \"Strand\" in Little Strand Street (Dublin, Ireland)."@en ;
          owl:sameAs  <https://inspire.ec.europa.eu/codelist/PartTypeValue/name>;
          rdfs:isDefinedBy  <https://inspire.ec.europa.eu/codelist/PartTypeValue/name>;
         rdfs:label "name"@no .

### http://inspire.ec.europa.eu/ont:PartTypeValue.namePrefix
:PartTypeValue.namePrefix a :PartTypeValue,skos:Concept ;
         skos:inScheme :PartTypeValueCode ;
         skos:definition "-- Definition -- The part of name is used to separate connecting words without sorting significance from the core of the thoroughfare name.  -- Description -- EXAMPLE \"da\" in Rua da Abelheira (Caçém, Portugal), \"de la \" in Place de la Madeleine (Paris, France) and \"del\" in Calle del Christo Canneregio (Venezia, Italy)."@en ;
          owl:sameAs  <https://inspire.ec.europa.eu/codelist/PartTypeValue/namePrefix>;
          rdfs:isDefinedBy  <https://inspire.ec.europa.eu/codelist/PartTypeValue/namePrefix>;
         rdfs:label "namePrefix"@no .

### http://inspire.ec.europa.eu/ont:PartTypeValue.type
:PartTypeValue.type a :PartTypeValue,skos:Concept ;
         skos:inScheme :PartTypeValueCode ;
         skos:definition "-- Definition -- The part of name indicates the category or type of thoroughfare.  -- Description -- EXAMPLE \"Rua\" in Rua da Abelheira (Caçém, Portugal), \"Place\" in Place de la Madeleine (Paris, France), \"Calle\" in Calle del Christo Canneregio (Venezia, Italy) and \"Street\" in Little Strand Street (Dublin, Ireland)."@en ;
          owl:sameAs  <https://inspire.ec.europa.eu/codelist/PartTypeValue/type>;
          rdfs:isDefinedBy  <https://inspire.ec.europa.eu/codelist/PartTypeValue/type>;
         rdfs:label "type"@no .

### http://inspire.ec.europa.eu/ont:PartTypeValue.qualifier
:PartTypeValue.qualifier a :PartTypeValue,skos:Concept ;
         skos:inScheme :PartTypeValueCode ;
         skos:definition "-- Definition -- The part of name qualifies the thoroughfare name.  -- Description -- EXAMPLE \"Unterer\" in Unterer Quai (German name in Biel/Bienne, Switzerland), \"Bas\" in Quai Bas (French name for same street) and \"Little\" in Little Strand Street (Dublin, Ireland)."@en ;
          owl:sameAs  <https://inspire.ec.europa.eu/codelist/PartTypeValue/qualifier>;
          rdfs:isDefinedBy  <https://inspire.ec.europa.eu/codelist/PartTypeValue/qualifier>;
         rdfs:label "qualifier"@no .

### http://inspire.ec.europa.eu/ont:StatusValue
:StatusValue a owl:Class ;
       rdfs:subClassOf :itnrCodeList ;
          rdfs:isDefinedBy  <https://inspire.ec.europa.eu/codelist/StatusValue>;
         skos:definition "-- Definition -- Current validity of the real world address or address component.   -- Description -- NOTE 1 This element enables the application schema to represent a full life-cycle of an address and address component, from proposed to reserved, current and retired, or even alternative.   NOTE 2 The status value relates to the real world address or address component and not to the property to which the address or address component is assigned (the addressable object)."@en ;
       rdfs:label "StatusValue"@en .

### http://inspire.ec.europa.eu/ont:StatusValueCode
:StatusValueCode a skos:ConceptScheme ;
         skos:definition "-- Definition -- Current validity of the real world address or address component.   -- Description -- NOTE 1 This element enables the application schema to represent a full life-cycle of an address and address component, from proposed to reserved, current and retired, or even alternative.   NOTE 2 The status value relates to the real world address or address component and not to the property to which the address or address component is assigned (the addressable object)."@en ;
          owl:sameAs  <https://inspire.ec.europa.eu/codelist/StatusValue>;
       dc:isFormatOf :StatusValue .

### http://inspire.ec.europa.eu/ont:StatusValue.current
:StatusValue.current a :StatusValue,skos:Concept ;
         skos:inScheme :StatusValueCode ;
         skos:definition "-- Definition -- Current and valid address according to official body responsible for address allocation or deemed, by the dataset custodian, to be the most appropriate, commonly used address."@en ;
          owl:sameAs  <https://inspire.ec.europa.eu/codelist/StatusValue/current>;
          rdfs:isDefinedBy  <https://inspire.ec.europa.eu/codelist/StatusValue/current>;
         rdfs:label "current"@no .

### http://inspire.ec.europa.eu/ont:StatusValue.retired
:StatusValue.retired a :StatusValue,skos:Concept ;
         skos:inScheme :StatusValueCode ;
         skos:definition "-- Definition -- An address no longer in every day use or abolished by the official body responsible for address allocation or by the dataset custodian."@en ;
          owl:sameAs  <https://inspire.ec.europa.eu/codelist/StatusValue/retired>;
          rdfs:isDefinedBy  <https://inspire.ec.europa.eu/codelist/StatusValue/retired>;
         rdfs:label "retired"@no .

### http://inspire.ec.europa.eu/ont:StatusValue.proposed
:StatusValue.proposed a :StatusValue,skos:Concept ;
         skos:inScheme :StatusValueCode ;
         skos:definition "-- Definition -- An address awaiting approval by the dataset custodian or official body responsible for address allocation."@en ;
          owl:sameAs  <https://inspire.ec.europa.eu/codelist/StatusValue/proposed>;
          rdfs:isDefinedBy  <https://inspire.ec.europa.eu/codelist/StatusValue/proposed>;
         rdfs:label "proposed"@no .

### http://inspire.ec.europa.eu/ont:StatusValue.reserved
:StatusValue.reserved a :StatusValue,skos:Concept ;
         skos:inScheme :StatusValueCode ;
         skos:definition "-- Definition -- An address approved by the by the official body responsible for address allocation or by the dataset custodian, but yet to be implemented."@en ;
          owl:sameAs  <https://inspire.ec.europa.eu/codelist/StatusValue/reserved>;
          rdfs:isDefinedBy  <https://inspire.ec.europa.eu/codelist/StatusValue/reserved>;
         rdfs:label "reserved"@no .

### http://inspire.ec.europa.eu/ont:StatusValue.alternative
:StatusValue.alternative a :StatusValue,skos:Concept ;
         skos:inScheme :StatusValueCode ;
         skos:definition "-- Definition -- An address in common use but different from the master address as determined by the official body responsible for address allocation or by the dataset custodian."@en ;
          owl:sameAs  <https://inspire.ec.europa.eu/codelist/StatusValue/alternative>;
          rdfs:isDefinedBy  <https://inspire.ec.europa.eu/codelist/StatusValue/alternative>;
         rdfs:label "alternative"@no .

### http://inspire.ec.europa.eu/ont:ThoroughfareName
:ThoroughfareName a owl:Class ;
         skos:definition "-- Definition -- An address component which represents the name of a passage or way through from one location to another.   -- Description -- NOTE 1 A thoroughfare can, e.g., be a road or a waterway  NOTE 2 Thoroughfare names includes names of squares and of cul de sacs, and they can also represent the network of smaller roads or paths e.g. in a small village or settlement."@en ;
       rdfs:label "ThoroughfareName"@en .

### http://inspire.ec.europa.eu/ont#ThoroughfareName.transportLink
:ThoroughfareName.transportLink rdf:type owl:ObjectProperty ;
         skos:definition "-- Definition -- One or several transport network links to which the spatial object of the thoroughfare name has been designated.  -- Description -- EXAMPLE The thoroughfare name \"Na Pankráci\" in Praha, The Czech Republic, has been designated as a road name for a number of road links (street segments) in the city."@en ;
         rdfs:domain :ThoroughfareName;
         rdfs:range :TransportLink;
         rdfs:label "ThoroughfareName.transportLink"@en .
:ThoroughfareName rdfs:subClassOf [ rdf:type owl:Restriction ;
         owl:onProperty :ThoroughfareName.transportLink;
         owl:allValuesFrom :TransportLink;
         ] .

:ThoroughfareName rdfs:subClassOf :AddressComponent .

### http://inspire.ec.europa.eu/ont#ThoroughfareName.name
:ThoroughfareName.name rdf:type owl:ObjectProperty ;
         skos:definition "-- Definition -- Name of the thoroughfare.  -- Description -- NOTE 1 The name can optionally include an often used alternative name, alternative spelling of the name, a historic name or spelling, which is still in use. It may also optionally include a subdivision of the name into parts.  NOTE 2 Most often thoroughfares are roads, in this situation the thoroughfare name is the road name.    NOTE 3 The data type also allows a representation of the thoroughfare name in separate parts e.g. \"rue\" + \"de la\" + \"Paix\""@en ;
         rdfs:domain :ThoroughfareName;
         rdfs:range :ThoroughfareNameValue;
         rdfs:label "ThoroughfareName.name"@en .
:ThoroughfareName rdfs:subClassOf [ rdf:type owl:Restriction ;
         owl:onProperty :ThoroughfareName.name;
         owl:onClass :ThoroughfareNameValue;
       owl:minQualifiedCardinality "1"^^xsd:nonNegativeInteger ;
         ] .
:ThoroughfareName rdfs:subClassOf [ rdf:type owl:Restriction ;
         owl:onProperty :ThoroughfareName.name;
         owl:allValuesFrom :ThoroughfareNameValue;
         ] .


### http://inspire.ec.europa.eu/ont:ThoroughfareNameValue
:ThoroughfareNameValue a owl:Class ;
       rdfs:subClassOf :itnrDataType ;
         skos:definition "-- Definition -- Proper noun applied to thoroughfare optionally including a subdivision of the name into parts.  -- Description -- NOTE 1 The data type allows names in different languages and scripts as well as inclusion of alternative name, alternative spellings, historical name and exonyms.   NOTE 2 The data type allows optionally a representation of the thoroughfare name subdivided into separate, semantic parts e.g. \"Avenue\" + \"de la\" + \"Poste\"."@en ;
       rdfs:label "ThoroughfareNameValue"@en .

### http://inspire.ec.europa.eu/ont#ThoroughfareNameValue.name
:ThoroughfareNameValue.name rdf:type owl:ObjectProperty ;
         skos:definition "-- Definition -- Proper noun applied to the thoroughfare.  -- Description -- NOTE 1 The complete name of the thoroughfare must be applied in this attribute, including type, prefix or qualifier, like for example \"Avenue de la Poste\", \"Calle del Christo Canneregio\" or \"Untere Quai\". The name part attribute enables a representation of the name subdivided into separate semantic parts.  NOTE 2 The data type allows names in different languages as well as inclusion of exonyms. "@en ;
         rdfs:domain :ThoroughfareNameValue;
         rdfs:range :GeographicalName;
         rdf:type owl:FunctionalProperty;
         rdfs:label "ThoroughfareNameValue.name"@en .
:ThoroughfareNameValue rdfs:subClassOf [ rdf:type owl:Restriction ;
         owl:onProperty :ThoroughfareNameValue.name;
         owl:onClass :GeographicalName;
       owl:qualifiedCardinality "1"^^xsd:nonNegativeInteger ;
         ] .
:ThoroughfareNameValue rdfs:subClassOf [ rdf:type owl:Restriction ;
         owl:onProperty :ThoroughfareNameValue.name;
         owl:allValuesFrom :GeographicalName;
         ] .


### http://inspire.ec.europa.eu/ont#nameParts
:nameParts rdf:type owl:ObjectProperty ;
         skos:definition "-- Definition -- One or several parts into which the thoroughfare name can be subdivided.  -- Description -- NOTE 1 This is a definition which is consistent with that adopted by the UPU  NOTE 2 A subdivision of a thoroughfare name into semantic parts could improve parsing (e.g. of abbreviated or misspelled names) and for sorting of address data for example for postal delivery purposes. It could also improve the creation of alphabetically sorted street gazetteers.   NOTE 3 The data type requires that each part of the subdivided thoroughfare name is qualified with information on the semantics e.g. if it is a thoroughfare type (e.g., Rua, Place, Calle, Street), a prefix (e.g., da, de la, del), a qualifier (e.g., Unterer, Little) or if it is the core of the name, which would normally be used for sorting or indexing.   NOTE 4 In some countries or regions and for some thoroughfare names it is not feasible or it does not add value to subdivide the thoroughfare name into parts.  EXAMPLE In France the thoroughfare name \"Avenue de la Poste\" could be subdivided into these parts: \"Avenue\" + \"de la\" + \"Poste\"."@en ;
         rdfs:domain :ThoroughfareNameValue;
         rdfs:range :PartOfName;
         rdfs:label "nameParts"@en .
:ThoroughfareNameValue rdfs:subClassOf [ rdf:type owl:Restriction ;
         owl:onProperty :nameParts;
         owl:allValuesFrom :PartOfName;
         ] .



### http://inspire.ec.europa.eu/ont:GeographicalName
:GeographicalName a owl:Class ;
       rdfs:subClassOf :itnrDataType ;
         skos:definition "-- Definition -- Proper noun applied to a real world entity."@en ;
       rdfs:label "GeographicalName"@en .

### http://inspire.ec.europa.eu/ont#language
:language rdf:type owl:DatatypeProperty ;
         skos:definition "-- Definition -- Language of the name, given as a three letters code, in accordance with either ISO 639-3 or ISO 639-5.  -- Description -- NOTE 1More precisely, this definition refers to the language used by the community that uses the name.  NOTE 2 The code \"mul\" for \"multilingual\" should not be used in general. However it can be used in rare cases like official names composed of two names in different languages. For example, \"Vitoria-Gasteiz\" is such a multilingual official name in Spain.  NOTE 3 Even if this attribute is \"voidable\" for pragmatic reasons, it is of first importance in several use cases in the multi-language context of Europe. "@en ;
         rdfs:domain :GeographicalName;
         rdfs:range xsd:string;
         rdf:type owl:FunctionalProperty;
         rdfs:label "language"@en .
:GeographicalName rdfs:subClassOf [ rdf:type owl:Restriction ;
         owl:onProperty :language;
         owl:onDataRange xsd:string;
       owl:qualifiedCardinality "1"^^xsd:nonNegativeInteger ;
         ] .
:GeographicalName rdfs:subClassOf [ rdf:type owl:Restriction ;
         owl:onProperty :language;
         owl:allValuesFrom xsd:string;
         ] .


### http://inspire.ec.europa.eu/ont#nativeness
:nativeness rdf:type owl:ObjectProperty ;
         skos:definition "-- Definition -- Information enabling to acknowledge if the name is the one that is/was used in the area where the spatial object is situated at the instant when the name is/was in use. "@en ;
         rdfs:domain :GeographicalName;
         rdfs:range :NativenessValue;
         rdf:type owl:FunctionalProperty;
         rdfs:label "nativeness"@en .
:GeographicalName rdfs:subClassOf [ rdf:type owl:Restriction ;
         owl:onProperty :nativeness;
         owl:onClass :NativenessValue;
       owl:qualifiedCardinality "1"^^xsd:nonNegativeInteger ;
         ] .
:GeographicalName rdfs:subClassOf [ rdf:type owl:Restriction ;
         owl:onProperty :nativeness;
         owl:allValuesFrom :NativenessValue;
         ] .


### http://inspire.ec.europa.eu/ont#nameStatus
:nameStatus rdf:type owl:ObjectProperty ;
         skos:definition "-- Definition -- Qualitative information enabling to discern which credit should be given to the name with respect to its standardisation and/or its topicality.  -- Description -- NOTE The Geographical Names application schema does not explicitly make a preference between different names (e.g. official endonyms) of a specific real world entity. The necessary information for making the preference (e.g. the linguistic status of the administrative or geographic area in question), for a certain use case, must be obtained from other data or information sources. For example, the status of the language of the name may be known through queries on the geometries of named places against the geometry of administrative units recorded in a certain source with the language statuses information. "@en ;
         rdfs:domain :GeographicalName;
         rdfs:range :NameStatusValue;
         rdf:type owl:FunctionalProperty;
         rdfs:label "nameStatus"@en .
:GeographicalName rdfs:subClassOf [ rdf:type owl:Restriction ;
         owl:onProperty :nameStatus;
         owl:onClass :NameStatusValue;
       owl:qualifiedCardinality "1"^^xsd:nonNegativeInteger ;
         ] .
:GeographicalName rdfs:subClassOf [ rdf:type owl:Restriction ;
         owl:onProperty :nameStatus;
         owl:allValuesFrom :NameStatusValue;
         ] .


### http://inspire.ec.europa.eu/ont#sourceOfName
:sourceOfName rdf:type owl:DatatypeProperty ;
         skos:definition "-- Definition -- Original data source from which the geographical name is taken from and integrated in the data set providing/publishing it. For some named spatial objects it might refer again to the publishing data set if no other information is available.  -- Description -- EXAMPLES Gazetteer, geographical names data set. "@en ;
         rdfs:domain :GeographicalName;
         rdfs:range xsd:string;
         rdf:type owl:FunctionalProperty;
         rdfs:label "sourceOfName"@en .
:GeographicalName rdfs:subClassOf [ rdf:type owl:Restriction ;
         owl:onProperty :sourceOfName;
         owl:onDataRange xsd:string;
       owl:qualifiedCardinality "1"^^xsd:nonNegativeInteger ;
         ] .
:GeographicalName rdfs:subClassOf [ rdf:type owl:Restriction ;
         owl:onProperty :sourceOfName;
         owl:allValuesFrom xsd:string;
         ] .


### http://inspire.ec.europa.eu/ont#pronunciation
:pronunciation rdf:type owl:ObjectProperty ;
         skos:definition "-- Definition -- Proper, correct or standard (standard within the linguistic community concerned) pronunciation of the geographical name.  -- Description -- SOURCE Adapted from [UNGEGN Manual 2006]. "@en ;
         rdfs:domain :GeographicalName;
         rdfs:range :PronunciationOfName;
         rdf:type owl:FunctionalProperty;
         rdfs:label "pronunciation"@en .
:GeographicalName rdfs:subClassOf [ rdf:type owl:Restriction ;
         owl:onProperty :pronunciation;
         owl:onClass :PronunciationOfName;
       owl:qualifiedCardinality "1"^^xsd:nonNegativeInteger ;
         ] .
:GeographicalName rdfs:subClassOf [ rdf:type owl:Restriction ;
         owl:onProperty :pronunciation;
         owl:allValuesFrom :PronunciationOfName;
         ] .


### http://inspire.ec.europa.eu/ont#spelling
:spelling rdf:type owl:ObjectProperty ;
         skos:definition "-- Definition -- A proper way of writing the geographical name.  -- Description -- NOTE 1 Different spellings should only be used for names rendered in different scripts. .  NOTE 2 While a particular GeographicalName should only have one spelling in a given script, providing different spellings in the same script should be done through the provision of different geographical names associated with the same named place. "@en ;
         rdfs:domain :GeographicalName;
         rdfs:range :SpellingOfName;
         rdfs:label "spelling"@en .
:GeographicalName rdfs:subClassOf [ rdf:type owl:Restriction ;
         owl:onProperty :spelling;
         owl:onClass :SpellingOfName;
       owl:minQualifiedCardinality "1"^^xsd:nonNegativeInteger ;
         ] .
:GeographicalName rdfs:subClassOf [ rdf:type owl:Restriction ;
         owl:onProperty :spelling;
         owl:allValuesFrom :SpellingOfName;
         ] .


### http://inspire.ec.europa.eu/ont#grammaticalGender
:grammaticalGender rdf:type owl:ObjectProperty ;
         skos:definition "-- Definition -- Class of nouns reflected in the behaviour of associated words.  -- Description -- NOTE the attribute has cardinality [0..1] and is voidable, which means that: <ul> 	<li>in case the concept of grammatical gender has no sense for a given name (i.e. the attribute is not applicable), the attribute should not be provided.</li> 	<li>in case the concept of grammatical gender has some sense for the name but is unknown, the attribute should be provided but <i>void</i>.  </li> </ul>  "@en ;
         rdfs:domain :GeographicalName;
         rdfs:range :GrammaticalGenderValue;
         rdfs:label "grammaticalGender"@en .
:GeographicalName rdfs:subClassOf [ rdf:type owl:Restriction ;
         owl:onProperty :grammaticalGender;
         owl:onClass :GrammaticalGenderValue;
       owl:maxQualifiedCardinality "1"^^xsd:nonNegativeInteger ;
         ] .
:GeographicalName rdfs:subClassOf [ rdf:type owl:Restriction ;
         owl:onProperty :grammaticalGender;
         owl:allValuesFrom :GrammaticalGenderValue;
         ] .


### http://inspire.ec.europa.eu/ont#grammaticalNumber
:grammaticalNumber rdf:type owl:ObjectProperty ;
         skos:definition "-- Definition -- Grammatical category of nouns that expresses count distinctions.  -- Description -- NOTE the attribute has cardinality [0..1] and is voidable, which means that: <ul> 	<li>in case the concept of grammatical number has no sense for a given name (i.e. the attribute is not applicable), the attribute should not be provided.</li> 	<li>in case the concept of grammatical number has some sense for the name but is unknown, the attribute should be provided but <i>void</i>.</li> </ul>  "@en ;
         rdfs:domain :GeographicalName;
         rdfs:range :GrammaticalNumberValue;
         rdfs:label "grammaticalNumber"@en .
:GeographicalName rdfs:subClassOf [ rdf:type owl:Restriction ;
         owl:onProperty :grammaticalNumber;
         owl:onClass :GrammaticalNumberValue;
       owl:maxQualifiedCardinality "1"^^xsd:nonNegativeInteger ;
         ] .
:GeographicalName rdfs:subClassOf [ rdf:type owl:Restriction ;
         owl:onProperty :grammaticalNumber;
         owl:allValuesFrom :GrammaticalNumberValue;
         ] .


### http://inspire.ec.europa.eu/ont:GrammaticalGenderValue
:GrammaticalGenderValue a owl:Class ;
       rdfs:subClassOf :itnrCodeList ;
          rdfs:isDefinedBy  <https://inspire.ec.europa.eu/codelist/GrammaticalGenderValue>;
         skos:definition "-- Definition -- The grammatical gender of a geographical name. "@en ;
       rdfs:label "GrammaticalGenderValue"@en .

### http://inspire.ec.europa.eu/ont:GrammaticalGenderValueCode
:GrammaticalGenderValueCode a skos:ConceptScheme ;
         skos:definition "-- Definition -- The grammatical gender of a geographical name. "@en ;
          owl:sameAs  <https://inspire.ec.europa.eu/codelist/GrammaticalGenderValue>;
       dc:isFormatOf :GrammaticalGenderValue .

### http://inspire.ec.europa.eu/ont:GrammaticalGenderValue.masculine
:GrammaticalGenderValue.masculine a :GrammaticalGenderValue,skos:Concept ;
         skos:inScheme :GrammaticalGenderValueCode ;
         skos:definition "-- Definition -- Masculine grammatical gender.  -- Description -- EXAMPLES Sena (Spanish), Schwarzwald (German). "@en ;
          owl:sameAs  <https://inspire.ec.europa.eu/codelist/GrammaticalGenderValue/masculine>;
          rdfs:isDefinedBy  <https://inspire.ec.europa.eu/codelist/GrammaticalGenderValue/masculine>;
         rdfs:label "masculine"@no .

### http://inspire.ec.europa.eu/ont:GrammaticalGenderValue.feminine
:GrammaticalGenderValue.feminine a :GrammaticalGenderValue,skos:Concept ;
         skos:inScheme :GrammaticalGenderValueCode ;
         skos:definition "-- Definition -- Feminine grammatical gender.  -- Description -- EXAMPLES Seine (French), Forêt Noire (French). "@en ;
          owl:sameAs  <https://inspire.ec.europa.eu/codelist/GrammaticalGenderValue/feminine>;
          rdfs:isDefinedBy  <https://inspire.ec.europa.eu/codelist/GrammaticalGenderValue/feminine>;
         rdfs:label "feminine"@no .

### http://inspire.ec.europa.eu/ont:GrammaticalGenderValue.neuter
:GrammaticalGenderValue.neuter a :GrammaticalGenderValue,skos:Concept ;
         skos:inScheme :GrammaticalGenderValueCode ;
         skos:definition "-- Definition -- Neuter grammatical gender.  -- Description -- EXAMPLES Zwarte Woud (Dutch), Rheinland (German). "@en ;
          owl:sameAs  <https://inspire.ec.europa.eu/codelist/GrammaticalGenderValue/neuter>;
          rdfs:isDefinedBy  <https://inspire.ec.europa.eu/codelist/GrammaticalGenderValue/neuter>;
         rdfs:label "neuter"@no .

### http://inspire.ec.europa.eu/ont:GrammaticalGenderValue.common
:GrammaticalGenderValue.common a :GrammaticalGenderValue,skos:Concept ;
         skos:inScheme :GrammaticalGenderValueCode ;
         skos:definition "-- Definition -- 'Common' grammatical gender (the merging of 'masculine' and 'feminine').  "@en ;
          owl:sameAs  <https://inspire.ec.europa.eu/codelist/GrammaticalGenderValue/common>;
          rdfs:isDefinedBy  <https://inspire.ec.europa.eu/codelist/GrammaticalGenderValue/common>;
         rdfs:label "common"@no .

### http://inspire.ec.europa.eu/ont:GrammaticalNumberValue
:GrammaticalNumberValue a owl:Class ;
       rdfs:subClassOf :itnrCodeList ;
          rdfs:isDefinedBy  <https://inspire.ec.europa.eu/codelist/GrammaticalNumberValue>;
         skos:definition "-- Definition -- The grammatical number of a geographical name. "@en ;
       rdfs:label "GrammaticalNumberValue"@en .

### http://inspire.ec.europa.eu/ont:GrammaticalNumberValueCode
:GrammaticalNumberValueCode a skos:ConceptScheme ;
         skos:definition "-- Definition -- The grammatical number of a geographical name. "@en ;
          owl:sameAs  <https://inspire.ec.europa.eu/codelist/GrammaticalNumberValue>;
       dc:isFormatOf :GrammaticalNumberValue .

### http://inspire.ec.europa.eu/ont:GrammaticalNumberValue.singular
:GrammaticalNumberValue.singular a :GrammaticalNumberValue,skos:Concept ;
         skos:inScheme :GrammaticalNumberValueCode ;
         skos:definition "-- Definition -- Singular grammatical number.  -- Description -- EXAMPLES Danube (English), Lac du Bourget (French), Praha (Czech), Nederland (Dutch). "@en ;
          owl:sameAs  <https://inspire.ec.europa.eu/codelist/GrammaticalNumberValue/singular>;
          rdfs:isDefinedBy  <https://inspire.ec.europa.eu/codelist/GrammaticalNumberValue/singular>;
         rdfs:label "singular"@no .

### http://inspire.ec.europa.eu/ont:GrammaticalNumberValue.plural
:GrammaticalNumberValue.plural a :GrammaticalNumberValue,skos:Concept ;
         skos:inScheme :GrammaticalNumberValueCode ;
         skos:definition "-- Definition -- Plural grammatical number.  -- Description -- EXAMPLES Alps (English), Pays-Bas (French), Waddeneilanden (Dutch), Cárpatos (Spanish). "@en ;
          owl:sameAs  <https://inspire.ec.europa.eu/codelist/GrammaticalNumberValue/plural>;
          rdfs:isDefinedBy  <https://inspire.ec.europa.eu/codelist/GrammaticalNumberValue/plural>;
         rdfs:label "plural"@no .

### http://inspire.ec.europa.eu/ont:GrammaticalNumberValue.dual
:GrammaticalNumberValue.dual a :GrammaticalNumberValue,skos:Concept ;
         skos:inScheme :GrammaticalNumberValueCode ;
         skos:definition "-- Definition -- Dual grammatical number. "@en ;
          owl:sameAs  <https://inspire.ec.europa.eu/codelist/GrammaticalNumberValue/dual>;
          rdfs:isDefinedBy  <https://inspire.ec.europa.eu/codelist/GrammaticalNumberValue/dual>;
         rdfs:label "dual"@no .

### http://inspire.ec.europa.eu/ont:NameStatusValue
:NameStatusValue a owl:Class ;
       rdfs:subClassOf :itnrCodeList ;
          rdfs:isDefinedBy  <https://inspire.ec.europa.eu/codelist/NameStatusValue>;
         skos:definition "-- Definition -- The status of a geographical name, that is the information enabling to discern which credit should be given to the name with respect to its standardisation and/or its topicality.  -- Description -- NOTE The precise definition of the values 'Official', 'Standardised', 'Historical' and 'Other' can only be decided by Member States according to their legislation and practice.  "@en ;
       rdfs:label "NameStatusValue"@en .

### http://inspire.ec.europa.eu/ont:NameStatusValueCode
:NameStatusValueCode a skos:ConceptScheme ;
         skos:definition "-- Definition -- The status of a geographical name, that is the information enabling to discern which credit should be given to the name with respect to its standardisation and/or its topicality.  -- Description -- NOTE The precise definition of the values 'Official', 'Standardised', 'Historical' and 'Other' can only be decided by Member States according to their legislation and practice.  "@en ;
          owl:sameAs  <https://inspire.ec.europa.eu/codelist/NameStatusValue>;
       dc:isFormatOf :NameStatusValue .

### http://inspire.ec.europa.eu/ont:NameStatusValue.official
:NameStatusValue.official a :NameStatusValue,skos:Concept ;
         skos:inScheme :NameStatusValueCode ;
         skos:definition "-- Definition -- Name in current use and officially approved or established by legislation."@en ;
          owl:sameAs  <https://inspire.ec.europa.eu/codelist/NameStatusValue/official>;
          rdfs:isDefinedBy  <https://inspire.ec.europa.eu/codelist/NameStatusValue/official>;
         rdfs:label "official"@no .

### http://inspire.ec.europa.eu/ont:NameStatusValue.standardised
:NameStatusValue.standardised a :NameStatusValue,skos:Concept ;
         skos:inScheme :NameStatusValueCode ;
         skos:definition "-- Definition -- Name in current use and accepted or recommended by a body assigned advisory function and/or power of decision in matters of toponymy."@en ;
          owl:sameAs  <https://inspire.ec.europa.eu/codelist/NameStatusValue/standardised>;
          rdfs:isDefinedBy  <https://inspire.ec.europa.eu/codelist/NameStatusValue/standardised>;
         rdfs:label "standardised"@no .

### http://inspire.ec.europa.eu/ont:NameStatusValue.historical
:NameStatusValue.historical a :NameStatusValue,skos:Concept ;
         skos:inScheme :NameStatusValueCode ;
         skos:definition "-- Definition -- Historical name not in current use."@en ;
          owl:sameAs  <https://inspire.ec.europa.eu/codelist/NameStatusValue/historical>;
          rdfs:isDefinedBy  <https://inspire.ec.europa.eu/codelist/NameStatusValue/historical>;
         rdfs:label "historical"@no .

### http://inspire.ec.europa.eu/ont:NameStatusValue.other
:NameStatusValue.other a :NameStatusValue,skos:Concept ;
         skos:inScheme :NameStatusValueCode ;
         skos:definition "-- Definition -- Current, but not official, nor approved name."@en ;
          owl:sameAs  <https://inspire.ec.europa.eu/codelist/NameStatusValue/other>;
          rdfs:isDefinedBy  <https://inspire.ec.europa.eu/codelist/NameStatusValue/other>;
         rdfs:label "other"@no .

### http://inspire.ec.europa.eu/ont:NativenessValue
:NativenessValue a owl:Class ;
       rdfs:subClassOf :itnrCodeList ;
          rdfs:isDefinedBy  <https://inspire.ec.europa.eu/codelist/NativenessValue>;
         skos:definition "-- Definition -- The nativeness of a geographical name.  "@en ;
       rdfs:label "NativenessValue"@en .

### http://inspire.ec.europa.eu/ont:NativenessValueCode
:NativenessValueCode a skos:ConceptScheme ;
         skos:definition "-- Definition -- The nativeness of a geographical name.  "@en ;
          owl:sameAs  <https://inspire.ec.europa.eu/codelist/NativenessValue>;
       dc:isFormatOf :NativenessValue .

### http://inspire.ec.europa.eu/ont:NativenessValue.endonym
:NativenessValue.endonym a :NativenessValue,skos:Concept ;
         skos:inScheme :NativenessValueCode ;
         skos:definition "-- Definition -- Name for a geographical feature in an official or well-established language occurring in that area where the feature is situated.  -- Description -- SOURCE [UNGEGN Glossary 2007]. "@en ;
          owl:sameAs  <https://inspire.ec.europa.eu/codelist/NativenessValue/endonym>;
          rdfs:isDefinedBy  <https://inspire.ec.europa.eu/codelist/NativenessValue/endonym>;
         rdfs:label "endonym"@no .

### http://inspire.ec.europa.eu/ont:NativenessValue.exonym
:NativenessValue.exonym a :NativenessValue,skos:Concept ;
         skos:inScheme :NativenessValueCode ;
         skos:definition "-- Definition -- Name used in a specific language for a geographical feature situated outside the area where that language is widely spoken, and differing in form from the respective endonym(s) in the area where the geographical feature is situated.  -- Description -- SOURCE [UNGEGN Glossary 2007]. "@en ;
          owl:sameAs  <https://inspire.ec.europa.eu/codelist/NativenessValue/exonym>;
          rdfs:isDefinedBy  <https://inspire.ec.europa.eu/codelist/NativenessValue/exonym>;
         rdfs:label "exonym"@no .

### http://inspire.ec.europa.eu/ont:PronunciationOfName
:PronunciationOfName a owl:Class ;
       rdfs:subClassOf :itnrDataType ;
         skos:definition "-- Definition -- Proper, correct or standard (standard within the linguistic community concerned) pronunciation of a name.  -- Description -- SOURCE Adapted from [UNGEGN Manual 2006]. "@en ;
       rdfs:label "PronunciationOfName"@en .

### http://inspire.ec.europa.eu/ont#pronunciationSoundLink
:pronunciationSoundLink rdf:type owl:DatatypeProperty ;
         skos:definition "-- Definition -- Proper, correct or standard (standard within the linguistic community concerned) pronunciation of a name, expressed by a link to any sound file.  -- Description -- SOURCE Adapted from [UNGEGN Manual 2006]. "@en ;
         rdfs:domain :PronunciationOfName;
         rdfs:range xsd:anyURI;
         rdfs:label "pronunciationSoundLink"@en .
:PronunciationOfName rdfs:subClassOf [ rdf:type owl:Restriction ;
         owl:onProperty :pronunciationSoundLink;
         owl:onDataRange xsd:anyURI;
       owl:maxQualifiedCardinality "1"^^xsd:nonNegativeInteger ;
         ] .
:PronunciationOfName rdfs:subClassOf [ rdf:type owl:Restriction ;
         owl:onProperty :pronunciationSoundLink;
         owl:allValuesFrom xsd:anyURI;
         ] .


### http://inspire.ec.europa.eu/ont#pronunciationIPA
:pronunciationIPA rdf:type owl:DatatypeProperty ;
         skos:definition "-- Definition -- Proper, correct or standard (standard within the linguistic community concerned) pronunciation of a name, expressed in International Phonetic Alphabet (IPA).  -- Description -- SOURCE Adapted from [UNGEGN Manual 2006]. "@en ;
         rdfs:domain :PronunciationOfName;
         rdfs:range xsd:string;
         rdfs:label "pronunciationIPA"@en .
:PronunciationOfName rdfs:subClassOf [ rdf:type owl:Restriction ;
         owl:onProperty :pronunciationIPA;
         owl:onDataRange xsd:string;
       owl:maxQualifiedCardinality "1"^^xsd:nonNegativeInteger ;
         ] .
:PronunciationOfName rdfs:subClassOf [ rdf:type owl:Restriction ;
         owl:onProperty :pronunciationIPA;
         owl:allValuesFrom xsd:string;
         ] .


### http://inspire.ec.europa.eu/ont:SpellingOfName
:SpellingOfName a owl:Class ;
       rdfs:subClassOf :itnrDataType ;
         skos:definition "-- Definition -- Proper way of writing a name.  -- Description -- SOURCE Adapted from [UNGEGN Manual 2006].  NOTE Proper spelling means the writing of a name with the correct capitalisation and the correct letters and diacritics present in an accepted standard order.   "@en ;
       rdfs:label "SpellingOfName"@en .

### http://inspire.ec.europa.eu/ont#text
:text rdf:type owl:DatatypeProperty ;
         skos:definition "-- Definition -- Way the name is written."@en ;
         rdfs:domain :SpellingOfName;
         rdfs:range xsd:string;
         rdf:type owl:FunctionalProperty;
         rdfs:label "text"@en .
:SpellingOfName rdfs:subClassOf [ rdf:type owl:Restriction ;
         owl:onProperty :text;
         owl:onDataRange xsd:string;
       owl:qualifiedCardinality "1"^^xsd:nonNegativeInteger ;
         ] .
:SpellingOfName rdfs:subClassOf [ rdf:type owl:Restriction ;
         owl:onProperty :text;
         owl:allValuesFrom xsd:string;
         ] .


### http://inspire.ec.europa.eu/ont#script
:script rdf:type owl:DatatypeProperty ;
         skos:definition "-- Definition -- Set of graphic symbols (for example an alphabet) employed in writing the name, expressed using the four letters codes defined in ISO 15924, where applicable.  -- Description -- SOURCE Adapted from [UNGEGN Glossary 2007].  EXAMPLES Cyrillic, Greek, Roman/Latin scripts.  NOTE 1The four letter codes for Latin (Roman), Cyrillic and Greek script are \"Latn\", \"Cyrl\" and \"Grek\", respectively.  NOTE 2 In rare cases other codes could be used (for other scripts than Latin, Greek and Cyrillic). However, this should mainly apply for historical names in historical scripts.  NOTE 3 This attribute is of first importance in the multi-scriptual context of Europe. "@en ;
         rdfs:domain :SpellingOfName;
         rdfs:range xsd:string;
         rdf:type owl:FunctionalProperty;
         rdfs:label "script"@en .
:SpellingOfName rdfs:subClassOf [ rdf:type owl:Restriction ;
         owl:onProperty :script;
         owl:onDataRange xsd:string;
       owl:qualifiedCardinality "1"^^xsd:nonNegativeInteger ;
         ] .
:SpellingOfName rdfs:subClassOf [ rdf:type owl:Restriction ;
         owl:onProperty :script;
         owl:allValuesFrom xsd:string;
         ] .


### http://inspire.ec.europa.eu/ont#transliterationScheme
:transliterationScheme rdf:type owl:DatatypeProperty ;
         skos:definition "-- Definition -- Method used for the names conversion between different scripts.  -- Description -- SOURCE Adapted from [UNGEGN Glossary 2007].  NOTE 1 This attribute should be filled for any transliterated spellings. If the transliteration scheme used is recorded in codelists maintained by ISO or UN, those codes should be preferred. "@en ;
         rdfs:domain :SpellingOfName;
         rdfs:range xsd:string;
         rdfs:label "transliterationScheme"@en .
:SpellingOfName rdfs:subClassOf [ rdf:type owl:Restriction ;
         owl:onProperty :transliterationScheme;
         owl:onDataRange xsd:string;
       owl:maxQualifiedCardinality "1"^^xsd:nonNegativeInteger ;
         ] .
:SpellingOfName rdfs:subClassOf [ rdf:type owl:Restriction ;
         owl:onProperty :transliterationScheme;
         owl:allValuesFrom xsd:string;
         ] .



### http://inspire.ec.europa.eu/ont:ConnectionTypeValue
:ConnectionTypeValue a owl:Class ;
       rdfs:subClassOf :itnrCodeList ;
          rdfs:isDefinedBy  <https://inspire.ec.europa.eu/codelist/ConnectionTypeValue>;
         skos:definition "-- Definition -- Types of connections between different networks."@en ;
       rdfs:label "ConnectionTypeValue"@en .

### http://inspire.ec.europa.eu/ont:ConnectionTypeValueCode
:ConnectionTypeValueCode a skos:ConceptScheme ;
         skos:definition "-- Definition -- Types of connections between different networks."@en ;
          owl:sameAs  <https://inspire.ec.europa.eu/codelist/ConnectionTypeValue>;
       dc:isFormatOf :ConnectionTypeValue .

### http://inspire.ec.europa.eu/ont:ConnectionTypeValue.crossBorderIdentical
:ConnectionTypeValue.crossBorderIdentical a :ConnectionTypeValue,skos:Concept ;
         skos:inScheme :ConnectionTypeValueCode ;
         skos:definition "-- Definition -- Connection between two network elements in different networks of the same type, but in adjacent areas. The referenced network elements represent the same real-world phenomena."@en ;
          owl:sameAs  <https://inspire.ec.europa.eu/codelist/ConnectionTypeValue/crossBorderIdentical>;
          rdfs:isDefinedBy  <https://inspire.ec.europa.eu/codelist/ConnectionTypeValue/crossBorderIdentical>;
         rdfs:label "crossBorderIdentical"@no .

### http://inspire.ec.europa.eu/ont:ConnectionTypeValue.crossBorderConnected
:ConnectionTypeValue.crossBorderConnected a :ConnectionTypeValue,skos:Concept ;
         skos:inScheme :ConnectionTypeValueCode ;
         skos:definition "-- Definition -- Connection between two network elements in different networks of the same type, but in adjacent areas. The referenced network elements represent the different, but spatially connected real-world phenomena."@en ;
          owl:sameAs  <https://inspire.ec.europa.eu/codelist/ConnectionTypeValue/crossBorderConnected>;
          rdfs:isDefinedBy  <https://inspire.ec.europa.eu/codelist/ConnectionTypeValue/crossBorderConnected>;
         rdfs:label "crossBorderConnected"@no .

### http://inspire.ec.europa.eu/ont:ConnectionTypeValue.intermodal
:ConnectionTypeValue.intermodal a :ConnectionTypeValue,skos:Concept ;
         skos:inScheme :ConnectionTypeValueCode ;
         skos:definition "-- Definition -- Connection between two network elements in different transport networks that use a different transport mode. The connection represents a possibility for the transported media (people, goods, etc) to change from one transport mode to another. "@en ;
          owl:sameAs  <https://inspire.ec.europa.eu/codelist/ConnectionTypeValue/intermodal>;
          rdfs:isDefinedBy  <https://inspire.ec.europa.eu/codelist/ConnectionTypeValue/intermodal>;
         rdfs:label "intermodal"@no .

### http://inspire.ec.europa.eu/ont:CrossReference
:CrossReference a owl:Class ;
       rdfs:subClassOf :itnrFeature ;
          rdfs:isDefinedBy  <http://inspire.ec.europa.eu/featureconcept/CrossReference>;
         skos:definition "-- Definition -- Represents a reference between two elements in the same network.   -- Description -- The cross reference may represent the case where two elements are different representations of the same spatial object. "@en ;
       rdfs:label "CrossReference"@en .

### http://inspire.ec.europa.eu/ont#CrossReference.element
:CrossReference.element rdf:type owl:ObjectProperty ;
         skos:definition "-- Definition -- The cross referenced elements"@en ;
         rdfs:domain :CrossReference;
         rdfs:range :NetworkElement;
         rdfs:label "CrossReference.element"@en .
:CrossReference rdfs:subClassOf [ rdf:type owl:Restriction ;
         owl:onProperty :CrossReference.element;
         owl:onClass :NetworkElement;
       owl:qualifiedCardinality "2"^^xsd:nonNegativeInteger ;
         ] .
:CrossReference rdfs:subClassOf [ rdf:type owl:Restriction ;
         owl:onProperty :CrossReference.element;
         owl:allValuesFrom :NetworkElement;
         ] .


### http://inspire.ec.europa.eu/ont:DirectedLink
:DirectedLink a owl:Class ;
       rdfs:subClassOf :itnrDataType ;
         skos:definition "-- Definition -- A link either in its positive or negative direction. "@en ;
       rdfs:label "DirectedLink"@en .

### http://inspire.ec.europa.eu/ont#DirectedLink.link
:DirectedLink.link rdf:type owl:ObjectProperty ;
         skos:definition "-- Definition -- The link"@en ;
         rdfs:domain :DirectedLink;
         rdfs:range :Link;
         rdf:type owl:FunctionalProperty;
         rdfs:label "DirectedLink.link"@en .
:DirectedLink rdfs:subClassOf [ rdf:type owl:Restriction ;
         owl:onProperty :DirectedLink.link;
         owl:onClass :Link;
       owl:qualifiedCardinality "1"^^xsd:nonNegativeInteger ;
         ] .
:DirectedLink rdfs:subClassOf [ rdf:type owl:Restriction ;
         owl:onProperty :DirectedLink.link;
         owl:allValuesFrom :Link;
         ] .


### http://inspire.ec.europa.eu/ont#DirectedLink.direction
:DirectedLink.direction rdf:type owl:DatatypeProperty ;
         skos:definition "-- Definition -- Indicates if the directed link agrees (positive) or disagrees (negative) with the positive direction of the link. "@en ;
         rdfs:domain :DirectedLink;
         rdfs:range <http://def.isotc211.org/iso19136/2007/BasicTypes#Sign>;
         rdf:type owl:FunctionalProperty;
         rdfs:label "DirectedLink.direction"@en .
:DirectedLink rdfs:subClassOf [ rdf:type owl:Restriction ;
         owl:onProperty :DirectedLink.direction;
         owl:onDataRange <http://def.isotc211.org/iso19136/2007/BasicTypes#Sign>;
       owl:qualifiedCardinality "1"^^xsd:nonNegativeInteger ;
         ] .
:DirectedLink rdfs:subClassOf [ rdf:type owl:Restriction ;
         owl:onProperty :DirectedLink.direction;
         owl:allValuesFrom <http://def.isotc211.org/iso19136/2007/BasicTypes#Sign>;
         ] .


### http://inspire.ec.europa.eu/ont:GeneralisedLink
:GeneralisedLink a owl:Class ;
         skos:definition "-- Definition -- Abstract base type representing a linear network element that may be used as a target in linear referencing. "@en ;
       rdfs:label "GeneralisedLink"@en .
:GeneralisedLink rdfs:subClassOf :NetworkElement .
:GeneralisedLink owl:disjointUnionOf ( :Link :LinkSequence  ) ; .

### http://inspire.ec.europa.eu/ont:GradeSeparatedCrossing
:GradeSeparatedCrossing a owl:Class ;
         skos:definition "-- Definition -- Indicator which of two or more intersecting elements is/are below and which is/are above, to be used if elevation coordinates are not present or cannot be trusted.  -- Description -- NOTE 1 In most cases, the number of elements will be two.  NOTE 2 In the normal case this is when elements intersect in the x/y-plane when the z coordinate is not present or is not accurate enough. "@en ;
       rdfs:label "GradeSeparatedCrossing"@en .

### http://inspire.ec.europa.eu/ont#GradeSeparatedCrossing.element
:GradeSeparatedCrossing.element rdf:type owl:ObjectProperty ;
         skos:definition "-- Definition -- Sequence of crossing links. The order reflects their elevation; the first link is the lower link."@en ;
         rdfs:domain :GradeSeparatedCrossing;
         rdfs:range :Link;
         rdfs:label "GradeSeparatedCrossing.element"@en .
:GradeSeparatedCrossing rdfs:subClassOf [ rdf:type owl:Restriction ;
         owl:onProperty :GradeSeparatedCrossing.element;
         owl:onClass :Link;
       owl:minQualifiedCardinality "2"^^xsd:nonNegativeInteger ;
         ] .
:GradeSeparatedCrossing rdfs:subClassOf [ rdf:type owl:Restriction ;
         owl:onProperty :GradeSeparatedCrossing.element;
         owl:allValuesFrom :Link;
         ] .

:GradeSeparatedCrossing rdfs:subClassOf :NetworkElement .

### http://inspire.ec.europa.eu/ont:Link
:Link a owl:Class ;
         skos:definition "-- Definition -- Curvilinear network element that connects two positions and represents a homogeneous path in the network. The connected positions may be represented as nodes. "@en ;
       rdfs:label "Link"@en .
:Link rdfs:subClassOf :GeneralisedLink .

### http://inspire.ec.europa.eu/ont#endNode
:endNode rdf:type owl:ObjectProperty ;
         skos:definition "-- Definition -- The optional end node for this link. The end node may be the same instance as the start node. "@en ;
         rdfs:domain :Link;
         rdfs:range :Node;
         owl:inverseOf :spokeEnd ;
         rdfs:label "endNode"@en .
:Link rdfs:subClassOf [ rdf:type owl:Restriction ;
         owl:onProperty :endNode;
         owl:onClass :Node;
       owl:maxQualifiedCardinality "1"^^xsd:nonNegativeInteger ;
         ] .
:Link rdfs:subClassOf [ rdf:type owl:Restriction ;
         owl:onProperty :endNode;
         owl:allValuesFrom :Node;
         ] .


### http://inspire.ec.europa.eu/ont#startNode
:startNode rdf:type owl:ObjectProperty ;
         skos:definition "-- Definition -- The optional start node for this link."@en ;
         rdfs:domain :Link;
         rdfs:range :Node;
         owl:inverseOf :spokeStart ;
         rdfs:label "startNode"@en .
:Link rdfs:subClassOf [ rdf:type owl:Restriction ;
         owl:onProperty :startNode;
         owl:onClass :Node;
       owl:maxQualifiedCardinality "1"^^xsd:nonNegativeInteger ;
         ] .
:Link rdfs:subClassOf [ rdf:type owl:Restriction ;
         owl:onProperty :startNode;
         owl:allValuesFrom :Node;
         ] .


### http://inspire.ec.europa.eu/ont#centrelineGeometry
:centrelineGeometry rdf:type owl:ObjectProperty ;
         skos:definition "-- Definition -- The geometry that represents the centreline of the link. "@en ;
         rdfs:domain :Link;
         rdfs:range <http://www.opengis.net/ont/sf#Curve>;
         rdf:type owl:FunctionalProperty;
         rdfs:label "centrelineGeometry"@en .
:Link rdfs:subClassOf [ rdf:type owl:Restriction ;
         owl:onProperty :centrelineGeometry;
         owl:onClass <http://www.opengis.net/ont/sf#Curve>;
       owl:qualifiedCardinality "1"^^xsd:nonNegativeInteger ;
         ] .
:Link rdfs:subClassOf [ rdf:type owl:Restriction ;
         owl:onProperty :centrelineGeometry;
         owl:allValuesFrom <http://www.opengis.net/ont/sf#Curve>;
         ] .


### http://inspire.ec.europa.eu/ont#fictitious
:fictitious rdf:type owl:DatatypeProperty ;
         skos:definition "-- Definition -- Indicator that the centreline geometry of the link is a straight line with no intermediate control points &ndash; unless the straight line represents the geography in the resolution of the data set appropriately. "@en ;
         rdfs:domain :Link;
         rdfs:range xsd:boolean;
         rdf:type owl:FunctionalProperty;
         rdfs:label "fictitious"@en .
:Link rdfs:subClassOf [ rdf:type owl:Restriction ;
         owl:onProperty :fictitious;
         owl:onDataRange xsd:boolean;
       owl:qualifiedCardinality "1"^^xsd:nonNegativeInteger ;
         ] .
:Link rdfs:subClassOf [ rdf:type owl:Restriction ;
         owl:onProperty :fictitious;
         owl:allValuesFrom xsd:boolean;
         ] .

:Link owl:disjointUnionOf ( :TransportLink  ) ; .

### http://inspire.ec.europa.eu/ont:LinkDirectionValue
:LinkDirectionValue a owl:Class ;
       rdfs:subClassOf :itnrCodeList ;
          rdfs:isDefinedBy  <https://inspire.ec.europa.eu/codelist/LinkDirectionValue>;
         skos:definition "-- Definition -- List of values for directions relative to a link"@en ;
       rdfs:label "LinkDirectionValue"@en .

### http://inspire.ec.europa.eu/ont:LinkDirectionValueCode
:LinkDirectionValueCode a skos:ConceptScheme ;
         skos:definition "-- Definition -- List of values for directions relative to a link"@en ;
          owl:sameAs  <https://inspire.ec.europa.eu/codelist/LinkDirectionValue>;
       dc:isFormatOf :LinkDirectionValue .

### http://inspire.ec.europa.eu/ont:LinkDirectionValue.bothDirections
:LinkDirectionValue.bothDirections a :LinkDirectionValue,skos:Concept ;
         skos:inScheme :LinkDirectionValueCode ;
         skos:definition "-- Definition -- In both directions. "@en ;
          owl:sameAs  <https://inspire.ec.europa.eu/codelist/LinkDirectionValue/bothDirections>;
          rdfs:isDefinedBy  <https://inspire.ec.europa.eu/codelist/LinkDirectionValue/bothDirections>;
         rdfs:label "bothDirections"@no .

### http://inspire.ec.europa.eu/ont:LinkDirectionValue.inDirection
:LinkDirectionValue.inDirection a :LinkDirectionValue,skos:Concept ;
         skos:inScheme :LinkDirectionValueCode ;
         skos:definition "-- Definition -- In direction of the link. "@en ;
          owl:sameAs  <https://inspire.ec.europa.eu/codelist/LinkDirectionValue/inDirection>;
          rdfs:isDefinedBy  <https://inspire.ec.europa.eu/codelist/LinkDirectionValue/inDirection>;
         rdfs:label "inDirection"@no .

### http://inspire.ec.europa.eu/ont:LinkDirectionValue.inOppositeDirection
:LinkDirectionValue.inOppositeDirection a :LinkDirectionValue,skos:Concept ;
         skos:inScheme :LinkDirectionValueCode ;
         skos:definition "-- Definition -- In the opposite direction of the link. "@en ;
          owl:sameAs  <https://inspire.ec.europa.eu/codelist/LinkDirectionValue/inOppositeDirection>;
          rdfs:isDefinedBy  <https://inspire.ec.europa.eu/codelist/LinkDirectionValue/inOppositeDirection>;
         rdfs:label "inOppositeDirection"@no .

### http://inspire.ec.europa.eu/ont:LinkReference
:LinkReference a owl:Class ;
         skos:definition "-- Definition -- A network reference to a linear network element. "@en ;
       rdfs:label "LinkReference"@en .
:LinkReference rdfs:subClassOf :NetworkReference .

### http://inspire.ec.europa.eu/ont#applicableDirection
:applicableDirection rdf:type owl:ObjectProperty ;
         skos:definition "-- Definition -- The directions of the generalised link to which the reference applies.  In cases where a property does not apply <i>to</i> a direction along a link, but represents a phenomenon <i>along</i> a link, &ldquo;inDirection&rdquo; refers to the right side in the direction of the link.  -- Description -- EXAMPLE A speed limit is a property that applies to a direction of the link (or both directions) while a house number is a phenomenon along a link. "@en ;
         rdfs:domain :LinkReference;
         rdfs:range :LinkDirectionValue;
         rdf:type owl:FunctionalProperty;
         rdfs:label "applicableDirection"@en .
:LinkReference rdfs:subClassOf [ rdf:type owl:Restriction ;
         owl:onProperty :applicableDirection;
         owl:onClass :LinkDirectionValue;
       owl:qualifiedCardinality "1"^^xsd:nonNegativeInteger ;
         ] .
:LinkReference rdfs:subClassOf [ rdf:type owl:Restriction ;
         owl:onProperty :applicableDirection;
         owl:allValuesFrom :LinkDirectionValue;
         ] .

:LinkReference owl:disjointUnionOf ( :SimpleLinearReference :SimplePointReference  ) ; .

### http://inspire.ec.europa.eu/ont:LinkSequence
:LinkSequence a owl:Class ;
         skos:definition "-- Definition -- A network element which represents a continuous path in the network without any branches. The element has a defined beginning and end and every position on the link sequence is identifiable with one single parameter such as length.   -- Description -- EXAMPLE A link sequence may represent a route.  "@en ;
       rdfs:label "LinkSequence"@en .
:LinkSequence rdfs:subClassOf :GeneralisedLink .

### http://inspire.ec.europa.eu/ont#LinkSequence.link
:LinkSequence.link rdf:type owl:ObjectProperty ;
         skos:definition "-- Definition -- The ordered collection of directed links that constitute the link sequence. "@en ;
         rdfs:domain :LinkSequence;
         rdfs:range :DirectedLink;
         rdfs:label "LinkSequence.link"@en .
:LinkSequence rdfs:subClassOf [ rdf:type owl:Restriction ;
         owl:onProperty :LinkSequence.link;
         owl:onClass :DirectedLink;
       owl:minQualifiedCardinality "1"^^xsd:nonNegativeInteger ;
         ] .
:LinkSequence rdfs:subClassOf [ rdf:type owl:Restriction ;
         owl:onProperty :LinkSequence.link;
         owl:allValuesFrom :DirectedLink;
         ] .

:LinkSequence owl:disjointUnionOf ( :TransportLinkSequence  ) ; .

### http://inspire.ec.europa.eu/ont:LinkSet
:LinkSet a owl:Class ;
         skos:definition "-- Definition -- A collection of link sequences and/or individual links that has a specific function or significance in a network.   -- Description -- NOTE This spatial object type supports the aggregation of links to form objects with branches, loops, parallel sequences of links, gaps, etc.  EXAMPLE A dual carriageway road, as a collection of the two link sequences that represent each carriageway.  "@en ;
       rdfs:label "LinkSet"@en .
:LinkSet rdfs:subClassOf :NetworkElement .

### http://inspire.ec.europa.eu/ont#LinkSet.link
:LinkSet.link rdf:type owl:ObjectProperty ;
         skos:definition "-- Definition -- The set of links and link sequences that constitute the link set."@en ;
         rdfs:domain :LinkSet;
         rdfs:range :GeneralisedLink;
         rdfs:label "LinkSet.link"@en .
:LinkSet rdfs:subClassOf [ rdf:type owl:Restriction ;
         owl:onProperty :LinkSet.link;
         owl:onClass :GeneralisedLink;
       owl:minQualifiedCardinality "1"^^xsd:nonNegativeInteger ;
         ] .
:LinkSet rdfs:subClassOf [ rdf:type owl:Restriction ;
         owl:onProperty :LinkSet.link;
         owl:allValuesFrom :GeneralisedLink;
         ] .

:LinkSet owl:disjointUnionOf ( :TransportLinkSet  ) ; .

### http://inspire.ec.europa.eu/ont:Network
:Network a owl:Class ;
       rdfs:subClassOf :itnrFeature ;
          rdfs:isDefinedBy  <http://inspire.ec.europa.eu/featureconcept/Network>;
         skos:definition "-- Definition -- A network is a collection of network elements.  -- Description -- The reason for collecting certain elements in a certain network may vary (e.g. connected elements for the same mode of transport) "@en ;
       rdfs:label "Network"@en .

### http://inspire.ec.europa.eu/ont#elements
:elements rdf:type owl:ObjectProperty ;
         skos:definition "-- Definition -- The collection of elements that constitutes the network. "@en ;
         rdfs:domain :Network;
         rdfs:range :NetworkElement;
         owl:inverseOf :inNetwork ;
         rdfs:label "elements"@en .
:Network rdfs:subClassOf [ rdf:type owl:Restriction ;
         owl:onProperty :elements;
         owl:allValuesFrom :NetworkElement;
         ] .


### http://inspire.ec.europa.eu/ont#geographicalName
:geographicalName rdf:type owl:ObjectProperty ;
         skos:definition "-- Definition -- Geographical name for this spatial object. "@en ;
         rdfs:range :GeographicalName;
         rdfs:label "geographicalName"@en .
:Network rdfs:subClassOf [ rdf:type owl:Restriction ;
         owl:onProperty :geographicalName;
         owl:allValuesFrom :GeographicalName;
         ] .

:Network owl:disjointUnionOf ( :TransportNetwork  ) ; .

### http://inspire.ec.europa.eu/ont:NetworkArea
:NetworkArea a owl:Class ;
         skos:definition "-- Definition -- A 2-dimensional element in a network.  "@en ;
       rdfs:label "NetworkArea"@en .
:NetworkArea rdfs:subClassOf :NetworkElement .

### http://inspire.ec.europa.eu/ont#geometry
:geometry rdf:type owl:ObjectProperty ;
         skos:definition "-- Definition -- Represents the geometric properties of the spatial object"@en ;
         rdfs:label "geometry"@en .
:NetworkArea rdfs:subClassOf [ rdf:type owl:Restriction ;
         owl:onProperty :geometry;
         owl:onClass <http://www.opengis.net/ont/sf#Surface>;
       owl:qualifiedCardinality "1"^^xsd:nonNegativeInteger ;
         ] .
:NetworkArea rdfs:subClassOf [ rdf:type owl:Restriction ;
         owl:onProperty :geometry;
         owl:allValuesFrom <http://www.opengis.net/ont/sf#Surface>;
         ] .

:NetworkArea owl:disjointUnionOf ( :TransportArea  ) ; .

### http://inspire.ec.europa.eu/ont:NetworkConnection
:NetworkConnection a owl:Class ;
         skos:definition "-- Definition -- Represents a logical connection between two or more network elements in different networks.  -- Description -- In the case where the networks are in different spatial data sets, a network connection object may exist in both data sets. "@en ;
       rdfs:label "NetworkConnection"@en .
:NetworkConnection rdfs:subClassOf :NetworkElement .

### http://inspire.ec.europa.eu/ont#NetworkConnection.element
:NetworkConnection.element rdf:type owl:ObjectProperty ;
         skos:definition "-- Definition -- Network elements in different networks "@en ;
         rdfs:domain :NetworkConnection;
         rdfs:label "NetworkConnection.element"@en .
:NetworkConnection rdfs:subClassOf [ rdf:type owl:Restriction ;
         owl:onProperty :NetworkConnection.element;
         owl:onClass :NetworkElement;
       owl:minQualifiedCardinality "2"^^xsd:nonNegativeInteger ;
         ] .
:NetworkConnection rdfs:subClassOf [ rdf:type owl:Restriction ;
         owl:onProperty :NetworkConnection.element;
         owl:allValuesFrom :NetworkElement;
         ] .


### http://inspire.ec.europa.eu/ont#NetworkConnection.type
:NetworkConnection.type rdf:type owl:ObjectProperty ;
         skos:definition "-- Definition -- Categorisation of the network connection."@en ;
         rdfs:domain :NetworkConnection;
         rdf:type owl:FunctionalProperty;
         rdfs:label "NetworkConnection.type"@en .
:NetworkConnection rdfs:subClassOf [ rdf:type owl:Restriction ;
         owl:onProperty :NetworkConnection.type;
         owl:onClass :ConnectionTypeValue;
       owl:qualifiedCardinality "1"^^xsd:nonNegativeInteger ;
         ] .
:NetworkConnection rdfs:subClassOf [ rdf:type owl:Restriction ;
         owl:onProperty :NetworkConnection.type;
         owl:allValuesFrom :ConnectionTypeValue;
         ] .


### http://inspire.ec.europa.eu/ont:NetworkElement
:NetworkElement a owl:Class ;
       rdfs:subClassOf :itnrFeature ;
          rdfs:isDefinedBy  <http://inspire.ec.europa.eu/featureconcept/NetworkElement>;
         skos:definition "-- Definition -- Abstract base type representing an element in a network. Every element in a network provides some function that is of interest in the network. "@en ;
       rdfs:label "NetworkElement"@en .

### http://inspire.ec.europa.eu/ont#inNetwork
:inNetwork rdf:type owl:ObjectProperty ;
         skos:definition "-- Definition -- The networks in which a network element is a member."@en ;
         rdfs:domain :NetworkElement;
         rdfs:range :Network;
         owl:inverseOf :elements ;
         rdfs:label "inNetwork"@en .
:NetworkElement rdfs:subClassOf [ rdf:type owl:Restriction ;
         owl:onProperty :inNetwork;
         owl:onClass :Network;
       owl:minQualifiedCardinality "1"^^xsd:nonNegativeInteger ;
         ] .
:NetworkElement rdfs:subClassOf [ rdf:type owl:Restriction ;
         owl:onProperty :inNetwork;
         owl:allValuesFrom :Network;
         ] .

:NetworkElement rdfs:subClassOf [ rdf:type owl:Restriction ;
         owl:onProperty :beginLifespanVersion;
         owl:onDataRange xsd:dateTime;
       owl:qualifiedCardinality "1"^^xsd:nonNegativeInteger ;
         ] .
:NetworkElement rdfs:subClassOf [ rdf:type owl:Restriction ;
         owl:onProperty :beginLifespanVersion;
         owl:allValuesFrom xsd:dateTime;
         ] .

:NetworkElement rdfs:subClassOf [ rdf:type owl:Restriction ;
         owl:onProperty :inspireId;
         owl:onClass :Identifier;
       owl:maxQualifiedCardinality "1"^^xsd:nonNegativeInteger ;
         ] .
:NetworkElement rdfs:subClassOf [ rdf:type owl:Restriction ;
         owl:onProperty :inspireId;
         owl:allValuesFrom :Identifier;
         ] .

:NetworkElement rdfs:subClassOf [ rdf:type owl:Restriction ;
         owl:onProperty :endLifespanVersion;
         owl:onDataRange xsd:dateTime;
       owl:maxQualifiedCardinality "1"^^xsd:nonNegativeInteger ;
         ] .
:NetworkElement rdfs:subClassOf [ rdf:type owl:Restriction ;
         owl:onProperty :endLifespanVersion;
         owl:allValuesFrom xsd:dateTime;
         ] .

:NetworkElement owl:disjointUnionOf ( :LinkSet :GradeSeparatedCrossing :GeneralisedLink :NetworkConnection :NetworkArea :Node :TransportPoint  ) ; .

### http://inspire.ec.europa.eu/ont:NetworkProperty
:NetworkProperty a owl:Class ;
       rdfs:subClassOf :itnrFeature ;
          rdfs:isDefinedBy  <http://inspire.ec.europa.eu/featureconcept/NetworkProperty>;
         skos:definition "-- Definition -- Abstract base type representing phenomena located at or along a network element. This base type provides general properties to associate the network-related phenomena (network properties) with the network elements.  -- Description -- In the simplest case (NetworkReference), the network property applies to the whole network element. In the case of a Link, the spatial reference may be restricted to part of the Link by using a linear reference. ISO/TC 211 is currently in the early stages of developing a standard for Linear Referencing (ISO 19148). A simple mechanism to express linear references is provided in this version of the network model; it is expected that the model will be extended once ISO 19148 is stable. The current simple model requires for all linear references two expressions representing a distance from the start of the Link along its curve geometry. The network property applies to the part of the Link between fromPosition and toPosition. "@en ;
       rdfs:label "NetworkProperty"@en .

### http://inspire.ec.europa.eu/ont#networkRef
:networkRef rdf:type owl:ObjectProperty ;
         skos:definition "-- Definition -- Spatial reference of the network-related property.  -- Description -- This attribute provides an indirect spatial reference based on a reference to an element of an underlying network. See the chapter on Object Referencing in the Generic Conceptual Model for a discussion on modelling object references. "@en ;
         rdfs:domain :NetworkProperty;
         rdfs:range :NetworkReference;
         rdfs:label "networkRef"@en .
:NetworkProperty rdfs:subClassOf [ rdf:type owl:Restriction ;
         owl:onProperty :networkRef;
         owl:onClass :NetworkReference;
       owl:minQualifiedCardinality "1"^^xsd:nonNegativeInteger ;
         ] .
:NetworkProperty rdfs:subClassOf [ rdf:type owl:Restriction ;
         owl:onProperty :networkRef;
         owl:allValuesFrom :NetworkReference;
         ] .

:NetworkProperty rdfs:subClassOf [ rdf:type owl:Restriction ;
         owl:onProperty :inspireId;
         owl:onClass :Identifier;
       owl:maxQualifiedCardinality "1"^^xsd:nonNegativeInteger ;
         ] .
:NetworkProperty rdfs:subClassOf [ rdf:type owl:Restriction ;
         owl:onProperty :inspireId;
         owl:allValuesFrom :Identifier;
         ] .

:NetworkProperty rdfs:subClassOf [ rdf:type owl:Restriction ;
         owl:onProperty :beginLifespanVersion;
         owl:onDataRange xsd:dateTime;
       owl:qualifiedCardinality "1"^^xsd:nonNegativeInteger ;
         ] .
:NetworkProperty rdfs:subClassOf [ rdf:type owl:Restriction ;
         owl:onProperty :beginLifespanVersion;
         owl:allValuesFrom xsd:dateTime;
         ] .

:NetworkProperty rdfs:subClassOf [ rdf:type owl:Restriction ;
         owl:onProperty :endLifespanVersion;
         owl:onDataRange xsd:dateTime;
       owl:maxQualifiedCardinality "1"^^xsd:nonNegativeInteger ;
         ] .
:NetworkProperty rdfs:subClassOf [ rdf:type owl:Restriction ;
         owl:onProperty :endLifespanVersion;
         owl:allValuesFrom xsd:dateTime;
         ] .

:NetworkProperty owl:disjointUnionOf ( :TransportProperty  ) ; .

### http://inspire.ec.europa.eu/ont:NetworkReference
:NetworkReference a owl:Class ;
       rdfs:subClassOf :itnrDataType ;
         skos:definition "-- Definition -- A reference to a network element. "@en ;
       rdfs:label "NetworkReference"@en .

### http://inspire.ec.europa.eu/ont#NetworkReference.element
:NetworkReference.element rdf:type owl:ObjectProperty ;
         skos:definition "-- Definition -- The referenced network element."@en ;
         rdfs:domain :NetworkReference;
         rdfs:range :NetworkElement;
         rdf:type owl:FunctionalProperty;
         rdfs:label "NetworkReference.element"@en .
:NetworkReference rdfs:subClassOf [ rdf:type owl:Restriction ;
         owl:onProperty :NetworkReference.element;
         owl:onClass :NetworkElement;
       owl:qualifiedCardinality "1"^^xsd:nonNegativeInteger ;
         ] .
:NetworkReference rdfs:subClassOf [ rdf:type owl:Restriction ;
         owl:onProperty :NetworkReference.element;
         owl:allValuesFrom :NetworkElement;
         ] .

:NetworkReference owl:disjointUnionOf ( :LinkReference  ) ; .

### http://inspire.ec.europa.eu/ont:Node
:Node a owl:Class ;
         skos:definition "-- Definition -- Represents a significant position in the network that always occurs at the beginning or the end of a link.  -- Description -- NOTE if a topological representation of the network is used the road node is either a topological connection between two or more links or the termination of a ink. If a geometric representation of the network is used road nodes are represented by points or alternatively another geometric shape. [EuroRoadS] "@en ;
       rdfs:label "Node"@en .

### http://inspire.ec.europa.eu/ont#spokeEnd
:spokeEnd rdf:type owl:ObjectProperty ;
         skos:definition "-- Definition -- The links that enter the node.  -- Description -- NOTE In the INSPIRE context, this spoke property is to be published when this information is published in current exchange formats of the data set."@en ;
         rdfs:domain :Node;
         rdfs:range :Link;
         owl:inverseOf :endNode ;
         rdfs:label "spokeEnd"@en .
:Node rdfs:subClassOf [ rdf:type owl:Restriction ;
         owl:onProperty :spokeEnd;
         owl:allValuesFrom :Link;
         ] .


### http://inspire.ec.europa.eu/ont#spokeStart
:spokeStart rdf:type owl:ObjectProperty ;
         skos:definition "-- Definition -- The links that leave the node.  -- Description -- NOTE In the INSPIRE context, this spoke property is to be published when this information is published in current exchange formats of the data set."@en ;
         rdfs:domain :Node;
         rdfs:range :Link;
         owl:inverseOf :startNode ;
         rdfs:label "spokeStart"@en .
:Node rdfs:subClassOf [ rdf:type owl:Restriction ;
         owl:onProperty :spokeStart;
         owl:allValuesFrom :Link;
         ] .

:Node rdfs:subClassOf :NetworkElement .
:Node rdfs:subClassOf [ rdf:type owl:Restriction ;
         owl:onProperty :geometry;
         owl:onClass <http://www.opengis.net/ont/sf#Point>;
       owl:qualifiedCardinality "1"^^xsd:nonNegativeInteger ;
         ] .
:Node rdfs:subClassOf [ rdf:type owl:Restriction ;
         owl:onProperty :geometry;
         owl:allValuesFrom <http://www.opengis.net/ont/sf#Point>;
         ] .

:Node owl:disjointUnionOf ( :TransportNode  ) ; .

### http://inspire.ec.europa.eu/ont:SimpleLinearReference
:SimpleLinearReference a owl:Class ;
         skos:definition "-- Definition -- A network reference that is restricted to part of a linear network element. The part is the part of the network element between fromPosition and toPosition. "@en ;
       rdfs:label "SimpleLinearReference"@en .
:SimpleLinearReference rdfs:subClassOf :LinkReference .

### http://inspire.ec.europa.eu/ont#fromPosition
:fromPosition rdf:type owl:ObjectProperty ;
         skos:definition "-- Definition -- The start position of the linear element, expressed as the distance from the start of the linear network element along its curve geometry. "@en ;
         rdfs:domain :SimpleLinearReference;
         rdfs:range <http://def.isotc211.org/iso19103/2015/MeasureTypes#Length>;
         rdf:type owl:FunctionalProperty;
         rdfs:label "fromPosition"@en .
:SimpleLinearReference rdfs:subClassOf [ rdf:type owl:Restriction ;
         owl:onProperty :fromPosition;
         owl:onClass <http://def.isotc211.org/iso19103/2015/MeasureTypes#Length>;
       owl:qualifiedCardinality "1"^^xsd:nonNegativeInteger ;
         ] .
:SimpleLinearReference rdfs:subClassOf [ rdf:type owl:Restriction ;
         owl:onProperty :fromPosition;
         owl:allValuesFrom <http://def.isotc211.org/iso19103/2015/MeasureTypes#Length>;
         ] .


### http://inspire.ec.europa.eu/ont#toPosition
:toPosition rdf:type owl:ObjectProperty ;
         skos:definition "-- Definition -- The end position of the linear element, expressed as the distance from the start of the linear network element along its curve geometry. "@en ;
         rdfs:domain :SimpleLinearReference;
         rdfs:range <http://def.isotc211.org/iso19103/2015/MeasureTypes#Length>;
         rdf:type owl:FunctionalProperty;
         rdfs:label "toPosition"@en .
:SimpleLinearReference rdfs:subClassOf [ rdf:type owl:Restriction ;
         owl:onProperty :toPosition;
         owl:onClass <http://def.isotc211.org/iso19103/2015/MeasureTypes#Length>;
       owl:qualifiedCardinality "1"^^xsd:nonNegativeInteger ;
         ] .
:SimpleLinearReference rdfs:subClassOf [ rdf:type owl:Restriction ;
         owl:onProperty :toPosition;
         owl:allValuesFrom <http://def.isotc211.org/iso19103/2015/MeasureTypes#Length>;
         ] .


### http://inspire.ec.europa.eu/ont#offset
:offset rdf:type owl:ObjectProperty ;
         skos:definition "-- Definition -- An offset from the centerline geometry of the generalised link, where applicable; a positive offset is to the right in the direction of the link, a negative offset is to the left. "@en ;
         rdfs:range <http://def.isotc211.org/iso19103/2015/MeasureTypes#Length>;
         rdfs:label "offset"@en .
:SimpleLinearReference rdfs:subClassOf [ rdf:type owl:Restriction ;
         owl:onProperty :offset;
         owl:onClass <http://def.isotc211.org/iso19103/2015/MeasureTypes#Length>;
       owl:maxQualifiedCardinality "1"^^xsd:nonNegativeInteger ;
         ] .
:SimpleLinearReference rdfs:subClassOf [ rdf:type owl:Restriction ;
         owl:onProperty :offset;
         owl:allValuesFrom <http://def.isotc211.org/iso19103/2015/MeasureTypes#Length>;
         ] .


### http://inspire.ec.europa.eu/ont:SimplePointReference
:SimplePointReference a owl:Class ;
         skos:definition "-- Definition -- A network reference that is restricted to a point on a linear network element. The point is the location on the network element at the position atPosition along the network.  "@en ;
       rdfs:label "SimplePointReference"@en .
:SimplePointReference rdfs:subClassOf :LinkReference .

### http://inspire.ec.europa.eu/ont#atPosition
:atPosition rdf:type owl:ObjectProperty ;
         skos:definition "-- Definition -- Position of the point, expressed as the distance from the start of the linear network element along its curve geometry. "@en ;
         rdfs:domain :SimplePointReference;
         rdfs:range <http://def.isotc211.org/iso19103/2015/MeasureTypes#Length>;
         rdf:type owl:FunctionalProperty;
         rdfs:label "atPosition"@en .
:SimplePointReference rdfs:subClassOf [ rdf:type owl:Restriction ;
         owl:onProperty :atPosition;
         owl:onClass <http://def.isotc211.org/iso19103/2015/MeasureTypes#Length>;
       owl:qualifiedCardinality "1"^^xsd:nonNegativeInteger ;
         ] .
:SimplePointReference rdfs:subClassOf [ rdf:type owl:Restriction ;
         owl:onProperty :atPosition;
         owl:allValuesFrom <http://def.isotc211.org/iso19103/2015/MeasureTypes#Length>;
         ] .

:SimplePointReference rdfs:subClassOf [ rdf:type owl:Restriction ;
         owl:onProperty :offset;
         owl:onClass <http://def.isotc211.org/iso19103/2015/MeasureTypes#Length>;
       owl:maxQualifiedCardinality "1"^^xsd:nonNegativeInteger ;
         ] .
:SimplePointReference rdfs:subClassOf [ rdf:type owl:Restriction ;
         owl:onProperty :offset;
         owl:allValuesFrom <http://def.isotc211.org/iso19103/2015/MeasureTypes#Length>;
         ] .



### http://inspire.ec.europa.eu/ont:AccessRestriction
:AccessRestriction a owl:Class ;
         skos:definition "-- Definition -- A restriction on the access to a transport element."@en ;
       rdfs:label "AccessRestriction"@en .
:AccessRestriction rdfs:subClassOf :TransportProperty .

### http://inspire.ec.europa.eu/ont#restriction
:restriction rdf:type owl:ObjectProperty ;
         skos:definition "-- Definition -- Nature of the access restriction."@en ;
         rdfs:domain :AccessRestriction;
         rdfs:range :AccessRestrictionValue;
         rdf:type owl:FunctionalProperty;
         rdfs:label "restriction"@en .
:AccessRestriction rdfs:subClassOf [ rdf:type owl:Restriction ;
         owl:onProperty :restriction;
         owl:onClass :AccessRestrictionValue;
       owl:qualifiedCardinality "1"^^xsd:nonNegativeInteger ;
         ] .
:AccessRestriction rdfs:subClassOf [ rdf:type owl:Restriction ;
         owl:onProperty :restriction;
         owl:allValuesFrom :AccessRestrictionValue;
         ] .


### http://inspire.ec.europa.eu/ont:ConditionOfFacility
:ConditionOfFacility a owl:Class ;
         skos:definition "-- Definition -- State of a transport network element with regards to its completion and use."@en ;
       rdfs:label "ConditionOfFacility"@en .
:ConditionOfFacility rdfs:subClassOf :TransportProperty .

### http://inspire.ec.europa.eu/ont#currentStatus
:currentStatus rdf:type owl:ObjectProperty ;
         skos:definition "-- Definition -- Current status value of a transport network element with regards to its completion and use."@en ;
         rdfs:domain :ConditionOfFacility;
         rdfs:range :ConditionOfFacilityValue;
         rdf:type owl:FunctionalProperty;
         rdfs:label "currentStatus"@en .
:ConditionOfFacility rdfs:subClassOf [ rdf:type owl:Restriction ;
         owl:onProperty :currentStatus;
         owl:onClass :ConditionOfFacilityValue;
       owl:qualifiedCardinality "1"^^xsd:nonNegativeInteger ;
         ] .
:ConditionOfFacility rdfs:subClassOf [ rdf:type owl:Restriction ;
         owl:onProperty :currentStatus;
         owl:allValuesFrom :ConditionOfFacilityValue;
         ] .


### http://inspire.ec.europa.eu/ont:MaintenanceAuthority
:MaintenanceAuthority a owl:Class ;
         skos:definition "-- Definition -- The authority responsible for maintenance of the transport element."@en ;
       rdfs:label "MaintenanceAuthority"@en .
:MaintenanceAuthority rdfs:subClassOf :TransportProperty .

### http://inspire.ec.europa.eu/ont#authority
:authority rdf:type owl:ObjectProperty ;
         skos:definition "-- Definition -- Identification of the authority."@en ;
         rdfs:range <http://def.isotc211.org/iso19115/2003/CitationAndResponsiblePartyInformation#CI_Citation>;
         rdfs:label "authority"@en .
:MaintenanceAuthority rdfs:subClassOf [ rdf:type owl:Restriction ;
         owl:onProperty :authority;
         owl:onClass <http://def.isotc211.org/iso19115/2003/CitationAndResponsiblePartyInformation#CI_Citation>;
       owl:qualifiedCardinality "1"^^xsd:nonNegativeInteger ;
         ] .
:MaintenanceAuthority rdfs:subClassOf [ rdf:type owl:Restriction ;
         owl:onProperty :authority;
         owl:allValuesFrom <http://def.isotc211.org/iso19115/2003/CitationAndResponsiblePartyInformation#CI_Citation>;
         ] .


### http://inspire.ec.europa.eu/ont:MarkerPost
:MarkerPost a owl:Class ;
         skos:definition "-- Definition -- Reference marker placed along a route in a transport network, mostly at regular intervals, indicating the distance from the beginning of the route, or some other reference point, to the point where the marker is located.  -- Description -- EXAMPLE Examples of routes along which marker posts can be found are roads, railway lines and navigable waterways. "@en ;
       rdfs:label "MarkerPost"@en .
:MarkerPost rdfs:subClassOf :TransportPoint .

### http://inspire.ec.europa.eu/ont#route
:route rdf:type owl:ObjectProperty ;
         skos:definition "-- Definition -- Route in a transport network along which the marker post is placed."@en ;
         rdfs:domain :MarkerPost;
         rdfs:range :TransportLinkSet;
         rdf:type owl:FunctionalProperty;
         owl:inverseOf :post ;
         rdfs:label "route"@en .
:MarkerPost rdfs:subClassOf [ rdf:type owl:Restriction ;
         owl:onProperty :route;
         owl:onClass :TransportLinkSet;
       owl:qualifiedCardinality "1"^^xsd:nonNegativeInteger ;
         ] .
:MarkerPost rdfs:subClassOf [ rdf:type owl:Restriction ;
         owl:onProperty :route;
         owl:allValuesFrom :TransportLinkSet;
         ] .


### http://inspire.ec.europa.eu/ont#location
:location rdf:type owl:ObjectProperty ;
         skos:definition "-- Definition -- Distance from the beginning of the route, or some other reference point, to the point where a marker post is located."@en ;
         rdfs:domain :MarkerPost;
         rdfs:range <http://def.isotc211.org/iso19103/2015/MeasureTypes#Distance>;
         rdf:type owl:FunctionalProperty;
         rdfs:label "location"@en .
:MarkerPost rdfs:subClassOf [ rdf:type owl:Restriction ;
         owl:onProperty :location;
         owl:onClass <http://def.isotc211.org/iso19103/2015/MeasureTypes#Distance>;
       owl:qualifiedCardinality "1"^^xsd:nonNegativeInteger ;
         ] .
:MarkerPost rdfs:subClassOf [ rdf:type owl:Restriction ;
         owl:onProperty :location;
         owl:allValuesFrom <http://def.isotc211.org/iso19103/2015/MeasureTypes#Distance>;
         ] .


### http://inspire.ec.europa.eu/ont:OwnerAuthority
:OwnerAuthority a owl:Class ;
         skos:definition "-- Definition -- The authority owning the transport element."@en ;
       rdfs:label "OwnerAuthority"@en .
:OwnerAuthority rdfs:subClassOf :TransportProperty .
:OwnerAuthority rdfs:subClassOf [ rdf:type owl:Restriction ;
         owl:onProperty :authority;
         owl:onClass <http://def.isotc211.org/iso19115/2003/CitationAndResponsiblePartyInformation#CI_Citation>;
       owl:qualifiedCardinality "1"^^xsd:nonNegativeInteger ;
         ] .
:OwnerAuthority rdfs:subClassOf [ rdf:type owl:Restriction ;
         owl:onProperty :authority;
         owl:allValuesFrom <http://def.isotc211.org/iso19115/2003/CitationAndResponsiblePartyInformation#CI_Citation>;
         ] .


### http://inspire.ec.europa.eu/ont:RestrictionForVehicles
:RestrictionForVehicles a owl:Class ;
         skos:definition "-- Definition -- Restriction on vehicles on a transport element."@en ;
       rdfs:label "RestrictionForVehicles"@en .
:RestrictionForVehicles rdfs:subClassOf :TransportProperty .

### http://inspire.ec.europa.eu/ont#measure
:measure rdf:type owl:ObjectProperty ;
         skos:definition "-- Definition -- The measure for the restriction .  -- Description -- SOURCE [Euroroads]. "@en ;
         rdfs:domain :RestrictionForVehicles;
         rdfs:range <http://def.isotc211.org/iso19103/2015/MeasureTypes#Measure>;
         rdf:type owl:FunctionalProperty;
         rdfs:label "measure"@en .
:RestrictionForVehicles rdfs:subClassOf [ rdf:type owl:Restriction ;
         owl:onProperty :measure;
         owl:onClass <http://def.isotc211.org/iso19103/2015/MeasureTypes#Measure>;
       owl:qualifiedCardinality "1"^^xsd:nonNegativeInteger ;
         ] .
:RestrictionForVehicles rdfs:subClassOf [ rdf:type owl:Restriction ;
         owl:onProperty :measure;
         owl:allValuesFrom <http://def.isotc211.org/iso19103/2015/MeasureTypes#Measure>;
         ] .


### http://inspire.ec.europa.eu/ont#restrictionType
:restrictionType rdf:type owl:ObjectProperty ;
         skos:definition "-- Definition -- The type of restriction .  -- Description -- SOURCE [Euroroads]. "@en ;
         rdfs:domain :RestrictionForVehicles;
         rdfs:range :RestrictionTypeValue;
         rdf:type owl:FunctionalProperty;
         rdfs:label "restrictionType"@en .
:RestrictionForVehicles rdfs:subClassOf [ rdf:type owl:Restriction ;
         owl:onProperty :restrictionType;
         owl:onClass :RestrictionTypeValue;
       owl:qualifiedCardinality "1"^^xsd:nonNegativeInteger ;
         ] .
:RestrictionForVehicles rdfs:subClassOf [ rdf:type owl:Restriction ;
         owl:onProperty :restrictionType;
         owl:allValuesFrom :RestrictionTypeValue;
         ] .


### http://inspire.ec.europa.eu/ont:RestrictionTypeValue
:RestrictionTypeValue a owl:Class ;
       rdfs:subClassOf :itnrCodeList ;
          rdfs:isDefinedBy  <https://inspire.ec.europa.eu/codelist/RestrictionTypeValue>;
         skos:definition "-- Definition -- Possible restrictions on vehicles that can access a transport element."@en ;
       rdfs:label "RestrictionTypeValue"@en .

### http://inspire.ec.europa.eu/ont:RestrictionTypeValueCode
:RestrictionTypeValueCode a skos:ConceptScheme ;
         skos:definition "-- Definition -- Possible restrictions on vehicles that can access a transport element."@en ;
          owl:sameAs  <https://inspire.ec.europa.eu/codelist/RestrictionTypeValue>;
       dc:isFormatOf :RestrictionTypeValue .

### http://inspire.ec.europa.eu/ont:RestrictionTypeValue.maximumDoubleAxleWeight
:RestrictionTypeValue.maximumDoubleAxleWeight a :RestrictionTypeValue,skos:Concept ;
         skos:inScheme :RestrictionTypeValueCode ;
         skos:definition "-- Definition -- The maximum weight per double axle of a vehicle allowed at a transport element.  -- Description -- SOURCE Adapted from [Euroroads].  NOTE This value applies to wheeled vehicles only. "@en ;
          owl:sameAs  <https://inspire.ec.europa.eu/codelist/RestrictionTypeValue/maximumDoubleAxleWeight>;
          rdfs:isDefinedBy  <https://inspire.ec.europa.eu/codelist/RestrictionTypeValue/maximumDoubleAxleWeight>;
         rdfs:label "maximumDoubleAxleWeight"@no .

### http://inspire.ec.europa.eu/ont:RestrictionTypeValue.maximumHeight
:RestrictionTypeValue.maximumHeight a :RestrictionTypeValue,skos:Concept ;
         skos:inScheme :RestrictionTypeValueCode ;
         skos:definition "-- Definition -- The maximum height of a vehicle which can pass under another object .  -- Description -- SOURCE [Euroroads]. "@en ;
          owl:sameAs  <https://inspire.ec.europa.eu/codelist/RestrictionTypeValue/maximumHeight>;
          rdfs:isDefinedBy  <https://inspire.ec.europa.eu/codelist/RestrictionTypeValue/maximumHeight>;
         rdfs:label "maximumHeight"@no .

### http://inspire.ec.europa.eu/ont:RestrictionTypeValue.maximumLength
:RestrictionTypeValue.maximumLength a :RestrictionTypeValue,skos:Concept ;
         skos:inScheme :RestrictionTypeValueCode ;
         skos:definition "-- Definition -- The maximum length of a vehicle allowed at a transport element.  -- Description -- SOURCE Adapted from [Euroroads]. "@en ;
          owl:sameAs  <https://inspire.ec.europa.eu/codelist/RestrictionTypeValue/maximumLength>;
          rdfs:isDefinedBy  <https://inspire.ec.europa.eu/codelist/RestrictionTypeValue/maximumLength>;
         rdfs:label "maximumLength"@no .

### http://inspire.ec.europa.eu/ont:RestrictionTypeValue.maximumSingleAxleWeight
:RestrictionTypeValue.maximumSingleAxleWeight a :RestrictionTypeValue,skos:Concept ;
         skos:inScheme :RestrictionTypeValueCode ;
         skos:definition "-- Definition -- The maximum weight per single axle of a vehicle allowed at a transport element.  -- Description -- SOURCE Adapted from [Euroroads].  NOTE This value applies to wheeled vehicles only. "@en ;
          owl:sameAs  <https://inspire.ec.europa.eu/codelist/RestrictionTypeValue/maximumSingleAxleWeight>;
          rdfs:isDefinedBy  <https://inspire.ec.europa.eu/codelist/RestrictionTypeValue/maximumSingleAxleWeight>;
         rdfs:label "maximumSingleAxleWeight"@no .

### http://inspire.ec.europa.eu/ont:RestrictionTypeValue.maximumTotalWeight
:RestrictionTypeValue.maximumTotalWeight a :RestrictionTypeValue,skos:Concept ;
         skos:inScheme :RestrictionTypeValueCode ;
         skos:definition "-- Definition -- The maximum total weight of a vehicle allowed at a transport element.  -- Description -- SOURCE Adapted from [Euroroads]. "@en ;
          owl:sameAs  <https://inspire.ec.europa.eu/codelist/RestrictionTypeValue/maximumTotalWeight>;
          rdfs:isDefinedBy  <https://inspire.ec.europa.eu/codelist/RestrictionTypeValue/maximumTotalWeight>;
         rdfs:label "maximumTotalWeight"@no .

### http://inspire.ec.europa.eu/ont:RestrictionTypeValue.maximumTripleAxleWeight
:RestrictionTypeValue.maximumTripleAxleWeight a :RestrictionTypeValue,skos:Concept ;
         skos:inScheme :RestrictionTypeValueCode ;
         skos:definition "-- Definition -- The maximum weight per triple axle of a vehicle allowed at a transport element.  -- Description -- SOURCE Adapted from [Euroroads].  NOTE This value applies to wheeled vehicles only. "@en ;
          owl:sameAs  <https://inspire.ec.europa.eu/codelist/RestrictionTypeValue/maximumTripleAxleWeight>;
          rdfs:isDefinedBy  <https://inspire.ec.europa.eu/codelist/RestrictionTypeValue/maximumTripleAxleWeight>;
         rdfs:label "maximumTripleAxleWeight"@no .

### http://inspire.ec.europa.eu/ont:RestrictionTypeValue.maximumWidth
:RestrictionTypeValue.maximumWidth a :RestrictionTypeValue,skos:Concept ;
         skos:inScheme :RestrictionTypeValueCode ;
         skos:definition "-- Definition -- The maximum width of a vehicle allowed on a transport element.  -- Description -- SOURCE Adapted from [Euroroads]. "@en ;
          owl:sameAs  <https://inspire.ec.europa.eu/codelist/RestrictionTypeValue/maximumWidth>;
          rdfs:isDefinedBy  <https://inspire.ec.europa.eu/codelist/RestrictionTypeValue/maximumWidth>;
         rdfs:label "maximumWidth"@no .

### http://inspire.ec.europa.eu/ont:TrafficFlowDirection
:TrafficFlowDirection a owl:Class ;
         skos:definition "-- Definition -- Indicates the direction of the flow of traffic in relation to the direction of the transport link vector. "@en ;
       rdfs:label "TrafficFlowDirection"@en .
:TrafficFlowDirection rdfs:subClassOf :TransportProperty .

### http://inspire.ec.europa.eu/ont#TrafficFlowDirection.direction
:TrafficFlowDirection.direction rdf:type owl:ObjectProperty ;
         skos:definition "-- Definition -- Indicates the direction of the flow of traffic."@en ;
         rdfs:domain :TrafficFlowDirection;
         rdfs:range :LinkDirectionValue;
         rdf:type owl:FunctionalProperty;
         rdfs:label "TrafficFlowDirection.direction"@en .
:TrafficFlowDirection rdfs:subClassOf [ rdf:type owl:Restriction ;
         owl:onProperty :TrafficFlowDirection.direction;
         owl:onClass :LinkDirectionValue;
       owl:qualifiedCardinality "1"^^xsd:nonNegativeInteger ;
         ] .
:TrafficFlowDirection rdfs:subClassOf [ rdf:type owl:Restriction ;
         owl:onProperty :TrafficFlowDirection.direction;
         owl:allValuesFrom :LinkDirectionValue;
         ] .


### http://inspire.ec.europa.eu/ont:TransportArea
:TransportArea a owl:Class ;
         skos:definition "-- Definition -- Surface that represents the spatial extent of an element of a transport network."@en ;
       rdfs:label "TransportArea"@en .
:TransportArea rdfs:subClassOf :NetworkArea .
:TransportArea rdfs:subClassOf :TransportObject .
:TransportArea rdfs:subClassOf [ rdf:type owl:Restriction ;
         owl:onProperty :validFrom;
         owl:onDataRange xsd:dateTime;
       owl:qualifiedCardinality "1"^^xsd:nonNegativeInteger ;
         ] .
:TransportArea rdfs:subClassOf [ rdf:type owl:Restriction ;
         owl:onProperty :validFrom;
         owl:allValuesFrom xsd:dateTime;
         ] .

:TransportArea rdfs:subClassOf [ rdf:type owl:Restriction ;
         owl:onProperty :validTo;
         owl:onDataRange xsd:dateTime;
       owl:maxQualifiedCardinality "1"^^xsd:nonNegativeInteger ;
         ] .
:TransportArea rdfs:subClassOf [ rdf:type owl:Restriction ;
         owl:onProperty :validTo;
         owl:allValuesFrom xsd:dateTime;
         ] .

:TransportArea owl:disjointUnionOf ( :RoadServiceArea :VehicleTrafficArea :RoadArea  ) ; .

### http://inspire.ec.europa.eu/ont:TransportLink
:TransportLink a owl:Class ;
         skos:definition "-- Definition -- A linear spatial object that describes the geometry and connectivity of a transport network between two points in the network."@en ;
       rdfs:label "TransportLink"@en .
:TransportLink rdfs:subClassOf :TransportObject .
:TransportLink rdfs:subClassOf :Link .
:TransportLink rdfs:subClassOf [ rdf:type owl:Restriction ;
         owl:onProperty :validFrom;
         owl:onDataRange xsd:dateTime;
       owl:qualifiedCardinality "1"^^xsd:nonNegativeInteger ;
         ] .
:TransportLink rdfs:subClassOf [ rdf:type owl:Restriction ;
         owl:onProperty :validFrom;
         owl:allValuesFrom xsd:dateTime;
         ] .

:TransportLink rdfs:subClassOf [ rdf:type owl:Restriction ;
         owl:onProperty :validTo;
         owl:onDataRange xsd:dateTime;
       owl:maxQualifiedCardinality "1"^^xsd:nonNegativeInteger ;
         ] .
:TransportLink rdfs:subClassOf [ rdf:type owl:Restriction ;
         owl:onProperty :validTo;
         owl:allValuesFrom xsd:dateTime;
         ] .

:TransportLink owl:disjointUnionOf ( :RoadLink  ) ; .

### http://inspire.ec.europa.eu/ont:TransportLinkSequence
:TransportLinkSequence a owl:Class ;
         skos:definition "-- Definition -- A linear spatial object, composed of an ordered collection of transport links, which represents a continuous path in the transport network without any branches. The element has a defined beginning and end and every position on the transport link sequence is identifiable with one single parameter such as length. It describes an element of the transport network, characterized by one or more thematical identifiers and/or properties. "@en ;
       rdfs:label "TransportLinkSequence"@en .
:TransportLinkSequence rdfs:subClassOf :LinkSequence .
:TransportLinkSequence rdfs:subClassOf :TransportObject .
:TransportLinkSequence rdfs:subClassOf [ rdf:type owl:Restriction ;
         owl:onProperty :validFrom;
         owl:onDataRange xsd:dateTime;
       owl:qualifiedCardinality "1"^^xsd:nonNegativeInteger ;
         ] .
:TransportLinkSequence rdfs:subClassOf [ rdf:type owl:Restriction ;
         owl:onProperty :validFrom;
         owl:allValuesFrom xsd:dateTime;
         ] .

:TransportLinkSequence rdfs:subClassOf [ rdf:type owl:Restriction ;
         owl:onProperty :validTo;
         owl:onDataRange xsd:dateTime;
       owl:maxQualifiedCardinality "1"^^xsd:nonNegativeInteger ;
         ] .
:TransportLinkSequence rdfs:subClassOf [ rdf:type owl:Restriction ;
         owl:onProperty :validTo;
         owl:allValuesFrom xsd:dateTime;
         ] .

:TransportLinkSequence owl:disjointUnionOf ( :RoadLinkSequence  ) ; .

### http://inspire.ec.europa.eu/ont:TransportLinkSet
:TransportLinkSet a owl:Class ;
         skos:definition "-- Definition -- A collection of transport link sequences and or individual transport links that has a specific function or significance in a transport network.   -- Description -- NOTE This spatial object type supports the aggregation of links to form objects with branches, loops, parallel sequences of links, gaps, etc.  EXAMPLE A dual carriageway road, as a collection of the two link sequences that represent each carriageway.  "@en ;
       rdfs:label "TransportLinkSet"@en .
:TransportLinkSet rdfs:subClassOf :LinkSet .
:TransportLinkSet rdfs:subClassOf :TransportObject .

### http://inspire.ec.europa.eu/ont#post
:post rdf:type owl:ObjectProperty ;
         skos:definition "-- Definition -- Marker post along a route in a transport network."@en ;
         rdfs:domain :TransportLinkSet;
         rdfs:range :MarkerPost;
         owl:inverseOf :route ;
         rdfs:label "post"@en .
:TransportLinkSet rdfs:subClassOf [ rdf:type owl:Restriction ;
         owl:onProperty :post;
         owl:allValuesFrom :MarkerPost;
         ] .

:TransportLinkSet rdfs:subClassOf [ rdf:type owl:Restriction ;
         owl:onProperty :validFrom;
         owl:onDataRange xsd:dateTime;
       owl:qualifiedCardinality "1"^^xsd:nonNegativeInteger ;
         ] .
:TransportLinkSet rdfs:subClassOf [ rdf:type owl:Restriction ;
         owl:onProperty :validFrom;
         owl:allValuesFrom xsd:dateTime;
         ] .

:TransportLinkSet rdfs:subClassOf [ rdf:type owl:Restriction ;
         owl:onProperty :validTo;
         owl:onDataRange xsd:dateTime;
       owl:maxQualifiedCardinality "1"^^xsd:nonNegativeInteger ;
         ] .
:TransportLinkSet rdfs:subClassOf [ rdf:type owl:Restriction ;
         owl:onProperty :validTo;
         owl:allValuesFrom xsd:dateTime;
         ] .

:TransportLinkSet owl:disjointUnionOf ( :ERoad :Road  ) ; .

### http://inspire.ec.europa.eu/ont:TransportNetwork
:TransportNetwork a owl:Class ;
         skos:definition "-- Definition -- Collection of network elements that belong to a single mode of transport.  -- Description -- NOTE Road, rail, water and air transport are always considered separate transport modes. Even within these four categories, multiple modes of transport can be defined, based on infrastructure, vehicle types, propulsion system, operation and/or other defining characteristics.  EXAMPLE All road transport can be considered one mode of transport for some applications. For other applications, it might be necessary to distinguish between different public road transport networks. Within water transport, marine and inland water transport can be considered to be separate modes of transport for some applications, as they use different types of ships. "@en ;
       rdfs:label "TransportNetwork"@en .
:TransportNetwork rdfs:subClassOf :Network .
:TransportNetwork rdfs:subClassOf [ rdf:type owl:Restriction ;
         owl:onProperty :inspireId;
         owl:onClass :Identifier;
       owl:qualifiedCardinality "1"^^xsd:nonNegativeInteger ;
         ] .
:TransportNetwork rdfs:subClassOf [ rdf:type owl:Restriction ;
         owl:onProperty :inspireId;
         owl:allValuesFrom :Identifier;
         ] .


### http://inspire.ec.europa.eu/ont#typeOfTransport
:typeOfTransport rdf:type owl:ObjectProperty ;
         skos:definition "-- Definition -- Type of transport network, based on the type of infrastructure the network uses."@en ;
         rdfs:domain :TransportNetwork;
         rdfs:range :TransportTypeValue;
         rdf:type owl:FunctionalProperty;
         rdfs:label "typeOfTransport"@en .
:TransportNetwork rdfs:subClassOf [ rdf:type owl:Restriction ;
         owl:onProperty :typeOfTransport;
         owl:onClass :TransportTypeValue;
       owl:qualifiedCardinality "1"^^xsd:nonNegativeInteger ;
         ] .
:TransportNetwork rdfs:subClassOf [ rdf:type owl:Restriction ;
         owl:onProperty :typeOfTransport;
         owl:allValuesFrom :TransportTypeValue;
         ] .


### http://inspire.ec.europa.eu/ont:TransportNode
:TransportNode a owl:Class ;
         skos:definition "-- Definition -- A point spatial object which is used for connectivity.  -- Description -- Nodes are found at either end of the TransportLink. "@en ;
       rdfs:label "TransportNode"@en .
:TransportNode rdfs:subClassOf :TransportObject .
:TransportNode rdfs:subClassOf :Node .
:TransportNode rdfs:subClassOf [ rdf:type owl:Restriction ;
         owl:onProperty :validFrom;
         owl:onDataRange xsd:dateTime;
       owl:qualifiedCardinality "1"^^xsd:nonNegativeInteger ;
         ] .
:TransportNode rdfs:subClassOf [ rdf:type owl:Restriction ;
         owl:onProperty :validFrom;
         owl:allValuesFrom xsd:dateTime;
         ] .

:TransportNode rdfs:subClassOf [ rdf:type owl:Restriction ;
         owl:onProperty :validTo;
         owl:onDataRange xsd:dateTime;
       owl:maxQualifiedCardinality "1"^^xsd:nonNegativeInteger ;
         ] .
:TransportNode rdfs:subClassOf [ rdf:type owl:Restriction ;
         owl:onProperty :validTo;
         owl:allValuesFrom xsd:dateTime;
         ] .

:TransportNode owl:disjointUnionOf ( :RoadNode  ) ; .

### http://inspire.ec.europa.eu/ont:TransportObject
:TransportObject a owl:Class ;
       rdfs:subClassOf :itnrFeature ;
          rdfs:isDefinedBy  <http://inspire.ec.europa.eu/featureconcept/TransportObject>;
         skos:definition "-- Definition -- An identity base for transport network objects in the real world.  -- Description -- NOTE Derived 'views' of real-world transport objects are represented through specialisations in other application schemas; all representations of the same real-world object share a common geographic name. "@en ;
       rdfs:label "TransportObject"@en .
:TransportObject rdfs:subClassOf [ rdf:type owl:Restriction ;
         owl:onProperty :geographicalName;
         owl:onClass <>;
       owl:maxQualifiedCardinality "1"^^xsd:nonNegativeInteger ;
         ] .
:TransportObject rdfs:subClassOf [ rdf:type owl:Restriction ;
         owl:onProperty :geographicalName;
         owl:allValuesFrom <>;
         ] .

:TransportObject owl:disjointUnionOf ( :TransportLink :TransportNode :TransportLinkSet :TransportPoint :TransportLinkSequence :TransportArea  ) ; .

### http://inspire.ec.europa.eu/ont:TransportPoint
:TransportPoint a owl:Class ;
         skos:definition "-- Definition -- A point spatial object - which is not a node - that represents the position of an element of a transport network."@en ;
       rdfs:label "TransportPoint"@en .
:TransportPoint rdfs:subClassOf :NetworkElement .
:TransportPoint rdfs:subClassOf :TransportObject .
:TransportPoint rdfs:subClassOf [ rdf:type owl:Restriction ;
         owl:onProperty :geometry;
         owl:onClass <http://www.opengis.net/ont/sf#Point>;
       owl:qualifiedCardinality "1"^^xsd:nonNegativeInteger ;
         ] .
:TransportPoint rdfs:subClassOf [ rdf:type owl:Restriction ;
         owl:onProperty :geometry;
         owl:allValuesFrom <http://www.opengis.net/ont/sf#Point>;
         ] .

:TransportPoint rdfs:subClassOf [ rdf:type owl:Restriction ;
         owl:onProperty :validFrom;
         owl:onDataRange xsd:dateTime;
       owl:qualifiedCardinality "1"^^xsd:nonNegativeInteger ;
         ] .
:TransportPoint rdfs:subClassOf [ rdf:type owl:Restriction ;
         owl:onProperty :validFrom;
         owl:allValuesFrom xsd:dateTime;
         ] .

:TransportPoint rdfs:subClassOf [ rdf:type owl:Restriction ;
         owl:onProperty :validTo;
         owl:onDataRange xsd:dateTime;
       owl:maxQualifiedCardinality "1"^^xsd:nonNegativeInteger ;
         ] .
:TransportPoint rdfs:subClassOf [ rdf:type owl:Restriction ;
         owl:onProperty :validTo;
         owl:allValuesFrom xsd:dateTime;
         ] .

:TransportPoint owl:disjointUnionOf ( :MarkerPost  ) ; .

### http://inspire.ec.europa.eu/ont:TransportProperty
:TransportProperty a owl:Class ;
         skos:definition "-- Definition -- A reference to a property that falls upon the network. This property can apply to the whole of the network element it is associated with or - for linear spatial objects - be described using linear referencing."@en ;
       rdfs:label "TransportProperty"@en .
:TransportProperty rdfs:subClassOf :NetworkProperty .
:TransportProperty rdfs:subClassOf [ rdf:type owl:Restriction ;
         owl:onProperty :validFrom;
         owl:onDataRange xsd:dateTime;
       owl:qualifiedCardinality "1"^^xsd:nonNegativeInteger ;
         ] .
:TransportProperty rdfs:subClassOf [ rdf:type owl:Restriction ;
         owl:onProperty :validFrom;
         owl:allValuesFrom xsd:dateTime;
         ] .

:TransportProperty rdfs:subClassOf [ rdf:type owl:Restriction ;
         owl:onProperty :validTo;
         owl:onDataRange xsd:dateTime;
       owl:maxQualifiedCardinality "1"^^xsd:nonNegativeInteger ;
         ] .
:TransportProperty rdfs:subClassOf [ rdf:type owl:Restriction ;
         owl:onProperty :validTo;
         owl:allValuesFrom xsd:dateTime;
         ] .

:TransportProperty owl:disjointUnionOf ( :RoadSurfaceCategory :NumberOfLanes :RoadServiceType :FormOfWay :RoadWidth :SpeedLimit :FunctionalRoadClass :RoadName :AccessRestriction :MaintenanceAuthority :RestrictionForVehicles :TrafficFlowDirection :OwnerAuthority :ConditionOfFacility :VerticalPosition  ) ; .

### http://inspire.ec.europa.eu/ont:TransportTypeValue
:TransportTypeValue a owl:Class ;
       rdfs:subClassOf :itnrEnumeration ;
          rdfs:isDefinedBy  <https://inspire.ec.europa.eu/enumeration/TransportTypeValue>;
         skos:definition "-- Definition -- Possible types on transport networks."@en ;
       rdfs:label "TransportTypeValue"@en .

### http://inspire.ec.europa.eu/ont:TransportTypeValueCode
:TransportTypeValueCode a skos:ConceptScheme ;
         skos:definition "-- Definition -- Possible types on transport networks."@en ;
          owl:sameAs  <https://inspire.ec.europa.eu/enumeration/TransportTypeValue>;
       dc:isFormatOf :TransportTypeValue .

### http://inspire.ec.europa.eu/ont:TransportTypeValue.air
:TransportTypeValue.air a :TransportTypeValue,skos:Concept ;
         skos:inScheme :TransportTypeValueCode ;
         skos:definition "-- Definition -- The transport network consists of transport by air."@en ;
          owl:sameAs  <https://inspire.ec.europa.eu/enumeration/TransportTypeValue/air>;
          rdfs:isDefinedBy  <https://inspire.ec.europa.eu/enumeration/TransportTypeValue/air>;
         rdfs:label "air"@no .

### http://inspire.ec.europa.eu/ont:TransportTypeValue.cable
:TransportTypeValue.cable a :TransportTypeValue,skos:Concept ;
         skos:inScheme :TransportTypeValueCode ;
         skos:definition "-- Definition -- The transport network consists of transport by cable. "@en ;
          owl:sameAs  <https://inspire.ec.europa.eu/enumeration/TransportTypeValue/cable>;
          rdfs:isDefinedBy  <https://inspire.ec.europa.eu/enumeration/TransportTypeValue/cable>;
         rdfs:label "cable"@no .

### http://inspire.ec.europa.eu/ont:TransportTypeValue.rail
:TransportTypeValue.rail a :TransportTypeValue,skos:Concept ;
         skos:inScheme :TransportTypeValueCode ;
         skos:definition "-- Definition -- The transport network consists of transport by rail. "@en ;
          owl:sameAs  <https://inspire.ec.europa.eu/enumeration/TransportTypeValue/rail>;
          rdfs:isDefinedBy  <https://inspire.ec.europa.eu/enumeration/TransportTypeValue/rail>;
         rdfs:label "rail"@no .

### http://inspire.ec.europa.eu/ont:TransportTypeValue.road
:TransportTypeValue.road a :TransportTypeValue,skos:Concept ;
         skos:inScheme :TransportTypeValueCode ;
         skos:definition "-- Definition -- The transport network consists of transport by road. "@en ;
          owl:sameAs  <https://inspire.ec.europa.eu/enumeration/TransportTypeValue/road>;
          rdfs:isDefinedBy  <https://inspire.ec.europa.eu/enumeration/TransportTypeValue/road>;
         rdfs:label "road"@no .

### http://inspire.ec.europa.eu/ont:TransportTypeValue.water
:TransportTypeValue.water a :TransportTypeValue,skos:Concept ;
         skos:inScheme :TransportTypeValueCode ;
         skos:definition "-- Definition -- The transport network consists of transport by water. "@en ;
          owl:sameAs  <https://inspire.ec.europa.eu/enumeration/TransportTypeValue/water>;
          rdfs:isDefinedBy  <https://inspire.ec.europa.eu/enumeration/TransportTypeValue/water>;
         rdfs:label "water"@no .
:TransportTypeValue owl:oneOf ( :TransportTypeValue.air :TransportTypeValue.cable :TransportTypeValue.rail :TransportTypeValue.road :TransportTypeValue.water  ) ; .

### http://inspire.ec.europa.eu/ont:VerticalPosition
:VerticalPosition a owl:Class ;
         skos:definition "-- Definition -- Vertical level relative to other transport network elements."@en ;
       rdfs:label "VerticalPosition"@en .
:VerticalPosition rdfs:subClassOf :TransportProperty .

### http://inspire.ec.europa.eu/ont#VerticalPosition.verticalPosition
:VerticalPosition.verticalPosition rdf:type owl:ObjectProperty ;
         skos:definition "-- Definition -- Relative vertical position of the transport element."@en ;
         rdfs:domain :VerticalPosition;
         rdfs:range :VerticalPositionValue;
         rdf:type owl:FunctionalProperty;
         rdfs:label "VerticalPosition.verticalPosition"@en .
:VerticalPosition rdfs:subClassOf [ rdf:type owl:Restriction ;
         owl:onProperty :VerticalPosition.verticalPosition;
         owl:onClass :VerticalPositionValue;
       owl:qualifiedCardinality "1"^^xsd:nonNegativeInteger ;
         ] .
:VerticalPosition rdfs:subClassOf [ rdf:type owl:Restriction ;
         owl:onProperty :VerticalPosition.verticalPosition;
         owl:allValuesFrom :VerticalPositionValue;
         ] .


### http://inspire.ec.europa.eu/ont:AccessRestrictionValue
:AccessRestrictionValue a owl:Class ;
       rdfs:subClassOf :itnrCodeList ;
          rdfs:isDefinedBy  <https://inspire.ec.europa.eu/codelist/AccessRestrictionValue>;
         skos:definition "-- Definition -- Types of access restrictions for a transport element. "@en ;
       rdfs:label "AccessRestrictionValue"@en .

### http://inspire.ec.europa.eu/ont:AccessRestrictionValueCode
:AccessRestrictionValueCode a skos:ConceptScheme ;
         skos:definition "-- Definition -- Types of access restrictions for a transport element. "@en ;
          owl:sameAs  <https://inspire.ec.europa.eu/codelist/AccessRestrictionValue>;
       dc:isFormatOf :AccessRestrictionValue .

### http://inspire.ec.europa.eu/ont:AccessRestrictionValue.forbiddenLegally
:AccessRestrictionValue.forbiddenLegally a :AccessRestrictionValue,skos:Concept ;
         skos:inScheme :AccessRestrictionValueCode ;
         skos:definition "-- Definition -- Access to the transport element is forbidden by law."@en ;
          owl:sameAs  <https://inspire.ec.europa.eu/codelist/AccessRestrictionValue/forbiddenLegally>;
          rdfs:isDefinedBy  <https://inspire.ec.europa.eu/codelist/AccessRestrictionValue/forbiddenLegally>;
         rdfs:label "forbiddenLegally"@no .

### http://inspire.ec.europa.eu/ont:AccessRestrictionValue.physicallyImpossible
:AccessRestrictionValue.physicallyImpossible a :AccessRestrictionValue,skos:Concept ;
         skos:inScheme :AccessRestrictionValueCode ;
         skos:definition "-- Definition -- Access to the transport element is physically impossible due to the presence of barriers or other physical obstacles."@en ;
          owl:sameAs  <https://inspire.ec.europa.eu/codelist/AccessRestrictionValue/physicallyImpossible>;
          rdfs:isDefinedBy  <https://inspire.ec.europa.eu/codelist/AccessRestrictionValue/physicallyImpossible>;
         rdfs:label "physicallyImpossible"@no .

### http://inspire.ec.europa.eu/ont:AccessRestrictionValue.private
:AccessRestrictionValue.private a :AccessRestrictionValue,skos:Concept ;
         skos:inScheme :AccessRestrictionValueCode ;
         skos:definition "-- Definition -- Access to the transport element is restricted because it is privately owned."@en ;
          owl:sameAs  <https://inspire.ec.europa.eu/codelist/AccessRestrictionValue/private>;
          rdfs:isDefinedBy  <https://inspire.ec.europa.eu/codelist/AccessRestrictionValue/private>;
         rdfs:label "private"@no .

### http://inspire.ec.europa.eu/ont:AccessRestrictionValue.publicAccess
:AccessRestrictionValue.publicAccess a :AccessRestrictionValue,skos:Concept ;
         skos:inScheme :AccessRestrictionValueCode ;
         skos:definition "-- Definition -- The transport element is open to public access."@en ;
          owl:sameAs  <https://inspire.ec.europa.eu/codelist/AccessRestrictionValue/publicAccess>;
          rdfs:isDefinedBy  <https://inspire.ec.europa.eu/codelist/AccessRestrictionValue/publicAccess>;
         rdfs:label "publicAccess"@no .

### http://inspire.ec.europa.eu/ont:AccessRestrictionValue.seasonal
:AccessRestrictionValue.seasonal a :AccessRestrictionValue,skos:Concept ;
         skos:inScheme :AccessRestrictionValueCode ;
         skos:definition "-- Definition -- Access to the transport element depends on the season."@en ;
          owl:sameAs  <https://inspire.ec.europa.eu/codelist/AccessRestrictionValue/seasonal>;
          rdfs:isDefinedBy  <https://inspire.ec.europa.eu/codelist/AccessRestrictionValue/seasonal>;
         rdfs:label "seasonal"@no .

### http://inspire.ec.europa.eu/ont:AccessRestrictionValue.toll
:AccessRestrictionValue.toll a :AccessRestrictionValue,skos:Concept ;
         skos:inScheme :AccessRestrictionValueCode ;
         skos:definition "-- Definition -- Access to the transport element is subject to toll."@en ;
          owl:sameAs  <https://inspire.ec.europa.eu/codelist/AccessRestrictionValue/toll>;
          rdfs:isDefinedBy  <https://inspire.ec.europa.eu/codelist/AccessRestrictionValue/toll>;
         rdfs:label "toll"@no .


### http://inspire.ec.europa.eu/ont:AreaConditionValue
:AreaConditionValue a owl:Class ;
       rdfs:subClassOf :itnrCodeList ;
          rdfs:isDefinedBy  <https://inspire.ec.europa.eu/codelist/AreaConditionValue>;
         skos:definition "-- Definition -- Speed limit restriction depending on the area.  -- Description -- SOURCE [Euroroads]. "@en ;
       rdfs:label "AreaConditionValue"@en .

### http://inspire.ec.europa.eu/ont:AreaConditionValueCode
:AreaConditionValueCode a skos:ConceptScheme ;
         skos:definition "-- Definition -- Speed limit restriction depending on the area.  -- Description -- SOURCE [Euroroads]. "@en ;
          owl:sameAs  <https://inspire.ec.europa.eu/codelist/AreaConditionValue>;
       dc:isFormatOf :AreaConditionValue .

### http://inspire.ec.europa.eu/ont:AreaConditionValue.inNationalPark
:AreaConditionValue.inNationalPark a :AreaConditionValue,skos:Concept ;
         skos:inScheme :AreaConditionValueCode ;
         skos:definition "-- Definition -- Speed limit restriction inside national park.  -- Description -- SOURCE [Euroroads]."@en ;
          owl:sameAs  <https://inspire.ec.europa.eu/codelist/AreaConditionValue/inNationalPark>;
          rdfs:isDefinedBy  <https://inspire.ec.europa.eu/codelist/AreaConditionValue/inNationalPark>;
         rdfs:label "inNationalPark"@no .

### http://inspire.ec.europa.eu/ont:AreaConditionValue.insideCities
:AreaConditionValue.insideCities a :AreaConditionValue,skos:Concept ;
         skos:inScheme :AreaConditionValueCode ;
         skos:definition "-- Definition -- Speed limit restriction inside cities.  -- Description -- SOURCE [Euroroads]."@en ;
          owl:sameAs  <https://inspire.ec.europa.eu/codelist/AreaConditionValue/insideCities>;
          rdfs:isDefinedBy  <https://inspire.ec.europa.eu/codelist/AreaConditionValue/insideCities>;
         rdfs:label "insideCities"@no .

### http://inspire.ec.europa.eu/ont:AreaConditionValue.nearRailroadCrossing
:AreaConditionValue.nearRailroadCrossing a :AreaConditionValue,skos:Concept ;
         skos:inScheme :AreaConditionValueCode ;
         skos:definition "-- Definition -- Speed limit restriction near rail road crossing.  -- Description -- SOURCE [Euroroads]."@en ;
          owl:sameAs  <https://inspire.ec.europa.eu/codelist/AreaConditionValue/nearRailroadCrossing>;
          rdfs:isDefinedBy  <https://inspire.ec.europa.eu/codelist/AreaConditionValue/nearRailroadCrossing>;
         rdfs:label "nearRailroadCrossing"@no .

### http://inspire.ec.europa.eu/ont:AreaConditionValue.nearSchool
:AreaConditionValue.nearSchool a :AreaConditionValue,skos:Concept ;
         skos:inScheme :AreaConditionValueCode ;
         skos:definition "-- Definition -- Speed limit restriction near school.  -- Description -- SOURCE [Euroroads]."@en ;
          owl:sameAs  <https://inspire.ec.europa.eu/codelist/AreaConditionValue/nearSchool>;
          rdfs:isDefinedBy  <https://inspire.ec.europa.eu/codelist/AreaConditionValue/nearSchool>;
         rdfs:label "nearSchool"@no .

### http://inspire.ec.europa.eu/ont:AreaConditionValue.outsideCities
:AreaConditionValue.outsideCities a :AreaConditionValue,skos:Concept ;
         skos:inScheme :AreaConditionValueCode ;
         skos:definition "-- Definition -- Speed limit restriction outside cities.  -- Description -- SOURCE [Euroroads]."@en ;
          owl:sameAs  <https://inspire.ec.europa.eu/codelist/AreaConditionValue/outsideCities>;
          rdfs:isDefinedBy  <https://inspire.ec.europa.eu/codelist/AreaConditionValue/outsideCities>;
         rdfs:label "outsideCities"@no .

### http://inspire.ec.europa.eu/ont:AreaConditionValue.trafficCalmingArea
:AreaConditionValue.trafficCalmingArea a :AreaConditionValue,skos:Concept ;
         skos:inScheme :AreaConditionValueCode ;
         skos:definition "-- Definition -- Speed limit restriction in traffic calming area.  -- Description -- SOURCE [Euroroads]."@en ;
          owl:sameAs  <https://inspire.ec.europa.eu/codelist/AreaConditionValue/trafficCalmingArea>;
          rdfs:isDefinedBy  <https://inspire.ec.europa.eu/codelist/AreaConditionValue/trafficCalmingArea>;
         rdfs:label "trafficCalmingArea"@no .

### http://inspire.ec.europa.eu/ont:ERoad
:ERoad a owl:Class ;
         skos:definition "-- Definition -- A collection of road link sequences and or individual road links that represents a route that is part of the international E-road network, characterized by its European route number.  -- Description -- EXAMPLE E40. "@en ;
       rdfs:label "ERoad"@en .
:ERoad rdfs:subClassOf :TransportLinkSet .

### http://inspire.ec.europa.eu/ont#europeanRouteNumber
:europeanRouteNumber rdf:type owl:DatatypeProperty ;
         skos:definition "-- Definition -- Code, identifying the route in the international E-road network. The code always starts with a letter 'E', followed by a one-, two- or three-digit number."@en ;
         rdfs:domain :ERoad;
         rdfs:range xsd:string;
         rdf:type owl:FunctionalProperty;
         rdfs:label "europeanRouteNumber"@en .
:ERoad rdfs:subClassOf [ rdf:type owl:Restriction ;
         owl:onProperty :europeanRouteNumber;
         owl:onDataRange xsd:string;
       owl:qualifiedCardinality "1"^^xsd:nonNegativeInteger ;
         ] .
:ERoad rdfs:subClassOf [ rdf:type owl:Restriction ;
         owl:onProperty :europeanRouteNumber;
         owl:allValuesFrom xsd:string;
         ] .


### http://inspire.ec.europa.eu/ont:FormOfWay
:FormOfWay a owl:Class ;
         skos:definition "-- Definition -- A classification based on the physical properties of the Road Link.  -- Description -- SOURCE Based on [EuroRoadS]. "@en ;
       rdfs:label "FormOfWay"@en .
:FormOfWay rdfs:subClassOf :TransportProperty .

### http://inspire.ec.europa.eu/ont#FormOfWay.formOfWay
:FormOfWay.formOfWay rdf:type owl:ObjectProperty ;
         skos:definition "-- Definition -- Physical form of the way."@en ;
         rdfs:domain :FormOfWay;
         rdfs:range :FormOfWayValue;
         rdf:type owl:FunctionalProperty;
         rdfs:label "FormOfWay.formOfWay"@en .
:FormOfWay rdfs:subClassOf [ rdf:type owl:Restriction ;
         owl:onProperty :FormOfWay.formOfWay;
         owl:onClass :FormOfWayValue;
       owl:qualifiedCardinality "1"^^xsd:nonNegativeInteger ;
         ] .
:FormOfWay rdfs:subClassOf [ rdf:type owl:Restriction ;
         owl:onProperty :FormOfWay.formOfWay;
         owl:allValuesFrom :FormOfWayValue;
         ] .


### http://inspire.ec.europa.eu/ont:FunctionalRoadClass
:FunctionalRoadClass a owl:Class ;
         skos:definition "-- Definition -- A classification based on the importance of the role that the road performs in the road network.   -- Description -- SOURCE Adapted from [GDF, EuroRoadS]. "@en ;
       rdfs:label "FunctionalRoadClass"@en .
:FunctionalRoadClass rdfs:subClassOf :TransportProperty .

### http://inspire.ec.europa.eu/ont#functionalClass
:functionalClass rdf:type owl:ObjectProperty ;
         skos:definition "-- Definition -- Functional rank of the road link in the road network.  -- Description -- NOTE Where functional classification systems are used that have fewer classes/ranks than the number provided by FunctionalRoadClassValues, classes with codes 1 to n will be used, where n corresponds to the number of classes that are used in the classification system. "@en ;
         rdfs:domain :FunctionalRoadClass;
         rdfs:range :FunctionalRoadClassValue;
         rdf:type owl:FunctionalProperty;
         rdfs:label "functionalClass"@en .
:FunctionalRoadClass rdfs:subClassOf [ rdf:type owl:Restriction ;
         owl:onProperty :functionalClass;
         owl:onClass :FunctionalRoadClassValue;
       owl:qualifiedCardinality "1"^^xsd:nonNegativeInteger ;
         ] .
:FunctionalRoadClass rdfs:subClassOf [ rdf:type owl:Restriction ;
         owl:onProperty :functionalClass;
         owl:allValuesFrom :FunctionalRoadClassValue;
         ] .


### http://inspire.ec.europa.eu/ont:MinMaxLaneValue
:MinMaxLaneValue a owl:Class ;
       rdfs:subClassOf :itnrEnumeration ;
          rdfs:isDefinedBy  <https://inspire.ec.europa.eu/enumeration/MinMaxLaneValue>;
         skos:definition "-- Definition -- Values to indicate whether number of lanes are counted as the maximum, minimum or average number.  -- Description -- SOURCE Adapted from [Euroroads]."@en ;
       rdfs:label "MinMaxLaneValue"@en .

### http://inspire.ec.europa.eu/ont:MinMaxLaneValueCode
:MinMaxLaneValueCode a skos:ConceptScheme ;
         skos:definition "-- Definition -- Values to indicate whether number of lanes are counted as the maximum, minimum or average number.  -- Description -- SOURCE Adapted from [Euroroads]."@en ;
          owl:sameAs  <https://inspire.ec.europa.eu/enumeration/MinMaxLaneValue>;
       dc:isFormatOf :MinMaxLaneValue .

### http://inspire.ec.europa.eu/ont:MinMaxLaneValue.maximum
:MinMaxLaneValue.maximum a :MinMaxLaneValue,skos:Concept ;
         skos:inScheme :MinMaxLaneValueCode ;
         skos:definition "-- Definition -- The number of lanes is the maximum value for a given part of the road network.  -- Description -- SOURCE Adapted from [Euroroads]. "@en ;
          owl:sameAs  <https://inspire.ec.europa.eu/enumeration/MinMaxLaneValue/maximum>;
          rdfs:isDefinedBy  <https://inspire.ec.europa.eu/enumeration/MinMaxLaneValue/maximum>;
         rdfs:label "maximum"@no .

### http://inspire.ec.europa.eu/ont:MinMaxLaneValue.minimum
:MinMaxLaneValue.minimum a :MinMaxLaneValue,skos:Concept ;
         skos:inScheme :MinMaxLaneValueCode ;
         skos:definition "-- Definition -- The number of lanes is the minimum value for a given part of the road network.  -- Description -- SOURCE [Euroroads]. "@en ;
          owl:sameAs  <https://inspire.ec.europa.eu/enumeration/MinMaxLaneValue/minimum>;
          rdfs:isDefinedBy  <https://inspire.ec.europa.eu/enumeration/MinMaxLaneValue/minimum>;
         rdfs:label "minimum"@no .

### http://inspire.ec.europa.eu/ont:MinMaxLaneValue.average
:MinMaxLaneValue.average a :MinMaxLaneValue,skos:Concept ;
         skos:inScheme :MinMaxLaneValueCode ;
         skos:definition "-- Definition -- The number of lanes is the average value for a given part of the road network.  -- Description -- SOURCE [Euroroads]. "@en ;
          owl:sameAs  <https://inspire.ec.europa.eu/enumeration/MinMaxLaneValue/average>;
          rdfs:isDefinedBy  <https://inspire.ec.europa.eu/enumeration/MinMaxLaneValue/average>;
         rdfs:label "average"@no .
:MinMaxLaneValue owl:oneOf ( :MinMaxLaneValue.maximum :MinMaxLaneValue.minimum :MinMaxLaneValue.average  ) ; .

### http://inspire.ec.europa.eu/ont:NumberOfLanes
:NumberOfLanes a owl:Class ;
         skos:definition "-- Definition -- The number of lanes of a road element.  -- Description -- SOURCE Adapated from [Euroroads]. "@en ;
       rdfs:label "NumberOfLanes"@en .
:NumberOfLanes rdfs:subClassOf :TransportProperty .

### http://inspire.ec.europa.eu/ont#NumberOfLanes.direction
:NumberOfLanes.direction rdf:type owl:ObjectProperty ;
         skos:definition "-- Definition -- Indicates which direction the number of lanes is valid for.  -- Description -- SOURCE [Euroroads]. NOTE When the value for this attribute is 'both', numberOfLanes contains the sum of the number of lanes in both directions of travel. NOTE This attribute only applies when the property is associated with a road link or road link sequence."@en ;
         rdfs:domain :NumberOfLanes;
         rdfs:range :LinkDirectionValue;
         rdfs:label "NumberOfLanes.direction"@en .
:NumberOfLanes rdfs:subClassOf [ rdf:type owl:Restriction ;
         owl:onProperty :NumberOfLanes.direction;
         owl:onClass :LinkDirectionValue;
       owl:maxQualifiedCardinality "1"^^xsd:nonNegativeInteger ;
         ] .
:NumberOfLanes rdfs:subClassOf [ rdf:type owl:Restriction ;
         owl:onProperty :NumberOfLanes.direction;
         owl:allValuesFrom :LinkDirectionValue;
         ] .


### http://inspire.ec.europa.eu/ont#minMaxNumberOfLanes
:minMaxNumberOfLanes rdf:type owl:ObjectProperty ;
         skos:definition "-- Definition -- Indicates if the number of lanes is counted as minimum or maximum value.  -- Description -- SOURCE [Euroroads].  NOTE This attribute only applies when the value in numberOfLanes is not an exact value. "@en ;
         rdfs:domain :NumberOfLanes;
         rdfs:range :MinMaxLaneValue;
         rdfs:label "minMaxNumberOfLanes"@en .
:NumberOfLanes rdfs:subClassOf [ rdf:type owl:Restriction ;
         owl:onProperty :minMaxNumberOfLanes;
         owl:onClass :MinMaxLaneValue;
       owl:maxQualifiedCardinality "1"^^xsd:nonNegativeInteger ;
         ] .
:NumberOfLanes rdfs:subClassOf [ rdf:type owl:Restriction ;
         owl:onProperty :minMaxNumberOfLanes;
         owl:allValuesFrom :MinMaxLaneValue;
         ] .


### http://inspire.ec.europa.eu/ont#NumberOfLanes.numberOfLanes
:NumberOfLanes.numberOfLanes rdf:type owl:DatatypeProperty ;
         skos:definition "-- Definition -- Number of lanes.  -- Description -- SOURCE [Euroroads]."@en ;
         rdfs:domain :NumberOfLanes;
         rdfs:range xsd:integer;
         rdf:type owl:FunctionalProperty;
         rdfs:label "NumberOfLanes.numberOfLanes"@en .
:NumberOfLanes rdfs:subClassOf [ rdf:type owl:Restriction ;
         owl:onProperty :NumberOfLanes.numberOfLanes;
         owl:onDataRange xsd:integer;
       owl:qualifiedCardinality "1"^^xsd:nonNegativeInteger ;
         ] .
:NumberOfLanes rdfs:subClassOf [ rdf:type owl:Restriction ;
         owl:onProperty :NumberOfLanes.numberOfLanes;
         owl:allValuesFrom xsd:integer;
         ] .


### http://inspire.ec.europa.eu/ont:RoadLinkSequence
:RoadLinkSequence a owl:Class ;
         skos:definition "-- Definition -- A linear spatial object, composed of an ordered collection of road links, which represents a continuous path in a road network without any branches. The element has a defined beginning and end and every position on the road link sequence is identifiable with one single parameter such as length. It describes an element of the road network, characterized by one or more thematic identifiers and/or properties. "@en ;
       rdfs:label "RoadLinkSequence"@en .
:RoadLinkSequence rdfs:subClassOf :TransportLinkSequence .

### http://inspire.ec.europa.eu/ont:RoadName
:RoadName a owl:Class ;
         skos:definition "-- Definition -- Name of a road, as assigned by the responsible authority. "@en ;
       rdfs:label "RoadName"@en .
:RoadName rdfs:subClassOf :TransportProperty .

### http://inspire.ec.europa.eu/ont#RoadName.name
:RoadName.name rdf:type owl:ObjectProperty ;
         skos:definition "-- Definition -- Name of the road."@en ;
         rdfs:domain :RoadName;
         rdfs:range :GeographicalName;
         rdf:type owl:FunctionalProperty;
         rdfs:label "RoadName.name"@en .
:RoadName rdfs:subClassOf [ rdf:type owl:Restriction ;
         owl:onProperty :RoadName.name;
         owl:onClass :GeographicalName;
       owl:qualifiedCardinality "1"^^xsd:nonNegativeInteger ;
         ] .
:RoadName rdfs:subClassOf [ rdf:type owl:Restriction ;
         owl:onProperty :RoadName.name;
         owl:allValuesFrom :GeographicalName;
         ] .


### http://inspire.ec.europa.eu/ont:RoadPartValue
:RoadPartValue a owl:Class ;
       rdfs:subClassOf :itnrCodeList ;
          rdfs:isDefinedBy  <https://inspire.ec.europa.eu/codelist/RoadPartValue>;
         skos:definition "-- Definition -- Indication to which part of a road the value of a measurement applies. "@en ;
       rdfs:label "RoadPartValue"@en .

### http://inspire.ec.europa.eu/ont:RoadPartValueCode
:RoadPartValueCode a skos:ConceptScheme ;
         skos:definition "-- Definition -- Indication to which part of a road the value of a measurement applies. "@en ;
          owl:sameAs  <https://inspire.ec.europa.eu/codelist/RoadPartValue>;
       dc:isFormatOf :RoadPartValue .

### http://inspire.ec.europa.eu/ont:RoadPartValue.carriageway
:RoadPartValue.carriageway a :RoadPartValue,skos:Concept ;
         skos:inScheme :RoadPartValueCode ;
         skos:definition "-- Definition -- The part of a road which is reserved for traffic."@en ;
          owl:sameAs  <https://inspire.ec.europa.eu/codelist/RoadPartValue/carriageway>;
          rdfs:isDefinedBy  <https://inspire.ec.europa.eu/codelist/RoadPartValue/carriageway>;
         rdfs:label "carriageway"@no .

### http://inspire.ec.europa.eu/ont:RoadPartValue.pavedSurface
:RoadPartValue.pavedSurface a :RoadPartValue,skos:Concept ;
         skos:inScheme :RoadPartValueCode ;
         skos:definition "-- Definition -- The part of the road which is paved."@en ;
          owl:sameAs  <https://inspire.ec.europa.eu/codelist/RoadPartValue/pavedSurface>;
          rdfs:isDefinedBy  <https://inspire.ec.europa.eu/codelist/RoadPartValue/pavedSurface>;
         rdfs:label "pavedSurface"@no .

### http://inspire.ec.europa.eu/ont:RoadServiceArea
:RoadServiceArea a owl:Class ;
         skos:definition "-- Definition -- Surface annexed to a road and devoted to offer particular services for it.  -- Description -- EXAMPLES Gas station, rest area, toll area. "@en ;
       rdfs:label "RoadServiceArea"@en .
:RoadServiceArea rdfs:subClassOf :TransportArea .

### http://inspire.ec.europa.eu/ont:RoadServiceType
:RoadServiceType a owl:Class ;
         skos:definition "-- Definition -- Description of the type of road service area and the available facilities. "@en ;
       rdfs:label "RoadServiceType"@en .
:RoadServiceType rdfs:subClassOf :TransportProperty .

### http://inspire.ec.europa.eu/ont#availableFacility
:availableFacility rdf:type owl:ObjectProperty ;
         skos:definition "-- Definition -- Facility that is available for a given road service area."@en ;
         rdfs:domain :RoadServiceType;
         rdfs:range :ServiceFacilityValue;
         rdfs:label "availableFacility"@en .
:RoadServiceType rdfs:subClassOf [ rdf:type owl:Restriction ;
         owl:onProperty :availableFacility;
         owl:allValuesFrom :ServiceFacilityValue;
         ] .


### http://inspire.ec.europa.eu/ont#RoadServiceType.type
:RoadServiceType.type rdf:type owl:ObjectProperty ;
         skos:definition "-- Definition -- Type of road service area."@en ;
         rdfs:domain :RoadServiceType;
         rdfs:range :RoadServiceTypeValue;
         rdf:type owl:FunctionalProperty;
         rdfs:label "RoadServiceType.type"@en .
:RoadServiceType rdfs:subClassOf [ rdf:type owl:Restriction ;
         owl:onProperty :RoadServiceType.type;
         owl:onClass :RoadServiceTypeValue;
       owl:qualifiedCardinality "1"^^xsd:nonNegativeInteger ;
         ] .
:RoadServiceType rdfs:subClassOf [ rdf:type owl:Restriction ;
         owl:onProperty :RoadServiceType.type;
         owl:allValuesFrom :RoadServiceTypeValue;
         ] .


### http://inspire.ec.europa.eu/ont:RoadSurfaceCategory
:RoadSurfaceCategory a owl:Class ;
         skos:definition "-- Definition -- Specification of the state of the surface of the associated Road Element. Indicates whether a road is paved or unpaved.  -- Description -- SOURCE [GDF3, Euroroads]. "@en ;
       rdfs:label "RoadSurfaceCategory"@en .
:RoadSurfaceCategory rdfs:subClassOf :TransportProperty .

### http://inspire.ec.europa.eu/ont#surfaceCategory
:surfaceCategory rdf:type owl:ObjectProperty ;
         skos:definition "-- Definition -- Type of road surface."@en ;
         rdfs:domain :RoadSurfaceCategory;
         rdfs:range :RoadSurfaceCategoryValue;
         rdf:type owl:FunctionalProperty;
         rdfs:label "surfaceCategory"@en .
:RoadSurfaceCategory rdfs:subClassOf [ rdf:type owl:Restriction ;
         owl:onProperty :surfaceCategory;
         owl:onClass :RoadSurfaceCategoryValue;
       owl:qualifiedCardinality "1"^^xsd:nonNegativeInteger ;
         ] .
:RoadSurfaceCategory rdfs:subClassOf [ rdf:type owl:Restriction ;
         owl:onProperty :surfaceCategory;
         owl:allValuesFrom :RoadSurfaceCategoryValue;
         ] .


### http://inspire.ec.europa.eu/ont:RoadSurfaceCategoryValue
:RoadSurfaceCategoryValue a owl:Class ;
       rdfs:subClassOf :itnrCodeList ;
          rdfs:isDefinedBy  <https://inspire.ec.europa.eu/codelist/RoadSurfaceCategoryValue>;
         skos:definition "-- Definition -- Values to indicate whether a road is paved or not paved."@en ;
       rdfs:label "RoadSurfaceCategoryValue"@en .

### http://inspire.ec.europa.eu/ont:RoadSurfaceCategoryValueCode
:RoadSurfaceCategoryValueCode a skos:ConceptScheme ;
         skos:definition "-- Definition -- Values to indicate whether a road is paved or not paved."@en ;
          owl:sameAs  <https://inspire.ec.europa.eu/codelist/RoadSurfaceCategoryValue>;
       dc:isFormatOf :RoadSurfaceCategoryValue .

### http://inspire.ec.europa.eu/ont:RoadSurfaceCategoryValue.paved
:RoadSurfaceCategoryValue.paved a :RoadSurfaceCategoryValue,skos:Concept ;
         skos:inScheme :RoadSurfaceCategoryValueCode ;
         skos:definition "-- Definition -- Road with a hard paved surface.  -- Description -- SOURCE [Euroroads].  EXAMPLES Asphalt or concrete. "@en ;
          owl:sameAs  <https://inspire.ec.europa.eu/codelist/RoadSurfaceCategoryValue/paved>;
          rdfs:isDefinedBy  <https://inspire.ec.europa.eu/codelist/RoadSurfaceCategoryValue/paved>;
         rdfs:label "paved"@no .

### http://inspire.ec.europa.eu/ont:RoadSurfaceCategoryValue.unpaved
:RoadSurfaceCategoryValue.unpaved a :RoadSurfaceCategoryValue,skos:Concept ;
         skos:inScheme :RoadSurfaceCategoryValueCode ;
         skos:definition "-- Definition -- Road not paved.  -- Description -- SOURCE [Euroroads].  EXAMPLE Gravelled road. "@en ;
          owl:sameAs  <https://inspire.ec.europa.eu/codelist/RoadSurfaceCategoryValue/unpaved>;
          rdfs:isDefinedBy  <https://inspire.ec.europa.eu/codelist/RoadSurfaceCategoryValue/unpaved>;
         rdfs:label "unpaved"@no .

### http://inspire.ec.europa.eu/ont:RoadWidth
:RoadWidth a owl:Class ;
         skos:definition "-- Definition -- The width of the road, measured as an average value.  -- Description -- SOURCE [Euroroads]. "@en ;
       rdfs:label "RoadWidth"@en .
:RoadWidth rdfs:subClassOf :TransportProperty .

### http://inspire.ec.europa.eu/ont#measuredRoadPart
:measuredRoadPart rdf:type owl:ObjectProperty ;
         skos:definition "-- Definition -- Indicates to which part of a road the value for the attribute 'width' applies."@en ;
         rdfs:domain :RoadWidth;
         rdfs:range :RoadPartValue;
         rdf:type owl:FunctionalProperty;
         rdfs:label "measuredRoadPart"@en .
:RoadWidth rdfs:subClassOf [ rdf:type owl:Restriction ;
         owl:onProperty :measuredRoadPart;
         owl:onClass :RoadPartValue;
       owl:qualifiedCardinality "1"^^xsd:nonNegativeInteger ;
         ] .
:RoadWidth rdfs:subClassOf [ rdf:type owl:Restriction ;
         owl:onProperty :measuredRoadPart;
         owl:allValuesFrom :RoadPartValue;
         ] .


### http://inspire.ec.europa.eu/ont#width
:width rdf:type owl:ObjectProperty ;
         skos:definition "-- Definition -- Road width value."@en ;
         rdfs:domain :RoadWidth;
         rdfs:range <http://def.isotc211.org/iso19103/2015/MeasureTypes#Measure>;
         rdf:type owl:FunctionalProperty;
         rdfs:label "width"@en .
:RoadWidth rdfs:subClassOf [ rdf:type owl:Restriction ;
         owl:onProperty :width;
         owl:onClass <http://def.isotc211.org/iso19103/2015/MeasureTypes#Measure>;
       owl:qualifiedCardinality "1"^^xsd:nonNegativeInteger ;
         ] .
:RoadWidth rdfs:subClassOf [ rdf:type owl:Restriction ;
         owl:onProperty :width;
         owl:allValuesFrom <http://def.isotc211.org/iso19103/2015/MeasureTypes#Measure>;
         ] .


### http://inspire.ec.europa.eu/ont:SpeedLimit
:SpeedLimit a owl:Class ;
         skos:definition "-- Definition -- Limit for the speed of a vehicle on a road..  -- Description -- SOURCE [Euroroads]. "@en ;
       rdfs:label "SpeedLimit"@en .
:SpeedLimit rdfs:subClassOf :TransportProperty .

### http://inspire.ec.europa.eu/ont#areaCondition
:areaCondition rdf:type owl:ObjectProperty ;
         skos:definition "-- Definition -- Speed limit is dependent on environmental circumstances.  -- Description -- SOURCE [Euroroads]."@en ;
         rdfs:domain :SpeedLimit;
         rdfs:range :AreaConditionValue;
         rdfs:label "areaCondition"@en .
:SpeedLimit rdfs:subClassOf [ rdf:type owl:Restriction ;
         owl:onProperty :areaCondition;
         owl:onClass :AreaConditionValue;
       owl:maxQualifiedCardinality "1"^^xsd:nonNegativeInteger ;
         ] .
:SpeedLimit rdfs:subClassOf [ rdf:type owl:Restriction ;
         owl:onProperty :areaCondition;
         owl:allValuesFrom :AreaConditionValue;
         ] .


### http://inspire.ec.europa.eu/ont#SpeedLimit.direction
:SpeedLimit.direction rdf:type owl:ObjectProperty ;
         skos:definition "-- Definition -- Indicates which direction the speed limit is valid for.  -- Description -- SOURCE [Euroroads]. NOTE This attribute only applies when the property is associated with a road link or road link sequence."@en ;
         rdfs:domain :SpeedLimit;
         rdfs:range :LinkDirectionValue;
         rdfs:label "SpeedLimit.direction"@en .
:SpeedLimit rdfs:subClassOf [ rdf:type owl:Restriction ;
         owl:onProperty :SpeedLimit.direction;
         owl:onClass :LinkDirectionValue;
       owl:maxQualifiedCardinality "1"^^xsd:nonNegativeInteger ;
         ] .
:SpeedLimit rdfs:subClassOf [ rdf:type owl:Restriction ;
         owl:onProperty :SpeedLimit.direction;
         owl:allValuesFrom :LinkDirectionValue;
         ] .


### http://inspire.ec.europa.eu/ont#laneExtension
:laneExtension rdf:type owl:DatatypeProperty ;
         skos:definition "-- Definition -- Number of lanes including the start lane counted from the right hand side for which the speed limit applies.  -- Description -- SOURCE [Euroroads]. NOTE This attribute only applies when the property is associated with a road link or road link sequence."@en ;
         rdfs:domain :SpeedLimit;
         rdfs:range xsd:integer;
         rdfs:label "laneExtension"@en .
:SpeedLimit rdfs:subClassOf [ rdf:type owl:Restriction ;
         owl:onProperty :laneExtension;
         owl:onDataRange xsd:integer;
       owl:maxQualifiedCardinality "1"^^xsd:nonNegativeInteger ;
         ] .
:SpeedLimit rdfs:subClassOf [ rdf:type owl:Restriction ;
         owl:onProperty :laneExtension;
         owl:allValuesFrom xsd:integer;
         ] .


### http://inspire.ec.europa.eu/ont#speedLimitMinMaxType
:speedLimitMinMaxType rdf:type owl:ObjectProperty ;
         skos:definition "-- Definition -- Indicates if the speed limit is maximum or minimum and if it is recommended.  -- Description -- SOURCE [Euroroads]."@en ;
         rdfs:domain :SpeedLimit;
         rdfs:range :SpeedLimitMinMaxValue;
         rdf:type owl:FunctionalProperty;
         rdfs:label "speedLimitMinMaxType"@en .
:SpeedLimit rdfs:subClassOf [ rdf:type owl:Restriction ;
         owl:onProperty :speedLimitMinMaxType;
         owl:onClass :SpeedLimitMinMaxValue;
       owl:qualifiedCardinality "1"^^xsd:nonNegativeInteger ;
         ] .
:SpeedLimit rdfs:subClassOf [ rdf:type owl:Restriction ;
         owl:onProperty :speedLimitMinMaxType;
         owl:allValuesFrom :SpeedLimitMinMaxValue;
         ] .


### http://inspire.ec.europa.eu/ont#speedLimitSource
:speedLimitSource rdf:type owl:ObjectProperty ;
         skos:definition "-- Definition -- Source for speed limit.  -- Description -- SOURCE [Euroroads]."@en ;
         rdfs:domain :SpeedLimit;
         rdfs:range :SpeedLimitSourceValue;
         rdfs:label "speedLimitSource"@en .
:SpeedLimit rdfs:subClassOf [ rdf:type owl:Restriction ;
         owl:onProperty :speedLimitSource;
         owl:onClass :SpeedLimitSourceValue;
       owl:maxQualifiedCardinality "1"^^xsd:nonNegativeInteger ;
         ] .
:SpeedLimit rdfs:subClassOf [ rdf:type owl:Restriction ;
         owl:onProperty :speedLimitSource;
         owl:allValuesFrom :SpeedLimitSourceValue;
         ] .


### http://inspire.ec.europa.eu/ont#speedLimitValue
:speedLimitValue rdf:type owl:ObjectProperty ;
         skos:definition "-- Definition -- Value for speed limit.  -- Description -- SOURCE [Euroroads]."@en ;
         rdfs:domain :SpeedLimit;
         rdfs:range <http://def.isotc211.org/iso19103/2015/MeasureTypes#Velocity>;
         rdf:type owl:FunctionalProperty;
         rdfs:label "speedLimitValue"@en .
:SpeedLimit rdfs:subClassOf [ rdf:type owl:Restriction ;
         owl:onProperty :speedLimitValue;
         owl:onClass <http://def.isotc211.org/iso19103/2015/MeasureTypes#Velocity>;
       owl:qualifiedCardinality "1"^^xsd:nonNegativeInteger ;
         ] .
:SpeedLimit rdfs:subClassOf [ rdf:type owl:Restriction ;
         owl:onProperty :speedLimitValue;
         owl:allValuesFrom <http://def.isotc211.org/iso19103/2015/MeasureTypes#Velocity>;
         ] .


### http://inspire.ec.europa.eu/ont#startLane
:startLane rdf:type owl:DatatypeProperty ;
         skos:definition "-- Definition -- Start lane counted from the right side for which speed limit applies.  -- Description -- SOURCE [Euroroads]. NOTE This attribute only applies when the property is associated with a road link or road link sequence."@en ;
         rdfs:domain :SpeedLimit;
         rdfs:range xsd:integer;
         rdfs:label "startLane"@en .
:SpeedLimit rdfs:subClassOf [ rdf:type owl:Restriction ;
         owl:onProperty :startLane;
         owl:onDataRange xsd:integer;
       owl:maxQualifiedCardinality "1"^^xsd:nonNegativeInteger ;
         ] .
:SpeedLimit rdfs:subClassOf [ rdf:type owl:Restriction ;
         owl:onProperty :startLane;
         owl:allValuesFrom xsd:integer;
         ] .


### http://inspire.ec.europa.eu/ont#validityPeriod
:validityPeriod rdf:type owl:ObjectProperty ;
         skos:definition "-- Definition -- Period during which the speed limit is valid."@en ;
         rdfs:domain :SpeedLimit;
         rdfs:range <http://def.isotc211.org/iso19108/2006/TemporalObjects#TM_Period>;
         rdfs:label "validityPeriod"@en .
:SpeedLimit rdfs:subClassOf [ rdf:type owl:Restriction ;
         owl:onProperty :validityPeriod;
         owl:onClass <http://def.isotc211.org/iso19108/2006/TemporalObjects#TM_Period>;
       owl:maxQualifiedCardinality "1"^^xsd:nonNegativeInteger ;
         ] .
:SpeedLimit rdfs:subClassOf [ rdf:type owl:Restriction ;
         owl:onProperty :validityPeriod;
         owl:allValuesFrom <http://def.isotc211.org/iso19108/2006/TemporalObjects#TM_Period>;
         ] .


### http://inspire.ec.europa.eu/ont#vehicleType
:vehicleType rdf:type owl:ObjectProperty ;
         skos:definition "-- Definition -- Vehicle type the speed limit is restricted to.  -- Description -- SOURCE Adapted from [Euroroads]. "@en ;
         rdfs:domain :SpeedLimit;
         rdfs:range :VehicleTypeValue;
         rdfs:label "vehicleType"@en .
:SpeedLimit rdfs:subClassOf [ rdf:type owl:Restriction ;
         owl:onProperty :vehicleType;
         owl:onClass :VehicleTypeValue;
       owl:maxQualifiedCardinality "1"^^xsd:nonNegativeInteger ;
         ] .
:SpeedLimit rdfs:subClassOf [ rdf:type owl:Restriction ;
         owl:onProperty :vehicleType;
         owl:allValuesFrom :VehicleTypeValue;
         ] .


### http://inspire.ec.europa.eu/ont#weatherCondition
:weatherCondition rdf:type owl:ObjectProperty ;
         skos:definition "-- Definition -- Weather condition the speed limit is dependent on.  -- Description -- SOURCE Adapted from [Euroroads]. "@en ;
         rdfs:domain :SpeedLimit;
         rdfs:range :WeatherConditionValue;
         rdfs:label "weatherCondition"@en .
:SpeedLimit rdfs:subClassOf [ rdf:type owl:Restriction ;
         owl:onProperty :weatherCondition;
         owl:onClass :WeatherConditionValue;
       owl:maxQualifiedCardinality "1"^^xsd:nonNegativeInteger ;
         ] .
:SpeedLimit rdfs:subClassOf [ rdf:type owl:Restriction ;
         owl:onProperty :weatherCondition;
         owl:allValuesFrom :WeatherConditionValue;
         ] .


### http://inspire.ec.europa.eu/ont:SpeedLimitMinMaxValue
:SpeedLimitMinMaxValue a owl:Class ;
       rdfs:subClassOf :itnrEnumeration ;
          rdfs:isDefinedBy  <https://inspire.ec.europa.eu/enumeration/SpeedLimitMinMaxValue>;
         skos:definition "-- Definition -- Possible values to indicate the nature of a speed limit."@en ;
       rdfs:label "SpeedLimitMinMaxValue"@en .

### http://inspire.ec.europa.eu/ont:SpeedLimitMinMaxValueCode
:SpeedLimitMinMaxValueCode a skos:ConceptScheme ;
         skos:definition "-- Definition -- Possible values to indicate the nature of a speed limit."@en ;
          owl:sameAs  <https://inspire.ec.europa.eu/enumeration/SpeedLimitMinMaxValue>;
       dc:isFormatOf :SpeedLimitMinMaxValue .

### http://inspire.ec.europa.eu/ont:SpeedLimitMinMaxValue.maximum
:SpeedLimitMinMaxValue.maximum a :SpeedLimitMinMaxValue,skos:Concept ;
         skos:inScheme :SpeedLimitMinMaxValueCode ;
         skos:definition "-- Definition -- Speed limit is a maximum value  -- Description -- SOURCE [Euroroads]. "@en ;
          owl:sameAs  <https://inspire.ec.europa.eu/enumeration/SpeedLimitMinMaxValue/maximum>;
          rdfs:isDefinedBy  <https://inspire.ec.europa.eu/enumeration/SpeedLimitMinMaxValue/maximum>;
         rdfs:label "maximum"@no .

### http://inspire.ec.europa.eu/ont:SpeedLimitMinMaxValue.minimum
:SpeedLimitMinMaxValue.minimum a :SpeedLimitMinMaxValue,skos:Concept ;
         skos:inScheme :SpeedLimitMinMaxValueCode ;
         skos:definition "-- Definition -- Speed limit is a minimum value  -- Description -- SOURCE [Euroroads]. "@en ;
          owl:sameAs  <https://inspire.ec.europa.eu/enumeration/SpeedLimitMinMaxValue/minimum>;
          rdfs:isDefinedBy  <https://inspire.ec.europa.eu/enumeration/SpeedLimitMinMaxValue/minimum>;
         rdfs:label "minimum"@no .

### http://inspire.ec.europa.eu/ont:SpeedLimitMinMaxValue.recommendedMaximum
:SpeedLimitMinMaxValue.recommendedMaximum a :SpeedLimitMinMaxValue,skos:Concept ;
         skos:inScheme :SpeedLimitMinMaxValueCode ;
         skos:definition "-- Definition -- Speed limit is a recommended maximum value  -- Description -- SOURCE [Euroroads]. "@en ;
          owl:sameAs  <https://inspire.ec.europa.eu/enumeration/SpeedLimitMinMaxValue/recommendedMaximum>;
          rdfs:isDefinedBy  <https://inspire.ec.europa.eu/enumeration/SpeedLimitMinMaxValue/recommendedMaximum>;
         rdfs:label "recommendedMaximum"@no .

### http://inspire.ec.europa.eu/ont:SpeedLimitMinMaxValue.recommendedMinimum
:SpeedLimitMinMaxValue.recommendedMinimum a :SpeedLimitMinMaxValue,skos:Concept ;
         skos:inScheme :SpeedLimitMinMaxValueCode ;
         skos:definition "-- Definition -- Speed limit is a recommended minimum value  -- Description -- SOURCE [Euroroads]. "@en ;
          owl:sameAs  <https://inspire.ec.europa.eu/enumeration/SpeedLimitMinMaxValue/recommendedMinimum>;
          rdfs:isDefinedBy  <https://inspire.ec.europa.eu/enumeration/SpeedLimitMinMaxValue/recommendedMinimum>;
         rdfs:label "recommendedMinimum"@no .
:SpeedLimitMinMaxValue owl:oneOf ( :SpeedLimitMinMaxValue.maximum :SpeedLimitMinMaxValue.minimum :SpeedLimitMinMaxValue.recommendedMaximum :SpeedLimitMinMaxValue.recommendedMinimum  ) ; .

### http://inspire.ec.europa.eu/ont:SpeedLimitSourceValue
:SpeedLimitSourceValue a owl:Class ;
       rdfs:subClassOf :itnrCodeList ;
          rdfs:isDefinedBy  <https://inspire.ec.europa.eu/codelist/SpeedLimitSourceValue>;
         skos:definition "-- Definition -- Possible sources for speed limits."@en ;
       rdfs:label "SpeedLimitSourceValue"@en .

### http://inspire.ec.europa.eu/ont:SpeedLimitSourceValueCode
:SpeedLimitSourceValueCode a skos:ConceptScheme ;
         skos:definition "-- Definition -- Possible sources for speed limits."@en ;
          owl:sameAs  <https://inspire.ec.europa.eu/codelist/SpeedLimitSourceValue>;
       dc:isFormatOf :SpeedLimitSourceValue .

### http://inspire.ec.europa.eu/ont:SpeedLimitSourceValue.fixedTrafficSign
:SpeedLimitSourceValue.fixedTrafficSign a :SpeedLimitSourceValue,skos:Concept ;
         skos:inScheme :SpeedLimitSourceValueCode ;
         skos:definition "-- Definition -- Source is a fixed traffic sign (site specific administrative order, explicit speed limit).  -- Description -- SOURCE [Euroroads]. "@en ;
          owl:sameAs  <https://inspire.ec.europa.eu/codelist/SpeedLimitSourceValue/fixedTrafficSign>;
          rdfs:isDefinedBy  <https://inspire.ec.europa.eu/codelist/SpeedLimitSourceValue/fixedTrafficSign>;
         rdfs:label "fixedTrafficSign"@no .

### http://inspire.ec.europa.eu/ont:SpeedLimitSourceValue.regulation
:SpeedLimitSourceValue.regulation a :SpeedLimitSourceValue,skos:Concept ;
         skos:inScheme :SpeedLimitSourceValueCode ;
         skos:definition "-- Definition -- Source is a regulation (national regulation, rule or 'implicit speed limit').  -- Description -- SOURCE [Euroroads]."@en ;
          owl:sameAs  <https://inspire.ec.europa.eu/codelist/SpeedLimitSourceValue/regulation>;
          rdfs:isDefinedBy  <https://inspire.ec.europa.eu/codelist/SpeedLimitSourceValue/regulation>;
         rdfs:label "regulation"@no .

### http://inspire.ec.europa.eu/ont:SpeedLimitSourceValue.variableTrafficSign
:SpeedLimitSourceValue.variableTrafficSign a :SpeedLimitSourceValue,skos:Concept ;
         skos:inScheme :SpeedLimitSourceValueCode ;
         skos:definition "-- Definition -- Source is a variable traffic sign.  -- Description -- SOURCE [Euroroads]."@en ;
          owl:sameAs  <https://inspire.ec.europa.eu/codelist/SpeedLimitSourceValue/variableTrafficSign>;
          rdfs:isDefinedBy  <https://inspire.ec.europa.eu/codelist/SpeedLimitSourceValue/variableTrafficSign>;
         rdfs:label "variableTrafficSign"@no .

### http://inspire.ec.europa.eu/ont:VehicleTrafficArea
:VehicleTrafficArea a owl:Class ;
         skos:definition "-- Definition -- Surface that represents the part of a road which is used for the normal traffic of vehicles."@en ;
       rdfs:label "VehicleTrafficArea"@en .
:VehicleTrafficArea rdfs:subClassOf :TransportArea .

### http://inspire.ec.europa.eu/ont:VehicleTypeValue
:VehicleTypeValue a owl:Class ;
       rdfs:subClassOf :itnrCodeList ;
          rdfs:isDefinedBy  <https://inspire.ec.europa.eu/codelist/VehicleTypeValue>;
         skos:definition "-- Definition -- Possible types of vehicles."@en ;
       rdfs:label "VehicleTypeValue"@en .

### http://inspire.ec.europa.eu/ont:VehicleTypeValueCode
:VehicleTypeValueCode a skos:ConceptScheme ;
         skos:definition "-- Definition -- Possible types of vehicles."@en ;
          owl:sameAs  <https://inspire.ec.europa.eu/codelist/VehicleTypeValue>;
       dc:isFormatOf :VehicleTypeValue .

### http://inspire.ec.europa.eu/ont:VehicleTypeValue.allVehicle
:VehicleTypeValue.allVehicle a :VehicleTypeValue,skos:Concept ;
         skos:inScheme :VehicleTypeValueCode ;
         skos:definition "-- Definition -- Any vehicle, not including pedestrians.  -- Description -- SOURCE [Euroroads]."@en ;
          owl:sameAs  <https://inspire.ec.europa.eu/codelist/VehicleTypeValue/allVehicle>;
          rdfs:isDefinedBy  <https://inspire.ec.europa.eu/codelist/VehicleTypeValue/allVehicle>;
         rdfs:label "allVehicle"@no .

### http://inspire.ec.europa.eu/ont:VehicleTypeValue.bicycle
:VehicleTypeValue.bicycle a :VehicleTypeValue,skos:Concept ;
         skos:inScheme :VehicleTypeValueCode ;
         skos:definition "-- Definition -- pedal-driven two-wheeled vehicle.  -- Description -- SOURCE [Euroroads]."@en ;
          owl:sameAs  <https://inspire.ec.europa.eu/codelist/VehicleTypeValue/bicycle>;
          rdfs:isDefinedBy  <https://inspire.ec.europa.eu/codelist/VehicleTypeValue/bicycle>;
         rdfs:label "bicycle"@no .

### http://inspire.ec.europa.eu/ont:VehicleTypeValue.carWithTrailer
:VehicleTypeValue.carWithTrailer a :VehicleTypeValue,skos:Concept ;
         skos:inScheme :VehicleTypeValueCode ;
         skos:definition "-- Definition -- A passenger car with an attached trailer.  -- Description -- SOURCE [Euroroads]."@en ;
          owl:sameAs  <https://inspire.ec.europa.eu/codelist/VehicleTypeValue/carWithTrailer>;
          rdfs:isDefinedBy  <https://inspire.ec.europa.eu/codelist/VehicleTypeValue/carWithTrailer>;
         rdfs:label "carWithTrailer"@no .

### http://inspire.ec.europa.eu/ont:VehicleTypeValue.deliveryTruck
:VehicleTypeValue.deliveryTruck a :VehicleTypeValue,skos:Concept ;
         skos:inScheme :VehicleTypeValueCode ;
         skos:definition "-- Definition -- A truck vehicle of relatively small size, whose principal use is for delivery of goods and materials.  -- Description -- SOURCE [Euroroads]."@en ;
          owl:sameAs  <https://inspire.ec.europa.eu/codelist/VehicleTypeValue/deliveryTruck>;
          rdfs:isDefinedBy  <https://inspire.ec.europa.eu/codelist/VehicleTypeValue/deliveryTruck>;
         rdfs:label "deliveryTruck"@no .

### http://inspire.ec.europa.eu/ont:VehicleTypeValue.emergencyVehicle
:VehicleTypeValue.emergencyVehicle a :VehicleTypeValue,skos:Concept ;
         skos:inScheme :VehicleTypeValueCode ;
         skos:definition "-- Definition -- A vehicle engaged in emergency response, included but not limited to police, ambulance and fire.  -- Description -- SOURCE [Euroroads]."@en ;
          owl:sameAs  <https://inspire.ec.europa.eu/codelist/VehicleTypeValue/emergencyVehicle>;
          rdfs:isDefinedBy  <https://inspire.ec.europa.eu/codelist/VehicleTypeValue/emergencyVehicle>;
         rdfs:label "emergencyVehicle"@no .

### http://inspire.ec.europa.eu/ont:VehicleTypeValue.employeeVehicle
:VehicleTypeValue.employeeVehicle a :VehicleTypeValue,skos:Concept ;
         skos:inScheme :VehicleTypeValueCode ;
         skos:definition "-- Definition -- A vehicle operated by an employee of an organization that is used within that organization's ground.  -- Description -- SOURCE [Euroroads]."@en ;
          owl:sameAs  <https://inspire.ec.europa.eu/codelist/VehicleTypeValue/employeeVehicle>;
          rdfs:isDefinedBy  <https://inspire.ec.europa.eu/codelist/VehicleTypeValue/employeeVehicle>;
         rdfs:label "employeeVehicle"@no .

### http://inspire.ec.europa.eu/ont:VehicleTypeValue.facilityVehicle
:VehicleTypeValue.facilityVehicle a :VehicleTypeValue,skos:Concept ;
         skos:inScheme :VehicleTypeValueCode ;
         skos:definition "-- Definition -- A vehicle dedicated to a localized area within a private or restricted estate.  -- Description -- SOURCE [Euroroads].  EXAMPLE Facilities roads within an airport or theme park. "@en ;
          owl:sameAs  <https://inspire.ec.europa.eu/codelist/VehicleTypeValue/facilityVehicle>;
          rdfs:isDefinedBy  <https://inspire.ec.europa.eu/codelist/VehicleTypeValue/facilityVehicle>;
         rdfs:label "facilityVehicle"@no .

### http://inspire.ec.europa.eu/ont:VehicleTypeValue.farmVehicle
:VehicleTypeValue.farmVehicle a :VehicleTypeValue,skos:Concept ;
         skos:inScheme :VehicleTypeValueCode ;
         skos:definition "-- Definition -- Vehicle commonly associated with farming activities.  -- Description -- SOURCE [Euroroads]."@en ;
          owl:sameAs  <https://inspire.ec.europa.eu/codelist/VehicleTypeValue/farmVehicle>;
          rdfs:isDefinedBy  <https://inspire.ec.europa.eu/codelist/VehicleTypeValue/farmVehicle>;
         rdfs:label "farmVehicle"@no .

### http://inspire.ec.europa.eu/ont:VehicleTypeValue.highOccupancyVehicle
:VehicleTypeValue.highOccupancyVehicle a :VehicleTypeValue,skos:Concept ;
         skos:inScheme :VehicleTypeValueCode ;
         skos:definition "-- Definition -- Vehicle populated with a number of occupants corresponding to (or exceeding) the specified minimum number of passengers.  -- Description -- SOURCE [Euroroads]."@en ;
          owl:sameAs  <https://inspire.ec.europa.eu/codelist/VehicleTypeValue/highOccupancyVehicle>;
          rdfs:isDefinedBy  <https://inspire.ec.europa.eu/codelist/VehicleTypeValue/highOccupancyVehicle>;
         rdfs:label "highOccupancyVehicle"@no .

### http://inspire.ec.europa.eu/ont:VehicleTypeValue.lightRail
:VehicleTypeValue.lightRail a :VehicleTypeValue,skos:Concept ;
         skos:inScheme :VehicleTypeValueCode ;
         skos:definition "-- Definition -- Train-like transport vehicle limited to a rail network within a limited area.  -- Description -- SOURCE [Euroroads].  NOTE Does not include heavy rail lines. "@en ;
          owl:sameAs  <https://inspire.ec.europa.eu/codelist/VehicleTypeValue/lightRail>;
          rdfs:isDefinedBy  <https://inspire.ec.europa.eu/codelist/VehicleTypeValue/lightRail>;
         rdfs:label "lightRail"@no .

### http://inspire.ec.europa.eu/ont:VehicleTypeValue.mailVehicle
:VehicleTypeValue.mailVehicle a :VehicleTypeValue,skos:Concept ;
         skos:inScheme :VehicleTypeValueCode ;
         skos:definition "-- Definition -- A vehicle that collects, carries or delivers mail.  -- Description -- SOURCE [Euroroads]."@en ;
          owl:sameAs  <https://inspire.ec.europa.eu/codelist/VehicleTypeValue/mailVehicle>;
          rdfs:isDefinedBy  <https://inspire.ec.europa.eu/codelist/VehicleTypeValue/mailVehicle>;
         rdfs:label "mailVehicle"@no .

### http://inspire.ec.europa.eu/ont:VehicleTypeValue.militaryVehicle
:VehicleTypeValue.militaryVehicle a :VehicleTypeValue,skos:Concept ;
         skos:inScheme :VehicleTypeValueCode ;
         skos:definition "-- Definition -- Vehicle authorized by a military authority.  -- Description -- SOURCE [Euroroads]."@en ;
          owl:sameAs  <https://inspire.ec.europa.eu/codelist/VehicleTypeValue/militaryVehicle>;
          rdfs:isDefinedBy  <https://inspire.ec.europa.eu/codelist/VehicleTypeValue/militaryVehicle>;
         rdfs:label "militaryVehicle"@no .

### http://inspire.ec.europa.eu/ont:VehicleTypeValue.moped
:VehicleTypeValue.moped a :VehicleTypeValue,skos:Concept ;
         skos:inScheme :VehicleTypeValueCode ;
         skos:definition "-- Definition -- Two or three wheeled vehicle equipped with internal combustion engine, with size less than 50 cc and maximum speed that does not exceed 45 km/h (28mph).   -- Description -- SOURCE Adapted from [CADaS/CARE]."@en ;
          owl:sameAs  <https://inspire.ec.europa.eu/codelist/VehicleTypeValue/moped>;
          rdfs:isDefinedBy  <https://inspire.ec.europa.eu/codelist/VehicleTypeValue/moped>;
         rdfs:label "moped"@no .

### http://inspire.ec.europa.eu/ont:VehicleTypeValue.motorcycle
:VehicleTypeValue.motorcycle a :VehicleTypeValue,skos:Concept ;
         skos:inScheme :VehicleTypeValueCode ;
         skos:definition "-- Definition -- Two or three wheeled vehicle equipped with internal combustion engine, with size more than 50 cc and maximum speed that does exceed 45 km/h (28mph).  -- Description -- SOURCE Adapted from [CADaS/CARE]."@en ;
          owl:sameAs  <https://inspire.ec.europa.eu/codelist/VehicleTypeValue/motorcycle>;
          rdfs:isDefinedBy  <https://inspire.ec.europa.eu/codelist/VehicleTypeValue/motorcycle>;
         rdfs:label "motorcycle"@no .

### http://inspire.ec.europa.eu/ont:VehicleTypeValue.passengerCar
:VehicleTypeValue.passengerCar a :VehicleTypeValue,skos:Concept ;
         skos:inScheme :VehicleTypeValueCode ;
         skos:definition "-- Definition -- A small vehicle designed for private transport of people.  -- Description -- SOURCE [Euroroads]."@en ;
          owl:sameAs  <https://inspire.ec.europa.eu/codelist/VehicleTypeValue/passengerCar>;
          rdfs:isDefinedBy  <https://inspire.ec.europa.eu/codelist/VehicleTypeValue/passengerCar>;
         rdfs:label "passengerCar"@no .

### http://inspire.ec.europa.eu/ont:VehicleTypeValue.pedestrian
:VehicleTypeValue.pedestrian a :VehicleTypeValue,skos:Concept ;
         skos:inScheme :VehicleTypeValueCode ;
         skos:definition "-- Definition -- A person on foot.  -- Description -- SOURCE [Euroroads]."@en ;
          owl:sameAs  <https://inspire.ec.europa.eu/codelist/VehicleTypeValue/pedestrian>;
          rdfs:isDefinedBy  <https://inspire.ec.europa.eu/codelist/VehicleTypeValue/pedestrian>;
         rdfs:label "pedestrian"@no .

### http://inspire.ec.europa.eu/ont:VehicleTypeValue.privateBus
:VehicleTypeValue.privateBus a :VehicleTypeValue,skos:Concept ;
         skos:inScheme :VehicleTypeValueCode ;
         skos:definition "-- Definition -- A vehicle designed for transport of large groups of people, privately owned or chartered.  -- Description -- SOURCE [Euroroads]."@en ;
          owl:sameAs  <https://inspire.ec.europa.eu/codelist/VehicleTypeValue/privateBus>;
          rdfs:isDefinedBy  <https://inspire.ec.europa.eu/codelist/VehicleTypeValue/privateBus>;
         rdfs:label "privateBus"@no .

### http://inspire.ec.europa.eu/ont:VehicleTypeValue.publicBus
:VehicleTypeValue.publicBus a :VehicleTypeValue,skos:Concept ;
         skos:inScheme :VehicleTypeValueCode ;
         skos:definition "-- Definition -- A vehicle designed for transport of large groups of people that is generally charterized by published routes and schedules.  -- Description -- SOURCE [Euroroads]."@en ;
          owl:sameAs  <https://inspire.ec.europa.eu/codelist/VehicleTypeValue/publicBus>;
          rdfs:isDefinedBy  <https://inspire.ec.europa.eu/codelist/VehicleTypeValue/publicBus>;
         rdfs:label "publicBus"@no .

### http://inspire.ec.europa.eu/ont:VehicleTypeValue.residentialVehicle
:VehicleTypeValue.residentialVehicle a :VehicleTypeValue,skos:Concept ;
         skos:inScheme :VehicleTypeValueCode ;
         skos:definition "-- Definition -- A vehicle whose owner is resident (or a guest) of particular street or town area.  -- Description -- SOURCE [Euroroads]."@en ;
          owl:sameAs  <https://inspire.ec.europa.eu/codelist/VehicleTypeValue/residentialVehicle>;
          rdfs:isDefinedBy  <https://inspire.ec.europa.eu/codelist/VehicleTypeValue/residentialVehicle>;
         rdfs:label "residentialVehicle"@no .

### http://inspire.ec.europa.eu/ont:VehicleTypeValue.schoolBus
:VehicleTypeValue.schoolBus a :VehicleTypeValue,skos:Concept ;
         skos:inScheme :VehicleTypeValueCode ;
         skos:definition "-- Definition -- Vehicle operated on behalf of a school to transport students.  -- Description -- SOURCE [Euroroads]."@en ;
          owl:sameAs  <https://inspire.ec.europa.eu/codelist/VehicleTypeValue/schoolBus>;
          rdfs:isDefinedBy  <https://inspire.ec.europa.eu/codelist/VehicleTypeValue/schoolBus>;
         rdfs:label "schoolBus"@no .

### http://inspire.ec.europa.eu/ont:VehicleTypeValue.snowChainEquippedVehicle
:VehicleTypeValue.snowChainEquippedVehicle a :VehicleTypeValue,skos:Concept ;
         skos:inScheme :VehicleTypeValueCode ;
         skos:definition "-- Definition -- Any vehicle equipped with snow chains.  -- Description -- SOURCE [Euroroads]."@en ;
          owl:sameAs  <https://inspire.ec.europa.eu/codelist/VehicleTypeValue/snowChainEquippedVehicle>;
          rdfs:isDefinedBy  <https://inspire.ec.europa.eu/codelist/VehicleTypeValue/snowChainEquippedVehicle>;
         rdfs:label "snowChainEquippedVehicle"@no .

### http://inspire.ec.europa.eu/ont:VehicleTypeValue.tanker
:VehicleTypeValue.tanker a :VehicleTypeValue,skos:Concept ;
         skos:inScheme :VehicleTypeValueCode ;
         skos:definition "-- Definition -- A truck with more than two axels used to transport liquid loads in bulk.  -- Description -- SOURCE [Euroroads]."@en ;
          owl:sameAs  <https://inspire.ec.europa.eu/codelist/VehicleTypeValue/tanker>;
          rdfs:isDefinedBy  <https://inspire.ec.europa.eu/codelist/VehicleTypeValue/tanker>;
         rdfs:label "tanker"@no .

### http://inspire.ec.europa.eu/ont:VehicleTypeValue.taxi
:VehicleTypeValue.taxi a :VehicleTypeValue,skos:Concept ;
         skos:inScheme :VehicleTypeValueCode ;
         skos:definition "-- Definition -- A vehicle licensed for hire usually fitted with a meter.  -- Description -- SOURCE [Euroroads]."@en ;
          owl:sameAs  <https://inspire.ec.europa.eu/codelist/VehicleTypeValue/taxi>;
          rdfs:isDefinedBy  <https://inspire.ec.europa.eu/codelist/VehicleTypeValue/taxi>;
         rdfs:label "taxi"@no .

### http://inspire.ec.europa.eu/ont:VehicleTypeValue.transportTruck
:VehicleTypeValue.transportTruck a :VehicleTypeValue,skos:Concept ;
         skos:inScheme :VehicleTypeValueCode ;
         skos:definition "-- Definition -- A truck vehicle for long range transport of goods.  -- Description -- SOURCE [Euroroads]."@en ;
          owl:sameAs  <https://inspire.ec.europa.eu/codelist/VehicleTypeValue/transportTruck>;
          rdfs:isDefinedBy  <https://inspire.ec.europa.eu/codelist/VehicleTypeValue/transportTruck>;
         rdfs:label "transportTruck"@no .

### http://inspire.ec.europa.eu/ont:VehicleTypeValue.trolleyBus
:VehicleTypeValue.trolleyBus a :VehicleTypeValue,skos:Concept ;
         skos:inScheme :VehicleTypeValueCode ;
         skos:definition "-- Definition -- A bus-like mass transport vehicle hooked up to an electrical network for power supply.  -- Description -- SOURCE [Euroroads]."@en ;
          owl:sameAs  <https://inspire.ec.europa.eu/codelist/VehicleTypeValue/trolleyBus>;
          rdfs:isDefinedBy  <https://inspire.ec.europa.eu/codelist/VehicleTypeValue/trolleyBus>;
         rdfs:label "trolleyBus"@no .

### http://inspire.ec.europa.eu/ont:VehicleTypeValue.vehicleForDisabledPerson
:VehicleTypeValue.vehicleForDisabledPerson a :VehicleTypeValue,skos:Concept ;
         skos:inScheme :VehicleTypeValueCode ;
         skos:definition "-- Definition -- A vehicle with supporting identification that designates a vehicle for disabled persons.  -- Description -- SOURCE [Euroroads]."@en ;
          owl:sameAs  <https://inspire.ec.europa.eu/codelist/VehicleTypeValue/vehicleForDisabledPerson>;
          rdfs:isDefinedBy  <https://inspire.ec.europa.eu/codelist/VehicleTypeValue/vehicleForDisabledPerson>;
         rdfs:label "vehicleForDisabledPerson"@no .

### http://inspire.ec.europa.eu/ont:VehicleTypeValue.vehicleWithExplosiveLoad
:VehicleTypeValue.vehicleWithExplosiveLoad a :VehicleTypeValue,skos:Concept ;
         skos:inScheme :VehicleTypeValueCode ;
         skos:definition "-- Definition -- Vehicle transporting explosive cargo.  -- Description -- SOURCE [Euroroads]."@en ;
          owl:sameAs  <https://inspire.ec.europa.eu/codelist/VehicleTypeValue/vehicleWithExplosiveLoad>;
          rdfs:isDefinedBy  <https://inspire.ec.europa.eu/codelist/VehicleTypeValue/vehicleWithExplosiveLoad>;
         rdfs:label "vehicleWithExplosiveLoad"@no .

### http://inspire.ec.europa.eu/ont:VehicleTypeValue.vehicleWithOtherDangerousLoad
:VehicleTypeValue.vehicleWithOtherDangerousLoad a :VehicleTypeValue,skos:Concept ;
         skos:inScheme :VehicleTypeValueCode ;
         skos:definition "-- Definition -- Vehicle transporting dangerous cargo, other than explosive or waterpollution loads.  -- Description -- SOURCE [Euroroads]."@en ;
          owl:sameAs  <https://inspire.ec.europa.eu/codelist/VehicleTypeValue/vehicleWithOtherDangerousLoad>;
          rdfs:isDefinedBy  <https://inspire.ec.europa.eu/codelist/VehicleTypeValue/vehicleWithOtherDangerousLoad>;
         rdfs:label "vehicleWithOtherDangerousLoad"@no .

### http://inspire.ec.europa.eu/ont:VehicleTypeValue.vehicleWithWaterPollutingLoad
:VehicleTypeValue.vehicleWithWaterPollutingLoad a :VehicleTypeValue,skos:Concept ;
         skos:inScheme :VehicleTypeValueCode ;
         skos:definition "-- Definition -- Vehicle transporting water-polluting cargo.  -- Description -- SOURCE [Euroroads]."@en ;
          owl:sameAs  <https://inspire.ec.europa.eu/codelist/VehicleTypeValue/vehicleWithWaterPollutingLoad>;
          rdfs:isDefinedBy  <https://inspire.ec.europa.eu/codelist/VehicleTypeValue/vehicleWithWaterPollutingLoad>;
         rdfs:label "vehicleWithWaterPollutingLoad"@no .

### http://inspire.ec.europa.eu/ont:WeatherConditionValue
:WeatherConditionValue a owl:Class ;
       rdfs:subClassOf :itnrCodeList ;
          rdfs:isDefinedBy  <https://inspire.ec.europa.eu/codelist/WeatherConditionValue>;
         skos:definition "-- Definition -- Values to indicate weather conditions that affect speed limits."@en ;
       rdfs:label "WeatherConditionValue"@en .

### http://inspire.ec.europa.eu/ont:WeatherConditionValueCode
:WeatherConditionValueCode a skos:ConceptScheme ;
         skos:definition "-- Definition -- Values to indicate weather conditions that affect speed limits."@en ;
          owl:sameAs  <https://inspire.ec.europa.eu/codelist/WeatherConditionValue>;
       dc:isFormatOf :WeatherConditionValue .

### http://inspire.ec.europa.eu/ont:WeatherConditionValue.fog
:WeatherConditionValue.fog a :WeatherConditionValue,skos:Concept ;
         skos:inScheme :WeatherConditionValueCode ;
         skos:definition "-- Definition -- Speed applies when fog is present.  -- Description -- SOURCE Adapted from [Euroroads]."@en ;
          owl:sameAs  <https://inspire.ec.europa.eu/codelist/WeatherConditionValue/fog>;
          rdfs:isDefinedBy  <https://inspire.ec.europa.eu/codelist/WeatherConditionValue/fog>;
         rdfs:label "fog"@no .

### http://inspire.ec.europa.eu/ont:WeatherConditionValue.ice
:WeatherConditionValue.ice a :WeatherConditionValue,skos:Concept ;
         skos:inScheme :WeatherConditionValueCode ;
         skos:definition "-- Definition -- Speed applies when ice is present.  -- Description -- SOURCE Adapted from [Euroroads]."@en ;
          owl:sameAs  <https://inspire.ec.europa.eu/codelist/WeatherConditionValue/ice>;
          rdfs:isDefinedBy  <https://inspire.ec.europa.eu/codelist/WeatherConditionValue/ice>;
         rdfs:label "ice"@no .

### http://inspire.ec.europa.eu/ont:WeatherConditionValue.rain
:WeatherConditionValue.rain a :WeatherConditionValue,skos:Concept ;
         skos:inScheme :WeatherConditionValueCode ;
         skos:definition "-- Definition -- Speed applies when rain is present.  -- Description -- SOURCE Adapted from [Euroroads]."@en ;
          owl:sameAs  <https://inspire.ec.europa.eu/codelist/WeatherConditionValue/rain>;
          rdfs:isDefinedBy  <https://inspire.ec.europa.eu/codelist/WeatherConditionValue/rain>;
         rdfs:label "rain"@no .

### http://inspire.ec.europa.eu/ont:WeatherConditionValue.smog
:WeatherConditionValue.smog a :WeatherConditionValue,skos:Concept ;
         skos:inScheme :WeatherConditionValueCode ;
         skos:definition "-- Definition -- Speed applies when a certain amount of smog is present."@en ;
          owl:sameAs  <https://inspire.ec.europa.eu/codelist/WeatherConditionValue/smog>;
          rdfs:isDefinedBy  <https://inspire.ec.europa.eu/codelist/WeatherConditionValue/smog>;
         rdfs:label "smog"@no .

### http://inspire.ec.europa.eu/ont:WeatherConditionValue.snow
:WeatherConditionValue.snow a :WeatherConditionValue,skos:Concept ;
         skos:inScheme :WeatherConditionValueCode ;
         skos:definition "-- Definition -- Speed applies when snow is present."@en ;
          owl:sameAs  <https://inspire.ec.europa.eu/codelist/WeatherConditionValue/snow>;
          rdfs:isDefinedBy  <https://inspire.ec.europa.eu/codelist/WeatherConditionValue/snow>;
         rdfs:label "snow"@no .

### http://inspire.ec.europa.eu/ont:FormOfRoadNodeValue
:FormOfRoadNodeValue a owl:Class ;
       rdfs:subClassOf :itnrCodeList ;
          rdfs:isDefinedBy  <https://inspire.ec.europa.eu/codelist/FormOfRoadNodeValue>;
         skos:definition "-- Definition -- Functions of road nodes within Euroroads."@en ;
       rdfs:label "FormOfRoadNodeValue"@en .

### http://inspire.ec.europa.eu/ont:FormOfRoadNodeValueCode
:FormOfRoadNodeValueCode a skos:ConceptScheme ;
         skos:definition "-- Definition -- Functions of road nodes within Euroroads."@en ;
          owl:sameAs  <https://inspire.ec.europa.eu/codelist/FormOfRoadNodeValue>;
       dc:isFormatOf :FormOfRoadNodeValue .

### http://inspire.ec.europa.eu/ont:FormOfRoadNodeValue.enclosedTrafficArea
:FormOfRoadNodeValue.enclosedTrafficArea a :FormOfRoadNodeValue,skos:Concept ;
         skos:inScheme :FormOfRoadNodeValueCode ;
         skos:definition "-- Definition -- The road node is situated inside and/or represents an enclosed traffic area. A traffic area is an area with no internal structure of legally defined driving directions. At least two roads are connected to the area..  -- Description -- SOURCE [Euroroads]."@en ;
          owl:sameAs  <https://inspire.ec.europa.eu/codelist/FormOfRoadNodeValue/enclosedTrafficArea>;
          rdfs:isDefinedBy  <https://inspire.ec.europa.eu/codelist/FormOfRoadNodeValue/enclosedTrafficArea>;
         rdfs:label "enclosedTrafficArea"@no .

### http://inspire.ec.europa.eu/ont:FormOfRoadNodeValue.junction
:FormOfRoadNodeValue.junction a :FormOfRoadNodeValue,skos:Concept ;
         skos:inScheme :FormOfRoadNodeValueCode ;
         skos:definition "-- Definition -- Three or more road links intersect at the road node."@en ;
          owl:sameAs  <https://inspire.ec.europa.eu/codelist/FormOfRoadNodeValue/junction>;
          rdfs:isDefinedBy  <https://inspire.ec.europa.eu/codelist/FormOfRoadNodeValue/junction>;
         rdfs:label "junction"@no .

### http://inspire.ec.europa.eu/ont:FormOfRoadNodeValue.levelCrossing
:FormOfRoadNodeValue.levelCrossing a :FormOfRoadNodeValue,skos:Concept ;
         skos:inScheme :FormOfRoadNodeValueCode ;
         skos:definition "-- Definition -- A railway crosses a road on the same level at the position of the road node."@en ;
          owl:sameAs  <https://inspire.ec.europa.eu/codelist/FormOfRoadNodeValue/levelCrossing>;
          rdfs:isDefinedBy  <https://inspire.ec.europa.eu/codelist/FormOfRoadNodeValue/levelCrossing>;
         rdfs:label "levelCrossing"@no .

### http://inspire.ec.europa.eu/ont:FormOfRoadNodeValue.pseudoNode
:FormOfRoadNodeValue.pseudoNode a :FormOfRoadNodeValue,skos:Concept ;
         skos:inScheme :FormOfRoadNodeValueCode ;
         skos:definition "-- Definition -- Exactly two road links connect to the road node."@en ;
          owl:sameAs  <https://inspire.ec.europa.eu/codelist/FormOfRoadNodeValue/pseudoNode>;
          rdfs:isDefinedBy  <https://inspire.ec.europa.eu/codelist/FormOfRoadNodeValue/pseudoNode>;
         rdfs:label "pseudoNode"@no .

### http://inspire.ec.europa.eu/ont:FormOfRoadNodeValue.roadEnd
:FormOfRoadNodeValue.roadEnd a :FormOfRoadNodeValue,skos:Concept ;
         skos:inScheme :FormOfRoadNodeValueCode ;
         skos:definition "-- Definition -- Only one road link connects to the road node. It signifies the end of a road."@en ;
          owl:sameAs  <https://inspire.ec.europa.eu/codelist/FormOfRoadNodeValue/roadEnd>;
          rdfs:isDefinedBy  <https://inspire.ec.europa.eu/codelist/FormOfRoadNodeValue/roadEnd>;
         rdfs:label "roadEnd"@no .

### http://inspire.ec.europa.eu/ont:FormOfRoadNodeValue.roundabout
:FormOfRoadNodeValue.roundabout a :FormOfRoadNodeValue,skos:Concept ;
         skos:inScheme :FormOfRoadNodeValueCode ;
         skos:definition "-- Definition -- The road node represents or is a part of a roundabout."@en ;
          owl:sameAs  <https://inspire.ec.europa.eu/codelist/FormOfRoadNodeValue/roundabout>;
          rdfs:isDefinedBy  <https://inspire.ec.europa.eu/codelist/FormOfRoadNodeValue/roundabout>;
         rdfs:label "roundabout"@no .

### http://inspire.ec.europa.eu/ont:FormOfRoadNodeValue.trafficSquare
:FormOfRoadNodeValue.trafficSquare a :FormOfRoadNodeValue,skos:Concept ;
         skos:inScheme :FormOfRoadNodeValueCode ;
         skos:definition "-- Definition -- The road node is situated inside and/or represents a traffic square. A traffic square is an area (partly) enclosed by roads which is used for non-traffic purposes and which is not a roundabout.   -- Description -- SOURCE [GDF, Euroroads]. "@en ;
          owl:sameAs  <https://inspire.ec.europa.eu/codelist/FormOfRoadNodeValue/trafficSquare>;
          rdfs:isDefinedBy  <https://inspire.ec.europa.eu/codelist/FormOfRoadNodeValue/trafficSquare>;
         rdfs:label "trafficSquare"@no .

### http://inspire.ec.europa.eu/ont:FormOfRoadNodeValue.roadServiceArea
:FormOfRoadNodeValue.roadServiceArea a :FormOfRoadNodeValue,skos:Concept ;
         skos:inScheme :FormOfRoadNodeValueCode ;
         skos:definition "-- Definition -- Surface annexed to a road and devoted to offer particular services for it.  -- Description -- EXAMPLES Gas station, rest area, toll area. "@en ;
          owl:sameAs  <https://inspire.ec.europa.eu/codelist/FormOfRoadNodeValue/roadServiceArea>;
          rdfs:isDefinedBy  <https://inspire.ec.europa.eu/codelist/FormOfRoadNodeValue/roadServiceArea>;
         rdfs:label "roadServiceArea"@no .

### http://inspire.ec.europa.eu/ont:FormOfWayValue
:FormOfWayValue a owl:Class ;
       rdfs:subClassOf :itnrCodeList ;
          rdfs:isDefinedBy  <https://inspire.ec.europa.eu/codelist/FormOfWayValue>;
         skos:definition "-- Definition -- Classification based on the physical properties of the road link.  -- Description -- SOURCE Based on [Euroroads]. "@en ;
       rdfs:label "FormOfWayValue"@en .

### http://inspire.ec.europa.eu/ont:FormOfWayValueCode
:FormOfWayValueCode a skos:ConceptScheme ;
         skos:definition "-- Definition -- Classification based on the physical properties of the road link.  -- Description -- SOURCE Based on [Euroroads]. "@en ;
          owl:sameAs  <https://inspire.ec.europa.eu/codelist/FormOfWayValue>;
       dc:isFormatOf :FormOfWayValue .

### http://inspire.ec.europa.eu/ont:FormOfWayValue.bicycleRoad
:FormOfWayValue.bicycleRoad a :FormOfWayValue,skos:Concept ;
         skos:inScheme :FormOfWayValueCode ;
         skos:definition "-- Definition -- Road where bicycles are the only vehicles allowed.  -- Description -- SOURCE Adapted from [Euroroads]."@en ;
          owl:sameAs  <https://inspire.ec.europa.eu/codelist/FormOfWayValue/bicycleRoad>;
          rdfs:isDefinedBy  <https://inspire.ec.europa.eu/codelist/FormOfWayValue/bicycleRoad>;
         rdfs:label "bicycleRoad"@no .

### http://inspire.ec.europa.eu/ont:FormOfWayValue.dualCarriageway
:FormOfWayValue.dualCarriageway a :FormOfWayValue,skos:Concept ;
         skos:inScheme :FormOfWayValueCode ;
         skos:definition "-- Definition -- Road with physically separated carriageways regardless of the number of lanes, which is not a motorway or a freeway.  -- Description -- SOURCE Based on [NVDB/GDF, Euroroads]. "@en ;
          owl:sameAs  <https://inspire.ec.europa.eu/codelist/FormOfWayValue/dualCarriageway>;
          rdfs:isDefinedBy  <https://inspire.ec.europa.eu/codelist/FormOfWayValue/dualCarriageway>;
         rdfs:label "dualCarriageway"@no .

### http://inspire.ec.europa.eu/ont:FormOfWayValue.enclosedTrafficArea
:FormOfWayValue.enclosedTrafficArea a :FormOfWayValue,skos:Concept ;
         skos:inScheme :FormOfWayValueCode ;
         skos:definition "-- Definition -- Area with no internal structure of legally defined driving directions. At least two roads are connected to the area.  -- Description -- SOURCE [Euroroads]. "@en ;
          owl:sameAs  <https://inspire.ec.europa.eu/codelist/FormOfWayValue/enclosedTrafficArea>;
          rdfs:isDefinedBy  <https://inspire.ec.europa.eu/codelist/FormOfWayValue/enclosedTrafficArea>;
         rdfs:label "enclosedTrafficArea"@no .

### http://inspire.ec.europa.eu/ont:FormOfWayValue.entranceOrExitCarPark
:FormOfWayValue.entranceOrExitCarPark a :FormOfWayValue,skos:Concept ;
         skos:inScheme :FormOfWayValueCode ;
         skos:definition "-- Definition -- Road specially designed to enter or to leave a parking area.   -- Description -- SOURCE [GDF], [Euroroads]. "@en ;
          owl:sameAs  <https://inspire.ec.europa.eu/codelist/FormOfWayValue/entranceOrExitCarPark>;
          rdfs:isDefinedBy  <https://inspire.ec.europa.eu/codelist/FormOfWayValue/entranceOrExitCarPark>;
         rdfs:label "entranceOrExitCarPark"@no .

### http://inspire.ec.europa.eu/ont:FormOfWayValue.entranceOrExitService
:FormOfWayValue.entranceOrExitService a :FormOfWayValue,skos:Concept ;
         skos:inScheme :FormOfWayValueCode ;
         skos:definition "-- Definition -- Road used only to enter or to leave a service.   -- Description -- SOURCE [GDF], [Euroroads]. "@en ;
          owl:sameAs  <https://inspire.ec.europa.eu/codelist/FormOfWayValue/entranceOrExitService>;
          rdfs:isDefinedBy  <https://inspire.ec.europa.eu/codelist/FormOfWayValue/entranceOrExitService>;
         rdfs:label "entranceOrExitService"@no .

### http://inspire.ec.europa.eu/ont:FormOfWayValue.freeway
:FormOfWayValue.freeway a :FormOfWayValue,skos:Concept ;
         skos:inScheme :FormOfWayValueCode ;
         skos:definition "-- Definition -- Road having no single level crossings with other roads.  -- Description -- SOURCE Adapted from [Euroroads]. NOTE This means that connections with other roads consist of slip roads.  "@en ;
          owl:sameAs  <https://inspire.ec.europa.eu/codelist/FormOfWayValue/freeway>;
          rdfs:isDefinedBy  <https://inspire.ec.europa.eu/codelist/FormOfWayValue/freeway>;
         rdfs:label "freeway"@no .

### http://inspire.ec.europa.eu/ont:FormOfWayValue.motorway
:FormOfWayValue.motorway a :FormOfWayValue,skos:Concept ;
         skos:inScheme :FormOfWayValueCode ;
         skos:definition "-- Definition -- Road permitted for motorized vehicles only in combination with a prescribed minimum speed. It has two or more mostly physically separated carriageways and no single level-crossings.  -- Description -- SOURCE [GDF], [Euroroads]. "@en ;
          owl:sameAs  <https://inspire.ec.europa.eu/codelist/FormOfWayValue/motorway>;
          rdfs:isDefinedBy  <https://inspire.ec.europa.eu/codelist/FormOfWayValue/motorway>;
         rdfs:label "motorway"@no .

### http://inspire.ec.europa.eu/ont:FormOfWayValue.pedestrianZone
:FormOfWayValue.pedestrianZone a :FormOfWayValue,skos:Concept ;
         skos:inScheme :FormOfWayValueCode ;
         skos:definition "-- Definition -- Area with a road network which is especially designed for use by pedestrians.  -- Description -- SOURCE [GDF], [Euroroads].  NOTE Pedestrian zones are usually located in urban areas. Except for emergency vehicles and for delivery vehicles during certain hours no traffic is allowed on the road network elements which are located inside the zone.  "@en ;
          owl:sameAs  <https://inspire.ec.europa.eu/codelist/FormOfWayValue/pedestrianZone>;
          rdfs:isDefinedBy  <https://inspire.ec.europa.eu/codelist/FormOfWayValue/pedestrianZone>;
         rdfs:label "pedestrianZone"@no .

### http://inspire.ec.europa.eu/ont:FormOfWayValue.roundabout
:FormOfWayValue.roundabout a :FormOfWayValue,skos:Concept ;
         skos:inScheme :FormOfWayValueCode ;
         skos:definition "-- Definition -- Road which forms a ring on which traffic travelling in only one direction is allowed.  -- Description -- SOURCE Based on [GDF], [Euroroads].  NOTE The Road elements which make up a roundabout are connected to one another and they form exactly one ring. "@en ;
          owl:sameAs  <https://inspire.ec.europa.eu/codelist/FormOfWayValue/roundabout>;
          rdfs:isDefinedBy  <https://inspire.ec.europa.eu/codelist/FormOfWayValue/roundabout>;
         rdfs:label "roundabout"@no .

### http://inspire.ec.europa.eu/ont:FormOfWayValue.serviceRoad
:FormOfWayValue.serviceRoad a :FormOfWayValue,skos:Concept ;
         skos:inScheme :FormOfWayValueCode ;
         skos:definition "-- Definition -- Road running parallel to and connecting to a road with a relatively high connectivity function, which is especially designed to enable access from the connecting roads to roads with a low connectivity function in its vicinity.  -- Description -- SOURCE Based on [GDF], [Euroroads].  NOTE Generally, service roads have the same name as the higher class road it runs parallel to and are only divided from it by small constructions like walkways, traffic islands etc. "@en ;
          owl:sameAs  <https://inspire.ec.europa.eu/codelist/FormOfWayValue/serviceRoad>;
          rdfs:isDefinedBy  <https://inspire.ec.europa.eu/codelist/FormOfWayValue/serviceRoad>;
         rdfs:label "serviceRoad"@no .

### http://inspire.ec.europa.eu/ont:FormOfWayValue.singleCarriageway
:FormOfWayValue.singleCarriageway a :FormOfWayValue,skos:Concept ;
         skos:inScheme :FormOfWayValueCode ;
         skos:definition "-- Definition -- Road where the traffic is not separated by any physical object.  -- Description -- SOURCE [GDF], [Euroroads].  NOTE All roads without separate carriageways are considered as roads with a single carriageway.   "@en ;
          owl:sameAs  <https://inspire.ec.europa.eu/codelist/FormOfWayValue/singleCarriageway>;
          rdfs:isDefinedBy  <https://inspire.ec.europa.eu/codelist/FormOfWayValue/singleCarriageway>;
         rdfs:label "singleCarriageway"@no .

### http://inspire.ec.europa.eu/ont:FormOfWayValue.slipRoad
:FormOfWayValue.slipRoad a :FormOfWayValue,skos:Concept ;
         skos:inScheme :FormOfWayValueCode ;
         skos:definition "-- Definition -- Road especially designed to enter or leave a road.  -- Description -- SOURCE Adapted from [Euroroads]."@en ;
          owl:sameAs  <https://inspire.ec.europa.eu/codelist/FormOfWayValue/slipRoad>;
          rdfs:isDefinedBy  <https://inspire.ec.europa.eu/codelist/FormOfWayValue/slipRoad>;
         rdfs:label "slipRoad"@no .

### http://inspire.ec.europa.eu/ont:FormOfWayValue.tractor
:FormOfWayValue.tractor a :FormOfWayValue,skos:Concept ;
         skos:inScheme :FormOfWayValueCode ;
         skos:definition "-- Definition -- Arranged road only usable for a tractor (farm vehicle or forest machine) or terrain vehicle (a vehicle with higher ground clearance, big wheels and 4 wheel drive).  -- Description -- SOURCE Based on [Euroroads]. "@en ;
          owl:sameAs  <https://inspire.ec.europa.eu/codelist/FormOfWayValue/tractor>;
          rdfs:isDefinedBy  <https://inspire.ec.europa.eu/codelist/FormOfWayValue/tractor>;
         rdfs:label "tractor"@no .

### http://inspire.ec.europa.eu/ont:FormOfWayValue.trafficSquare
:FormOfWayValue.trafficSquare a :FormOfWayValue,skos:Concept ;
         skos:inScheme :FormOfWayValueCode ;
         skos:definition "-- Definition -- Area (partly) enclosed by roads which is used for non-traffic purposes and which is not a roundabout.   -- Description -- SOURCE [GDF], [Euroroads]. "@en ;
          owl:sameAs  <https://inspire.ec.europa.eu/codelist/FormOfWayValue/trafficSquare>;
          rdfs:isDefinedBy  <https://inspire.ec.europa.eu/codelist/FormOfWayValue/trafficSquare>;
         rdfs:label "trafficSquare"@no .

### http://inspire.ec.europa.eu/ont:FormOfWayValue.walkway
:FormOfWayValue.walkway a :FormOfWayValue,skos:Concept ;
         skos:inScheme :FormOfWayValueCode ;
         skos:definition "-- Definition -- Road reserved for pedestrian use and closed for regular vehicular use by a physically barrier.  -- Description -- SOURCE Adapted from [Euroroads].  NOTE Occasional use by (emergency) services may occur. "@en ;
          owl:sameAs  <https://inspire.ec.europa.eu/codelist/FormOfWayValue/walkway>;
          rdfs:isDefinedBy  <https://inspire.ec.europa.eu/codelist/FormOfWayValue/walkway>;
         rdfs:label "walkway"@no .

### http://inspire.ec.europa.eu/ont:FunctionalRoadClassValue
:FunctionalRoadClassValue a owl:Class ;
       rdfs:subClassOf :itnrEnumeration ;
          rdfs:isDefinedBy  <https://inspire.ec.europa.eu/enumeration/FunctionalRoadClassValue>;
         skos:definition "-- Definition -- Values for the functional road classification. This classification is based on the importance of the role that the road performs in the road network.   -- Description -- SOURCE Adapted from [GDF, EuroRoadS]."@en ;
       rdfs:label "FunctionalRoadClassValue"@en .

### http://inspire.ec.europa.eu/ont:FunctionalRoadClassValueCode
:FunctionalRoadClassValueCode a skos:ConceptScheme ;
         skos:definition "-- Definition -- Values for the functional road classification. This classification is based on the importance of the role that the road performs in the road network.   -- Description -- SOURCE Adapted from [GDF, EuroRoadS]."@en ;
          owl:sameAs  <https://inspire.ec.europa.eu/enumeration/FunctionalRoadClassValue>;
       dc:isFormatOf :FunctionalRoadClassValue .

### http://inspire.ec.europa.eu/ont:FunctionalRoadClassValue.mainRoad
:FunctionalRoadClassValue.mainRoad a :FunctionalRoadClassValue,skos:Concept ;
         skos:inScheme :FunctionalRoadClassValueCode ;
         skos:definition "-- Definition -- The most important roads in a given network.   -- Description -- SOURCE [GDF], [Euroroads]."@en ;
          owl:sameAs  <https://inspire.ec.europa.eu/enumeration/FunctionalRoadClassValue/mainRoad>;
          rdfs:isDefinedBy  <https://inspire.ec.europa.eu/enumeration/FunctionalRoadClassValue/mainRoad>;
         rdfs:label "mainRoad"@no .

### http://inspire.ec.europa.eu/ont:FunctionalRoadClassValue.firstClass
:FunctionalRoadClassValue.firstClass a :FunctionalRoadClassValue,skos:Concept ;
         skos:inScheme :FunctionalRoadClassValueCode ;
         skos:definition "-- Definition -- The second most important roads in a given network.  -- Description -- SOURCE [Euroroads]. "@en ;
          owl:sameAs  <https://inspire.ec.europa.eu/enumeration/FunctionalRoadClassValue/firstClass>;
          rdfs:isDefinedBy  <https://inspire.ec.europa.eu/enumeration/FunctionalRoadClassValue/firstClass>;
         rdfs:label "firstClass"@no .

### http://inspire.ec.europa.eu/ont:FunctionalRoadClassValue.secondClass
:FunctionalRoadClassValue.secondClass a :FunctionalRoadClassValue,skos:Concept ;
         skos:inScheme :FunctionalRoadClassValueCode ;
         skos:definition "-- Definition -- The third most important roads in a given network.  -- Description -- SOURCE [Euroroads]. "@en ;
          owl:sameAs  <https://inspire.ec.europa.eu/enumeration/FunctionalRoadClassValue/secondClass>;
          rdfs:isDefinedBy  <https://inspire.ec.europa.eu/enumeration/FunctionalRoadClassValue/secondClass>;
         rdfs:label "secondClass"@no .

### http://inspire.ec.europa.eu/ont:FunctionalRoadClassValue.thirdClass
:FunctionalRoadClassValue.thirdClass a :FunctionalRoadClassValue,skos:Concept ;
         skos:inScheme :FunctionalRoadClassValueCode ;
         skos:definition "-- Definition -- The fourth most important roads in a given network.  -- Description -- SOURCE [Euroroads]. "@en ;
          owl:sameAs  <https://inspire.ec.europa.eu/enumeration/FunctionalRoadClassValue/thirdClass>;
          rdfs:isDefinedBy  <https://inspire.ec.europa.eu/enumeration/FunctionalRoadClassValue/thirdClass>;
         rdfs:label "thirdClass"@no .

### http://inspire.ec.europa.eu/ont:FunctionalRoadClassValue.fourthClass
:FunctionalRoadClassValue.fourthClass a :FunctionalRoadClassValue,skos:Concept ;
         skos:inScheme :FunctionalRoadClassValueCode ;
         skos:definition "-- Definition -- The fifth most important roads in a given network.  -- Description -- SOURCE [Euroroads]. "@en ;
          owl:sameAs  <https://inspire.ec.europa.eu/enumeration/FunctionalRoadClassValue/fourthClass>;
          rdfs:isDefinedBy  <https://inspire.ec.europa.eu/enumeration/FunctionalRoadClassValue/fourthClass>;
         rdfs:label "fourthClass"@no .

### http://inspire.ec.europa.eu/ont:FunctionalRoadClassValue.fifthClass
:FunctionalRoadClassValue.fifthClass a :FunctionalRoadClassValue,skos:Concept ;
         skos:inScheme :FunctionalRoadClassValueCode ;
         skos:definition "-- Definition -- The sixth most important roads in a given network.  -- Description -- SOURCE [Euroroads]. "@en ;
          owl:sameAs  <https://inspire.ec.europa.eu/enumeration/FunctionalRoadClassValue/fifthClass>;
          rdfs:isDefinedBy  <https://inspire.ec.europa.eu/enumeration/FunctionalRoadClassValue/fifthClass>;
         rdfs:label "fifthClass"@no .

### http://inspire.ec.europa.eu/ont:FunctionalRoadClassValue.sixthClass
:FunctionalRoadClassValue.sixthClass a :FunctionalRoadClassValue,skos:Concept ;
         skos:inScheme :FunctionalRoadClassValueCode ;
         skos:definition "-- Definition -- The seventh most important roads in a given network.  -- Description -- SOURCE [Euroroads]. "@en ;
          owl:sameAs  <https://inspire.ec.europa.eu/enumeration/FunctionalRoadClassValue/sixthClass>;
          rdfs:isDefinedBy  <https://inspire.ec.europa.eu/enumeration/FunctionalRoadClassValue/sixthClass>;
         rdfs:label "sixthClass"@no .

### http://inspire.ec.europa.eu/ont:FunctionalRoadClassValue.seventhClass
:FunctionalRoadClassValue.seventhClass a :FunctionalRoadClassValue,skos:Concept ;
         skos:inScheme :FunctionalRoadClassValueCode ;
         skos:definition "-- Definition -- The eighth most important roads in a given network.  -- Description -- SOURCE [Euroroads]. "@en ;
          owl:sameAs  <https://inspire.ec.europa.eu/enumeration/FunctionalRoadClassValue/seventhClass>;
          rdfs:isDefinedBy  <https://inspire.ec.europa.eu/enumeration/FunctionalRoadClassValue/seventhClass>;
         rdfs:label "seventhClass"@no .

### http://inspire.ec.europa.eu/ont:FunctionalRoadClassValue.eighthClass
:FunctionalRoadClassValue.eighthClass a :FunctionalRoadClassValue,skos:Concept ;
         skos:inScheme :FunctionalRoadClassValueCode ;
         skos:definition "-- Definition -- The ninth most important roads in a given network.  -- Description -- SOURCE [Euroroads]. "@en ;
          owl:sameAs  <https://inspire.ec.europa.eu/enumeration/FunctionalRoadClassValue/eighthClass>;
          rdfs:isDefinedBy  <https://inspire.ec.europa.eu/enumeration/FunctionalRoadClassValue/eighthClass>;
         rdfs:label "eighthClass"@no .

### http://inspire.ec.europa.eu/ont:FunctionalRoadClassValue.ninthClass
:FunctionalRoadClassValue.ninthClass a :FunctionalRoadClassValue,skos:Concept ;
         skos:inScheme :FunctionalRoadClassValueCode ;
         skos:definition "-- Definition -- The least important roads in a given network.  -- Description -- SOURCE [GDF]  NOTE The farthest ways in the forest road network. It has no regular maintenance. [NVDB] [Euroroads]. "@en ;
          owl:sameAs  <https://inspire.ec.europa.eu/enumeration/FunctionalRoadClassValue/ninthClass>;
          rdfs:isDefinedBy  <https://inspire.ec.europa.eu/enumeration/FunctionalRoadClassValue/ninthClass>;
         rdfs:label "ninthClass"@no .
:FunctionalRoadClassValue owl:oneOf ( :FunctionalRoadClassValue.mainRoad :FunctionalRoadClassValue.firstClass :FunctionalRoadClassValue.secondClass :FunctionalRoadClassValue.thirdClass :FunctionalRoadClassValue.fourthClass :FunctionalRoadClassValue.fifthClass :FunctionalRoadClassValue.sixthClass :FunctionalRoadClassValue.seventhClass :FunctionalRoadClassValue.eighthClass :FunctionalRoadClassValue.ninthClass  ) ; .

### http://inspire.ec.europa.eu/ont:Road
:Road a owl:Class ;
         skos:definition "-- Definition -- A collection of road link sequences and/or individual road links that are characterized by one or more thematic identifiers and/or properties.  -- Description -- EXAMPLE Examples are roads characterized by a specific identification code, used by road management authorities or tourist routes, identified by a specific name. "@en ;
       rdfs:label "Road"@en .
:Road rdfs:subClassOf :TransportLinkSet .

### http://inspire.ec.europa.eu/ont#localRoadCode
:localRoadCode rdf:type owl:DatatypeProperty ;
         skos:definition "-- Definition -- Identification code assigned to the road by the local road authority."@en ;
         rdfs:domain :Road;
         rdfs:range xsd:string;
         rdfs:label "localRoadCode"@en .
:Road rdfs:subClassOf [ rdf:type owl:Restriction ;
         owl:onProperty :localRoadCode;
         owl:onDataRange xsd:string;
       owl:maxQualifiedCardinality "1"^^xsd:nonNegativeInteger ;
         ] .
:Road rdfs:subClassOf [ rdf:type owl:Restriction ;
         owl:onProperty :localRoadCode;
         owl:allValuesFrom xsd:string;
         ] .


### http://inspire.ec.europa.eu/ont#nationalRoadCode
:nationalRoadCode rdf:type owl:DatatypeProperty ;
         skos:definition "-- Definition -- The national number of the road.  -- Description -- SOURCE [Euroroads]. "@en ;
         rdfs:domain :Road;
         rdfs:range xsd:string;
         rdfs:label "nationalRoadCode"@en .
:Road rdfs:subClassOf [ rdf:type owl:Restriction ;
         owl:onProperty :nationalRoadCode;
         owl:onDataRange xsd:string;
       owl:maxQualifiedCardinality "1"^^xsd:nonNegativeInteger ;
         ] .
:Road rdfs:subClassOf [ rdf:type owl:Restriction ;
         owl:onProperty :nationalRoadCode;
         owl:allValuesFrom xsd:string;
         ] .


### http://inspire.ec.europa.eu/ont:RoadArea
:RoadArea a owl:Class ;
         skos:definition "-- Definition -- Surface which extends to the limits of a road, including vehicular areas and other parts of it.  -- Description -- EAXMPLE Pedestrian areas. "@en ;
       rdfs:label "RoadArea"@en .
:RoadArea rdfs:subClassOf :TransportArea .

### http://inspire.ec.europa.eu/ont:RoadLink
:RoadLink a owl:Class ;
         skos:definition "-- Definition -- A linear spatial object that describes the geometry and connectivity of a road network between two points in the network. Road links can represent paths, bicycle roads, single carriageways, multiple carriageway roads and even fictitious trajectories across traffic squares."@en ;
       rdfs:label "RoadLink"@en .
:RoadLink rdfs:subClassOf :TransportLink .

### http://inspire.ec.europa.eu/ont:RoadNode
:RoadNode a owl:Class ;
         skos:definition "-- Definition -- A point spatial object that is used to either represent connectivity between two road links or to represent a significant spatial object such as a services station or  roundabout."@en ;
       rdfs:label "RoadNode"@en .
:RoadNode rdfs:subClassOf :TransportNode .

### http://inspire.ec.europa.eu/ont#formOfRoadNode
:formOfRoadNode rdf:type owl:ObjectProperty ;
         skos:definition "-- Definition -- Description of the function of a road node in the road transport network."@en ;
         rdfs:domain :RoadNode;
         rdfs:range :FormOfRoadNodeValue;
         rdf:type owl:FunctionalProperty;
         rdfs:label "formOfRoadNode"@en .
:RoadNode rdfs:subClassOf [ rdf:type owl:Restriction ;
         owl:onProperty :formOfRoadNode;
         owl:onClass :FormOfRoadNodeValue;
       owl:qualifiedCardinality "1"^^xsd:nonNegativeInteger ;
         ] .
:RoadNode rdfs:subClassOf [ rdf:type owl:Restriction ;
         owl:onProperty :formOfRoadNode;
         owl:allValuesFrom :FormOfRoadNodeValue;
         ] .


### http://inspire.ec.europa.eu/ont:RoadServiceTypeValue
:RoadServiceTypeValue a owl:Class ;
       rdfs:subClassOf :itnrCodeList ;
          rdfs:isDefinedBy  <https://inspire.ec.europa.eu/codelist/RoadServiceTypeValue>;
         skos:definition "-- Definition -- Types of road service areas."@en ;
       rdfs:label "RoadServiceTypeValue"@en .

### http://inspire.ec.europa.eu/ont:RoadServiceTypeValueCode
:RoadServiceTypeValueCode a skos:ConceptScheme ;
         skos:definition "-- Definition -- Types of road service areas."@en ;
          owl:sameAs  <https://inspire.ec.europa.eu/codelist/RoadServiceTypeValue>;
       dc:isFormatOf :RoadServiceTypeValue .

### http://inspire.ec.europa.eu/ont:RoadServiceTypeValue.busStation
:RoadServiceTypeValue.busStation a :RoadServiceTypeValue,skos:Concept ;
         skos:inScheme :RoadServiceTypeValueCode ;
         skos:definition "-- Definition -- The road service is a bus stop."@en ;
          owl:sameAs  <https://inspire.ec.europa.eu/codelist/RoadServiceTypeValue/busStation>;
          rdfs:isDefinedBy  <https://inspire.ec.europa.eu/codelist/RoadServiceTypeValue/busStation>;
         rdfs:label "busStation"@no .

### http://inspire.ec.europa.eu/ont:RoadServiceTypeValue.parking
:RoadServiceTypeValue.parking a :RoadServiceTypeValue,skos:Concept ;
         skos:inScheme :RoadServiceTypeValueCode ;
         skos:definition "-- Definition -- The road service areea is a parking facility."@en ;
          owl:sameAs  <https://inspire.ec.europa.eu/codelist/RoadServiceTypeValue/parking>;
          rdfs:isDefinedBy  <https://inspire.ec.europa.eu/codelist/RoadServiceTypeValue/parking>;
         rdfs:label "parking"@no .

### http://inspire.ec.europa.eu/ont:RoadServiceTypeValue.restArea
:RoadServiceTypeValue.restArea a :RoadServiceTypeValue,skos:Concept ;
         skos:inScheme :RoadServiceTypeValueCode ;
         skos:definition "-- Definition -- The road service is a rest area."@en ;
          owl:sameAs  <https://inspire.ec.europa.eu/codelist/RoadServiceTypeValue/restArea>;
          rdfs:isDefinedBy  <https://inspire.ec.europa.eu/codelist/RoadServiceTypeValue/restArea>;
         rdfs:label "restArea"@no .

### http://inspire.ec.europa.eu/ont:RoadServiceTypeValue.toll
:RoadServiceTypeValue.toll a :RoadServiceTypeValue,skos:Concept ;
         skos:inScheme :RoadServiceTypeValueCode ;
         skos:definition "-- Definition -- Area that provides toll services such as ticket dispensers or toll payment services."@en ;
          owl:sameAs  <https://inspire.ec.europa.eu/codelist/RoadServiceTypeValue/toll>;
          rdfs:isDefinedBy  <https://inspire.ec.europa.eu/codelist/RoadServiceTypeValue/toll>;
         rdfs:label "toll"@no .

### http://inspire.ec.europa.eu/ont:ServiceFacilityValue
:ServiceFacilityValue a owl:Class ;
       rdfs:subClassOf :itnrCodeList ;
          rdfs:isDefinedBy  <https://inspire.ec.europa.eu/codelist/ServiceFacilityValue>;
         skos:definition "-- Definition -- Possible service facilities available at a road service area. "@en ;
       rdfs:label "ServiceFacilityValue"@en .

### http://inspire.ec.europa.eu/ont:ServiceFacilityValueCode
:ServiceFacilityValueCode a skos:ConceptScheme ;
         skos:definition "-- Definition -- Possible service facilities available at a road service area. "@en ;
          owl:sameAs  <https://inspire.ec.europa.eu/codelist/ServiceFacilityValue>;
       dc:isFormatOf :ServiceFacilityValue .

### http://inspire.ec.europa.eu/ont:ServiceFacilityValue.drinks
:ServiceFacilityValue.drinks a :ServiceFacilityValue,skos:Concept ;
         skos:inScheme :ServiceFacilityValueCode ;
         skos:definition "-- Definition -- Drinks are available."@en ;
          owl:sameAs  <https://inspire.ec.europa.eu/codelist/ServiceFacilityValue/drinks>;
          rdfs:isDefinedBy  <https://inspire.ec.europa.eu/codelist/ServiceFacilityValue/drinks>;
         rdfs:label "drinks"@no .

### http://inspire.ec.europa.eu/ont:ServiceFacilityValue.food
:ServiceFacilityValue.food a :ServiceFacilityValue,skos:Concept ;
         skos:inScheme :ServiceFacilityValueCode ;
         skos:definition "-- Definition -- Food is available."@en ;
          owl:sameAs  <https://inspire.ec.europa.eu/codelist/ServiceFacilityValue/food>;
          rdfs:isDefinedBy  <https://inspire.ec.europa.eu/codelist/ServiceFacilityValue/food>;
         rdfs:label "food"@no .

### http://inspire.ec.europa.eu/ont:ServiceFacilityValue.fuel
:ServiceFacilityValue.fuel a :ServiceFacilityValue,skos:Concept ;
         skos:inScheme :ServiceFacilityValueCode ;
         skos:definition "-- Definition -- Fuel is available."@en ;
          owl:sameAs  <https://inspire.ec.europa.eu/codelist/ServiceFacilityValue/fuel>;
          rdfs:isDefinedBy  <https://inspire.ec.europa.eu/codelist/ServiceFacilityValue/fuel>;
         rdfs:label "fuel"@no .

### http://inspire.ec.europa.eu/ont:ServiceFacilityValue.picnicArea
:ServiceFacilityValue.picnicArea a :ServiceFacilityValue,skos:Concept ;
         skos:inScheme :ServiceFacilityValueCode ;
         skos:definition "-- Definition -- A picnic area is present."@en ;
          owl:sameAs  <https://inspire.ec.europa.eu/codelist/ServiceFacilityValue/picnicArea>;
          rdfs:isDefinedBy  <https://inspire.ec.europa.eu/codelist/ServiceFacilityValue/picnicArea>;
         rdfs:label "picnicArea"@no .

### http://inspire.ec.europa.eu/ont:ServiceFacilityValue.playground
:ServiceFacilityValue.playground a :ServiceFacilityValue,skos:Concept ;
         skos:inScheme :ServiceFacilityValueCode ;
         skos:definition "-- Definition -- A playground area is present."@en ;
          owl:sameAs  <https://inspire.ec.europa.eu/codelist/ServiceFacilityValue/playground>;
          rdfs:isDefinedBy  <https://inspire.ec.europa.eu/codelist/ServiceFacilityValue/playground>;
         rdfs:label "playground"@no .

### http://inspire.ec.europa.eu/ont:ServiceFacilityValue.shop
:ServiceFacilityValue.shop a :ServiceFacilityValue,skos:Concept ;
         skos:inScheme :ServiceFacilityValueCode ;
         skos:definition "-- Definition -- A shop is present. "@en ;
          owl:sameAs  <https://inspire.ec.europa.eu/codelist/ServiceFacilityValue/shop>;
          rdfs:isDefinedBy  <https://inspire.ec.europa.eu/codelist/ServiceFacilityValue/shop>;
         rdfs:label "shop"@no .

### http://inspire.ec.europa.eu/ont:ServiceFacilityValue.toilets
:ServiceFacilityValue.toilets a :ServiceFacilityValue,skos:Concept ;
         skos:inScheme :ServiceFacilityValueCode ;
         skos:definition "-- Definition -- Toilets are present."@en ;
          owl:sameAs  <https://inspire.ec.europa.eu/codelist/ServiceFacilityValue/toilets>;
          rdfs:isDefinedBy  <https://inspire.ec.europa.eu/codelist/ServiceFacilityValue/toilets>;
         rdfs:label "toilets"@no .
:itnrFeature owl:disjointUnionOf ( :AddressComponent :CrossReference :Network :NetworkElement :NetworkProperty :TransportObject     ) ; .
:itnrEnumeration owl:disjointUnionOf ( :VerticalPositionValue :TransportTypeValue :MinMaxLaneValue :SpeedLimitMinMaxValue :FunctionalRoadClassValue     ) ; .
:itnrDataType owl:disjointUnionOf ( :Identifier :PartOfName :ThoroughfareNameValue :GeographicalName :PronunciationOfName :SpellingOfName :DirectedLink :NetworkReference     ) ; .
