# baseURI: http://spec.tn-its.eu/owl/tnits-owl
# imports: http://def.isotc211.org/iso19115/-1/2014/MetadataInformation
# imports: http://schemas.opengis.net/geosparql/1.0/geosparql_vocab_all.rdf
# imports: http://spec.tn-its.eu/codelists/allcodes
# imports: http://www.roadotl.eu/iso19148/def/
# imports: http://www.w3.org/2004/02/skos/core

@prefix : <http://spec.tn-its.eu/owl/tnits-owl#> .
@prefix dc: <http://purl.org/dc/terms/> .
@prefix gsp: <http://www.opengis.net/ont/geosparql#> .
@prefix lr: <http://www.roadotl.eu/iso19148/def/> .
@prefix owl: <http://www.w3.org/2002/07/owl#> .
@prefix rdf: <http://www.w3.org/1999/02/22-rdf-syntax-ns#> .
@prefix rdfs: <http://www.w3.org/2000/01/rdf-schema#> .
@prefix sf: <http://www.opengis.net/ont/sf#> .
@prefix skos: <http://www.w3.org/2004/02/skos/core#> .
@prefix xml: <http://www.w3.org/XML/1998/namespace> .
@prefix xsd: <http://www.w3.org/2001/XMLSchema#> .

<http://def.isotc211.org/iso19109/2015/GeneralFeatureModel#AnyFeature>
  rdf:type owl:Class ;
.
dc:date
  rdf:type owl:AnnotationProperty ;
.
<http://spec.tn-its.eu/owl/tnits-owl>
  rdf:type owl:Ontology ;
  dc:abstract "Ontology for exchange of changes in road attributes" ;
  dc:creator "TN-ITS" ;
  dc:date "29.03.2022" ;
  dc:description "Ontology for the TN-ITS model for exchange of changes in road attributes"@en ;
  dc:title "TN-ITS"@en ;
  owl:imports <http://def.isotc211.org/iso19115/-1/2014/MetadataInformation> ;
  owl:imports <http://schemas.opengis.net/geosparql/1.0/geosparql_vocab_all.rdf> ;
  owl:imports <http://spec.tn-its.eu/codelists/allcodes> ;
  owl:imports lr: ;
  owl:imports <http://www.w3.org/2004/02/skos/core> ;
.
:AbstractRoadFeatureProperty
  rdf:type owl:Class ;
  rdfs:label "AbstractRoadFeatureProperty"@en ;
  rdfs:subClassOf :tnitsDataType ;
  owl:disjointUnionOf (
      :GenericRoadFeatureProperty
      :RoadSignProperty
    ) ;
  skos:definition "An abstract generic (type independent) representation of a road feature property value "@en ;
.
:AgoraBinaryVersion
  rdf:type owl:Class ;
  rdfs:label "AgoraBinaryVersion"@en ;
  rdfs:subClassOf :tnitsCodeList ;
  skos:definition "Specifies the available list of enumerations for the version of the AGORA binary specification being used"@en ;
.
:AgoraBinaryVersionCode
  rdf:type owl:NamedIndividual ;
  rdf:type skos:ConceptScheme ;
  dc:isFormatOf :AgoraBinaryVersion ;
  skos:definition "Specifies the available list of enumerations for the version of the AGORA binary specification being used"@en ;
.
:AgoraLocationReference
  rdf:type owl:Class ;
  rdfs:label "AgoraLocationReference"@en ;
  rdfs:subClassOf :DynamicLocationReference ;
  rdfs:subClassOf [
      rdf:type owl:Restriction ;
      owl:allValuesFrom :AgoraBinaryVersion ;
      owl:onProperty <http://spec.tn-its.eu/owl/tnits-owl#AgoraLocationReference.agoraBinaryVersion> ;
    ] ;
  rdfs:subClassOf [
      rdf:type owl:Restriction ;
      owl:allValuesFrom xsd:string ;
      owl:onProperty <http://spec.tn-its.eu/owl/tnits-owl#AgoraLocationReference.base64String> ;
    ] ;
  rdfs:subClassOf [
      rdf:type owl:Restriction ;
      owl:onClass :AgoraBinaryVersion ;
      owl:onProperty <http://spec.tn-its.eu/owl/tnits-owl#AgoraLocationReference.agoraBinaryVersion> ;
      owl:qualifiedCardinality "1"^^xsd:nonNegativeInteger ;
    ] ;
  rdfs:subClassOf [
      rdf:type owl:Restriction ;
      owl:onDataRange xsd:string ;
      owl:onProperty <http://spec.tn-its.eu/owl/tnits-owl#AgoraLocationReference.base64String> ;
      owl:qualifiedCardinality "1"^^xsd:nonNegativeInteger ;
    ] ;
  skos:definition "A type of dynamic location reference that uses coordinates and core attribution according to ISO 17572-3.  "@en ;
.
<http://spec.tn-its.eu/owl/tnits-owl#AgoraLocationReference.agoraBinaryVersion>
  rdf:type owl:FunctionalProperty ;
  rdf:type owl:ObjectProperty ;
  rdfs:domain :AgoraLocationReference ;
  rdfs:label "AgoraLocationReference.agoraBinaryVersion"@en ;
  rdfs:range :AgoraBinaryVersion ;
  skos:definition "Provides reference to the version of the AGORA Binary string encoding used by reference to an item in an external code list (see AgoraBinaryVersion Class)"@en ;
.
<http://spec.tn-its.eu/owl/tnits-owl#AgoraLocationReference.base64String>
  rdf:type owl:DatatypeProperty ;
  rdf:type owl:FunctionalProperty ;
  rdfs:domain :AgoraLocationReference ;
  rdfs:label "AgoraLocationReference.base64String"@en ;
  rdfs:range xsd:string ;
  skos:definition "The AGORA binary string encoded using base64 "@en ;
.
:Any
  rdf:type owl:Class ;
.
:AreaCondition
  rdf:type owl:Class ;
  rdfs:label "AreaCondition"@en ;
  rdfs:subClassOf :Condition ;
  rdfs:subClassOf [
      rdf:type owl:Restriction ;
      owl:allValuesFrom :AreaType ;
      owl:onProperty <http://spec.tn-its.eu/owl/tnits-owl#AreaCondition.areaType> ;
    ] ;
  rdfs:subClassOf [
      rdf:type owl:Restriction ;
      owl:onClass :AreaType ;
      owl:onProperty <http://spec.tn-its.eu/owl/tnits-owl#AreaCondition.areaType> ;
      owl:qualifiedCardinality "1"^^xsd:nonNegativeInteger ;
    ] ;
  skos:definition "Specifies area type condition applicability relating to a road feature  "@en ;
.
<http://spec.tn-its.eu/owl/tnits-owl#AreaCondition.areaType>
  rdf:type owl:FunctionalProperty ;
  rdf:type owl:ObjectProperty ;
  rdfs:domain :AreaCondition ;
  rdfs:label "AreaCondition.areaType"@en ;
  rdfs:range :AreaType ;
  skos:definition "Specifies the available list of enumerations for the area type condition for a road feature by reference to an item in an external code list "@en ;
.
:AreaType
  rdf:type owl:Class ;
  rdfs:label "AreaType"@en ;
  rdfs:subClassOf :tnitsCodeList ;
  skos:definition "Specifies the available list of enumerations for the area type condition for a road feature "@en ;
.
:AreaTypeCode
  rdf:type owl:NamedIndividual ;
  rdf:type skos:ConceptScheme ;
  dc:isFormatOf :AreaType ;
  skos:definition "Specifies the available list of enumerations for the area type condition for a road feature "@en ;
.
:BinaryLocationReference
  rdf:type owl:Class ;
  rdfs:label "BinaryLocationReference"@en ;
  rdfs:subClassOf :tnitsDataType ;
  rdfs:subClassOf [
      rdf:type owl:Restriction ;
      owl:allValuesFrom :OpenLRBinaryVersion ;
      owl:onProperty <http://spec.tn-its.eu/owl/tnits-owl#BinaryLocationReference.openLRBinaryVersion> ;
    ] ;
  rdfs:subClassOf [
      rdf:type owl:Restriction ;
      owl:allValuesFrom xsd:string ;
      owl:onProperty <http://spec.tn-its.eu/owl/tnits-owl#BinaryLocationReference.base64String> ;
    ] ;
  rdfs:subClassOf [
      rdf:type owl:Restriction ;
      owl:onClass :OpenLRBinaryVersion ;
      owl:onProperty <http://spec.tn-its.eu/owl/tnits-owl#BinaryLocationReference.openLRBinaryVersion> ;
      owl:qualifiedCardinality "1"^^xsd:nonNegativeInteger ;
    ] ;
  rdfs:subClassOf [
      rdf:type owl:Restriction ;
      owl:onDataRange xsd:string ;
      owl:onProperty <http://spec.tn-its.eu/owl/tnits-owl#BinaryLocationReference.base64String> ;
      owl:qualifiedCardinality "1"^^xsd:nonNegativeInteger ;
    ] ;
  skos:definition "OpenLR location reference using binary encoding "@en ;
.
<http://spec.tn-its.eu/owl/tnits-owl#BinaryLocationReference.base64String>
  rdf:type owl:DatatypeProperty ;
  rdf:type owl:FunctionalProperty ;
  rdfs:domain :BinaryLocationReference ;
  rdfs:label "BinaryLocationReference.base64String"@en ;
  rdfs:range xsd:string ;
  skos:definition "The OpenRL binary string encoded using base64"@en ;
.
<http://spec.tn-its.eu/owl/tnits-owl#BinaryLocationReference.openLRBinaryVersion>
  rdf:type owl:FunctionalProperty ;
  rdf:type owl:ObjectProperty ;
  rdfs:domain :BinaryLocationReference ;
  rdfs:label "BinaryLocationReference.openLRBinaryVersion"@en ;
  rdfs:range :OpenLRBinaryVersion ;
  skos:definition "Provides reference to the version of the OpenLR Binary string encoding used by reference to an item in an external code list (see OpenLRBinaryVersion Class)"@en ;
.
:ChargingPointUsageType
  rdf:type owl:Class ;
  rdfs:label "ChargingPointUsageType"@en ;
  rdfs:subClassOf :tnitsCodeList ;
  skos:definition "Specifies the available list of enumerations for the use of electric charging point "@en ;
.
:ChargingPointUsageTypeCode
  rdf:type owl:NamedIndividual ;
  rdf:type skos:ConceptScheme ;
  dc:isFormatOf :ChargingPointUsageType ;
  skos:definition "Specifies the available list of enumerations for the use of electric charging point "@en ;
.
:ComparisonOperator
  rdf:type owl:Class ;
  rdfs:label "ComparisonOperator"@en ;
  rdfs:subClassOf :tnitsEnumeration ;
  owl:equivalentClass [
      rdf:type owl:Class ;
      owl:oneOf (
          <http://spec.tn-its.eu/owl/tnits-owl#ComparisonOperator.equalTo>
          <http://spec.tn-its.eu/owl/tnits-owl#ComparisonOperator.greaterThan>
          <http://spec.tn-its.eu/owl/tnits-owl#ComparisonOperator.greaterThanOrEqualTo>
          <http://spec.tn-its.eu/owl/tnits-owl#ComparisonOperator.lessThan>
          <http://spec.tn-its.eu/owl/tnits-owl#ComparisonOperator.lessThanOrEqualTo>
        ) ;
    ] ;
  skos:definition "The logical operator to be used in a comparison operation. "@en ;
.
<http://spec.tn-its.eu/owl/tnits-owl#ComparisonOperator.equalTo>
  rdf:type :ComparisonOperator ;
  rdf:type owl:NamedIndividual ;
  rdf:type skos:Concept ;
  rdfs:label "equalTo"@no ;
  skos:definition "Logical comparison operator of \"equal to\". "@en ;
  skos:inScheme :ComparisonOperatorCode ;
.
<http://spec.tn-its.eu/owl/tnits-owl#ComparisonOperator.greaterThan>
  rdf:type :ComparisonOperator ;
  rdf:type owl:NamedIndividual ;
  rdf:type skos:Concept ;
  rdfs:label "greaterThan"@no ;
  skos:definition "Logical comparison operator of \"greater than\". "@en ;
  skos:inScheme :ComparisonOperatorCode ;
.
<http://spec.tn-its.eu/owl/tnits-owl#ComparisonOperator.greaterThanOrEqualTo>
  rdf:type :ComparisonOperator ;
  rdf:type owl:NamedIndividual ;
  rdf:type skos:Concept ;
  rdfs:label "greaterThanOrEqualTo"@no ;
  skos:definition "Logical comparison operator of \"greater than or equal to\". "@en ;
  skos:inScheme :ComparisonOperatorCode ;
.
<http://spec.tn-its.eu/owl/tnits-owl#ComparisonOperator.lessThan>
  rdf:type :ComparisonOperator ;
  rdf:type owl:NamedIndividual ;
  rdf:type skos:Concept ;
  rdfs:label "lessThan"@no ;
  skos:definition "Logical comparison operator of \"less than\". "@en ;
  skos:inScheme :ComparisonOperatorCode ;
.
<http://spec.tn-its.eu/owl/tnits-owl#ComparisonOperator.lessThanOrEqualTo>
  rdf:type :ComparisonOperator ;
  rdf:type owl:NamedIndividual ;
  rdf:type skos:Concept ;
  rdfs:label "lessThanOrEqualTo"@no ;
  skos:definition "Logical comparison operator of \"less than or equal to\". "@en ;
  skos:inScheme :ComparisonOperatorCode ;
.
:ComparisonOperatorCode
  rdf:type owl:NamedIndividual ;
  rdf:type skos:ConceptScheme ;
  dc:isFormatOf :ComparisonOperator ;
  skos:definition "The logical operator to be used in a comparison operation. "@en ;
.
:Condition
  rdf:type owl:Class ;
  rdfs:label "Condition"@en ;
  rdfs:subClassOf :tnitsDataType ;
  rdfs:subClassOf [
      rdf:type owl:Restriction ;
      owl:allValuesFrom xsd:boolean ;
      owl:onProperty :negate ;
    ] ;
  rdfs:subClassOf [
      rdf:type owl:Restriction ;
      owl:maxQualifiedCardinality "1"^^xsd:nonNegativeInteger ;
      owl:onDataRange xsd:boolean ;
      owl:onProperty :negate ;
    ] ;
  owl:disjointUnionOf (
      :AreaCondition
      :ConditionSet
      :LaneCondition
      :RoadCategoryCondition
      :TimeCondition
      :VehicleCondition
      :WeatherCondition
    ) ;
  skos:definition "Abstract class that specifies a condition for the validity of a certain road feature such as time, weather conditions, vehicle type, vehicle propulsion fuel, vehicle occupancy, vehicle usage, restrictions of the vehicle driverâ€™s licence permissions, vehicle dimensions or weight characteristics."@en ;
.
:ConditionOperator
  rdf:type owl:Class ;
  rdfs:label "ConditionOperator"@en ;
  rdfs:subClassOf :tnitsEnumeration ;
  owl:equivalentClass [
      rdf:type owl:Class ;
      owl:oneOf (
          <http://spec.tn-its.eu/owl/tnits-owl#ConditionOperator.AND>
          <http://spec.tn-its.eu/owl/tnits-owl#ConditionOperator.OR>
          <http://spec.tn-its.eu/owl/tnits-owl#ConditionOperator.XOR>
        ) ;
    ] ;
  skos:definition "The logical operator to be used in a test of conditions "@en ;
.
<http://spec.tn-its.eu/owl/tnits-owl#ConditionOperator.AND>
  rdf:type :ConditionOperator ;
  rdf:type owl:NamedIndividual ;
  rdf:type skos:Concept ;
  rdfs:label "AND"@no ;
  skos:definition "The AND logical operator – a logical operation to determine if all conditions in a test are TRUE "@en ;
  skos:inScheme :ConditionOperatorCode ;
.
<http://spec.tn-its.eu/owl/tnits-owl#ConditionOperator.OR>
  rdf:type :ConditionOperator ;
  rdf:type owl:NamedIndividual ;
  rdf:type skos:Concept ;
  rdfs:label "OR"@no ;
  skos:definition "The OR logical operator – a logical operation to determine if any conditions in a test are TRUE "@en ;
  skos:inScheme :ConditionOperatorCode ;
.
<http://spec.tn-its.eu/owl/tnits-owl#ConditionOperator.XOR>
  rdf:type :ConditionOperator ;
  rdf:type owl:NamedIndividual ;
  rdf:type skos:Concept ;
  rdfs:label "XOR"@no ;
  skos:definition "The XOR logical operator - a logical operation that outputs true only when inputs differ (one is true, the other is false). "@en ;
  skos:inScheme :ConditionOperatorCode ;
.
:ConditionOperatorCode
  rdf:type owl:NamedIndividual ;
  rdf:type skos:ConceptScheme ;
  dc:isFormatOf :ConditionOperator ;
  skos:definition "The logical operator to be used in a test of conditions "@en ;
.
:ConditionSet
  rdf:type owl:Class ;
  rdfs:label "ConditionSet"@en ;
  rdfs:subClassOf :Condition ;
  rdfs:subClassOf [
      rdf:type owl:Restriction ;
      owl:allValuesFrom :Condition ;
      owl:onProperty :conditions ;
    ] ;
  rdfs:subClassOf [
      rdf:type owl:Restriction ;
      owl:allValuesFrom :ConditionOperator ;
      owl:onProperty :operator ;
    ] ;
  rdfs:subClassOf [
      rdf:type owl:Restriction ;
      owl:minQualifiedCardinality "1"^^xsd:nonNegativeInteger ;
      owl:onClass :Condition ;
      owl:onProperty :conditions ;
    ] ;
  rdfs:subClassOf [
      rdf:type owl:Restriction ;
      owl:onClass :ConditionOperator ;
      owl:onProperty :operator ;
      owl:qualifiedCardinality "1"^^xsd:nonNegativeInteger ;
    ] ;
  skos:definition "Groups a number of conditions into a condition set"@en ;
.
:Dataset
  rdf:type owl:Class ;
  rdfs:label "Dataset"@en ;
  rdfs:subClassOf :tnitsFeature ;
  rdfs:subClassOf [
      rdf:type owl:Restriction ;
      owl:allValuesFrom :Metadata ;
      owl:onProperty <http://spec.tn-its.eu/owl/tnits-owl#Dataset.metadata> ;
    ] ;
  rdfs:subClassOf [
      rdf:type owl:Restriction ;
      owl:maxQualifiedCardinality "1"^^xsd:nonNegativeInteger ;
      owl:onClass :Metadata ;
      owl:onProperty <http://spec.tn-its.eu/owl/tnits-owl#Dataset.metadata> ;
    ] ;
  owl:disjointUnionOf (
      :FeedbackDataset
      :RoadFeatureDataset
    ) ;
  skos:definition "Abstract class that represents any type of dataset that may be exchanged using TN-ITS  "@en ;
.
<http://spec.tn-its.eu/owl/tnits-owl#Dataset.metadata>
  rdf:type owl:ObjectProperty ;
  rdfs:domain :Dataset ;
  rdfs:label "Dataset.metadata"@en ;
  rdfs:range :Metadata ;
  skos:definition "Metadata for the dataset. "@en ;
.
:DatasetType
  rdf:type owl:Class ;
  rdfs:label "DatasetType"@en ;
  rdfs:subClassOf :tnitsEnumeration ;
  owl:equivalentClass [
      rdf:type owl:Class ;
      owl:oneOf (
          <http://spec.tn-its.eu/owl/tnits-owl#DatasetType.Snapshot>
          <http://spec.tn-its.eu/owl/tnits-owl#DatasetType.Update>
        ) ;
    ] ;
  skos:definition "Specifies the different possible types of datasets for road features  "@en ;
.
<http://spec.tn-its.eu/owl/tnits-owl#DatasetType.Snapshot>
  rdf:type :DatasetType ;
  rdf:type owl:NamedIndividual ;
  rdf:type skos:Concept ;
  rdfs:label "Snapshot"@no ;
  skos:definition "A snapshot dataset contains information (current status) of all road features in an area, or of all occurrences of one or more specified types of road features"@en ;
  skos:inScheme :DatasetTypeCode ;
.
<http://spec.tn-its.eu/owl/tnits-owl#DatasetType.Update>
  rdf:type :DatasetType ;
  rdf:type owl:NamedIndividual ;
  rdf:type skos:Concept ;
  rdfs:label "Update"@no ;
  skos:definition "A dataset consisting of only incremental updates for road features "@en ;
  skos:inScheme :DatasetTypeCode ;
.
:DatasetTypeCode
  rdf:type owl:NamedIndividual ;
  rdf:type skos:ConceptScheme ;
  dc:isFormatOf :DatasetType ;
  skos:definition "Specifies the different possible types of datasets for road features  "@en ;
.
:DayOfWeek
  rdf:type owl:Class ;
  rdfs:label "DayOfWeek"@en ;
  rdfs:subClassOf :tnitsEnumeration ;
  owl:equivalentClass [
      rdf:type owl:Class ;
      owl:oneOf (
          <http://spec.tn-its.eu/owl/tnits-owl#DayOfWeek.friday>
          <http://spec.tn-its.eu/owl/tnits-owl#DayOfWeek.monday>
          <http://spec.tn-its.eu/owl/tnits-owl#DayOfWeek.saturday>
          <http://spec.tn-its.eu/owl/tnits-owl#DayOfWeek.sunday>
          <http://spec.tn-its.eu/owl/tnits-owl#DayOfWeek.thursday>
          <http://spec.tn-its.eu/owl/tnits-owl#DayOfWeek.tuesday>
          <http://spec.tn-its.eu/owl/tnits-owl#DayOfWeek.wednesday>
        ) ;
    ] ;
  skos:definition "Applicable day of the week."@en ;
.
<http://spec.tn-its.eu/owl/tnits-owl#DayOfWeek.friday>
  rdf:type :DayOfWeek ;
  rdf:type owl:NamedIndividual ;
  rdf:type skos:Concept ;
  rdfs:label "friday"@no ;
  skos:inScheme :DayOfWeekCode ;
.
<http://spec.tn-its.eu/owl/tnits-owl#DayOfWeek.monday>
  rdf:type :DayOfWeek ;
  rdf:type owl:NamedIndividual ;
  rdf:type skos:Concept ;
  rdfs:label "monday"@no ;
  skos:inScheme :DayOfWeekCode ;
.
<http://spec.tn-its.eu/owl/tnits-owl#DayOfWeek.saturday>
  rdf:type :DayOfWeek ;
  rdf:type owl:NamedIndividual ;
  rdf:type skos:Concept ;
  rdfs:label "saturday"@no ;
  skos:inScheme :DayOfWeekCode ;
.
<http://spec.tn-its.eu/owl/tnits-owl#DayOfWeek.sunday>
  rdf:type :DayOfWeek ;
  rdf:type owl:NamedIndividual ;
  rdf:type skos:Concept ;
  rdfs:label "sunday"@no ;
  skos:inScheme :DayOfWeekCode ;
.
<http://spec.tn-its.eu/owl/tnits-owl#DayOfWeek.thursday>
  rdf:type :DayOfWeek ;
  rdf:type owl:NamedIndividual ;
  rdf:type skos:Concept ;
  rdfs:label "thursday"@no ;
  skos:inScheme :DayOfWeekCode ;
.
<http://spec.tn-its.eu/owl/tnits-owl#DayOfWeek.tuesday>
  rdf:type :DayOfWeek ;
  rdf:type owl:NamedIndividual ;
  rdf:type skos:Concept ;
  rdfs:label "tuesday"@no ;
  skos:inScheme :DayOfWeekCode ;
.
<http://spec.tn-its.eu/owl/tnits-owl#DayOfWeek.wednesday>
  rdf:type :DayOfWeek ;
  rdf:type owl:NamedIndividual ;
  rdf:type skos:Concept ;
  rdfs:label "wednesday"@no ;
  skos:inScheme :DayOfWeekCode ;
.
:DayOfWeekCode
  rdf:type owl:NamedIndividual ;
  rdf:type skos:ConceptScheme ;
  dc:isFormatOf :DayOfWeek ;
  skos:definition "Applicable day of the week."@en ;
.
:DayWeekMonth
  rdf:type owl:Class ;
  rdfs:label "DayWeekMonth"@en ;
  rdfs:subClassOf :tnitsDataType ;
  rdfs:subClassOf [
      rdf:type owl:Restriction ;
      owl:allValuesFrom :DayOfWeek ;
      owl:onProperty :applicableDay ;
    ] ;
  rdfs:subClassOf [
      rdf:type owl:Restriction ;
      owl:allValuesFrom :MonthOfYear ;
      owl:onProperty :applicableMonth ;
    ] ;
  rdfs:subClassOf [
      rdf:type owl:Restriction ;
      owl:allValuesFrom :WeekOfMonth ;
      owl:onProperty :applicableWeek ;
    ] ;
  rdfs:subClassOf [
      rdf:type owl:Restriction ;
      owl:maxQualifiedCardinality "12"^^xsd:nonNegativeInteger ;
      owl:onClass :MonthOfYear ;
      owl:onProperty :applicableMonth ;
    ] ;
  rdfs:subClassOf [
      rdf:type owl:Restriction ;
      owl:maxQualifiedCardinality "5"^^xsd:nonNegativeInteger ;
      owl:onClass :WeekOfMonth ;
      owl:onProperty :applicableWeek ;
    ] ;
  rdfs:subClassOf [
      rdf:type owl:Restriction ;
      owl:maxQualifiedCardinality "7"^^xsd:nonNegativeInteger ;
      owl:onClass :DayOfWeek ;
      owl:onProperty :applicableDay ;
    ] ;
  skos:definition "A recurring period defined in terms of days of the week, weeks of the month and months of the year. [SOURCE: CEN/TS16157-3:2011]"@en ;
.
:DynamicLocationReference
  rdf:type owl:Class ;
  rdfs:label "DynamicLocationReference"@en ;
  rdfs:subClassOf :LocationReference ;
  owl:disjointUnionOf (
      :AgoraLocationReference
      :OpenLRLocationReference
    ) ;
  skos:definition "Abstract class that specifies all types of dynamic location references in accordance with ISO 19111. "@en ;
.
:EmissionClassificationEuro
  rdf:type owl:Class ;
  rdfs:label "EmissionClassificationEuro"@en ;
  rdfs:subClassOf :tnitsCodeList ;
  skos:definition "Specifies the available list of enumerations for the minimum Euro emission classification the vehicle(s) have to comply with according to the 1970 Directive 70/220/EEC and its several amendments. Note that vehicleType and fuelType need to be provided in order to make this classification explicit. [SOURCE - DATEX 3.0 Part 7 (proposed EN/16157-7:2018)]"@en ;
.
:EmissionClassificationEuroCode
  rdf:type owl:NamedIndividual ;
  rdf:type skos:ConceptScheme ;
  dc:isFormatOf :EmissionClassificationEuro ;
  skos:definition "Specifies the available list of enumerations for the minimum Euro emission classification the vehicle(s) have to comply with according to the 1970 Directive 70/220/EEC and its several amendments. Note that vehicleType and fuelType need to be provided in order to make this classification explicit. [SOURCE - DATEX 3.0 Part 7 (proposed EN/16157-7:2018)]"@en ;
.
:Emissions
  rdf:type owl:Class ;
  rdfs:label "Emissions"@en ;
  rdfs:subClassOf :tnitsDataType ;
  rdfs:subClassOf [
      rdf:type owl:Restriction ;
      owl:allValuesFrom :EmissionClassificationEuro ;
      owl:onProperty <http://spec.tn-its.eu/owl/tnits-owl#Emissions.emissionClassificationEuro> ;
    ] ;
  rdfs:subClassOf [
      rdf:type owl:Restriction ;
      owl:allValuesFrom :LowEmissionLevel ;
      owl:onProperty :emissionLevel ;
    ] ;
  rdfs:subClassOf [
      rdf:type owl:Restriction ;
      owl:allValuesFrom xsd:string ;
      owl:onProperty :emissionClassificationOther ;
    ] ;
  rdfs:subClassOf [
      rdf:type owl:Restriction ;
      owl:maxQualifiedCardinality "1"^^xsd:nonNegativeInteger ;
      owl:onClass :EmissionClassificationEuro ;
      owl:onProperty <http://spec.tn-its.eu/owl/tnits-owl#Emissions.emissionClassificationEuro> ;
    ] ;
  rdfs:subClassOf [
      rdf:type owl:Restriction ;
      owl:maxQualifiedCardinality "1"^^xsd:nonNegativeInteger ;
      owl:onClass :LowEmissionLevel ;
      owl:onProperty :emissionLevel ;
    ] ;
  skos:definition "Emission characteristics of vehicles. [SOURCE: DATEX 3.0 Part 7 (proposed EN 16157-7:2018)]  "@en ;
.
<http://spec.tn-its.eu/owl/tnits-owl#Emissions.emissionClassificationEuro>
  rdf:type owl:ObjectProperty ;
  rdfs:domain :Emissions ;
  rdfs:label "Emissions.emissionClassificationEuro"@en ;
  rdfs:range :EmissionClassificationEuro ;
  skos:definition "The minimum Euro emission classification the vehicle(s) have to comply with according to the 1970 Directive 70/220/EEC and its several amendments. Note that vehicleType and fuelType need to be provided in order to make this classification explicit. [SOURCE: DATEX 3.0 Part 7 (proposed EN 161577:2018)] "@en ;
.
:FeedbackDataset
  rdf:type owl:Class ;
  rdfs:label "FeedbackDataset"@en ;
  rdfs:subClassOf :Dataset ;
  rdfs:subClassOf [
      rdf:type owl:Restriction ;
      owl:allValuesFrom :FeedbackInformation ;
      owl:onProperty :feedbackInfo ;
    ] ;
  rdfs:subClassOf [
      rdf:type owl:Restriction ;
      owl:onClass :FeedbackInformation ;
      owl:onProperty :feedbackInfo ;
      owl:qualifiedCardinality "1"^^xsd:nonNegativeInteger ;
    ] ;
  skos:definition "A dataset containing feedback to the road authorities/road operators from an information provider/map provider in response to data download and integration  "@en ;
.
:FeedbackInformation
  rdf:type owl:Class ;
  rdfs:label "FeedbackInformation"@en ;
  rdfs:subClassOf :tnitsFeature ;
  rdfs:subClassOf [
      rdf:type owl:Restriction ;
      owl:allValuesFrom :FeedbackLog ;
      owl:onProperty :log ;
    ] ;
  rdfs:subClassOf [
      rdf:type owl:Restriction ;
      owl:allValuesFrom :Identifier ;
      owl:onProperty :datasetId ;
    ] ;
  rdfs:subClassOf [
      rdf:type owl:Restriction ;
      owl:allValuesFrom xsd:dateTime ;
      owl:onProperty :processed ;
    ] ;
  rdfs:subClassOf [
      rdf:type owl:Restriction ;
      owl:onClass :FeedbackLog ;
      owl:onProperty :log ;
      owl:qualifiedCardinality "1"^^xsd:nonNegativeInteger ;
    ] ;
  rdfs:subClassOf [
      rdf:type owl:Restriction ;
      owl:onClass :Identifier ;
      owl:onProperty :datasetId ;
      owl:qualifiedCardinality "1"^^xsd:nonNegativeInteger ;
    ] ;
  rdfs:subClassOf [
      rdf:type owl:Restriction ;
      owl:onDataRange xsd:dateTime ;
      owl:onProperty :processed ;
      owl:qualifiedCardinality "1"^^xsd:nonNegativeInteger ;
    ] ;
  skos:definition "Represents the information sent back from a downloading client to the provider of road attributes  "@en ;
.
:FeedbackLog
  rdf:type owl:Class ;
  rdfs:label "FeedbackLog"@en ;
  rdfs:subClassOf :tnitsFeature ;
  rdfs:subClassOf [
      rdf:type owl:Restriction ;
      owl:allValuesFrom :FeedbackLogEvent ;
      owl:onProperty :events ;
    ] ;
  rdfs:subClassOf [
      rdf:type owl:Restriction ;
      owl:allValuesFrom :SummaryInfo ;
      owl:onProperty :summary ;
    ] ;
  rdfs:subClassOf [
      rdf:type owl:Restriction ;
      owl:onClass :SummaryInfo ;
      owl:onProperty :summary ;
      owl:qualifiedCardinality "1"^^xsd:nonNegativeInteger ;
    ] ;
  skos:definition "Represents a log which records all events that are reported back from a client as a result of download and integration of data  "@en ;
.
:FeedbackLogEvent
  rdf:type owl:Class ;
  rdfs:label "FeedbackLogEvent"@en ;
  rdfs:subClassOf :tnitsFeature ;
  owl:disjointUnionOf (
      :FreeTextEvent
      :GeneralFeedbackEvent
      :RoadFeatureEvent
    ) ;
  skos:definition "Abstract base class that represents any type of event that may occur during download and integration of data that needs to be reported back to the provider  "@en ;
.
:FreeTextEvent
  rdf:type owl:Class ;
  rdfs:label "FreeTextEvent"@en ;
  rdfs:subClassOf :FeedbackLogEvent ;
  rdfs:subClassOf [
      rdf:type owl:Restriction ;
      owl:allValuesFrom xsd:string ;
      owl:onProperty <http://spec.tn-its.eu/owl/tnits-owl#FreeTextEvent.text> ;
    ] ;
  rdfs:subClassOf [
      rdf:type owl:Restriction ;
      owl:onDataRange xsd:string ;
      owl:onProperty <http://spec.tn-its.eu/owl/tnits-owl#FreeTextEvent.text> ;
      owl:qualifiedCardinality "1"^^xsd:nonNegativeInteger ;
    ] ;
  skos:definition "Represents one event that is described using free text  "@en ;
.
<http://spec.tn-its.eu/owl/tnits-owl#FreeTextEvent.text>
  rdf:type owl:DatatypeProperty ;
  rdf:type owl:FunctionalProperty ;
  rdfs:domain :FreeTextEvent ;
  rdfs:label "FreeTextEvent.text"@en ;
  rdfs:range xsd:string ;
  skos:definition "The text describing the event "@en ;
.
:FuelType
  rdf:type owl:Class ;
  rdfs:label "FuelType"@en ;
  rdfs:subClassOf :tnitsCodeList ;
  skos:definition "Specifies the available list of enumerations for the type of fuel used by the vehicle."@en ;
.
:FuelTypeCode
  rdf:type owl:NamedIndividual ;
  rdf:type skos:ConceptScheme ;
  dc:isFormatOf :FuelType ;
  skos:definition "Specifies the available list of enumerations for the type of fuel used by the vehicle."@en ;
.
:FuzzyTimePeriod
  rdf:type owl:Class ;
  rdfs:label "FuzzyTimePeriod"@en ;
  rdfs:subClassOf :tnitsDataType ;
  rdfs:subClassOf [
      rdf:type owl:Restriction ;
      owl:allValuesFrom :FuzzyTimeType ;
      owl:onProperty :beginOrDuration ;
    ] ;
  rdfs:subClassOf [
      rdf:type owl:Restriction ;
      owl:allValuesFrom :FuzzyTimeType ;
      owl:onProperty :endOrDuration ;
    ] ;
  rdfs:subClassOf [
      rdf:type owl:Restriction ;
      owl:maxQualifiedCardinality "1"^^xsd:nonNegativeInteger ;
      owl:onClass :FuzzyTimeType ;
      owl:onProperty :endOrDuration ;
    ] ;
  rdfs:subClassOf [
      rdf:type owl:Restriction ;
      owl:onClass :FuzzyTimeType ;
      owl:onProperty :beginOrDuration ;
      owl:qualifiedCardinality "1"^^xsd:nonNegativeInteger ;
    ] ;
  skos:definition "Specifies the time period with non-precise characteristics  "@en ;
.
:FuzzyTimeType
  rdf:type owl:Class ;
  rdfs:label "FuzzyTimeType"@en ;
  rdfs:subClassOf :tnitsCodeList ;
  skos:definition "Specifies the available list of enumerations for the fuzzy time concepts, which provided the definition of start, end or duration time concepts that support the expression of a non-precise or variable qualified concept, resulting in a non-precise, potentially circumstantial defined time period.  Note: Example roads closed at the start of winter in mountainous areas, which is based on actual experienced weather conditions and therefore is not pre-defined.  "@en ;
.
:FuzzyTimeTypeCode
  rdf:type owl:NamedIndividual ;
  rdf:type skos:ConceptScheme ;
  dc:isFormatOf :FuzzyTimeType ;
  skos:definition "Specifies the available list of enumerations for the fuzzy time concepts, which provided the definition of start, end or duration time concepts that support the expression of a non-precise or variable qualified concept, resulting in a non-precise, potentially circumstantial defined time period.  Note: Example roads closed at the start of winter in mountainous areas, which is based on actual experienced weather conditions and therefore is not pre-defined.  "@en ;
.
:GasType
  rdf:type owl:Class ;
  rdfs:label "GasType"@en ;
  rdfs:subClassOf :tnitsCodeList ;
  skos:definition "Specifies the available list of enumerations for types of propellant gas."@en ;
.
:GasTypeCode
  rdf:type owl:NamedIndividual ;
  rdf:type skos:ConceptScheme ;
  dc:isFormatOf :GasType ;
  skos:definition "Specifies the available list of enumerations for types of propellant gas."@en ;
.
:GeneralFeedbackEvent
  rdf:type owl:Class ;
  rdfs:label "GeneralFeedbackEvent"@en ;
  rdfs:subClassOf :FeedbackLogEvent ;
  rdfs:subClassOf [
      rdf:type owl:Restriction ;
      owl:allValuesFrom :GeneralFeedbackEventType ;
      owl:onProperty :eventCode ;
    ] ;
  rdfs:subClassOf [
      rdf:type owl:Restriction ;
      owl:onClass :GeneralFeedbackEventType ;
      owl:onProperty :eventCode ;
      owl:qualifiedCardinality "1"^^xsd:nonNegativeInteger ;
    ] ;
  skos:definition "Represents one event that may occur during download and integration of data that needs to be reported back to the provider  "@en ;
.
:GeneralFeedbackEventType
  rdf:type owl:Class ;
  rdfs:label "GeneralFeedbackEventType"@en ;
  rdfs:subClassOf :tnitsCodeList ;
  skos:definition "Specifies the available list of enumerations for types of general feedback events."@en ;
.
:GeneralFeedbackEventTypeCode
  rdf:type owl:NamedIndividual ;
  rdf:type skos:ConceptScheme ;
  dc:isFormatOf :GeneralFeedbackEventType ;
  skos:definition "Specifies the available list of enumerations for types of general feedback events."@en ;
.
:GenericRoadFeatureProperty
  rdf:type owl:Class ;
  rdfs:label "GenericRoadFeatureProperty"@en ;
  rdfs:subClassOf :AbstractRoadFeatureProperty ;
  rdfs:subClassOf [
      rdf:type owl:Restriction ;
      owl:allValuesFrom :Any ;
      owl:onProperty <http://spec.tn-its.eu/owl/tnits-owl#GenericRoadFeatureProperty.value> ;
    ] ;
  rdfs:subClassOf [
      rdf:type owl:Restriction ;
      owl:allValuesFrom :PropertyValueReferenceType ;
      owl:onProperty :valueReference ;
    ] ;
  rdfs:subClassOf [
      rdf:type owl:Restriction ;
      owl:allValuesFrom :RoadFeaturePropertyType ;
      owl:onProperty <http://spec.tn-its.eu/owl/tnits-owl#GenericRoadFeatureProperty.type> ;
    ] ;
  rdfs:subClassOf [
      rdf:type owl:Restriction ;
      owl:onClass :RoadFeaturePropertyType ;
      owl:onProperty <http://spec.tn-its.eu/owl/tnits-owl#GenericRoadFeatureProperty.type> ;
      owl:qualifiedCardinality "1"^^xsd:nonNegativeInteger ;
    ] ;
  skos:definition "A representation of a road feature property value "@en ;
.
<http://spec.tn-its.eu/owl/tnits-owl#GenericRoadFeatureProperty.type>
  rdf:type owl:FunctionalProperty ;
  rdf:type owl:ObjectProperty ;
  rdfs:domain :GenericRoadFeatureProperty ;
  rdfs:label "GenericRoadFeatureProperty.type"@en ;
  rdfs:range :RoadFeaturePropertyType ;
  skos:definition "The type of road feature property by reference to an item in an external code list"@en ;
.
<http://spec.tn-its.eu/owl/tnits-owl#GenericRoadFeatureProperty.value>
  rdf:type owl:ObjectProperty ;
  rdfs:domain :GenericRoadFeatureProperty ;
  rdfs:label "GenericRoadFeatureProperty.value"@en ;
  rdfs:range :Any ;
  skos:definition "The value of the road feature property"@en ;
.
:GeometryLocationReference
  rdf:type owl:Class ;
  rdfs:label "GeometryLocationReference"@en ;
  rdfs:subClassOf :LocationReference ;
  rdfs:subClassOf [
      rdf:type owl:Restriction ;
      owl:allValuesFrom gsp:Geometry ;
      owl:onProperty :encodedGeometry ;
    ] ;
  rdfs:subClassOf [
      rdf:type owl:Restriction ;
      owl:onClass gsp:Geometry ;
      owl:onProperty :encodedGeometry ;
      owl:qualifiedCardinality "1"^^xsd:nonNegativeInteger ;
    ] ;
  skos:definition "Class that references location by use of a geometry reference "@en ;
.
:GrossWeightCharacteristic
  rdf:type owl:Class ;
  rdfs:label "GrossWeightCharacteristic"@en ;
  rdfs:subClassOf :tnitsDataType ;
  rdfs:subClassOf [
      rdf:type owl:Restriction ;
      owl:allValuesFrom :ComparisonOperator ;
      owl:onProperty :comparisonOperator ;
    ] ;
  rdfs:subClassOf [
      rdf:type owl:Restriction ;
      owl:allValuesFrom :Measure ;
      owl:onProperty :grossVehicleWeight ;
    ] ;
  rdfs:subClassOf [
      rdf:type owl:Restriction ;
      owl:allValuesFrom :WeightType ;
      owl:onProperty :typeOfWeight ;
    ] ;
  rdfs:subClassOf [
      rdf:type owl:Restriction ;
      owl:onClass :ComparisonOperator ;
      owl:onProperty :comparisonOperator ;
      owl:qualifiedCardinality "1"^^xsd:nonNegativeInteger ;
    ] ;
  rdfs:subClassOf [
      rdf:type owl:Restriction ;
      owl:onClass :Measure ;
      owl:onProperty :grossVehicleWeight ;
      owl:qualifiedCardinality "1"^^xsd:nonNegativeInteger ;
    ] ;
  rdfs:subClassOf [
      rdf:type owl:Restriction ;
      owl:onClass :WeightType ;
      owl:onProperty :typeOfWeight ;
      owl:qualifiedCardinality "1"^^xsd:nonNegativeInteger ;
    ] ;
  skos:definition "Gross weight characteristic of a vehicle. [SOURCE: CEN/TS16157-3:2011] "@en ;
.
:HeaviestAxleWeightCharacteristic
  rdf:type owl:Class ;
  rdfs:label "HeaviestAxleWeightCharacteristic"@en ;
  rdfs:subClassOf :tnitsDataType ;
  rdfs:subClassOf [
      rdf:type owl:Restriction ;
      owl:allValuesFrom :ComparisonOperator ;
      owl:onProperty :comparisonOperator ;
    ] ;
  rdfs:subClassOf [
      rdf:type owl:Restriction ;
      owl:allValuesFrom :Measure ;
      owl:onProperty :heaviestAxleWeight ;
    ] ;
  rdfs:subClassOf [
      rdf:type owl:Restriction ;
      owl:onClass :ComparisonOperator ;
      owl:onProperty :comparisonOperator ;
      owl:qualifiedCardinality "1"^^xsd:nonNegativeInteger ;
    ] ;
  rdfs:subClassOf [
      rdf:type owl:Restriction ;
      owl:onClass :Measure ;
      owl:onProperty :heaviestAxleWeight ;
      owl:qualifiedCardinality "1"^^xsd:nonNegativeInteger ;
    ] ;
  skos:definition "Weight characteristic of the heaviest axle on the vehicle. [SOURCE: CEN/TS16157-3:2011] "@en ;
.
:HeightCharacteristic
  rdf:type owl:Class ;
  rdfs:label "HeightCharacteristic"@en ;
  rdfs:subClassOf :tnitsDataType ;
  rdfs:subClassOf [
      rdf:type owl:Restriction ;
      owl:allValuesFrom :ComparisonOperator ;
      owl:onProperty :comparisonOperator ;
    ] ;
  rdfs:subClassOf [
      rdf:type owl:Restriction ;
      owl:allValuesFrom :Measure ;
      owl:onProperty :vehicleHeight ;
    ] ;
  rdfs:subClassOf [
      rdf:type owl:Restriction ;
      owl:onClass :ComparisonOperator ;
      owl:onProperty :comparisonOperator ;
      owl:qualifiedCardinality "1"^^xsd:nonNegativeInteger ;
    ] ;
  rdfs:subClassOf [
      rdf:type owl:Restriction ;
      owl:onClass :Measure ;
      owl:onProperty :vehicleHeight ;
      owl:qualifiedCardinality "1"^^xsd:nonNegativeInteger ;
    ] ;
  skos:definition "Height characteristic of a vehicle. [SOURCE: CEN/TS16157-3:2011] "@en ;
.
:ISO19115Metadata
  rdf:type owl:ObjectProperty ;
  rdfs:domain :Metadata ;
  rdfs:label "ISO19115Metadata"@en ;
  rdfs:range <http://def.isotc211.org/iso19115/-1/2014/MetadataInformation#MD_Metadata> ;
.
:Identifier
  rdf:type owl:Class ;
  rdfs:label "Identifier"@en ;
  rdfs:subClassOf :tnitsDataType ;
  rdfs:subClassOf [
      rdf:type owl:Restriction ;
      owl:allValuesFrom xsd:string ;
      owl:onProperty :localId ;
    ] ;
  rdfs:subClassOf [
      rdf:type owl:Restriction ;
      owl:allValuesFrom xsd:string ;
      owl:onProperty :namespace ;
    ] ;
  rdfs:subClassOf [
      rdf:type owl:Restriction ;
      owl:allValuesFrom xsd:string ;
      owl:onProperty :versionId ;
    ] ;
  rdfs:subClassOf [
      rdf:type owl:Restriction ;
      owl:maxQualifiedCardinality "1"^^xsd:nonNegativeInteger ;
      owl:onDataRange xsd:string ;
      owl:onProperty :versionId ;
    ] ;
  rdfs:subClassOf [
      rdf:type owl:Restriction ;
      owl:onDataRange xsd:string ;
      owl:onProperty :localId ;
      owl:qualifiedCardinality "1"^^xsd:nonNegativeInteger ;
    ] ;
  rdfs:subClassOf [
      rdf:type owl:Restriction ;
      owl:onDataRange xsd:string ;
      owl:onProperty :namespace ;
      owl:qualifiedCardinality "1"^^xsd:nonNegativeInteger ;
    ] ;
  skos:definition "External unique object identifier published by the responsible body, which may be used by external applications to reference the spatial object."@en ;
.
:LaneCondition
  rdf:type owl:Class ;
  rdfs:label "LaneCondition"@en ;
  rdfs:subClassOf :Condition ;
  rdfs:subClassOf [
      rdf:type owl:Restriction ;
      owl:allValuesFrom xsd:integer ;
      owl:onProperty :laneExtension ;
    ] ;
  rdfs:subClassOf [
      rdf:type owl:Restriction ;
      owl:allValuesFrom xsd:integer ;
      owl:onProperty :startLane ;
    ] ;
  rdfs:subClassOf [
      rdf:type owl:Restriction ;
      owl:onDataRange xsd:integer ;
      owl:onProperty :laneExtension ;
      owl:qualifiedCardinality "1"^^xsd:nonNegativeInteger ;
    ] ;
  rdfs:subClassOf [
      rdf:type owl:Restriction ;
      owl:onDataRange xsd:integer ;
      owl:onProperty :startLane ;
      owl:qualifiedCardinality "1"^^xsd:nonNegativeInteger ;
    ] ;
  skos:definition "Specifies the applicability of a condition to specific lanes "@en ;
.
:LengthCharacteristic
  rdf:type owl:Class ;
  rdfs:label "LengthCharacteristic"@en ;
  rdfs:subClassOf :tnitsDataType ;
  rdfs:subClassOf [
      rdf:type owl:Restriction ;
      owl:allValuesFrom :ComparisonOperator ;
      owl:onProperty :comparisonOperator ;
    ] ;
  rdfs:subClassOf [
      rdf:type owl:Restriction ;
      owl:allValuesFrom :Measure ;
      owl:onProperty :vehicleLength ;
    ] ;
  rdfs:subClassOf [
      rdf:type owl:Restriction ;
      owl:onClass :ComparisonOperator ;
      owl:onProperty :comparisonOperator ;
      owl:qualifiedCardinality "1"^^xsd:nonNegativeInteger ;
    ] ;
  rdfs:subClassOf [
      rdf:type owl:Restriction ;
      owl:onClass :Measure ;
      owl:onProperty :vehicleLength ;
      owl:qualifiedCardinality "1"^^xsd:nonNegativeInteger ;
    ] ;
  skos:definition "Length characteristic of a vehicle. [SOURCE: CEN/TS16157-3:2011] "@en ;
.
:LinearLocationReference
  rdf:type owl:Class ;
  rdfs:label "LinearLocationReference"@en ;
  rdfs:subClassOf :PreCodedLocationReference ;
  rdfs:subClassOf [
      rdf:type owl:Restriction ;
      owl:allValuesFrom :NetworkReference ;
      owl:onProperty <http://spec.tn-its.eu/owl/tnits-owl#LinearLocationReference.networkReference> ;
    ] ;
  rdfs:subClassOf [
      rdf:type owl:Restriction ;
      owl:allValuesFrom xsd:string ;
      owl:onProperty :description ;
    ] ;
  rdfs:subClassOf [
      rdf:type owl:Restriction ;
      owl:allValuesFrom xsd:string ;
      owl:onProperty :name ;
    ] ;
  rdfs:subClassOf [
      rdf:type owl:Restriction ;
      owl:maxQualifiedCardinality "1"^^xsd:nonNegativeInteger ;
      owl:onDataRange xsd:string ;
      owl:onProperty :description ;
    ] ;
  rdfs:subClassOf [
      rdf:type owl:Restriction ;
      owl:maxQualifiedCardinality "1"^^xsd:nonNegativeInteger ;
      owl:onDataRange xsd:string ;
      owl:onProperty :name ;
    ] ;
  rdfs:subClassOf [
      rdf:type owl:Restriction ;
      owl:minQualifiedCardinality "1"^^xsd:nonNegativeInteger ;
      owl:onClass :NetworkReference ;
      owl:onProperty <http://spec.tn-its.eu/owl/tnits-owl#LinearLocationReference.networkReference> ;
    ] ;
  skos:definition "A type of precoded location reference that references a location by use of a specified reference  "@en ;
.
<http://spec.tn-its.eu/owl/tnits-owl#LinearLocationReference.networkReference>
  rdf:type owl:ObjectProperty ;
  rdfs:domain :LinearLocationReference ;
  rdfs:label "LinearLocationReference.networkReference"@en ;
  rdfs:range :NetworkReference ;
  skos:definition "A link to a specific network reference "@en ;
.
:LinkDirectionValue
  rdf:type owl:Class ;
  rdfs:label "LinkDirectionValue"@en ;
  rdfs:subClassOf :tnitsCodeList ;
  skos:definition "-- Definition -- List of values for directions relative to a link"@en ;
.
<http://spec.tn-its.eu/owl/tnits-owl#LinkDirectionValue.bothDirections>
  rdf:type :LinkDirectionValue ;
  rdf:type owl:NamedIndividual ;
  rdf:type skos:Concept ;
  rdfs:label "bothDirections"@no ;
  skos:definition "-- Definition -- In both directions. "@en ;
  skos:inScheme :LinkDirectionValueCode ;
.
<http://spec.tn-its.eu/owl/tnits-owl#LinkDirectionValue.inDirection>
  rdf:type :LinkDirectionValue ;
  rdf:type owl:NamedIndividual ;
  rdf:type skos:Concept ;
  rdfs:label "inDirection"@no ;
  skos:definition "-- Definition -- In direction of the link. "@en ;
  skos:inScheme :LinkDirectionValueCode ;
.
<http://spec.tn-its.eu/owl/tnits-owl#LinkDirectionValue.inOppositeDirection>
  rdf:type :LinkDirectionValue ;
  rdf:type owl:NamedIndividual ;
  rdf:type skos:Concept ;
  rdfs:label "inOppositeDirection"@no ;
  skos:definition "-- Definition -- In the opposite direction of the link. "@en ;
  skos:inScheme :LinkDirectionValueCode ;
.
:LinkDirectionValueCode
  rdf:type owl:NamedIndividual ;
  rdf:type skos:ConceptScheme ;
  dc:isFormatOf :LinkDirectionValue ;
  skos:definition "-- Definition -- List of values for directions relative to a link"@en ;
.
:LinkReference
  rdf:type owl:Class ;
  rdfs:label "LinkReference"@en ;
  rdfs:subClassOf :NetworkReference ;
  rdfs:subClassOf [
      rdf:type owl:Restriction ;
      owl:allValuesFrom :LinkDirectionValue ;
      owl:onProperty :applicableDirection ;
    ] ;
  rdfs:subClassOf [
      rdf:type owl:Restriction ;
      owl:onClass :LinkDirectionValue ;
      owl:onProperty :applicableDirection ;
      owl:qualifiedCardinality "1"^^xsd:nonNegativeInteger ;
    ] ;
  owl:disjointUnionOf (
      :SimpleLinearReference
      :SimplePointReference
    ) ;
  skos:definition "A specialisation of a network reference to provide a reference to a network link "@en ;
.
:LoadType
  rdf:type owl:Class ;
  rdfs:label "LoadType"@en ;
  rdfs:subClassOf :tnitsCodeList ;
  skos:definition "Specifies the available list of enumerations for types of vehicle loads"@en ;
.
:LoadTypeCode
  rdf:type owl:NamedIndividual ;
  rdf:type skos:ConceptScheme ;
  dc:isFormatOf :LoadType ;
  skos:definition "Specifies the available list of enumerations for types of vehicle loads"@en ;
.
:LocationByExternalReference
  rdf:type owl:Class ;
  rdfs:label "LocationByExternalReference"@en ;
  rdfs:subClassOf :PreCodedLocationReference ;
  rdfs:subClassOf [
      rdf:type owl:Restriction ;
      owl:allValuesFrom :PredefinedLocation ;
      owl:onProperty :predefinedLocationReference ;
    ] ;
  rdfs:subClassOf [
      rdf:type owl:Restriction ;
      owl:onClass :PredefinedLocation ;
      owl:onProperty :predefinedLocationReference ;
      owl:qualifiedCardinality "1"^^xsd:nonNegativeInteger ;
    ] ;
  skos:definition "A type of precoded location reference that references a location by use of a specified reference  "@en ;
.
:LocationReference
  rdf:type owl:Class ;
  rdfs:label "LocationReference"@en ;
  rdfs:subClassOf :tnitsDataType ;
  owl:disjointUnionOf (
      :DynamicLocationReference
      :GeometryLocationReference
      :PreCodedLocationReference
    ) ;
  skos:definition "Abstract class that specifies any type of location reference for TN-ITS "@en ;
.
:LowEmissionLevel
  rdf:type owl:Class ;
  rdfs:label "LowEmissionLevel"@en ;
  rdfs:subClassOf :tnitsCodeList ;
  skos:definition "Specifies the available list of enumerations for vehicle emission levels"@en ;
.
:LowEmissionLevelCode
  rdf:type owl:NamedIndividual ;
  rdf:type skos:ConceptScheme ;
  dc:isFormatOf :LowEmissionLevel ;
  skos:definition "Specifies the available list of enumerations for vehicle emission levels"@en ;
.
:Measure
  rdf:type owl:Class ;
.
:Metadata
  rdf:type owl:Class ;
  rdfs:label "Metadata"@en ;
  rdfs:subClassOf :tnitsDataType ;
  rdfs:subClassOf [
      rdf:type owl:Restriction ;
      owl:allValuesFrom <http://def.isotc211.org/iso19115/-1/2014/MetadataInformation#MD_Metadata> ;
      owl:onProperty :ISO19115Metadata ;
    ] ;
  rdfs:subClassOf [
      rdf:type owl:Restriction ;
      owl:allValuesFrom :Identifier ;
      owl:onProperty :datasetId ;
    ] ;
  rdfs:subClassOf [
      rdf:type owl:Restriction ;
      owl:allValuesFrom xsd:dateTime ;
      owl:onProperty :datasetCreationTime ;
    ] ;
  rdfs:subClassOf [
      rdf:type owl:Restriction ;
      owl:maxQualifiedCardinality "1"^^xsd:nonNegativeInteger ;
      owl:onClass <http://def.isotc211.org/iso19115/-1/2014/MetadataInformation#MD_Metadata> ;
      owl:onProperty :ISO19115Metadata ;
    ] ;
  rdfs:subClassOf [
      rdf:type owl:Restriction ;
      owl:onClass :Identifier ;
      owl:onProperty :datasetId ;
      owl:qualifiedCardinality "1"^^xsd:nonNegativeInteger ;
    ] ;
  rdfs:subClassOf [
      rdf:type owl:Restriction ;
      owl:onDataRange xsd:dateTime ;
      owl:onProperty :datasetCreationTime ;
      owl:qualifiedCardinality "1"^^xsd:nonNegativeInteger ;
    ] ;
  skos:definition "Characterises the type of metadata "@en ;
.
:MonthOfYear
  rdf:type owl:Class ;
  rdfs:label "MonthOfYear"@en ;
  rdfs:subClassOf :tnitsEnumeration ;
  owl:equivalentClass [
      rdf:type owl:Class ;
      owl:oneOf (
          <http://spec.tn-its.eu/owl/tnits-owl#MonthOfYear.april>
          <http://spec.tn-its.eu/owl/tnits-owl#MonthOfYear.august>
          <http://spec.tn-its.eu/owl/tnits-owl#MonthOfYear.december>
          <http://spec.tn-its.eu/owl/tnits-owl#MonthOfYear.february>
          <http://spec.tn-its.eu/owl/tnits-owl#MonthOfYear.january>
          <http://spec.tn-its.eu/owl/tnits-owl#MonthOfYear.july>
          <http://spec.tn-its.eu/owl/tnits-owl#MonthOfYear.june>
          <http://spec.tn-its.eu/owl/tnits-owl#MonthOfYear.march>
          <http://spec.tn-its.eu/owl/tnits-owl#MonthOfYear.may>
          <http://spec.tn-its.eu/owl/tnits-owl#MonthOfYear.november>
          <http://spec.tn-its.eu/owl/tnits-owl#MonthOfYear.october>
          <http://spec.tn-its.eu/owl/tnits-owl#MonthOfYear.september>
        ) ;
    ] ;
  skos:definition "Applicable month of the year."@en ;
.
<http://spec.tn-its.eu/owl/tnits-owl#MonthOfYear.april>
  rdf:type :MonthOfYear ;
  rdf:type owl:NamedIndividual ;
  rdf:type skos:Concept ;
  rdfs:label "april"@no ;
  skos:inScheme :MonthOfYearCode ;
.
<http://spec.tn-its.eu/owl/tnits-owl#MonthOfYear.august>
  rdf:type :MonthOfYear ;
  rdf:type owl:NamedIndividual ;
  rdf:type skos:Concept ;
  rdfs:label "august"@no ;
  skos:inScheme :MonthOfYearCode ;
.
<http://spec.tn-its.eu/owl/tnits-owl#MonthOfYear.december>
  rdf:type :MonthOfYear ;
  rdf:type owl:NamedIndividual ;
  rdf:type skos:Concept ;
  rdfs:label "december"@no ;
  skos:inScheme :MonthOfYearCode ;
.
<http://spec.tn-its.eu/owl/tnits-owl#MonthOfYear.february>
  rdf:type :MonthOfYear ;
  rdf:type owl:NamedIndividual ;
  rdf:type skos:Concept ;
  rdfs:label "february"@no ;
  skos:inScheme :MonthOfYearCode ;
.
<http://spec.tn-its.eu/owl/tnits-owl#MonthOfYear.january>
  rdf:type :MonthOfYear ;
  rdf:type owl:NamedIndividual ;
  rdf:type skos:Concept ;
  rdfs:label "january"@no ;
  skos:inScheme :MonthOfYearCode ;
.
<http://spec.tn-its.eu/owl/tnits-owl#MonthOfYear.july>
  rdf:type :MonthOfYear ;
  rdf:type owl:NamedIndividual ;
  rdf:type skos:Concept ;
  rdfs:label "july"@no ;
  skos:inScheme :MonthOfYearCode ;
.
<http://spec.tn-its.eu/owl/tnits-owl#MonthOfYear.june>
  rdf:type :MonthOfYear ;
  rdf:type owl:NamedIndividual ;
  rdf:type skos:Concept ;
  rdfs:label "june"@no ;
  skos:inScheme :MonthOfYearCode ;
.
<http://spec.tn-its.eu/owl/tnits-owl#MonthOfYear.march>
  rdf:type :MonthOfYear ;
  rdf:type owl:NamedIndividual ;
  rdf:type skos:Concept ;
  rdfs:label "march"@no ;
  skos:inScheme :MonthOfYearCode ;
.
<http://spec.tn-its.eu/owl/tnits-owl#MonthOfYear.may>
  rdf:type :MonthOfYear ;
  rdf:type owl:NamedIndividual ;
  rdf:type skos:Concept ;
  rdfs:label "may"@no ;
  skos:inScheme :MonthOfYearCode ;
.
<http://spec.tn-its.eu/owl/tnits-owl#MonthOfYear.november>
  rdf:type :MonthOfYear ;
  rdf:type owl:NamedIndividual ;
  rdf:type skos:Concept ;
  rdfs:label "november"@no ;
  skos:inScheme :MonthOfYearCode ;
.
<http://spec.tn-its.eu/owl/tnits-owl#MonthOfYear.october>
  rdf:type :MonthOfYear ;
  rdf:type owl:NamedIndividual ;
  rdf:type skos:Concept ;
  rdfs:label "october"@no ;
  skos:inScheme :MonthOfYearCode ;
.
<http://spec.tn-its.eu/owl/tnits-owl#MonthOfYear.september>
  rdf:type :MonthOfYear ;
  rdf:type owl:NamedIndividual ;
  rdf:type skos:Concept ;
  rdfs:label "september"@no ;
  skos:inScheme :MonthOfYearCode ;
.
:MonthOfYearCode
  rdf:type owl:NamedIndividual ;
  rdf:type skos:ConceptScheme ;
  dc:isFormatOf :MonthOfYear ;
  skos:definition "Applicable month of the year."@en ;
.
:NatureOfDistanceMeasure
  rdf:type owl:Class ;
  rdfs:label "NatureOfDistanceMeasure"@en ;
  rdfs:subClassOf :tnitsCodeList ;
  skos:definition "Specifies the available list of enumerations for contexts of forms of interpreting distance measures"@en ;
.
:NatureOfDistanceMeasureCode
  rdf:type owl:NamedIndividual ;
  rdf:type skos:ConceptScheme ;
  dc:isFormatOf :NatureOfDistanceMeasure ;
  skos:definition "Specifies the available list of enumerations for contexts of forms of interpreting distance measures"@en ;
.
:NetworkElement
  rdf:type owl:Class ;
  rdfs:label "NetworkElement"@en ;
  rdfs:subClassOf :tnitsFeature ;
  rdfs:subClassOf lr:LinearElement ;
  rdfs:subClassOf [
      rdf:type owl:Restriction ;
      owl:allValuesFrom :Identifier ;
      owl:onProperty :id ;
    ] ;
  rdfs:subClassOf [
      rdf:type owl:Restriction ;
      owl:maxQualifiedCardinality "1"^^xsd:nonNegativeInteger ;
      owl:onClass :Identifier ;
      owl:onProperty :id ;
    ] ;
  skos:definition "Base type representing an element in a network. Every element in a network provides some function that is of interest in the network. "@en ;
.
:NetworkReference
  rdf:type owl:Class ;
  rdfs:label "NetworkReference"@en ;
  rdfs:subClassOf :tnitsDataType ;
  rdfs:subClassOf [
      rdf:type owl:Restriction ;
      owl:allValuesFrom :NetworkElement ;
      owl:onProperty :element ;
    ] ;
  rdfs:subClassOf [
      rdf:type owl:Restriction ;
      owl:allValuesFrom lr:LinearReferencingMethod ;
      owl:onProperty :overridingLRM ;
    ] ;
  rdfs:subClassOf [
      rdf:type owl:Restriction ;
      owl:maxQualifiedCardinality "1"^^xsd:nonNegativeInteger ;
      owl:onClass lr:LinearReferencingMethod ;
      owl:onProperty :overridingLRM ;
    ] ;
  rdfs:subClassOf [
      rdf:type owl:Restriction ;
      owl:onClass :NetworkElement ;
      owl:onProperty :element ;
      owl:qualifiedCardinality "1"^^xsd:nonNegativeInteger ;
    ] ;
  owl:disjointUnionOf (
      :LinkReference
    ) ;
  owl:equivalentClass lr:LinearEventLocation ;
  skos:definition "A general class defining a location reference by reference to a Network Reference "@en ;
.
:NumberOfAxlesCharacteristic
  rdf:type owl:Class ;
  rdfs:label "NumberOfAxlesCharacteristic"@en ;
  rdfs:subClassOf :tnitsDataType ;
  rdfs:subClassOf [
      rdf:type owl:Restriction ;
      owl:allValuesFrom :ComparisonOperator ;
      owl:onProperty :comparisonOperator ;
    ] ;
  rdfs:subClassOf [
      rdf:type owl:Restriction ;
      owl:allValuesFrom xsd:integer ;
      owl:onProperty :numberOfAxles ;
    ] ;
  rdfs:subClassOf [
      rdf:type owl:Restriction ;
      owl:onClass :ComparisonOperator ;
      owl:onProperty :comparisonOperator ;
      owl:qualifiedCardinality "1"^^xsd:nonNegativeInteger ;
    ] ;
  rdfs:subClassOf [
      rdf:type owl:Restriction ;
      owl:onDataRange xsd:integer ;
      owl:onProperty :numberOfAxles ;
      owl:qualifiedCardinality "1"^^xsd:nonNegativeInteger ;
    ] ;
  skos:definition "Number of axles characteristic of a vehicle. [SOURCE: CEN/TS16157-3:2011] "@en ;
.
:OpenLRBinaryVersion
  rdf:type owl:Class ;
  rdfs:label "OpenLRBinaryVersion"@en ;
  rdfs:subClassOf :tnitsCodeList ;
  skos:definition "Specifies the available list of enumerations for the version of the OpenLR binary specification"@en ;
.
:OpenLRBinaryVersionCode
  rdf:type owl:NamedIndividual ;
  rdf:type skos:ConceptScheme ;
  dc:isFormatOf :OpenLRBinaryVersion ;
  skos:definition "Specifies the available list of enumerations for the version of the OpenLR binary specification"@en ;
.
:OpenLRLocationReference
  rdf:type owl:Class ;
  rdfs:label "OpenLRLocationReference"@en ;
  rdfs:subClassOf :DynamicLocationReference ;
  rdfs:subClassOf [
      rdf:type owl:Restriction ;
      owl:allValuesFrom :BinaryLocationReference ;
      owl:onProperty <http://spec.tn-its.eu/owl/tnits-owl#OpenLRLocationReference.binaryLocationReference> ;
    ] ;
  rdfs:subClassOf [
      rdf:type owl:Restriction ;
      owl:allValuesFrom :XMLLocationReference ;
      owl:onProperty <http://spec.tn-its.eu/owl/tnits-owl#OpenLRLocationReference.xMLLocationReference> ;
    ] ;
  rdfs:subClassOf [
      rdf:type owl:Restriction ;
      owl:maxQualifiedCardinality "1"^^xsd:nonNegativeInteger ;
      owl:onClass :BinaryLocationReference ;
      owl:onProperty <http://spec.tn-its.eu/owl/tnits-owl#OpenLRLocationReference.binaryLocationReference> ;
    ] ;
  rdfs:subClassOf [
      rdf:type owl:Restriction ;
      owl:maxQualifiedCardinality "1"^^xsd:nonNegativeInteger ;
      owl:onClass :XMLLocationReference ;
      owl:onProperty <http://spec.tn-its.eu/owl/tnits-owl#OpenLRLocationReference.xMLLocationReference> ;
    ] ;
  skos:definition "A type of dynamic location reference that uses coordinates and core attribution according to the OpenLR specification (see bibliography)  "@en ;
.
<http://spec.tn-its.eu/owl/tnits-owl#OpenLRLocationReference.binaryLocationReference>
  rdf:type owl:ObjectProperty ;
  rdfs:domain :OpenLRLocationReference ;
  rdfs:label "OpenLRLocationReference.binaryLocationReference"@en ;
  rdfs:range :BinaryLocationReference ;
  skos:definition "OpenLR location reference using binary encoding "@en ;
.
<http://spec.tn-its.eu/owl/tnits-owl#OpenLRLocationReference.xMLLocationReference>
  rdf:type owl:ObjectProperty ;
  rdfs:domain :OpenLRLocationReference ;
  rdfs:label "OpenLRLocationReference.xMLLocationReference"@en ;
  rdfs:range :XMLLocationReference ;
  skos:definition "OpenLR location reference using XML encoding "@en ;
.
:OverallPeriod
  rdf:type owl:Class ;
  rdfs:label "OverallPeriod"@en ;
  rdfs:subClassOf :tnitsDataType ;
  rdfs:subClassOf [
      rdf:type owl:Restriction ;
      owl:allValuesFrom :Period ;
      owl:onProperty :exceptionPeriod ;
    ] ;
  rdfs:subClassOf [
      rdf:type owl:Restriction ;
      owl:allValuesFrom :Period ;
      owl:onProperty :validPeriod ;
    ] ;
  rdfs:subClassOf [
      rdf:type owl:Restriction ;
      owl:allValuesFrom xsd:dateTime ;
      owl:onProperty :overallEndTime ;
    ] ;
  rdfs:subClassOf [
      rdf:type owl:Restriction ;
      owl:allValuesFrom xsd:dateTime ;
      owl:onProperty :overallStartTime ;
    ] ;
  rdfs:subClassOf [
      rdf:type owl:Restriction ;
      owl:maxQualifiedCardinality "1"^^xsd:nonNegativeInteger ;
      owl:onDataRange xsd:dateTime ;
      owl:onProperty :overallEndTime ;
    ] ;
  rdfs:subClassOf [
      rdf:type owl:Restriction ;
      owl:onDataRange xsd:dateTime ;
      owl:onProperty :overallStartTime ;
      owl:qualifiedCardinality "1"^^xsd:nonNegativeInteger ;
    ] ;
  skos:definition "A continuous or discontinuous period of validity defined by overall bounding start and end times and the possible intersection of valid periods (potentially recurring) with the complement of exception periods (also potentially recurring). [SOURCE: CEN/TS16157-3:2011] "@en ;
.
:ParkingSiteType
  rdf:type owl:Class ;
  rdfs:label "ParkingSiteType"@en ;
  rdfs:subClassOf :tnitsCodeList ;
  skos:definition "Specifies the available list of enumerations for the types of parking sites"@en ;
.
:ParkingSiteTypeCode
  rdf:type owl:NamedIndividual ;
  rdf:type skos:ConceptScheme ;
  dc:isFormatOf :ParkingSiteType ;
  skos:definition "Specifies the available list of enumerations for the types of parking sites"@en ;
.
:PaymentMethod
  rdf:type owl:Class ;
  rdfs:label "PaymentMethod"@en ;
  rdfs:subClassOf :tnitsCodeList ;
  skos:definition "Specifies the available list of enumerations for the methods of payment"@en ;
.
:PaymentMethodCode
  rdf:type owl:NamedIndividual ;
  rdf:type skos:ConceptScheme ;
  dc:isFormatOf :PaymentMethod ;
  skos:definition "Specifies the available list of enumerations for the methods of payment"@en ;
.
:Period
  rdf:type owl:Class ;
  rdfs:label "Period"@en ;
  rdfs:subClassOf :tnitsDataType ;
  rdfs:subClassOf [
      rdf:type owl:Restriction ;
      owl:allValuesFrom :DayWeekMonth ;
      owl:onProperty :recurringDayWeekMonthPeriod ;
    ] ;
  rdfs:subClassOf [
      rdf:type owl:Restriction ;
      owl:allValuesFrom :FuzzyTimePeriod ;
      owl:onProperty :recurringFuzzyTimePeriod ;
    ] ;
  rdfs:subClassOf [
      rdf:type owl:Restriction ;
      owl:allValuesFrom :SpecialDay ;
      owl:onProperty :recurringSpecialDay ;
    ] ;
  rdfs:subClassOf [
      rdf:type owl:Restriction ;
      owl:allValuesFrom :TimePeriodOfDay ;
      owl:onProperty :recurringTimePeriodOfDay ;
    ] ;
  rdfs:subClassOf [
      rdf:type owl:Restriction ;
      owl:allValuesFrom xsd:dateTime ;
      owl:onProperty :endOfPeriod ;
    ] ;
  rdfs:subClassOf [
      rdf:type owl:Restriction ;
      owl:allValuesFrom xsd:dateTime ;
      owl:onProperty :startOfPeriod ;
    ] ;
  rdfs:subClassOf [
      rdf:type owl:Restriction ;
      owl:allValuesFrom xsd:string ;
      owl:onProperty :periodName ;
    ] ;
  rdfs:subClassOf [
      rdf:type owl:Restriction ;
      owl:maxQualifiedCardinality "1"^^xsd:nonNegativeInteger ;
      owl:onDataRange xsd:dateTime ;
      owl:onProperty :endOfPeriod ;
    ] ;
  rdfs:subClassOf [
      rdf:type owl:Restriction ;
      owl:maxQualifiedCardinality "1"^^xsd:nonNegativeInteger ;
      owl:onDataRange xsd:dateTime ;
      owl:onProperty :startOfPeriod ;
    ] ;
  rdfs:subClassOf [
      rdf:type owl:Restriction ;
      owl:maxQualifiedCardinality "1"^^xsd:nonNegativeInteger ;
      owl:onDataRange xsd:string ;
      owl:onProperty :periodName ;
    ] ;
  skos:definition "A continuous time period or a set of discontinuous time periods defined by the intersection of a set of criteria all within an overall delimiting interval.  [SOURCE: CEN/TS16157-3:2011] "@en ;
.
:PreCodedLocationReference
  rdf:type owl:Class ;
  rdfs:label "PreCodedLocationReference"@en ;
  rdfs:subClassOf :LocationReference ;
  owl:disjointUnionOf (
      :LinearLocationReference
      :LocationByExternalReference
    ) ;
  skos:definition "Abstract class that serves as a placeholder for any type of precoded location reference that may be used in TN-ITS. NOTE 1 Examples of precoded location references are: linear reference;  address; location code. NOTE 2 Linear referencing is the preferred location referencing method for data associated with the road network in INSPIRE.   NOTE 3 This kind of location reference is classified as \"PreCoded\" in ISO 17572."@en ;
.
:PredefinedLocation
  rdf:type owl:Class ;
  rdfs:label "PredefinedLocation"@en ;
  rdfs:subClassOf :tnitsCodeList ;
  skos:definition "Specifies the available list of enumerations for predefined locations "@en ;
.
:PredefinedLocationCode
  rdf:type owl:NamedIndividual ;
  rdf:type skos:ConceptScheme ;
  dc:isFormatOf :PredefinedLocation ;
  skos:definition "Specifies the available list of enumerations for predefined locations "@en ;
.
:PropertyValueReferenceType
  rdf:type owl:Class ;
  rdfs:label "PropertyValueReferenceType"@en ;
  rdfs:subClassOf :tnitsCodeList ;
  skos:definition "A list of externally defined values "@en ;
.
:PropertyValueReferenceTypeCode
  rdf:type owl:NamedIndividual ;
  rdf:type skos:ConceptScheme ;
  dc:isFormatOf :PropertyValueReferenceType ;
  skos:definition "A list of externally defined values "@en ;
.
:PublicHoliday
  rdf:type owl:Class ;
  rdfs:label "PublicHoliday"@en ;
  rdfs:subClassOf :SpecialDay ;
  rdfs:subClassOf [
      rdf:type owl:Restriction ;
      owl:allValuesFrom xsd:string ;
      owl:onProperty :publicHolidayName ;
    ] ;
  rdfs:subClassOf [
      rdf:type owl:Restriction ;
      owl:onDataRange xsd:string ;
      owl:onProperty :publicHolidayName ;
      owl:qualifiedCardinality "1"^^xsd:nonNegativeInteger ;
    ] ;
  skos:definition "Specification of a specific public holiday in case specialDayType is set to 'publicHoliday'. [SOURCE: DATEX 3.0 Part 7 (proposed EN 16157-7:2018)] "@en ;
.
:RoadCategory
  rdf:type owl:Class ;
  rdfs:label "RoadCategory"@en ;
  rdfs:subClassOf :tnitsCodeList ;
  skos:definition "Specifies the available list of enumerations for the road category types"@en ;
.
:RoadCategoryCode
  rdf:type owl:NamedIndividual ;
  rdf:type skos:ConceptScheme ;
  dc:isFormatOf :RoadCategory ;
  skos:definition "Specifies the available list of enumerations for the road category types"@en ;
.
:RoadCategoryCondition
  rdf:type owl:Class ;
  rdfs:label "RoadCategoryCondition"@en ;
  rdfs:subClassOf :Condition ;
  rdfs:subClassOf [
      rdf:type owl:Restriction ;
      owl:allValuesFrom :RoadCategory ;
      owl:onProperty <http://spec.tn-its.eu/owl/tnits-owl#RoadCategoryCondition.roadCategory> ;
    ] ;
  rdfs:subClassOf [
      rdf:type owl:Restriction ;
      owl:onClass :RoadCategory ;
      owl:onProperty <http://spec.tn-its.eu/owl/tnits-owl#RoadCategoryCondition.roadCategory> ;
      owl:qualifiedCardinality "1"^^xsd:nonNegativeInteger ;
    ] ;
  skos:definition "Specifies road category condition applicability relating to a road feature "@en ;
.
<http://spec.tn-its.eu/owl/tnits-owl#RoadCategoryCondition.roadCategory>
  rdf:type owl:FunctionalProperty ;
  rdf:type owl:ObjectProperty ;
  rdfs:domain :RoadCategoryCondition ;
  rdfs:label "RoadCategoryCondition.roadCategory"@en ;
  rdfs:range :RoadCategory ;
  skos:definition "Specifies the available list of enumerations for the category of road for a road feature by reference to an item in an external code list "@en ;
.
:RoadFeature
  rdf:type owl:Class ;
  rdfs:label "RoadFeature"@en ;
  rdfs:subClassOf :tnitsFeature ;
  rdfs:subClassOf [
      rdf:type owl:Restriction ;
      owl:allValuesFrom :AbstractRoadFeatureProperty ;
      owl:onProperty :properties ;
    ] ;
  rdfs:subClassOf [
      rdf:type owl:Restriction ;
      owl:allValuesFrom :Condition ;
      owl:onProperty <http://spec.tn-its.eu/owl/tnits-owl#RoadFeature.condition> ;
    ] ;
  rdfs:subClassOf [
      rdf:type owl:Restriction ;
      owl:allValuesFrom :Identifier ;
      owl:onProperty :roadFeatureId ;
    ] ;
  rdfs:subClassOf [
      rdf:type owl:Restriction ;
      owl:allValuesFrom :LocationReference ;
      owl:onProperty <http://spec.tn-its.eu/owl/tnits-owl#RoadFeature.locationReference> ;
    ] ;
  rdfs:subClassOf [
      rdf:type owl:Restriction ;
      owl:allValuesFrom :RoadFeatureSource ;
      owl:onProperty :source ;
    ] ;
  rdfs:subClassOf [
      rdf:type owl:Restriction ;
      owl:allValuesFrom :RoadFeatureType ;
      owl:onProperty <http://spec.tn-its.eu/owl/tnits-owl#RoadFeature.type> ;
    ] ;
  rdfs:subClassOf [
      rdf:type owl:Restriction ;
      owl:allValuesFrom :UpdateInfo ;
      owl:onProperty <http://spec.tn-its.eu/owl/tnits-owl#RoadFeature.updateInfo> ;
    ] ;
  rdfs:subClassOf [
      rdf:type owl:Restriction ;
      owl:allValuesFrom xsd:date ;
      owl:onProperty :validFrom ;
    ] ;
  rdfs:subClassOf [
      rdf:type owl:Restriction ;
      owl:allValuesFrom xsd:date ;
      owl:onProperty :validTo ;
    ] ;
  rdfs:subClassOf [
      rdf:type owl:Restriction ;
      owl:allValuesFrom xsd:dateTime ;
      owl:onProperty :beginLifespanVersion ;
    ] ;
  rdfs:subClassOf [
      rdf:type owl:Restriction ;
      owl:allValuesFrom xsd:dateTime ;
      owl:onProperty :endLifespanVersion ;
    ] ;
  rdfs:subClassOf [
      rdf:type owl:Restriction ;
      owl:maxQualifiedCardinality "1"^^xsd:nonNegativeInteger ;
      owl:onClass :Condition ;
      owl:onProperty <http://spec.tn-its.eu/owl/tnits-owl#RoadFeature.condition> ;
    ] ;
  rdfs:subClassOf [
      rdf:type owl:Restriction ;
      owl:maxQualifiedCardinality "1"^^xsd:nonNegativeInteger ;
      owl:onClass :UpdateInfo ;
      owl:onProperty <http://spec.tn-its.eu/owl/tnits-owl#RoadFeature.updateInfo> ;
    ] ;
  rdfs:subClassOf [
      rdf:type owl:Restriction ;
      owl:maxQualifiedCardinality "1"^^xsd:nonNegativeInteger ;
      owl:onDataRange xsd:date ;
      owl:onProperty :validTo ;
    ] ;
  rdfs:subClassOf [
      rdf:type owl:Restriction ;
      owl:maxQualifiedCardinality "1"^^xsd:nonNegativeInteger ;
      owl:onDataRange xsd:dateTime ;
      owl:onProperty :endLifespanVersion ;
    ] ;
  rdfs:subClassOf [
      rdf:type owl:Restriction ;
      owl:minQualifiedCardinality "1"^^xsd:nonNegativeInteger ;
      owl:onClass :LocationReference ;
      owl:onProperty <http://spec.tn-its.eu/owl/tnits-owl#RoadFeature.locationReference> ;
    ] ;
  rdfs:subClassOf [
      rdf:type owl:Restriction ;
      owl:onClass :Identifier ;
      owl:onProperty :roadFeatureId ;
      owl:qualifiedCardinality "1"^^xsd:nonNegativeInteger ;
    ] ;
  rdfs:subClassOf [
      rdf:type owl:Restriction ;
      owl:onClass :RoadFeatureSource ;
      owl:onProperty :source ;
      owl:qualifiedCardinality "1"^^xsd:nonNegativeInteger ;
    ] ;
  rdfs:subClassOf [
      rdf:type owl:Restriction ;
      owl:onClass :RoadFeatureType ;
      owl:onProperty <http://spec.tn-its.eu/owl/tnits-owl#RoadFeature.type> ;
      owl:qualifiedCardinality "1"^^xsd:nonNegativeInteger ;
    ] ;
  rdfs:subClassOf [
      rdf:type owl:Restriction ;
      owl:onDataRange xsd:date ;
      owl:onProperty :validFrom ;
      owl:qualifiedCardinality "1"^^xsd:nonNegativeInteger ;
    ] ;
  rdfs:subClassOf [
      rdf:type owl:Restriction ;
      owl:onDataRange xsd:dateTime ;
      owl:onProperty :beginLifespanVersion ;
      owl:qualifiedCardinality "1"^^xsd:nonNegativeInteger ;
    ] ;
  skos:definition "The base class for any type of road feature. A road feature represents static road data, such as traffic regulations, traffic signs (like speed limits, compulsory signs and warning signs) and road infrastructure (such as charging points). Each road feature must be described by a geo-referenced by providing a point or linear location reference and can be further described by a set of conditions specifying the validity of the road feature (using combinations of conditions such as time restrictions, area, lane, vehicle type, weather, loading or road category)."@en ;
.
<http://spec.tn-its.eu/owl/tnits-owl#RoadFeature.condition>
  rdf:type owl:ObjectProperty ;
  rdfs:domain :RoadFeature ;
  rdfs:label "RoadFeature.condition"@en ;
  rdfs:range :Condition ;
  skos:definition "Describes the circumstances when the road feature is applicable.  "@en ;
.
<http://spec.tn-its.eu/owl/tnits-owl#RoadFeature.locationReference>
  rdf:type owl:ObjectProperty ;
  rdfs:domain :RoadFeature ;
  rdfs:label "RoadFeature.locationReference"@en ;
  rdfs:range :LocationReference ;
  skos:definition "A reference to the location of the road feature either described by either a precoded or a dynamic location referencing method  "@en ;
.
<http://spec.tn-its.eu/owl/tnits-owl#RoadFeature.type>
  rdf:type owl:FunctionalProperty ;
  rdf:type owl:ObjectProperty ;
  rdfs:domain :RoadFeature ;
  rdfs:label "RoadFeature.type"@en ;
  rdfs:range :RoadFeatureType ;
  skos:definition "A characterisation identifying the type of the road feature by reference to an item in an external code list "@en ;
.
<http://spec.tn-its.eu/owl/tnits-owl#RoadFeature.updateInfo>
  rdf:type owl:ObjectProperty ;
  rdfs:domain :RoadFeature ;
  rdfs:label "RoadFeature.updateInfo"@en ;
  rdfs:range :UpdateInfo ;
  skos:definition "Specifies the necessary update information if this is a representation of an update event. "@en ;
.
:RoadFeatureDataset
  rdf:type owl:Class ;
  rdfs:label "RoadFeatureDataset"@en ;
  rdfs:subClassOf :Dataset ;
  rdfs:subClassOf [
      rdf:type owl:Restriction ;
      owl:allValuesFrom :DatasetType ;
      owl:onProperty <http://spec.tn-its.eu/owl/tnits-owl#RoadFeatureDataset.type> ;
    ] ;
  rdfs:subClassOf [
      rdf:type owl:Restriction ;
      owl:allValuesFrom :RoadFeature ;
      owl:onProperty :roadFeatures ;
    ] ;
  rdfs:subClassOf [
      rdf:type owl:Restriction ;
      owl:allValuesFrom lr:LinearReferencingMethod ;
      owl:onProperty :defaultLRM ;
    ] ;
  rdfs:subClassOf [
      rdf:type owl:Restriction ;
      owl:maxQualifiedCardinality "1"^^xsd:nonNegativeInteger ;
      owl:onClass lr:LinearReferencingMethod ;
      owl:onProperty :defaultLRM ;
    ] ;
  rdfs:subClassOf [
      rdf:type owl:Restriction ;
      owl:minQualifiedCardinality "1"^^xsd:nonNegativeInteger ;
      owl:onClass :RoadFeature ;
      owl:onProperty :roadFeatures ;
    ] ;
  rdfs:subClassOf [
      rdf:type owl:Restriction ;
      owl:onClass :DatasetType ;
      owl:onProperty <http://spec.tn-its.eu/owl/tnits-owl#RoadFeatureDataset.type> ;
      owl:qualifiedCardinality "1"^^xsd:nonNegativeInteger ;
    ] ;
  skos:definition "A dataset containing road feature with optional update information.  "@en ;
.
<http://spec.tn-its.eu/owl/tnits-owl#RoadFeatureDataset.type>
  rdf:type owl:FunctionalProperty ;
  rdf:type owl:ObjectProperty ;
  rdfs:domain :RoadFeatureDataset ;
  rdfs:label "RoadFeatureDataset.type"@en ;
  rdfs:range :DatasetType ;
  skos:definition "Specifies the type of dataset "@en ;
.
:RoadFeatureEvent
  rdf:type owl:Class ;
  rdfs:label "RoadFeatureEvent"@en ;
  rdfs:subClassOf :FeedbackLogEvent ;
  rdfs:subClassOf [
      rdf:type owl:Restriction ;
      owl:allValuesFrom :Identifier ;
      owl:onProperty :roadFeatureId ;
    ] ;
  rdfs:subClassOf [
      rdf:type owl:Restriction ;
      owl:allValuesFrom :RoadFeatureEventType ;
      owl:onProperty :eventCode ;
    ] ;
  rdfs:subClassOf [
      rdf:type owl:Restriction ;
      owl:allValuesFrom :RoadFeaturePropertyType ;
      owl:onProperty <http://spec.tn-its.eu/owl/tnits-owl#RoadFeatureEvent.roadFeaturePropertyType> ;
    ] ;
  rdfs:subClassOf [
      rdf:type owl:Restriction ;
      owl:onClass :Identifier ;
      owl:onProperty :roadFeatureId ;
      owl:qualifiedCardinality "1"^^xsd:nonNegativeInteger ;
    ] ;
  rdfs:subClassOf [
      rdf:type owl:Restriction ;
      owl:onClass :RoadFeatureEventType ;
      owl:onProperty :eventCode ;
      owl:qualifiedCardinality "1"^^xsd:nonNegativeInteger ;
    ] ;
  rdfs:subClassOf [
      rdf:type owl:Restriction ;
      owl:onClass :RoadFeaturePropertyType ;
      owl:onProperty <http://spec.tn-its.eu/owl/tnits-owl#RoadFeatureEvent.roadFeaturePropertyType> ;
      owl:qualifiedCardinality "1"^^xsd:nonNegativeInteger ;
    ] ;
  skos:definition "Represents one event that may occur during download and integration of data that needs to be reported back to the provider  "@en ;
.
<http://spec.tn-its.eu/owl/tnits-owl#RoadFeatureEvent.roadFeaturePropertyType>
  rdf:type owl:FunctionalProperty ;
  rdf:type owl:ObjectProperty ;
  rdfs:domain :RoadFeatureEvent ;
  rdfs:label "RoadFeatureEvent.roadFeaturePropertyType"@en ;
  rdfs:range :RoadFeaturePropertyType ;
  skos:definition "The identification of the road feature property type that is concerned by the event. If unset, this event does not concern any road feature property type in particular. "@en ;
.
:RoadFeatureEventType
  rdf:type owl:Class ;
  rdfs:label "RoadFeatureEventType"@en ;
  rdfs:subClassOf :tnitsCodeList ;
  skos:definition "Specifies the available list of enumerations for the types of Road Feature Events"@en ;
.
:RoadFeatureEventTypeCode
  rdf:type owl:NamedIndividual ;
  rdf:type skos:ConceptScheme ;
  dc:isFormatOf :RoadFeatureEventType ;
  skos:definition "Specifies the available list of enumerations for the types of Road Feature Events"@en ;
.
:RoadFeaturePropertyType
  rdf:type owl:Class ;
  rdfs:label "RoadFeaturePropertyType"@en ;
  rdfs:subClassOf :tnitsCodeList ;
  skos:definition "Specifies the available list of enumerations for the various types of road features"@en ;
.
:RoadFeaturePropertyTypeCode
  rdf:type owl:NamedIndividual ;
  rdf:type skos:ConceptScheme ;
  dc:isFormatOf :RoadFeaturePropertyType ;
  skos:definition "Specifies the available list of enumerations for the various types of road features"@en ;
.
:RoadFeatureSource
  rdf:type owl:Class ;
  rdfs:label "RoadFeatureSource"@en ;
  rdfs:subClassOf :tnitsCodeList ;
  skos:definition "Specifies the available list of enumerations for the various types source concerning road features"@en ;
.
:RoadFeatureSourceCode
  rdf:type owl:NamedIndividual ;
  rdf:type skos:ConceptScheme ;
  dc:isFormatOf :RoadFeatureSource ;
  skos:definition "Specifies the available list of enumerations for the various types source concerning road features"@en ;
.
:RoadFeatureType
  rdf:type owl:Class ;
  rdfs:label "RoadFeatureType"@en ;
  rdfs:subClassOf :tnitsCodeList ;
  skos:definition "Specifies the available list of enumerations for the various types of road features"@en ;
.
:RoadFeatureTypeCode
  rdf:type owl:NamedIndividual ;
  rdf:type skos:ConceptScheme ;
  dc:isFormatOf :RoadFeatureType ;
  skos:definition "Specifies the available list of enumerations for the various types of road features"@en ;
.
:RoadSignContent
  rdf:type owl:Class ;
  rdfs:label "RoadSignContent"@en ;
  rdfs:subClassOf :tnitsDataType ;
  rdfs:subClassOf [
      rdf:type owl:Restriction ;
      owl:allValuesFrom :Measure ;
      owl:onProperty <http://spec.tn-its.eu/owl/tnits-owl#RoadSignContent.value> ;
    ] ;
  rdfs:subClassOf [
      rdf:type owl:Restriction ;
      owl:allValuesFrom :NatureOfDistanceMeasure ;
      owl:onProperty :natureOfDistance ;
    ] ;
  rdfs:subClassOf [
      rdf:type owl:Restriction ;
      owl:allValuesFrom xsd:string ;
      owl:onProperty <http://spec.tn-its.eu/owl/tnits-owl#RoadSignContent.text> ;
    ] ;
  rdfs:subClassOf [
      rdf:type owl:Restriction ;
      owl:maxQualifiedCardinality "1"^^xsd:nonNegativeInteger ;
      owl:onClass :Measure ;
      owl:onProperty <http://spec.tn-its.eu/owl/tnits-owl#RoadSignContent.value> ;
    ] ;
  rdfs:subClassOf [
      rdf:type owl:Restriction ;
      owl:maxQualifiedCardinality "1"^^xsd:nonNegativeInteger ;
      owl:onClass :NatureOfDistanceMeasure ;
      owl:onProperty :natureOfDistance ;
    ] ;
  rdfs:subClassOf [
      rdf:type owl:Restriction ;
      owl:maxQualifiedCardinality "1"^^xsd:nonNegativeInteger ;
      owl:onDataRange xsd:string ;
      owl:onProperty <http://spec.tn-its.eu/owl/tnits-owl#RoadSignContent.text> ;
    ] ;
  skos:definition "Defines one instance of content providing context of the semantics of a road sign "@en ;
.
<http://spec.tn-its.eu/owl/tnits-owl#RoadSignContent.text>
  rdf:type owl:DatatypeProperty ;
  rdfs:domain :RoadSignContent ;
  rdfs:label "RoadSignContent.text"@en ;
  rdfs:range xsd:string ;
  skos:definition "A free-text description relevant to the specific road sign"@en ;
.
<http://spec.tn-its.eu/owl/tnits-owl#RoadSignContent.value>
  rdf:type owl:ObjectProperty ;
  rdfs:domain :RoadSignContent ;
  rdfs:label "RoadSignContent.value"@en ;
  rdfs:range :Measure ;
  skos:definition "The value of the road sign property "@en ;
.
:RoadSignProperty
  rdf:type owl:Class ;
  rdfs:label "RoadSignProperty"@en ;
  rdfs:subClassOf :AbstractRoadFeatureProperty ;
  rdfs:subClassOf [
      rdf:type owl:Restriction ;
      owl:allValuesFrom :RoadSignContent ;
      owl:onProperty :content ;
    ] ;
  rdfs:subClassOf [
      rdf:type owl:Restriction ;
      owl:allValuesFrom :RoadSignType ;
      owl:onProperty :gddCode ;
    ] ;
  rdfs:subClassOf [
      rdf:type owl:Restriction ;
      owl:onClass :RoadSignType ;
      owl:onProperty :gddCode ;
      owl:qualifiedCardinality "1"^^xsd:nonNegativeInteger ;
    ] ;
  skos:definition "A representation of a road feature property value in the case of the road feature being a road sign "@en ;
.
:RoadSignType
  rdf:type owl:Class ;
  rdfs:label "RoadSignType"@en ;
  rdfs:subClassOf :tnitsCodeList ;
  skos:definition "Specifies the available list of enumerations for the road sign types, defined in accordance with ISO 14823"@en ;
.
:RoadSignTypeCode
  rdf:type owl:NamedIndividual ;
  rdf:type skos:ConceptScheme ;
  dc:isFormatOf :RoadSignType ;
  skos:definition "Specifies the available list of enumerations for the road sign types, defined in accordance with ISO 14823"@en ;
.
:SimpleLinearReference
  rdf:type owl:Class ;
  rdfs:label "SimpleLinearReference"@en ;
  rdfs:subClassOf :LinkReference ;
  rdfs:subClassOf [
      rdf:type owl:Restriction ;
      owl:allValuesFrom lr:DistanceExpression ;
      owl:onProperty lr:fromPosition ;
    ] ;
  rdfs:subClassOf [
      rdf:type owl:Restriction ;
      owl:allValuesFrom lr:DistanceExpression ;
      owl:onProperty lr:toPosition ;
    ] ;
  rdfs:subClassOf [
      rdf:type owl:Restriction ;
      owl:onClass lr:DistanceExpression ;
      owl:onProperty lr:fromPosition ;
      owl:qualifiedCardinality "1"^^xsd:nonNegativeInteger ;
    ] ;
  rdfs:subClassOf [
      rdf:type owl:Restriction ;
      owl:onClass lr:DistanceExpression ;
      owl:onProperty lr:toPosition ;
      owl:qualifiedCardinality "1"^^xsd:nonNegativeInteger ;
    ] ;
  owl:equivalentClass lr:LinearFromToLocation ;
  skos:definition "A network reference that is restricted to part of a linear network element. The part is the part of the network element between fromPosition and toPosition. "@en ;
.
:SimplePointReference
  rdf:type owl:Class ;
  rdfs:label "SimplePointReference"@en ;
  rdfs:subClassOf :LinkReference ;
  rdfs:subClassOf [
      rdf:type owl:Restriction ;
      owl:allValuesFrom lr:DistanceExpression ;
      owl:onProperty lr:atPosition ;
    ] ;
  rdfs:subClassOf [
      rdf:type owl:Restriction ;
      owl:onClass lr:DistanceExpression ;
      owl:onProperty lr:atPosition ;
      owl:qualifiedCardinality "1"^^xsd:nonNegativeInteger ;
    ] ;
  owl:equivalentClass lr:LinearAtLocation ;
  skos:definition "A network reference that is restricted to a point on a linear network element. The point is the location on the network element at the position atPosition along the network.  "@en ;
.
:SiteAccessibilityType
  rdf:type owl:Class ;
  rdfs:label "SiteAccessibilityType"@en ;
  rdfs:subClassOf :tnitsCodeList ;
  skos:definition "Specifies the available list of enumerations for types of site accessibility"@en ;
.
:SiteAccessibilityTypeCode
  rdf:type owl:NamedIndividual ;
  rdf:type skos:ConceptScheme ;
  dc:isFormatOf :SiteAccessibilityType ;
  skos:definition "Specifies the available list of enumerations for types of site accessibility"@en ;
.
:SpecialDay
  rdf:type owl:Class ;
  rdfs:label "SpecialDay"@en ;
  rdfs:subClassOf :tnitsDataType ;
  rdfs:subClassOf [
      rdf:type owl:Restriction ;
      owl:allValuesFrom :SpecialDayType ;
      owl:onProperty <http://spec.tn-its.eu/owl/tnits-owl#SpecialDay.specialDayType> ;
    ] ;
  rdfs:subClassOf [
      rdf:type owl:Restriction ;
      owl:allValuesFrom xsd:boolean ;
      owl:onProperty :intersectWithApplicableDays ;
    ] ;
  rdfs:subClassOf [
      rdf:type owl:Restriction ;
      owl:allValuesFrom xsd:string ;
      owl:onProperty :publicEvent ;
    ] ;
  rdfs:subClassOf [
      rdf:type owl:Restriction ;
      owl:maxQualifiedCardinality "1"^^xsd:nonNegativeInteger ;
      owl:onDataRange xsd:string ;
      owl:onProperty :publicEvent ;
    ] ;
  rdfs:subClassOf [
      rdf:type owl:Restriction ;
      owl:onClass :SpecialDayType ;
      owl:onProperty <http://spec.tn-its.eu/owl/tnits-owl#SpecialDay.specialDayType> ;
      owl:qualifiedCardinality "1"^^xsd:nonNegativeInteger ;
    ] ;
  rdfs:subClassOf [
      rdf:type owl:Restriction ;
      owl:onDataRange xsd:boolean ;
      owl:onProperty :intersectWithApplicableDays ;
      owl:qualifiedCardinality "1"^^xsd:nonNegativeInteger ;
    ] ;
  owl:disjointUnionOf (
      :PublicHoliday
    ) ;
  skos:definition "Specification of a special type of day, possibly also a public holiday. Can be country or region specific. [SOURCE: DATEX 3.0 Part 7 (proposed EN 161577:2018)] "@en ;
.
<http://spec.tn-its.eu/owl/tnits-owl#SpecialDay.specialDayType>
  rdf:type owl:FunctionalProperty ;
  rdf:type owl:ObjectProperty ;
  rdfs:domain :SpecialDay ;
  rdfs:label "SpecialDay.specialDayType"@en ;
  rdfs:range :SpecialDayType ;
  skos:definition "Specification of a special day, for example schoolDay, publicHoliday, ... [SOURCE: DATEX 3.0 Part 7 (proposed EN 16157-7:2018)] "@en ;
.
:SpecialDayType
  rdf:type owl:Class ;
  rdfs:label "SpecialDayType"@en ;
  rdfs:subClassOf :tnitsCodeList ;
  skos:definition "Specifies the available list of enumerations for the special days"@en ;
.
:SpecialDayTypeCode
  rdf:type owl:NamedIndividual ;
  rdf:type skos:ConceptScheme ;
  dc:isFormatOf :SpecialDayType ;
  skos:definition "Specifies the available list of enumerations for the special days"@en ;
.
:SummaryInfo
  rdf:type owl:Class ;
  rdfs:label "SummaryInfo"@en ;
  rdfs:subClassOf :tnitsDataType ;
  rdfs:subClassOf [
      rdf:type owl:Restriction ;
      owl:allValuesFrom xsd:integer ;
      owl:onProperty :nrFail ;
    ] ;
  rdfs:subClassOf [
      rdf:type owl:Restriction ;
      owl:allValuesFrom xsd:integer ;
      owl:onProperty :nrSuccess ;
    ] ;
  rdfs:subClassOf [
      rdf:type owl:Restriction ;
      owl:onDataRange xsd:integer ;
      owl:onProperty :nrFail ;
      owl:qualifiedCardinality "1"^^xsd:nonNegativeInteger ;
    ] ;
  rdfs:subClassOf [
      rdf:type owl:Restriction ;
      owl:onDataRange xsd:integer ;
      owl:onProperty :nrSuccess ;
      owl:qualifiedCardinality "1"^^xsd:nonNegativeInteger ;
    ] ;
  skos:definition "Information that summarizes a feedback result "@en ;
.
:Time
  rdf:type owl:Class ;
.
:TimeCondition
  rdf:type owl:Class ;
  rdfs:label "TimeCondition"@en ;
  rdfs:subClassOf :Condition ;
  rdfs:subClassOf [
      rdf:type owl:Restriction ;
      owl:allValuesFrom :Validity ;
      owl:onProperty :validityPeriod ;
    ] ;
  rdfs:subClassOf [
      rdf:type owl:Restriction ;
      owl:onClass :Validity ;
      owl:onProperty :validityPeriod ;
      owl:qualifiedCardinality "1"^^xsd:nonNegativeInteger ;
    ] ;
  skos:definition "Specifies timing applicability relating to a road feature  "@en ;
.
:TimePeriodOfDay
  rdf:type owl:Class ;
  rdfs:label "TimePeriodOfDay"@en ;
  rdfs:subClassOf :tnitsDataType ;
  rdfs:subClassOf [
      rdf:type owl:Restriction ;
      owl:allValuesFrom :Time ;
      owl:onProperty :endTimeOfPeriod ;
    ] ;
  rdfs:subClassOf [
      rdf:type owl:Restriction ;
      owl:allValuesFrom :Time ;
      owl:onProperty :startTimeOfPeriod ;
    ] ;
  rdfs:subClassOf [
      rdf:type owl:Restriction ;
      owl:onClass :Time ;
      owl:onProperty :endTimeOfPeriod ;
      owl:qualifiedCardinality "1"^^xsd:nonNegativeInteger ;
    ] ;
  rdfs:subClassOf [
      rdf:type owl:Restriction ;
      owl:onClass :Time ;
      owl:onProperty :startTimeOfPeriod ;
      owl:qualifiedCardinality "1"^^xsd:nonNegativeInteger ;
    ] ;
  skos:definition "Specification of a continuous period of time within a 24 hour period. [SOURCE: CEN/TS16157-3:2011] "@en ;
.
:TunnelCategory
  rdf:type owl:Class ;
  rdfs:label "TunnelCategory"@en ;
  rdfs:subClassOf :tnitsCodeList ;
  skos:definition "Specifies the available list of enumerations for the categories of tunnel access"@en ;
.
:TunnelCategoryCode
  rdf:type owl:NamedIndividual ;
  rdf:type skos:ConceptScheme ;
  dc:isFormatOf :TunnelCategory ;
  skos:definition "Specifies the available list of enumerations for the categories of tunnel access"@en ;
.
:UomIdentifier
  rdf:type owl:Class ;
  rdfs:label "UomIdentifier"@en ;
  rdfs:subClassOf :tnitsCodeList ;
  skos:definition "Specifies the available list of preferred enumerations for identifiers for units of measure"@en ;
.
:UomIdentifierCode
  rdf:type owl:NamedIndividual ;
  rdf:type skos:ConceptScheme ;
  dc:isFormatOf :UomIdentifier ;
  skos:definition "Specifies the available list of preferred enumerations for identifiers for units of measure"@en ;
.
:UpdateInfo
  rdf:type owl:Class ;
  rdfs:label "UpdateInfo"@en ;
  rdfs:subClassOf :tnitsDataType ;
  rdfs:subClassOf [
      rdf:type owl:Restriction ;
      owl:allValuesFrom :UpdateType ;
      owl:onProperty <http://spec.tn-its.eu/owl/tnits-owl#UpdateInfo.type> ;
    ] ;
  rdfs:subClassOf [
      rdf:type owl:Restriction ;
      owl:onClass :UpdateType ;
      owl:onProperty <http://spec.tn-its.eu/owl/tnits-owl#UpdateInfo.type> ;
      owl:qualifiedCardinality "1"^^xsd:nonNegativeInteger ;
    ] ;
  skos:definition "Characterises the nature of the update for a road feature "@en ;
.
<http://spec.tn-its.eu/owl/tnits-owl#UpdateInfo.type>
  rdf:type owl:FunctionalProperty ;
  rdf:type owl:ObjectProperty ;
  rdfs:domain :UpdateInfo ;
  rdfs:label "UpdateInfo.type"@en ;
  rdfs:range :UpdateType ;
  skos:definition "The type of update "@en ;
.
:UpdateType
  rdf:type owl:Class ;
  rdfs:label "UpdateType"@en ;
  rdfs:subClassOf :tnitsEnumeration ;
  owl:equivalentClass [
      rdf:type owl:Class ;
      owl:oneOf (
          <http://spec.tn-its.eu/owl/tnits-owl#UpdateType.Add>
          <http://spec.tn-its.eu/owl/tnits-owl#UpdateType.Modify>
          <http://spec.tn-its.eu/owl/tnits-owl#UpdateType.Remove>
        ) ;
    ] ;
  skos:definition "Defines the different update types "@en ;
.
<http://spec.tn-its.eu/owl/tnits-owl#UpdateType.Add>
  rdf:type :UpdateType ;
  rdf:type owl:NamedIndividual ;
  rdf:type skos:Concept ;
  rdfs:label "Add"@no ;
  skos:definition "A new feature is inserted at the referenced location, without affecting any existing attribute feature "@en ;
  skos:inScheme :UpdateTypeCode ;
.
<http://spec.tn-its.eu/owl/tnits-owl#UpdateType.Modify>
  rdf:type :UpdateType ;
  rdf:type owl:NamedIndividual ;
  rdf:type skos:Concept ;
  rdfs:label "Modify"@no ;
  skos:definition "Signals a modification of the attributes of an existing road feature referenced by an object identifier "@en ;
  skos:inScheme :UpdateTypeCode ;
.
<http://spec.tn-its.eu/owl/tnits-owl#UpdateType.Remove>
  rdf:type :UpdateType ;
  rdf:type owl:NamedIndividual ;
  rdf:type skos:Concept ;
  rdfs:label "Remove"@no ;
  skos:definition "Signals a removal of the existing road feature referenced by an object identifier "@en ;
  skos:inScheme :UpdateTypeCode ;
.
:UpdateTypeCode
  rdf:type owl:NamedIndividual ;
  rdf:type skos:ConceptScheme ;
  dc:isFormatOf :UpdateType ;
  skos:definition "Defines the different update types "@en ;
.
:Validity
  rdf:type owl:Class ;
  rdfs:label "Validity"@en ;
  rdfs:subClassOf :tnitsDataType ;
  rdfs:subClassOf [
      rdf:type owl:Restriction ;
      owl:allValuesFrom :OverallPeriod ;
      owl:onProperty :validityTimeSpecification ;
    ] ;
  rdfs:subClassOf [
      rdf:type owl:Restriction ;
      owl:onClass :OverallPeriod ;
      owl:onProperty :validityTimeSpecification ;
      owl:qualifiedCardinality "1"^^xsd:nonNegativeInteger ;
    ] ;
  skos:definition "Specifies the periods of validity that relate to a road feature  "@en ;
.
:VehicleCharacteristics
  rdf:type owl:Class ;
  rdfs:label "VehicleCharacteristics"@en ;
  rdfs:subClassOf :tnitsDataType ;
  rdfs:subClassOf [
      rdf:type owl:Restriction ;
      owl:allValuesFrom :Emissions ;
      owl:onProperty <http://spec.tn-its.eu/owl/tnits-owl#VehicleCharacteristics.emissions> ;
    ] ;
  rdfs:subClassOf [
      rdf:type owl:Restriction ;
      owl:allValuesFrom :FuelType ;
      owl:onProperty <http://spec.tn-its.eu/owl/tnits-owl#VehicleCharacteristics.fuelType> ;
    ] ;
  rdfs:subClassOf [
      rdf:type owl:Restriction ;
      owl:allValuesFrom :GrossWeightCharacteristic ;
      owl:onProperty <http://spec.tn-its.eu/owl/tnits-owl#VehicleCharacteristics.grossWeightCharacteristic> ;
    ] ;
  rdfs:subClassOf [
      rdf:type owl:Restriction ;
      owl:allValuesFrom :HeaviestAxleWeightCharacteristic ;
      owl:onProperty <http://spec.tn-its.eu/owl/tnits-owl#VehicleCharacteristics.heaviestAxleWeightCharacteristic> ;
    ] ;
  rdfs:subClassOf [
      rdf:type owl:Restriction ;
      owl:allValuesFrom :HeightCharacteristic ;
      owl:onProperty <http://spec.tn-its.eu/owl/tnits-owl#VehicleCharacteristics.heightCharacteristic> ;
    ] ;
  rdfs:subClassOf [
      rdf:type owl:Restriction ;
      owl:allValuesFrom :LengthCharacteristic ;
      owl:onProperty <http://spec.tn-its.eu/owl/tnits-owl#VehicleCharacteristics.lengthCharacteristic> ;
    ] ;
  rdfs:subClassOf [
      rdf:type owl:Restriction ;
      owl:allValuesFrom :LoadType ;
      owl:onProperty <http://spec.tn-its.eu/owl/tnits-owl#VehicleCharacteristics.loadType> ;
    ] ;
  rdfs:subClassOf [
      rdf:type owl:Restriction ;
      owl:allValuesFrom :NumberOfAxlesCharacteristic ;
      owl:onProperty <http://spec.tn-its.eu/owl/tnits-owl#VehicleCharacteristics.numberOfAxlesCharacteristic> ;
    ] ;
  rdfs:subClassOf [
      rdf:type owl:Restriction ;
      owl:allValuesFrom :VehicleEquipment ;
      owl:onProperty <http://spec.tn-its.eu/owl/tnits-owl#VehicleCharacteristics.vehicleEquipment> ;
    ] ;
  rdfs:subClassOf [
      rdf:type owl:Restriction ;
      owl:allValuesFrom :VehicleType ;
      owl:onProperty <http://spec.tn-its.eu/owl/tnits-owl#VehicleCharacteristics.vehicleType> ;
    ] ;
  rdfs:subClassOf [
      rdf:type owl:Restriction ;
      owl:allValuesFrom :VehicleUsage ;
      owl:onProperty <http://spec.tn-its.eu/owl/tnits-owl#VehicleCharacteristics.vehicleUsage> ;
    ] ;
  rdfs:subClassOf [
      rdf:type owl:Restriction ;
      owl:allValuesFrom :WidthCharacteristic ;
      owl:onProperty <http://spec.tn-its.eu/owl/tnits-owl#VehicleCharacteristics.widthCharacteristic> ;
    ] ;
  rdfs:subClassOf [
      rdf:type owl:Restriction ;
      owl:allValuesFrom xsd:integer ;
      owl:onProperty :yearOfFirstRegistration ;
    ] ;
  rdfs:subClassOf [
      rdf:type owl:Restriction ;
      owl:maxQualifiedCardinality "1"^^xsd:nonNegativeInteger ;
      owl:onClass :LoadType ;
      owl:onProperty <http://spec.tn-its.eu/owl/tnits-owl#VehicleCharacteristics.loadType> ;
    ] ;
  rdfs:subClassOf [
      rdf:type owl:Restriction ;
      owl:maxQualifiedCardinality "1"^^xsd:nonNegativeInteger ;
      owl:onClass :VehicleEquipment ;
      owl:onProperty <http://spec.tn-its.eu/owl/tnits-owl#VehicleCharacteristics.vehicleEquipment> ;
    ] ;
  rdfs:subClassOf [
      rdf:type owl:Restriction ;
      owl:maxQualifiedCardinality "1"^^xsd:nonNegativeInteger ;
      owl:onClass :VehicleUsage ;
      owl:onProperty <http://spec.tn-its.eu/owl/tnits-owl#VehicleCharacteristics.vehicleUsage> ;
    ] ;
  rdfs:subClassOf [
      rdf:type owl:Restriction ;
      owl:maxQualifiedCardinality "1"^^xsd:nonNegativeInteger ;
      owl:onDataRange xsd:integer ;
      owl:onProperty :yearOfFirstRegistration ;
    ] ;
  skos:definition "A collection of parameters which characterise a vehicle. [SOURCE: DATEX 3.0 Part 7 (proposed EN 16157-7:2018)] "@en ;
.
<http://spec.tn-its.eu/owl/tnits-owl#VehicleCharacteristics.emissions>
  rdf:type owl:ObjectProperty ;
  rdfs:domain :VehicleCharacteristics ;
  rdfs:label "VehicleCharacteristics.emissions"@en ;
  rdfs:range :Emissions ;
  skos:definition "Emission characteristics of vehicles. [SOURCE: DATEX 3.0 Part 7 (proposed EN 16157-7:2018)] "@en ;
.
<http://spec.tn-its.eu/owl/tnits-owl#VehicleCharacteristics.fuelType>
  rdf:type owl:ObjectProperty ;
  rdfs:domain :VehicleCharacteristics ;
  rdfs:label "VehicleCharacteristics.fuelType"@en ;
  rdfs:range :FuelType ;
  skos:definition "The type of fuel used by the vehicle. [SOURCE: CEN/TS16157-3:2011] "@en ;
.
<http://spec.tn-its.eu/owl/tnits-owl#VehicleCharacteristics.grossWeightCharacteristic>
  rdf:type owl:ObjectProperty ;
  rdfs:domain :VehicleCharacteristics ;
  rdfs:label "VehicleCharacteristics.grossWeightCharacteristic"@en ;
  rdfs:range :GrossWeightCharacteristic ;
  skos:definition "Gross weight characteristic of a vehicle. [SOURCE: CEN/TS16157-3:2011] "@en ;
.
<http://spec.tn-its.eu/owl/tnits-owl#VehicleCharacteristics.heaviestAxleWeightCharacteristic>
  rdf:type owl:ObjectProperty ;
  rdfs:domain :VehicleCharacteristics ;
  rdfs:label "VehicleCharacteristics.heaviestAxleWeightCharacteristic"@en ;
  rdfs:range :HeaviestAxleWeightCharacteristic ;
  skos:definition "Weight characteristic of the heaviest axle on the vehicle. [SOURCE: CEN/TS16157-3:2011] "@en ;
.
<http://spec.tn-its.eu/owl/tnits-owl#VehicleCharacteristics.heightCharacteristic>
  rdf:type owl:ObjectProperty ;
  rdfs:domain :VehicleCharacteristics ;
  rdfs:label "VehicleCharacteristics.heightCharacteristic"@en ;
  rdfs:range :HeightCharacteristic ;
  skos:definition "Height characteristic of a vehicle. [SOURCE: CEN/TS16157-3:2011] "@en ;
.
<http://spec.tn-its.eu/owl/tnits-owl#VehicleCharacteristics.lengthCharacteristic>
  rdf:type owl:ObjectProperty ;
  rdfs:domain :VehicleCharacteristics ;
  rdfs:label "VehicleCharacteristics.lengthCharacteristic"@en ;
  rdfs:range :LengthCharacteristic ;
  skos:definition "Length characteristic of a vehicle. [SOURCE: CEN/TS16157-3:2011] "@en ;
.
<http://spec.tn-its.eu/owl/tnits-owl#VehicleCharacteristics.loadType>
  rdf:type owl:ObjectProperty ;
  rdfs:domain :VehicleCharacteristics ;
  rdfs:label "VehicleCharacteristics.loadType"@en ;
  rdfs:range :LoadType ;
  skos:definition "The type of load carried by the vehicle, especially in respect of hazardous loads. [SOURCE: CEN/TS16157-3:2011] "@en ;
.
<http://spec.tn-its.eu/owl/tnits-owl#VehicleCharacteristics.numberOfAxlesCharacteristic>
  rdf:type owl:ObjectProperty ;
  rdfs:domain :VehicleCharacteristics ;
  rdfs:label "VehicleCharacteristics.numberOfAxlesCharacteristic"@en ;
  rdfs:range :NumberOfAxlesCharacteristic ;
  skos:definition "Number of axles characteristic of a vehicle. [SOURCE: CEN/TS16157-3:2011] "@en ;
.
<http://spec.tn-its.eu/owl/tnits-owl#VehicleCharacteristics.vehicleEquipment>
  rdf:type owl:ObjectProperty ;
  rdfs:domain :VehicleCharacteristics ;
  rdfs:label "VehicleCharacteristics.vehicleEquipment"@en ;
  rdfs:range :VehicleEquipment ;
  skos:definition "The type of equipment in use or on board the vehicle. [SOURCE: CEN/TS16157-3:2011] "@en ;
.
<http://spec.tn-its.eu/owl/tnits-owl#VehicleCharacteristics.vehicleType>
  rdf:type owl:ObjectProperty ;
  rdfs:domain :VehicleCharacteristics ;
  rdfs:label "VehicleCharacteristics.vehicleType"@en ;
  rdfs:range :VehicleType ;
  skos:definition "Vehicle type. [SOURCE: CEN/TS16157-3:2011] "@en ;
.
<http://spec.tn-its.eu/owl/tnits-owl#VehicleCharacteristics.vehicleUsage>
  rdf:type owl:ObjectProperty ;
  rdfs:domain :VehicleCharacteristics ;
  rdfs:label "VehicleCharacteristics.vehicleUsage"@en ;
  rdfs:range :VehicleUsage ;
  skos:definition "The type of usage of the vehicle (i.e. for what purpose is the vehicle being used). [SOURCE: CEN/TS16157-3:2011] "@en ;
.
<http://spec.tn-its.eu/owl/tnits-owl#VehicleCharacteristics.widthCharacteristic>
  rdf:type owl:ObjectProperty ;
  rdfs:domain :VehicleCharacteristics ;
  rdfs:label "VehicleCharacteristics.widthCharacteristic"@en ;
  rdfs:range :WidthCharacteristic ;
  skos:definition "Width characteristic of a vehicle. [SOURCE: CEN/TS16157-3:2011] "@en ;
.
:VehicleCondition
  rdf:type owl:Class ;
  rdfs:label "VehicleCondition"@en ;
  rdfs:subClassOf :Condition ;
  rdfs:subClassOf [
      rdf:type owl:Restriction ;
      owl:allValuesFrom :VehicleCharacteristics ;
      owl:onProperty <http://spec.tn-its.eu/owl/tnits-owl#VehicleCondition.vehicleCharacteristics> ;
    ] ;
  rdfs:subClassOf [
      rdf:type owl:Restriction ;
      owl:onClass :VehicleCharacteristics ;
      owl:onProperty <http://spec.tn-its.eu/owl/tnits-owl#VehicleCondition.vehicleCharacteristics> ;
      owl:qualifiedCardinality "1"^^xsd:nonNegativeInteger ;
    ] ;
  skos:definition "Specifies vehicle type condition applicability relating to a road feature  "@en ;
.
<http://spec.tn-its.eu/owl/tnits-owl#VehicleCondition.vehicleCharacteristics>
  rdf:type owl:FunctionalProperty ;
  rdf:type owl:ObjectProperty ;
  rdfs:domain :VehicleCondition ;
  rdfs:label "VehicleCondition.vehicleCharacteristics"@en ;
  rdfs:range :VehicleCharacteristics ;
  skos:definition "Specifies the vehicle characteristics that are applicable to the vehicle type condition for a road feature "@en ;
.
:VehicleEquipment
  rdf:type owl:Class ;
  rdfs:label "VehicleEquipment"@en ;
  rdfs:subClassOf :tnitsCodeList ;
  skos:definition "Specifies the available list of enumerations for the vehicle equipment types"@en ;
.
:VehicleEquipmentCode
  rdf:type owl:NamedIndividual ;
  rdf:type skos:ConceptScheme ;
  dc:isFormatOf :VehicleEquipment ;
  skos:definition "Specifies the available list of enumerations for the vehicle equipment types"@en ;
.
:VehicleType
  rdf:type owl:Class ;
  rdfs:label "VehicleType"@en ;
  rdfs:subClassOf :tnitsCodeList ;
  skos:definition "Specifies the available list of enumerations for types of vehicle."@en ;
.
:VehicleTypeCode
  rdf:type owl:NamedIndividual ;
  rdf:type skos:ConceptScheme ;
  dc:isFormatOf :VehicleType ;
  skos:definition "Specifies the available list of enumerations for types of vehicle."@en ;
.
:VehicleUsage
  rdf:type owl:Class ;
  rdfs:label "VehicleUsage"@en ;
  rdfs:subClassOf :tnitsCodeList ;
  skos:definition "Specifies the available list of enumerations for types of usage of vehicles."@en ;
.
:VehicleUsageCode
  rdf:type owl:NamedIndividual ;
  rdf:type skos:ConceptScheme ;
  dc:isFormatOf :VehicleUsage ;
  skos:definition "Specifies the available list of enumerations for types of usage of vehicles."@en ;
.
:WeatherCondition
  rdf:type owl:Class ;
  rdfs:label "WeatherCondition"@en ;
  rdfs:subClassOf :Condition ;
  rdfs:subClassOf [
      rdf:type owl:Restriction ;
      owl:allValuesFrom :WeatherType ;
      owl:onProperty <http://spec.tn-its.eu/owl/tnits-owl#WeatherCondition.weatherType> ;
    ] ;
  rdfs:subClassOf [
      rdf:type owl:Restriction ;
      owl:onClass :WeatherType ;
      owl:onProperty <http://spec.tn-its.eu/owl/tnits-owl#WeatherCondition.weatherType> ;
      owl:qualifiedCardinality "1"^^xsd:nonNegativeInteger ;
    ] ;
  skos:definition "Specifies weather type condition applicability relating to a road feature  "@en ;
.
<http://spec.tn-its.eu/owl/tnits-owl#WeatherCondition.weatherType>
  rdf:type owl:FunctionalProperty ;
  rdf:type owl:ObjectProperty ;
  rdfs:domain :WeatherCondition ;
  rdfs:label "WeatherCondition.weatherType"@en ;
  rdfs:range :WeatherType ;
  skos:definition "Specifies the available list of enumerations for the weather type condition for a road feature by reference to an item in an external code list "@en ;
.
:WeatherType
  rdf:type owl:Class ;
  rdfs:label "WeatherType"@en ;
  rdfs:subClassOf :tnitsCodeList ;
  skos:definition "Types of weather conditions which affect driving conditions."@en ;
.
:WeatherTypeCode
  rdf:type owl:NamedIndividual ;
  rdf:type skos:ConceptScheme ;
  dc:isFormatOf :WeatherType ;
  skos:definition "Types of weather conditions which affect driving conditions."@en ;
.
:WeekOfMonth
  rdf:type owl:Class ;
  rdfs:label "WeekOfMonth"@en ;
  rdfs:subClassOf :tnitsEnumeration ;
  owl:equivalentClass [
      rdf:type owl:Class ;
      owl:oneOf (
          <http://spec.tn-its.eu/owl/tnits-owl#WeekOfMonth.fifthWeekOfMonth>
          <http://spec.tn-its.eu/owl/tnits-owl#WeekOfMonth.firstWeekOfMonth>
          <http://spec.tn-its.eu/owl/tnits-owl#WeekOfMonth.fourthWeekOfMonth>
          <http://spec.tn-its.eu/owl/tnits-owl#WeekOfMonth.secondWeekOfMonth>
          <http://spec.tn-its.eu/owl/tnits-owl#WeekOfMonth.sixthWeekOfMonth>
          <http://spec.tn-its.eu/owl/tnits-owl#WeekOfMonth.thirdWeekOfMonth>
        ) ;
    ] ;
  skos:definition "Applicable week of the month"@en ;
.
<http://spec.tn-its.eu/owl/tnits-owl#WeekOfMonth.fifthWeekOfMonth>
  rdf:type :WeekOfMonth ;
  rdf:type owl:NamedIndividual ;
  rdf:type skos:Concept ;
  rdfs:label "fifthWeekOfMonth"@no ;
  skos:inScheme :WeekOfMonthCode ;
.
<http://spec.tn-its.eu/owl/tnits-owl#WeekOfMonth.firstWeekOfMonth>
  rdf:type :WeekOfMonth ;
  rdf:type owl:NamedIndividual ;
  rdf:type skos:Concept ;
  rdfs:label "firstWeekOfMonth"@no ;
  skos:inScheme :WeekOfMonthCode ;
.
<http://spec.tn-its.eu/owl/tnits-owl#WeekOfMonth.fourthWeekOfMonth>
  rdf:type :WeekOfMonth ;
  rdf:type owl:NamedIndividual ;
  rdf:type skos:Concept ;
  rdfs:label "fourthWeekOfMonth"@no ;
  skos:inScheme :WeekOfMonthCode ;
.
<http://spec.tn-its.eu/owl/tnits-owl#WeekOfMonth.secondWeekOfMonth>
  rdf:type :WeekOfMonth ;
  rdf:type owl:NamedIndividual ;
  rdf:type skos:Concept ;
  rdfs:label "secondWeekOfMonth"@no ;
  skos:inScheme :WeekOfMonthCode ;
.
<http://spec.tn-its.eu/owl/tnits-owl#WeekOfMonth.sixthWeekOfMonth>
  rdf:type :WeekOfMonth ;
  rdf:type owl:NamedIndividual ;
  rdf:type skos:Concept ;
  rdfs:label "sixthWeekOfMonth"@no ;
  skos:inScheme :WeekOfMonthCode ;
.
<http://spec.tn-its.eu/owl/tnits-owl#WeekOfMonth.thirdWeekOfMonth>
  rdf:type :WeekOfMonth ;
  rdf:type owl:NamedIndividual ;
  rdf:type skos:Concept ;
  rdfs:label "thirdWeekOfMonth"@no ;
  skos:inScheme :WeekOfMonthCode ;
.
:WeekOfMonthCode
  rdf:type owl:NamedIndividual ;
  rdf:type skos:ConceptScheme ;
  dc:isFormatOf :WeekOfMonth ;
  skos:definition "Applicable week of the month"@en ;
.
:WeightType
  rdf:type owl:Class ;
  rdfs:label "WeightType"@en ;
  rdfs:subClassOf :tnitsCodeList ;
  skos:definition "Type of weight - describing the meaning of a vehicle weight value"@en ;
.
:WeightTypeCode
  rdf:type owl:NamedIndividual ;
  rdf:type skos:ConceptScheme ;
  dc:isFormatOf :WeightType ;
  skos:definition "Type of weight - describing the meaning of a vehicle weight value"@en ;
.
:WidthCharacteristic
  rdf:type owl:Class ;
  rdfs:label "WidthCharacteristic"@en ;
  rdfs:subClassOf :tnitsDataType ;
  rdfs:subClassOf [
      rdf:type owl:Restriction ;
      owl:allValuesFrom :ComparisonOperator ;
      owl:onProperty :comparisonOperator ;
    ] ;
  rdfs:subClassOf [
      rdf:type owl:Restriction ;
      owl:allValuesFrom :Measure ;
      owl:onProperty :vehicleWidth ;
    ] ;
  rdfs:subClassOf [
      rdf:type owl:Restriction ;
      owl:onClass :ComparisonOperator ;
      owl:onProperty :comparisonOperator ;
      owl:qualifiedCardinality "1"^^xsd:nonNegativeInteger ;
    ] ;
  rdfs:subClassOf [
      rdf:type owl:Restriction ;
      owl:onClass :Measure ;
      owl:onProperty :vehicleWidth ;
      owl:qualifiedCardinality "1"^^xsd:nonNegativeInteger ;
    ] ;
  skos:definition "Width characteristic of a vehicle. [SOURCE: CEN/TS16157-3:2011] "@en ;
.
:XMLLocationReference
  rdf:type owl:Class ;
  rdfs:label "XMLLocationReference"@en ;
  rdfs:subClassOf :tnitsDataType ;
  skos:definition "A OpenLR location reference encoded using XML according to the OpenLR specification (see bibliography)  "@en ;
.
:applicableDay
  rdf:type owl:ObjectProperty ;
  rdfs:domain :DayWeekMonth ;
  rdfs:label "applicableDay"@en ;
  rdfs:range :DayOfWeek ;
  skos:definition "Applicable day of the week. \"All days of the week\" is expressed by noninclusion of this attribute. [SOURCE: CEN/TS16157-3:2011] "@en ;
.
:applicableDirection
  rdf:type owl:FunctionalProperty ;
  rdf:type owl:ObjectProperty ;
  rdfs:domain :LinkReference ;
  rdfs:label "applicableDirection"@en ;
  rdfs:range :LinkDirectionValue ;
  skos:definition "Indicates the applicable direction "@en ;
.
:applicableMonth
  rdf:type owl:ObjectProperty ;
  rdfs:domain :DayWeekMonth ;
  rdfs:label "applicableMonth"@en ;
  rdfs:range :MonthOfYear ;
  skos:definition "Applicable month of the year.  \"All months of the year\" is expressed by noninclusion of this attribute. [SOURCE: CEN/TS16157-3:2011] "@en ;
.
:applicableWeek
  rdf:type owl:ObjectProperty ;
  rdfs:domain :DayWeekMonth ;
  rdfs:label "applicableWeek"@en ;
  rdfs:range :WeekOfMonth ;
  skos:definition "Applicable week of the month (1 to 5). \"All weeks of the month\" is expressed by non-inclusion of this attribute.  [SOURCE: CEN/TS16157-3:2011] "@en ;
.
:beginLifespanVersion
  rdf:type owl:DatatypeProperty ;
  rdf:type owl:FunctionalProperty ;
  rdfs:domain :RoadFeature ;
  rdfs:label "beginLifespanVersion"@en ;
  rdfs:range xsd:dateTime ;
  skos:definition "Date and time at which this version of the spatial object was inserted or changed in the spatial data set. "@en ;
.
:beginOrDuration
  rdf:type owl:FunctionalProperty ;
  rdf:type owl:ObjectProperty ;
  rdfs:domain :FuzzyTimePeriod ;
  rdfs:label "beginOrDuration"@en ;
  rdfs:range :FuzzyTimeType ;
  skos:definition "Time period begins with a fuzzy time or the duration is a fuzzy time "@en ;
.
:comparisonOperator
  rdf:type owl:ObjectProperty ;
  rdfs:label "comparisonOperator"@en ;
  rdfs:range :ComparisonOperator ;
  skos:definition "The operator to be used in the vehicle characteristic comparison operation. [SOURCE: CEN/TS16157-3:2011] "@en ;
.
:conditions
  rdf:type owl:ObjectProperty ;
  rdfs:domain :ConditionSet ;
  rdfs:label "conditions"@en ;
  rdfs:range :Condition ;
  skos:definition "Specifies the conditions that are present in the set "@en ;
.
:content
  rdf:type owl:ObjectProperty ;
  rdfs:domain :RoadSignProperty ;
  rdfs:label "content"@en ;
  rdfs:range :RoadSignContent ;
  skos:definition "Defines quantifiable content of the traffic sign "@en ;
.
:datasetCreationTime
  rdf:type owl:DatatypeProperty ;
  rdf:type owl:FunctionalProperty ;
  rdfs:domain :Metadata ;
  rdfs:label "datasetCreationTime"@en ;
  rdfs:range xsd:dateTime ;
  skos:definition "Indicates when the metadata are created "@en ;
.
:datasetId
  rdf:type owl:ObjectProperty ;
  rdfs:label "datasetId"@en ;
  rdfs:range :Identifier ;
  skos:definition "The identification of the dataset which is the source of this feedback information. This identifier shall correspond to the metadata element Unique resource identifier in the dataset for which the feedback is created."@en ;
.
:defaultLRM
  rdf:type owl:ObjectProperty ;
  rdfs:domain :RoadFeatureDataset ;
  rdfs:label "defaultLRM"@en ;
  rdfs:range lr:LinearReferencingMethod ;
  skos:definition "Default linear referencing method to be used in the dataset."@en ;
.
:description
  rdf:type owl:DatatypeProperty ;
  rdfs:domain :LinearLocationReference ;
  rdfs:label "description"@en ;
  rdfs:range xsd:string ;
  skos:definition "A free text string providing a description for the linear location "@en ;
.
:element
  rdf:type owl:FunctionalProperty ;
  rdf:type owl:ObjectProperty ;
  rdfs:domain :NetworkReference ;
  rdfs:label "element"@en ;
  rdfs:range :NetworkElement ;
  owl:equivalentProperty lr:hasLinearElement ;
  skos:definition "The referenced network element."@en ;
.
:emissionClassificationOther
  rdf:type owl:DatatypeProperty ;
  rdfs:domain :Emissions ;
  rdfs:label "emissionClassificationOther"@en ;
  rdfs:range xsd:string ;
  skos:definition "Some other (probably locally defined) value(s) for emission classification. [SOURCE: DATEX 3.0 Part 7 (proposed EN 16157-7:2018)] "@en ;
.
:emissionLevel
  rdf:type owl:ObjectProperty ;
  rdfs:domain :Emissions ;
  rdfs:label "emissionLevel"@en ;
  rdfs:range :LowEmissionLevel ;
  skos:definition "The low emission level of a vehicle. [SOURCE: DATEX 3.0 Part 7 (proposed EN 16157-7:2018)] "@en ;
.
:encodedGeometry
  rdf:type owl:FunctionalProperty ;
  rdf:type owl:ObjectProperty ;
  rdfs:domain :GeometryLocationReference ;
  rdfs:label "encodedGeometry"@en ;
  rdfs:range gsp:Geometry ;
  skos:definition "the geometry in the source road database that was used to encode the location reference of the referenced location "@en ;
.
:endLifespanVersion
  rdf:type owl:DatatypeProperty ;
  rdfs:domain :RoadFeature ;
  rdfs:label "endLifespanVersion"@en ;
  rdfs:range xsd:dateTime ;
  skos:definition "Date and time at which this version of the spatial object was superseded or retired in the spatial data set. "@en ;
.
:endOfPeriod
  rdf:type owl:DatatypeProperty ;
  rdfs:domain :Period ;
  rdfs:label "endOfPeriod"@en ;
  rdfs:range xsd:dateTime ;
  skos:definition "End of a period. [SOURCE: CEN/TS16157-3:2011]  Specifies the end date and time of this period. If not present, the end of the period is considered to be continuously on-going to an undefined date in the future."@en ;
.
:endOrDuration
  rdf:type owl:ObjectProperty ;
  rdfs:domain :FuzzyTimePeriod ;
  rdfs:label "endOrDuration"@en ;
  rdfs:range :FuzzyTimeType ;
  skos:definition "time period ends with a fuzzy time or the duration is a fuzzy time"@en ;
.
:endTimeOfPeriod
  rdf:type owl:FunctionalProperty ;
  rdf:type owl:ObjectProperty ;
  rdfs:domain :TimePeriodOfDay ;
  rdfs:label "endTimeOfPeriod"@en ;
  rdfs:range :Time ;
  skos:definition "End of time period. [SOURCE: CEN/TS16157-3:2011] "@en ;
.
:eventCode
  rdf:type owl:ObjectProperty ;
  rdfs:label "eventCode"@en ;
  skos:definition "Indicates the type of event that occurred "@en ;
.
:events
  rdf:type owl:ObjectProperty ;
  rdfs:domain :FeedbackLog ;
  rdfs:label "events"@en ;
  rdfs:range :FeedbackLogEvent ;
  skos:definition "The set of Refers to a log which records all the interesting events during download and integration of road features. "@en ;
.
:exceptionPeriod
  rdf:type owl:ObjectProperty ;
  rdfs:domain :OverallPeriod ;
  rdfs:label "exceptionPeriod"@en ;
  rdfs:range :Period ;
  skos:definition "A single time period, a recurring time period or a set of different recurring time periods during which validity is false. [SOURCE: CEN/TS16157-3:2011] "@en ;
.
:feedbackInfo
  rdf:type owl:FunctionalProperty ;
  rdf:type owl:ObjectProperty ;
  rdfs:domain :FeedbackDataset ;
  rdfs:label "feedbackInfo"@en ;
  rdfs:range :FeedbackInformation ;
  skos:definition "The feedback information  "@en ;
.
:gddCode
  rdf:type owl:FunctionalProperty ;
  rdf:type owl:ObjectProperty ;
  rdfs:domain :RoadSignProperty ;
  rdfs:label "gddCode"@en ;
  rdfs:range :RoadSignType ;
  skos:definition "The type of the road sign by reference to an item in the RoadSignType external code list "@en ;
.
:grossVehicleWeight
  rdf:type owl:FunctionalProperty ;
  rdf:type owl:ObjectProperty ;
  rdfs:domain :GrossWeightCharacteristic ;
  rdfs:label "grossVehicleWeight"@en ;
  rdfs:range :Measure ;
  skos:definition "The gross weight of the vehicle and its load, including any trailers. [SOURCE: CEN/TS16157-3:2011] "@en ;
.
:heaviestAxleWeight
  rdf:type owl:FunctionalProperty ;
  rdf:type owl:ObjectProperty ;
  rdfs:domain :HeaviestAxleWeightCharacteristic ;
  rdfs:label "heaviestAxleWeight"@en ;
  rdfs:range :Measure ;
  skos:definition "The weight of the heaviest axle on the vehicle. [SOURCE: CEN/TS161573:2011] "@en ;
.
:id
  rdf:type owl:ObjectProperty ;
  rdfs:domain :NetworkElement ;
  rdfs:label "id"@en ;
  rdfs:range :Identifier ;
  skos:definition "External identifier of the network element."@en ;
.
:intersectWithApplicableDays
  rdf:type owl:DatatypeProperty ;
  rdf:type owl:FunctionalProperty ;
  rdfs:domain :SpecialDay ;
  rdfs:label "intersectWithApplicableDays"@en ;
  rdfs:range xsd:boolean ;
  skos:definition "When true, the period is the intersection of applicable days and this special day. When false, the period is the union of applicable days and this special day. [SOURCE: DATEX 3.0 Part 7 (proposed EN 16157-7:2018)] "@en ;
.
:laneExtension
  rdf:type owl:DatatypeProperty ;
  rdf:type owl:FunctionalProperty ;
  rdfs:domain :LaneCondition ;
  rdfs:label "laneExtension"@en ;
  rdfs:range xsd:integer ;
  skos:definition "Number of lanes including the start lane counted from the right-hand side for which the condition applies. "@en ;
.
:localId
  rdf:type owl:DatatypeProperty ;
  rdf:type owl:FunctionalProperty ;
  rdfs:domain :Identifier ;
  rdfs:label "localId"@en ;
  rdfs:range xsd:string ;
  skos:definition "A local identifier, assigned by the data provider. The local identifier is unique within the namespace, that is no other spatial object carries the same unique identifier. "@en ;
.
:log
  rdf:type owl:FunctionalProperty ;
  rdf:type owl:ObjectProperty ;
  rdfs:domain :FeedbackInformation ;
  rdfs:label "log"@en ;
  rdfs:range :FeedbackLog ;
  skos:definition "Refers to a log which records all the interesting events during download and integration of road features. "@en ;
.
:name
  rdf:type owl:DatatypeProperty ;
  rdfs:domain :LinearLocationReference ;
  rdfs:label "name"@en ;
  rdfs:range xsd:string ;
  skos:definition "A free text string providing the name for the linear location "@en ;
.
:namespace
  rdf:type owl:DatatypeProperty ;
  rdf:type owl:FunctionalProperty ;
  rdfs:domain :Identifier ;
  rdfs:label "namespace"@en ;
  rdfs:range xsd:string ;
  skos:definition "Namespace uniquely identifying the data source of the spatial object."@en ;
.
:natureOfDistance
  rdf:type owl:ObjectProperty ;
  rdfs:domain :RoadSignContent ;
  rdfs:label "natureOfDistance"@en ;
  rdfs:range :NatureOfDistanceMeasure ;
  skos:definition "Defines the semantics of a distance measure provided within the RoadSignContent"@en ;
.
:negate
  rdf:type owl:DatatypeProperty ;
  rdfs:domain :Condition ;
  rdfs:label "negate"@en ;
  rdfs:range xsd:boolean ;
  skos:definition "If set to true means that the entire condition shall be negated. Note:  A condition stating VehicleType=EmergencyVehicle and negate = true would mean all vehicles except those of type EmergencyVehicle. "@en ;
.
:nrFail
  rdf:type owl:DatatypeProperty ;
  rdf:type owl:FunctionalProperty ;
  rdfs:domain :SummaryInfo ;
  rdfs:label "nrFail"@en ;
  rdfs:range xsd:integer ;
  skos:definition "Number of road features for which integration failed. "@en ;
.
:nrSuccess
  rdf:type owl:DatatypeProperty ;
  rdf:type owl:FunctionalProperty ;
  rdfs:domain :SummaryInfo ;
  rdfs:label "nrSuccess"@en ;
  rdfs:range xsd:integer ;
  skos:definition "Number of successfully decoded and integrated road features. "@en ;
.
:numberOfAxles
  rdf:type owl:DatatypeProperty ;
  rdf:type owl:FunctionalProperty ;
  rdfs:domain :NumberOfAxlesCharacteristic ;
  rdfs:label "numberOfAxles"@en ;
  rdfs:range xsd:integer ;
  skos:definition "The total number of axles of an individual vehicle.  [SOURCE: CEN/TS161573:2011] "@en ;
.
:operator
  rdf:type owl:FunctionalProperty ;
  rdf:type owl:ObjectProperty ;
  rdfs:domain :ConditionSet ;
  rdfs:label "operator"@en ;
  rdfs:range :ConditionOperator ;
  skos:definition "Specifies the operator to be applied between the conditions in the set "@en ;
.
:overallEndTime
  rdf:type owl:DatatypeProperty ;
  rdfs:domain :OverallPeriod ;
  rdfs:label "overallEndTime"@en ;
  rdfs:range xsd:dateTime ;
  skos:definition "End of bounding period of validity defined by date and time. [SOURCE: CEN/TS16157-3:2011]  If not present the overall period is considered to continue indefinitely into the future. "@en ;
.
:overallStartTime
  rdf:type owl:DatatypeProperty ;
  rdf:type owl:FunctionalProperty ;
  rdfs:domain :OverallPeriod ;
  rdfs:label "overallStartTime"@en ;
  rdfs:range xsd:dateTime ;
  skos:definition "Start of bounding period of validity defined by date and time. [SOURCE: CEN/TS16157-3:2011] "@en ;
.
:overridingLRM
  rdf:type owl:ObjectProperty ;
  rdfs:domain :NetworkReference ;
  rdfs:label "overridingLRM"@en ;
  rdfs:range lr:LinearReferencingMethod ;
  owl:equivalentProperty lr:hasOverridingLRM ;
  skos:definition "linear referencing method overriding default method for the data set"@en ;
.
:periodName
  rdf:type owl:DatatypeProperty ;
  rdfs:domain :Period ;
  rdfs:label "periodName"@en ;
  rdfs:range xsd:string ;
  skos:definition "The name of the period. [SOURCE: CEN/TS16157-3:2011] "@en ;
.
:predefinedLocationReference
  rdf:type owl:FunctionalProperty ;
  rdf:type owl:ObjectProperty ;
  rdfs:domain :LocationByExternalReference ;
  rdfs:label "predefinedLocationReference"@en ;
  rdfs:range :PredefinedLocation ;
  skos:definition "A location reference to an object that has pre-defined and stored for future reference "@en ;
.
:processed
  rdf:type owl:DatatypeProperty ;
  rdf:type owl:FunctionalProperty ;
  rdfs:domain :FeedbackInformation ;
  rdfs:label "processed"@en ;
  rdfs:range xsd:dateTime ;
  skos:definition "The declared date and time when the dataset was processed "@en ;
.
:properties
  rdf:type owl:ObjectProperty ;
  rdfs:domain :RoadFeature ;
  rdfs:label "properties"@en ;
  rdfs:range :AbstractRoadFeatureProperty ;
  skos:definition "The property values of interest for the road feature "@en ;
.
:publicEvent
  rdf:type owl:DatatypeProperty ;
  rdfs:domain :SpecialDay ;
  rdfs:label "publicEvent"@en ;
  rdfs:range xsd:string ;
  skos:definition "Type of public event on this special day. [SOURCE: DATEX 3.0 Part 7 (proposed EN 16157-7:2018)] "@en ;
.
:publicHolidayName
  rdf:type owl:DatatypeProperty ;
  rdf:type owl:FunctionalProperty ;
  rdfs:domain :PublicHoliday ;
  rdfs:label "publicHolidayName"@en ;
  rdfs:range xsd:string ;
  skos:definition "Specification of a specific public holiday by its name. [SOURCE: DATEX 3.0 Part 7 (proposed EN 16157-7:2018)] "@en ;
.
:recurringDayWeekMonthPeriod
  rdf:type owl:ObjectProperty ;
  rdfs:domain :Period ;
  rdfs:label "recurringDayWeekMonthPeriod"@en ;
  rdfs:range :DayWeekMonth ;
  skos:definition "Specification of periods defined by the intersection of days, weeks and months. [SOURCE: CEN/TS16157-3:2011] "@en ;
.
:recurringFuzzyTimePeriod
  rdf:type owl:ObjectProperty ;
  rdfs:domain :Period ;
  rdfs:label "recurringFuzzyTimePeriod"@en ;
  rdfs:range :FuzzyTimePeriod ;
  skos:definition "defines a time period whose start, end or duration is based upon a non-precise or variable qualified concept, resulting in a non-precise, potentially circumstantial defined time period"@en ;
.
:recurringSpecialDay
  rdf:type owl:ObjectProperty ;
  rdfs:domain :Period ;
  rdfs:label "recurringSpecialDay"@en ;
  rdfs:range :SpecialDay ;
  skos:definition "A recurring period of a special type of day, possibly also a public holiday. Can be country or region specific. [SOURCE: DATEX 3.0 Part 7 (proposed EN 16157-7:2018)] "@en ;
.
:recurringTimePeriodOfDay
  rdf:type owl:ObjectProperty ;
  rdfs:domain :Period ;
  rdfs:label "recurringTimePeriodOfDay"@en ;
  rdfs:range :TimePeriodOfDay ;
  skos:definition "A recurring period of a day. [SOURCE: CEN/TS16157-3:2011] "@en ;
.
:roadFeatureId
  rdf:type owl:ObjectProperty ;
  rdfs:label "roadFeatureId"@en ;
  rdfs:range :Identifier ;
  skos:definition "The identity for the road feature. Permanent identifier for the road feature in the database of the data provider. "@en ;
.
:roadFeatures
  rdf:type owl:ObjectProperty ;
  rdfs:domain :RoadFeatureDataset ;
  rdfs:label "roadFeatures"@en ;
  rdfs:range :RoadFeature ;
  skos:definition "The set of RoadFeatures contained in this dataset "@en ;
.
:source
  rdf:type owl:FunctionalProperty ;
  rdf:type owl:ObjectProperty ;
  rdfs:domain :RoadFeature ;
  rdfs:label "source"@en ;
  rdfs:range :RoadFeatureSource ;
  skos:definition "Identifies the evidence base that has been used by the authorised authority supplying the data. "@en ;
.
:startLane
  rdf:type owl:DatatypeProperty ;
  rdf:type owl:FunctionalProperty ;
  rdfs:domain :LaneCondition ;
  rdfs:label "startLane"@en ;
  rdfs:range xsd:integer ;
  skos:definition "Start lane counted from the right side for which the condition applies. NOTE \"Right side\" is to be interpreted in relation to the direction of the location reference.  Numbering starts from 1.  All lanes should be considered, e.g. including emergency lanes, special purpose lanes, etc."@en ;
.
:startOfPeriod
  rdf:type owl:DatatypeProperty ;
  rdfs:domain :Period ;
  rdfs:label "startOfPeriod"@en ;
  rdfs:range xsd:dateTime ;
  skos:definition "Start of period. [SOURCE: CEN/TS16157-3:2011]  Specifies the start date and time of this period. If not present, the start of the period is considered to be continuously on-going from an undefined date in the past. "@en ;
.
:startTimeOfPeriod
  rdf:type owl:FunctionalProperty ;
  rdf:type owl:ObjectProperty ;
  rdfs:domain :TimePeriodOfDay ;
  rdfs:label "startTimeOfPeriod"@en ;
  rdfs:range :Time ;
  skos:definition "Start of time period. [SOURCE: CEN/TS16157-3:2011] "@en ;
.
:summary
  rdf:type owl:FunctionalProperty ;
  rdf:type owl:ObjectProperty ;
  rdfs:domain :FeedbackLog ;
  rdfs:label "summary"@en ;
  rdfs:range :SummaryInfo ;
  skos:definition "A result summary "@en ;
.
:tnits
  rdf:type owl:Class ;
  rdfs:label "TN-ITS Root"@en ;
  owl:disjointUnionOf (
      :tnitsCodeList
      :tnitsDataType
      :tnitsEnumeration
      :tnitsFeature
    ) ;
.
:tnitsCodeList
  rdf:type owl:Class ;
  rdfs:label "TN-ITS Code value"@en ;
  rdfs:subClassOf :tnits ;
  rdfs:subClassOf skos:Concept ;
.
:tnitsDataType
  rdf:type owl:Class ;
  rdfs:label "TN-ITS Data type"@en ;
  rdfs:subClassOf :tnits ;
  owl:disjointUnionOf (
      :AbstractRoadFeatureProperty
      :BinaryLocationReference
      :Condition
      :DayWeekMonth
      :Emissions
      :FuzzyTimePeriod
      :GrossWeightCharacteristic
      :HeaviestAxleWeightCharacteristic
      :HeightCharacteristic
      :Identifier
      :LengthCharacteristic
      :LocationReference
      :Metadata
      :NetworkReference
      :NumberOfAxlesCharacteristic
      :OverallPeriod
      :Period
      :RoadSignContent
      :SpecialDay
      :SummaryInfo
      :TimePeriodOfDay
      :UpdateInfo
      :Validity
      :VehicleCharacteristics
      :WidthCharacteristic
      :XMLLocationReference
    ) ;
.
:tnitsEnumeration
  rdf:type owl:Class ;
  rdfs:label "TN-ITS Enumeration value"@en ;
  rdfs:subClassOf :tnits ;
  rdfs:subClassOf skos:Concept ;
  owl:disjointUnionOf (
      :ComparisonOperator
      :ConditionOperator
      :DatasetType
      :DayOfWeek
      :MonthOfYear
      :UpdateType
      :WeekOfMonth
    ) ;
.
:tnitsFeature
  rdf:type owl:Class ;
  rdfs:label "TN-ITS Feature"@en ;
  rdfs:subClassOf <http://def.isotc211.org/iso19109/2015/GeneralFeatureModel#AnyFeature> ;
  rdfs:subClassOf :tnits ;
  rdfs:subClassOf gsp:Feature ;
  owl:disjointUnionOf (
      :Dataset
      :FeedbackInformation
      :FeedbackLog
      :FeedbackLogEvent
      :NetworkElement
      :RoadFeature
    ) ;
.
:typeOfWeight
  rdf:type owl:FunctionalProperty ;
  rdf:type owl:ObjectProperty ;
  rdfs:domain :GrossWeightCharacteristic ;
  rdfs:label "typeOfWeight"@en ;
  rdfs:range :WeightType ;
  skos:definition "The meaning of the weight value [SOURCE: CEN/TS16157-3:2011] "@en ;
.
:validFrom
  rdf:type owl:DatatypeProperty ;
  rdf:type owl:FunctionalProperty ;
  rdfs:domain :RoadFeature ;
  rdfs:label "validFrom"@en ;
  rdfs:range xsd:date ;
  skos:definition "The date from which this road feature is valid and in use "@en ;
.
:validPeriod
  rdf:type owl:ObjectProperty ;
  rdfs:domain :OverallPeriod ;
  rdfs:label "validPeriod"@en ;
  rdfs:range :Period ;
  skos:definition "A single time period, a recurring time period or a set of different recurring time periods during which validity is true. [SOURCE: CEN/TS16157-3:2011] "@en ;
.
:validTo
  rdf:type owl:DatatypeProperty ;
  rdfs:domain :RoadFeature ;
  rdfs:label "validTo"@en ;
  rdfs:range xsd:date ;
  skos:definition "The date from which this road feature is no longer valid "@en ;
.
:validityPeriod
  rdf:type owl:FunctionalProperty ;
  rdf:type owl:ObjectProperty ;
  rdfs:domain :TimeCondition ;
  rdfs:label "validityPeriod"@en ;
  rdfs:range :Validity ;
  skos:definition "Specifies the time period for which this time condition applies "@en ;
.
:validityTimeSpecification
  rdf:type owl:FunctionalProperty ;
  rdf:type owl:ObjectProperty ;
  rdfs:domain :Validity ;
  rdfs:label "validityTimeSpecification"@en ;
  rdfs:range :OverallPeriod ;
  skos:definition "A specification of periods of validity defined by overall bounding start and end times and the possible intersection of valid periods with exception periods (exception periods overriding valid periods). [SOURCE: CEN/TS161573:2011] "@en ;
.
:valueReference
  rdf:type owl:ObjectProperty ;
  rdfs:domain :GenericRoadFeatureProperty ;
  rdfs:label "valueReference"@en ;
  rdfs:range :PropertyValueReferenceType ;
  skos:definition "A reference to an externally defined value"@en ;
.
:vehicleHeight
  rdf:type owl:FunctionalProperty ;
  rdf:type owl:ObjectProperty ;
  rdfs:domain :HeightCharacteristic ;
  rdfs:label "vehicleHeight"@en ;
  rdfs:range :Measure ;
  skos:definition "The height of the highest part, excluding antennae, of an individual vehicle above the road surface, in metres. [SOURCE: CEN/TS16157-3:2011] "@en ;
.
:vehicleLength
  rdf:type owl:FunctionalProperty ;
  rdf:type owl:ObjectProperty ;
  rdfs:domain :LengthCharacteristic ;
  rdfs:label "vehicleLength"@en ;
  rdfs:range :Measure ;
  skos:definition "The overall distance between the front and back of an individual vehicle, including the length of any trailers, couplings, etc. [SOURCE: CEN/TS161573:2011] "@en ;
.
:vehicleWidth
  rdf:type owl:FunctionalProperty ;
  rdf:type owl:ObjectProperty ;
  rdfs:domain :WidthCharacteristic ;
  rdfs:label "vehicleWidth"@en ;
  rdfs:range :Measure ;
  skos:definition "The maximum width of an individual vehicle, in metres. [SOURCE: CEN/TS16157-3:2011] "@en ;
.
:versionId
  rdf:type owl:DatatypeProperty ;
  rdfs:domain :Identifier ;
  rdfs:label "versionId"@en ;
  rdfs:range xsd:string ;
  skos:definition "The identifier of the particular version of the spatial object, with a maximum length of 25 characters. If the specification of a spatial object type with an external object identifier includes life-cycle information, the version identifier is used to distinguish between the different versions of a spatial object. Within the set of all versions of a spatial object, the version identifier is unique. "@en ;
.
:yearOfFirstRegistration
  rdf:type owl:DatatypeProperty ;
  rdfs:domain :VehicleCharacteristics ;
  rdfs:label "yearOfFirstRegistration"@en ;
  rdfs:range xsd:integer ;
  skos:definition "Year of first registration of the vehicle [SOURCE: DATEX 3.0 Part 7 (proposed EN 16157-7:2018)] "@en ;
.
