@prefix : <http://spec.tn-its.eu/owl/tnits-owl#> .
@prefix lr: <http://www.roadotl.eu/iso19148/def/> .
@prefix sf: <http://www.opengis.net/ont/sf#> .
@prefix gsp: <http://www.opengis.net/ont/geosparql#> .
@prefix owl: <http://www.w3.org/2002/07/owl#> .
@prefix rdf: <http://www.w3.org/1999/02/22-rdf-syntax-ns#> .
@prefix xml: <http://www.w3.org/XML/1998/namespace> .
@prefix xsd: <http://www.w3.org/2001/XMLSchema#> .
@prefix rdfs: <http://www.w3.org/2000/01/rdf-schema#> .
@prefix skos: <http://www.w3.org/2004/02/skos/core#> .
@prefix dc: <http://purl.org/dc/terms/> .

<http://spec.tn-its.eu/owl/tnits-owl> a owl:Ontology ;
	owl:imports <http://www.w3.org/2004/02/skos/core> ;
	owl:imports gsp: ;
	owl:imports lr: ;
	owl:imports <http://def.isotc211.org/iso19115/-1/2014/MetadataInformation> ;
	owl:imports <http://spec.tn-its.eu/codelists/allcodes> ;

	### GeoSPARQL rdf file: http://schemas.opengis.net/geosparql/1.0/geosparql_vocab_all.rdf
	### ISO 19148 ttl file: https://ontologi.atlas.vegvesen.no/nvdb/core/iso-19148.ttl
	### ISO 19115 rdf file: http://def.isotc211.org/iso19115/-1/2014/MetadataInformation.rdf

	dc:creator "TN-ITS" ;
	dc:date "08.06.2022" ;
	dc:description "Ontology for the TN-ITS model for exchange of changes in road attributes"@en ;
	dc:title "TN-ITS"@en ;
	dc:abstract "Ontology for exchange of changes in road attributes" .

### http://spec.tn-its.eu/owl/tnits-owl#tnits
:tnits a owl:Class ;
         owl:disjointUnionOf ( :tnitsFeature :tnitsCodeList :tnitsEnumeration :tnitsDataType ) ;
         rdfs:label "TN-ITS Root"@en .
### http://spec.tn-its.eu/owl/tnits-owl#Feature
:tnitsFeature a owl:Class ;
         rdfs:subClassOf <http://def.isotc211.org/iso19109/2015/GeneralFeatureModel#AnyFeature> ,
                          :tnits ,
                       gsp:Feature ;
         rdfs:label "TN-ITS Feature"@en .
### http://spec.tn-its.eu/owl/tnits-owl#CodeList
:tnitsCodeList a owl:Class ;
         rdfs:subClassOf :tnits, skos:Concept ;
         rdfs:label "TN-ITS Code value"@en .
### http://spec.tn-its.eu/owl/tnits-owl#Enumeration
:tnitsEnumeration a owl:Class ;
         rdfs:subClassOf :tnits, skos:Concept ;
         rdfs:label "TN-ITS Enumeration value"@en .
### http://spec.tn-its.eu/owl/tnits-owl#DataType
:tnitsDataType a owl:Class ;
         rdfs:subClassOf :tnits ;
         rdfs:label "TN-ITS Data type"@en .



### http://spec.tn-its.eu/owl/tnits-owl:Identifier
:Identifier a owl:Class ;
       rdfs:subClassOf :tnitsDataType ;
         skos:definition "External unique object identifier published by the responsible body, which may be used by external applications to reference the spatial object."@en ;
       rdfs:label "Identifier"@en .

### http://spec.tn-its.eu/owl/tnits-owl#localId
:localId rdf:type owl:DatatypeProperty ;
         skos:definition "A local identifier, assigned by the data provider. The local identifier is unique within the namespace, that is no other spatial object carries the same unique identifier. "@en ;
         rdfs:domain :Identifier;
         rdfs:range xsd:string;
         rdf:type owl:FunctionalProperty;
         rdfs:label "localId"@en .
:Identifier rdfs:subClassOf [ rdf:type owl:Restriction ;
         owl:onProperty :localId;
         owl:onDataRange xsd:string;
       owl:qualifiedCardinality "1"^^xsd:nonNegativeInteger ;
         ] .
:Identifier rdfs:subClassOf [ rdf:type owl:Restriction ;
         owl:onProperty :localId;
         owl:allValuesFrom xsd:string;
         ] .


### http://spec.tn-its.eu/owl/tnits-owl#namespace
:namespace rdf:type owl:DatatypeProperty ;
         skos:definition "Namespace uniquely identifying the data source of the spatial object."@en ;
         rdfs:domain :Identifier;
         rdfs:range xsd:string;
         rdf:type owl:FunctionalProperty;
         rdfs:label "namespace"@en .
:Identifier rdfs:subClassOf [ rdf:type owl:Restriction ;
         owl:onProperty :namespace;
         owl:onDataRange xsd:string;
       owl:qualifiedCardinality "1"^^xsd:nonNegativeInteger ;
         ] .
:Identifier rdfs:subClassOf [ rdf:type owl:Restriction ;
         owl:onProperty :namespace;
         owl:allValuesFrom xsd:string;
         ] .


### http://spec.tn-its.eu/owl/tnits-owl#versionId
:versionId rdf:type owl:DatatypeProperty ;
         skos:definition "The identifier of the particular version of the spatial object, with a maximum length of 25 characters. If the specification of a spatial object type with an external object identifier includes life-cycle information, the version identifier is used to distinguish between the different versions of a spatial object. Within the set of all versions of a spatial object, the version identifier is unique. "@en ;
         rdfs:domain :Identifier;
         rdfs:range xsd:string;
         rdfs:label "versionId"@en .
:Identifier rdfs:subClassOf [ rdf:type owl:Restriction ;
         owl:onProperty :versionId;
         owl:onDataRange xsd:string;
       owl:maxQualifiedCardinality "1"^^xsd:nonNegativeInteger ;
         ] .
:Identifier rdfs:subClassOf [ rdf:type owl:Restriction ;
         owl:onProperty :versionId;
         owl:allValuesFrom xsd:string;
         ] .



### http://spec.tn-its.eu/owl/tnits-owl:Dataset
:Dataset a owl:Class ;
       rdfs:subClassOf :tnitsFeature ;
         skos:definition "Abstract class that represents any type of dataset that may be exchanged using TN-ITS  "@en ;
       rdfs:label "Dataset"@en .

### http://spec.tn-its.eu/owl/tnits-owl#Dataset.metadata
:Dataset.metadata rdf:type owl:ObjectProperty ;
         skos:definition "Metadata for the dataset. "@en ;
         rdfs:domain :Dataset;
         rdfs:range :Metadata;
         rdfs:label "Dataset.metadata"@en .
:Dataset rdfs:subClassOf [ rdf:type owl:Restriction ;
         owl:onProperty :Dataset.metadata;
         owl:onClass :Metadata;
       owl:maxQualifiedCardinality "1"^^xsd:nonNegativeInteger ;
         ] .
:Dataset rdfs:subClassOf [ rdf:type owl:Restriction ;
         owl:onProperty :Dataset.metadata;
         owl:allValuesFrom :Metadata;
         ] .

:Dataset owl:disjointUnionOf ( :RoadFeatureDataset :FeedbackDataset  ) ; .

### http://spec.tn-its.eu/owl/tnits-owl:FeedbackDataset
:FeedbackDataset a owl:Class ;
         skos:definition "A dataset containing feedback to the road authorities/road operators from an information provider/map provider in response to data download and integration  "@en ;
       rdfs:label "FeedbackDataset"@en .
:FeedbackDataset rdfs:subClassOf :Dataset .

### http://spec.tn-its.eu/owl/tnits-owl#feedbackInfo
:feedbackInfo rdf:type owl:ObjectProperty ;
         skos:definition "The feedback information  "@en ;
         rdfs:domain :FeedbackDataset;
         rdfs:range :FeedbackInformation;
         rdf:type owl:FunctionalProperty;
         rdfs:label "feedbackInfo"@en .
:FeedbackDataset rdfs:subClassOf [ rdf:type owl:Restriction ;
         owl:onProperty :feedbackInfo;
         owl:onClass :FeedbackInformation;
       owl:qualifiedCardinality "1"^^xsd:nonNegativeInteger ;
         ] .
:FeedbackDataset rdfs:subClassOf [ rdf:type owl:Restriction ;
         owl:onProperty :feedbackInfo;
         owl:allValuesFrom :FeedbackInformation;
         ] .


### http://spec.tn-its.eu/owl/tnits-owl:RoadFeatureDataset
:RoadFeatureDataset a owl:Class ;
         skos:definition "A dataset containing road feature with optional update information.  "@en ;
       rdfs:label "RoadFeatureDataset"@en .

### http://spec.tn-its.eu/owl/tnits-owl#roadFeatures
:roadFeatures rdf:type owl:ObjectProperty ;
         skos:definition "The set of RoadFeatures contained in this dataset "@en ;
         rdfs:domain :RoadFeatureDataset;
         rdfs:range :RoadFeature;
         rdfs:label "roadFeatures"@en .
:RoadFeatureDataset rdfs:subClassOf [ rdf:type owl:Restriction ;
         owl:onProperty :roadFeatures;
         owl:onClass :RoadFeature;
       owl:minQualifiedCardinality "1"^^xsd:nonNegativeInteger ;
         ] .
:RoadFeatureDataset rdfs:subClassOf [ rdf:type owl:Restriction ;
         owl:onProperty :roadFeatures;
         owl:allValuesFrom :RoadFeature;
         ] .

:RoadFeatureDataset rdfs:subClassOf :Dataset .

### http://spec.tn-its.eu/owl/tnits-owl#RoadFeatureDataset.type
:RoadFeatureDataset.type rdf:type owl:ObjectProperty ;
         skos:definition "Specifies the type of dataset "@en ;
         rdfs:domain :RoadFeatureDataset;
         rdfs:range :DatasetType;
         rdf:type owl:FunctionalProperty;
         rdfs:label "RoadFeatureDataset.type"@en .
:RoadFeatureDataset rdfs:subClassOf [ rdf:type owl:Restriction ;
         owl:onProperty :RoadFeatureDataset.type;
         owl:onClass :DatasetType;
       owl:qualifiedCardinality "1"^^xsd:nonNegativeInteger ;
         ] .
:RoadFeatureDataset rdfs:subClassOf [ rdf:type owl:Restriction ;
         owl:onProperty :RoadFeatureDataset.type;
         owl:allValuesFrom :DatasetType;
         ] .


### http://spec.tn-its.eu/owl/tnits-owl#defaultLRM
:defaultLRM rdf:type owl:ObjectProperty ;
         skos:definition "Default linear referencing method to be used in the dataset."@en ;
         rdfs:domain :RoadFeatureDataset;
         rdfs:range <http://www.roadotl.eu/iso19148/def/LinearReferencingMethod>;
         rdfs:label "defaultLRM"@en .
:RoadFeatureDataset rdfs:subClassOf [ rdf:type owl:Restriction ;
         owl:onProperty :defaultLRM;
         owl:onClass <http://www.roadotl.eu/iso19148/def/LinearReferencingMethod>;
       owl:maxQualifiedCardinality "1"^^xsd:nonNegativeInteger ;
         ] .
:RoadFeatureDataset rdfs:subClassOf [ rdf:type owl:Restriction ;
         owl:onProperty :defaultLRM;
         owl:allValuesFrom <http://www.roadotl.eu/iso19148/def/LinearReferencingMethod>;
         ] .


### http://spec.tn-its.eu/owl/tnits-owl:DatasetType
:DatasetType a owl:Class ;
       rdfs:subClassOf :tnitsEnumeration ;
         skos:definition "Specifies the different possible types of datasets for road features  "@en ;
       rdfs:label "DatasetType"@en .

### http://spec.tn-its.eu/owl/tnits-owl:DatasetTypeCode
:DatasetTypeCode a skos:ConceptScheme ;
         skos:definition "Specifies the different possible types of datasets for road features  "@en ;
       dc:isFormatOf :DatasetType .

### http://spec.tn-its.eu/owl/tnits-owl:DatasetType.Update
:DatasetType.Update a :DatasetType,skos:Concept ;
         skos:inScheme :DatasetTypeCode ;
         skos:definition "A dataset consisting of only incremental updates for road features "@en ;
         rdfs:label "Update"@no .

### http://spec.tn-its.eu/owl/tnits-owl:DatasetType.Snapshot
:DatasetType.Snapshot a :DatasetType,skos:Concept ;
         skos:inScheme :DatasetTypeCode ;
         skos:definition "A snapshot dataset contains information (current status) of all road features in an area, or of all occurrences of one or more specified types of road features"@en ;
         rdfs:label "Snapshot"@no .
:DatasetType owl:oneOf ( :DatasetType.Update :DatasetType.Snapshot  ) ; .


### http://spec.tn-its.eu/owl/tnits-owl:AbstractRoadFeatureProperty
:AbstractRoadFeatureProperty a owl:Class ;
       rdfs:subClassOf :tnitsDataType ;
         skos:definition "An abstract generic (type independent) representation of a road feature property value "@en ;
       rdfs:label "AbstractRoadFeatureProperty"@en .
:AbstractRoadFeatureProperty owl:disjointUnionOf ( :GenericRoadFeatureProperty :RoadSignProperty  ) ; .

### http://spec.tn-its.eu/owl/tnits-owl:ChargingPointUsageType
:ChargingPointUsageType a owl:Class ;
       rdfs:subClassOf :tnitsCodeList ;
         skos:definition "Specifies the available list of enumerations for the use of electric charging point "@en ;
       rdfs:label "ChargingPointUsageType"@en .

### http://spec.tn-its.eu/owl/tnits-owl:ChargingPointUsageTypeCode
:ChargingPointUsageTypeCode a skos:ConceptScheme ;
         skos:definition "Specifies the available list of enumerations for the use of electric charging point "@en ;
       dc:isFormatOf :ChargingPointUsageType .

### http://spec.tn-its.eu/owl/tnits-owl:GasType
:GasType a owl:Class ;
       rdfs:subClassOf :tnitsCodeList ;
         skos:definition "Specifies the available list of enumerations for types of propellant gas."@en ;
       rdfs:label "GasType"@en .

### http://spec.tn-its.eu/owl/tnits-owl:GasTypeCode
:GasTypeCode a skos:ConceptScheme ;
         skos:definition "Specifies the available list of enumerations for types of propellant gas."@en ;
       dc:isFormatOf :GasType .

### http://spec.tn-its.eu/owl/tnits-owl:GenericRoadFeatureProperty
:GenericRoadFeatureProperty a owl:Class ;
         skos:definition "A representation of a road feature property value "@en ;
       rdfs:label "GenericRoadFeatureProperty"@en .
:GenericRoadFeatureProperty rdfs:subClassOf :AbstractRoadFeatureProperty .

### http://spec.tn-its.eu/owl/tnits-owl#GenericRoadFeatureProperty.type
:GenericRoadFeatureProperty.type rdf:type owl:ObjectProperty ;
         skos:definition "The type of road feature property by reference to an item in an external code list"@en ;
         rdfs:domain :GenericRoadFeatureProperty;
         rdfs:range :RoadFeaturePropertyType;
         rdf:type owl:FunctionalProperty;
         rdfs:label "GenericRoadFeatureProperty.type"@en .
:GenericRoadFeatureProperty rdfs:subClassOf [ rdf:type owl:Restriction ;
         owl:onProperty :GenericRoadFeatureProperty.type;
         owl:onClass :RoadFeaturePropertyType;
       owl:qualifiedCardinality "1"^^xsd:nonNegativeInteger ;
         ] .
:GenericRoadFeatureProperty rdfs:subClassOf [ rdf:type owl:Restriction ;
         owl:onProperty :GenericRoadFeatureProperty.type;
         owl:allValuesFrom :RoadFeaturePropertyType;
         ] .


### http://spec.tn-its.eu/owl/tnits-owl#GenericRoadFeatureProperty.value
:GenericRoadFeatureProperty.value rdf:type owl:ObjectProperty ;
         skos:definition "The value of the road feature property"@en ;
         rdfs:domain :GenericRoadFeatureProperty;
         rdfs:range :Any;
         rdfs:label "GenericRoadFeatureProperty.value"@en .
:GenericRoadFeatureProperty rdfs:subClassOf [ rdf:type owl:Restriction ;
         owl:onProperty :GenericRoadFeatureProperty.value;
         owl:allValuesFrom :Any;
         ] .


### http://spec.tn-its.eu/owl/tnits-owl#valueReference
:valueReference rdf:type owl:ObjectProperty ;
         skos:definition "A reference to an externally defined value"@en ;
         rdfs:domain :GenericRoadFeatureProperty;
         rdfs:range :PropertyValueReferenceType;
         rdfs:label "valueReference"@en .
:GenericRoadFeatureProperty rdfs:subClassOf [ rdf:type owl:Restriction ;
         owl:onProperty :valueReference;
         owl:allValuesFrom :PropertyValueReferenceType;
         ] .


### http://spec.tn-its.eu/owl/tnits-owl:NatureOfDistanceMeasure
:NatureOfDistanceMeasure a owl:Class ;
       rdfs:subClassOf :tnitsCodeList ;
         skos:definition "Specifies the available list of enumerations for contexts of forms of interpreting distance measures"@en ;
       rdfs:label "NatureOfDistanceMeasure"@en .

### http://spec.tn-its.eu/owl/tnits-owl:NatureOfDistanceMeasureCode
:NatureOfDistanceMeasureCode a skos:ConceptScheme ;
         skos:definition "Specifies the available list of enumerations for contexts of forms of interpreting distance measures"@en ;
       dc:isFormatOf :NatureOfDistanceMeasure .

### http://spec.tn-its.eu/owl/tnits-owl:ParkingSiteType
:ParkingSiteType a owl:Class ;
       rdfs:subClassOf :tnitsCodeList ;
         skos:definition "Specifies the available list of enumerations for the types of parking sites"@en ;
       rdfs:label "ParkingSiteType"@en .

### http://spec.tn-its.eu/owl/tnits-owl:ParkingSiteTypeCode
:ParkingSiteTypeCode a skos:ConceptScheme ;
         skos:definition "Specifies the available list of enumerations for the types of parking sites"@en ;
       dc:isFormatOf :ParkingSiteType .

### http://spec.tn-its.eu/owl/tnits-owl:PaymentMethod
:PaymentMethod a owl:Class ;
       rdfs:subClassOf :tnitsCodeList ;
         skos:definition "Specifies the available list of enumerations for the methods of payment"@en ;
       rdfs:label "PaymentMethod"@en .

### http://spec.tn-its.eu/owl/tnits-owl:PaymentMethodCode
:PaymentMethodCode a skos:ConceptScheme ;
         skos:definition "Specifies the available list of enumerations for the methods of payment"@en ;
       dc:isFormatOf :PaymentMethod .

### http://spec.tn-its.eu/owl/tnits-owl:PropertyValueReferenceType
:PropertyValueReferenceType a owl:Class ;
       rdfs:subClassOf :tnitsCodeList ;
         skos:definition "A list of externally defined values "@en ;
       rdfs:label "PropertyValueReferenceType"@en .

### http://spec.tn-its.eu/owl/tnits-owl:PropertyValueReferenceTypeCode
:PropertyValueReferenceTypeCode a skos:ConceptScheme ;
         skos:definition "A list of externally defined values "@en ;
       dc:isFormatOf :PropertyValueReferenceType .

### http://spec.tn-its.eu/owl/tnits-owl:RoadFeature
:RoadFeature a owl:Class ;
       rdfs:subClassOf :tnitsFeature ;
         skos:definition "The base class for any type of road feature. A road feature represents static road data, such as traffic regulations, traffic signs (like speed limits, compulsory signs and warning signs) and road infrastructure (such as charging points). Each road feature must be described by a geo-referenced by providing a point or linear location reference and can be further described by a set of conditions specifying the validity of the road feature (using combinations of conditions such as time restrictions, area, lane, vehicle type, weather, loading or road category)."@en ;
       rdfs:label "RoadFeature"@en .

### http://spec.tn-its.eu/owl/tnits-owl#roadFeatureId
:roadFeatureId rdf:type owl:ObjectProperty ;
         skos:definition "The identity for the road feature. Permanent identifier for the road feature in the database of the data provider. "@en ;
         rdfs:range :Identifier;
         rdfs:label "roadFeatureId"@en .
:RoadFeature rdfs:subClassOf [ rdf:type owl:Restriction ;
         owl:onProperty :roadFeatureId;
         owl:onClass :Identifier;
       owl:qualifiedCardinality "1"^^xsd:nonNegativeInteger ;
         ] .
:RoadFeature rdfs:subClassOf [ rdf:type owl:Restriction ;
         owl:onProperty :roadFeatureId;
         owl:allValuesFrom :Identifier;
         ] .


### http://spec.tn-its.eu/owl/tnits-owl#properties
:properties rdf:type owl:ObjectProperty ;
         skos:definition "The property values of interest for the road feature "@en ;
         rdfs:domain :RoadFeature;
         rdfs:range :AbstractRoadFeatureProperty;
         rdfs:label "properties"@en .
:RoadFeature rdfs:subClassOf [ rdf:type owl:Restriction ;
         owl:onProperty :properties;
         owl:allValuesFrom :AbstractRoadFeatureProperty;
         ] .


### http://spec.tn-its.eu/owl/tnits-owl#RoadFeature.condition
:RoadFeature.condition rdf:type owl:ObjectProperty ;
         skos:definition "Describes the circumstances when the road feature is applicable.  "@en ;
         rdfs:domain :RoadFeature;
         rdfs:range :Condition;
         rdfs:label "RoadFeature.condition"@en .
:RoadFeature rdfs:subClassOf [ rdf:type owl:Restriction ;
         owl:onProperty :RoadFeature.condition;
         owl:onClass :Condition;
       owl:maxQualifiedCardinality "1"^^xsd:nonNegativeInteger ;
         ] .
:RoadFeature rdfs:subClassOf [ rdf:type owl:Restriction ;
         owl:onProperty :RoadFeature.condition;
         owl:allValuesFrom :Condition;
         ] .


### http://spec.tn-its.eu/owl/tnits-owl#RoadFeature.locationReference
:RoadFeature.locationReference rdf:type owl:ObjectProperty ;
         skos:definition "A reference to the location of the road feature either described by either a precoded or a dynamic location referencing method  "@en ;
         rdfs:domain :RoadFeature;
         rdfs:range :LocationReference;
         rdfs:label "RoadFeature.locationReference"@en .
:RoadFeature rdfs:subClassOf [ rdf:type owl:Restriction ;
         owl:onProperty :RoadFeature.locationReference;
         owl:onClass :LocationReference;
       owl:minQualifiedCardinality "1"^^xsd:nonNegativeInteger ;
         ] .
:RoadFeature rdfs:subClassOf [ rdf:type owl:Restriction ;
         owl:onProperty :RoadFeature.locationReference;
         owl:allValuesFrom :LocationReference;
         ] .


### http://spec.tn-its.eu/owl/tnits-owl#validFrom
:validFrom rdf:type owl:DatatypeProperty ;
         skos:definition "The date from which this road feature is valid and in use "@en ;
         rdfs:domain :RoadFeature;
         rdfs:range xsd:date;
         rdf:type owl:FunctionalProperty;
         rdfs:label "validFrom"@en .
:RoadFeature rdfs:subClassOf [ rdf:type owl:Restriction ;
         owl:onProperty :validFrom;
         owl:onDataRange xsd:date;
       owl:qualifiedCardinality "1"^^xsd:nonNegativeInteger ;
         ] .
:RoadFeature rdfs:subClassOf [ rdf:type owl:Restriction ;
         owl:onProperty :validFrom;
         owl:allValuesFrom xsd:date;
         ] .


### http://spec.tn-its.eu/owl/tnits-owl#validTo
:validTo rdf:type owl:DatatypeProperty ;
         skos:definition "The date from which this road feature is no longer valid "@en ;
         rdfs:domain :RoadFeature;
         rdfs:range xsd:date;
         rdfs:label "validTo"@en .
:RoadFeature rdfs:subClassOf [ rdf:type owl:Restriction ;
         owl:onProperty :validTo;
         owl:onDataRange xsd:date;
       owl:maxQualifiedCardinality "1"^^xsd:nonNegativeInteger ;
         ] .
:RoadFeature rdfs:subClassOf [ rdf:type owl:Restriction ;
         owl:onProperty :validTo;
         owl:allValuesFrom xsd:date;
         ] .


### http://spec.tn-its.eu/owl/tnits-owl#beginLifespanVersion
:beginLifespanVersion rdf:type owl:DatatypeProperty ;
         skos:definition "Date and time at which this version of the spatial object was inserted or changed in the spatial data set. "@en ;
         rdfs:domain :RoadFeature;
         rdfs:range xsd:dateTime;
         rdf:type owl:FunctionalProperty;
         rdfs:label "beginLifespanVersion"@en .
:RoadFeature rdfs:subClassOf [ rdf:type owl:Restriction ;
         owl:onProperty :beginLifespanVersion;
         owl:onDataRange xsd:dateTime;
       owl:qualifiedCardinality "1"^^xsd:nonNegativeInteger ;
         ] .
:RoadFeature rdfs:subClassOf [ rdf:type owl:Restriction ;
         owl:onProperty :beginLifespanVersion;
         owl:allValuesFrom xsd:dateTime;
         ] .


### http://spec.tn-its.eu/owl/tnits-owl#endLifespanVersion
:endLifespanVersion rdf:type owl:DatatypeProperty ;
         skos:definition "Date and time at which this version of the spatial object was superseded or retired in the spatial data set. "@en ;
         rdfs:domain :RoadFeature;
         rdfs:range xsd:dateTime;
         rdfs:label "endLifespanVersion"@en .
:RoadFeature rdfs:subClassOf [ rdf:type owl:Restriction ;
         owl:onProperty :endLifespanVersion;
         owl:onDataRange xsd:dateTime;
       owl:maxQualifiedCardinality "1"^^xsd:nonNegativeInteger ;
         ] .
:RoadFeature rdfs:subClassOf [ rdf:type owl:Restriction ;
         owl:onProperty :endLifespanVersion;
         owl:allValuesFrom xsd:dateTime;
         ] .


### http://spec.tn-its.eu/owl/tnits-owl#RoadFeature.updateInfo
:RoadFeature.updateInfo rdf:type owl:ObjectProperty ;
         skos:definition "Specifies the necessary update information if this is a representation of an update event. "@en ;
         rdfs:domain :RoadFeature;
         rdfs:range :UpdateInfo;
         rdfs:label "RoadFeature.updateInfo"@en .
:RoadFeature rdfs:subClassOf [ rdf:type owl:Restriction ;
         owl:onProperty :RoadFeature.updateInfo;
         owl:onClass :UpdateInfo;
       owl:maxQualifiedCardinality "1"^^xsd:nonNegativeInteger ;
         ] .
:RoadFeature rdfs:subClassOf [ rdf:type owl:Restriction ;
         owl:onProperty :RoadFeature.updateInfo;
         owl:allValuesFrom :UpdateInfo;
         ] .


### http://spec.tn-its.eu/owl/tnits-owl#source
:source rdf:type owl:ObjectProperty ;
         skos:definition "Identifies the evidence base that has been used by the authorised authority supplying the data. "@en ;
         rdfs:domain :RoadFeature;
         rdfs:range :RoadFeatureSource;
         rdf:type owl:FunctionalProperty;
         rdfs:label "source"@en .
:RoadFeature rdfs:subClassOf [ rdf:type owl:Restriction ;
         owl:onProperty :source;
         owl:onClass :RoadFeatureSource;
       owl:qualifiedCardinality "1"^^xsd:nonNegativeInteger ;
         ] .
:RoadFeature rdfs:subClassOf [ rdf:type owl:Restriction ;
         owl:onProperty :source;
         owl:allValuesFrom :RoadFeatureSource;
         ] .


### http://spec.tn-its.eu/owl/tnits-owl#RoadFeature.type
:RoadFeature.type rdf:type owl:ObjectProperty ;
         skos:definition "A characterisation identifying the type of the road feature by reference to an item in an external code list "@en ;
         rdfs:domain :RoadFeature;
         rdfs:range :RoadFeatureType;
         rdf:type owl:FunctionalProperty;
         rdfs:label "RoadFeature.type"@en .
:RoadFeature rdfs:subClassOf [ rdf:type owl:Restriction ;
         owl:onProperty :RoadFeature.type;
         owl:onClass :RoadFeatureType;
       owl:qualifiedCardinality "1"^^xsd:nonNegativeInteger ;
         ] .
:RoadFeature rdfs:subClassOf [ rdf:type owl:Restriction ;
         owl:onProperty :RoadFeature.type;
         owl:allValuesFrom :RoadFeatureType;
         ] .


### http://spec.tn-its.eu/owl/tnits-owl:RoadFeaturePropertyType
:RoadFeaturePropertyType a owl:Class ;
       rdfs:subClassOf :tnitsCodeList ;
         skos:definition "Specifies the available list of enumerations for the various types of road features"@en ;
       rdfs:label "RoadFeaturePropertyType"@en .

### http://spec.tn-its.eu/owl/tnits-owl:RoadFeaturePropertyTypeCode
:RoadFeaturePropertyTypeCode a skos:ConceptScheme ;
         skos:definition "Specifies the available list of enumerations for the various types of road features"@en ;
       dc:isFormatOf :RoadFeaturePropertyType .

### http://spec.tn-its.eu/owl/tnits-owl:RoadFeatureSource
:RoadFeatureSource a owl:Class ;
       rdfs:subClassOf :tnitsCodeList ;
         skos:definition "Specifies the available list of enumerations for the various types source concerning road features"@en ;
       rdfs:label "RoadFeatureSource"@en .

### http://spec.tn-its.eu/owl/tnits-owl:RoadFeatureSourceCode
:RoadFeatureSourceCode a skos:ConceptScheme ;
         skos:definition "Specifies the available list of enumerations for the various types source concerning road features"@en ;
       dc:isFormatOf :RoadFeatureSource .

### http://spec.tn-its.eu/owl/tnits-owl:RoadFeatureType
:RoadFeatureType a owl:Class ;
       rdfs:subClassOf :tnitsCodeList ;
         skos:definition "Specifies the available list of enumerations for the various types of road features"@en ;
       rdfs:label "RoadFeatureType"@en .

### http://spec.tn-its.eu/owl/tnits-owl:RoadFeatureTypeCode
:RoadFeatureTypeCode a skos:ConceptScheme ;
         skos:definition "Specifies the available list of enumerations for the various types of road features"@en ;
       dc:isFormatOf :RoadFeatureType .

### http://spec.tn-its.eu/owl/tnits-owl:RoadSignContent
:RoadSignContent a owl:Class ;
       rdfs:subClassOf :tnitsDataType ;
         skos:definition "Defines one instance of content providing context of the semantics of a road sign "@en ;
       rdfs:label "RoadSignContent"@en .

### http://spec.tn-its.eu/owl/tnits-owl#RoadSignContent.value
:RoadSignContent.value rdf:type owl:ObjectProperty ;
         skos:definition "The value of the road sign property "@en ;
         rdfs:domain :RoadSignContent;
         rdfs:range :Measure;
         rdfs:label "RoadSignContent.value"@en .
:RoadSignContent rdfs:subClassOf [ rdf:type owl:Restriction ;
         owl:onProperty :RoadSignContent.value;
         owl:onClass :Measure;
       owl:maxQualifiedCardinality "1"^^xsd:nonNegativeInteger ;
         ] .
:RoadSignContent rdfs:subClassOf [ rdf:type owl:Restriction ;
         owl:onProperty :RoadSignContent.value;
         owl:allValuesFrom :Measure;
         ] .


### http://spec.tn-its.eu/owl/tnits-owl#RoadSignContent.text
:RoadSignContent.text rdf:type owl:DatatypeProperty ;
         skos:definition "A free-text description relevant to the specific road sign"@en ;
         rdfs:domain :RoadSignContent;
         rdfs:range xsd:string;
         rdfs:label "RoadSignContent.text"@en .
:RoadSignContent rdfs:subClassOf [ rdf:type owl:Restriction ;
         owl:onProperty :RoadSignContent.text;
         owl:onDataRange xsd:string;
       owl:maxQualifiedCardinality "1"^^xsd:nonNegativeInteger ;
         ] .
:RoadSignContent rdfs:subClassOf [ rdf:type owl:Restriction ;
         owl:onProperty :RoadSignContent.text;
         owl:allValuesFrom xsd:string;
         ] .


### http://spec.tn-its.eu/owl/tnits-owl#natureOfDistance
:natureOfDistance rdf:type owl:ObjectProperty ;
         skos:definition "Defines the semantics of a distance measure provided within the RoadSignContent"@en ;
         rdfs:domain :RoadSignContent;
         rdfs:range :NatureOfDistanceMeasure;
         rdfs:label "natureOfDistance"@en .
:RoadSignContent rdfs:subClassOf [ rdf:type owl:Restriction ;
         owl:onProperty :natureOfDistance;
         owl:onClass :NatureOfDistanceMeasure;
       owl:maxQualifiedCardinality "1"^^xsd:nonNegativeInteger ;
         ] .
:RoadSignContent rdfs:subClassOf [ rdf:type owl:Restriction ;
         owl:onProperty :natureOfDistance;
         owl:allValuesFrom :NatureOfDistanceMeasure;
         ] .


### http://spec.tn-its.eu/owl/tnits-owl:RoadSignProperty
:RoadSignProperty a owl:Class ;
         skos:definition "A representation of a road feature property value in the case of the road feature being a road sign "@en ;
       rdfs:label "RoadSignProperty"@en .
:RoadSignProperty rdfs:subClassOf :AbstractRoadFeatureProperty .

### http://spec.tn-its.eu/owl/tnits-owl#gddCode
:gddCode rdf:type owl:ObjectProperty ;
         skos:definition "The type of the road sign by reference to an item in the RoadSignType external code list "@en ;
         rdfs:domain :RoadSignProperty;
         rdfs:range :RoadSignType;
         rdf:type owl:FunctionalProperty;
         rdfs:label "gddCode"@en .
:RoadSignProperty rdfs:subClassOf [ rdf:type owl:Restriction ;
         owl:onProperty :gddCode;
         owl:onClass :RoadSignType;
       owl:qualifiedCardinality "1"^^xsd:nonNegativeInteger ;
         ] .
:RoadSignProperty rdfs:subClassOf [ rdf:type owl:Restriction ;
         owl:onProperty :gddCode;
         owl:allValuesFrom :RoadSignType;
         ] .


### http://spec.tn-its.eu/owl/tnits-owl#content
:content rdf:type owl:ObjectProperty ;
         skos:definition "Defines quantifiable content of the traffic sign "@en ;
         rdfs:domain :RoadSignProperty;
         rdfs:range :RoadSignContent;
         rdfs:label "content"@en .
:RoadSignProperty rdfs:subClassOf [ rdf:type owl:Restriction ;
         owl:onProperty :content;
         owl:allValuesFrom :RoadSignContent;
         ] .


### http://spec.tn-its.eu/owl/tnits-owl:RoadSignType
:RoadSignType a owl:Class ;
       rdfs:subClassOf :tnitsCodeList ;
         skos:definition "Specifies the available list of enumerations for the road sign types, defined in accordance with ISO 14823"@en ;
       rdfs:label "RoadSignType"@en .

### http://spec.tn-its.eu/owl/tnits-owl:RoadSignTypeCode
:RoadSignTypeCode a skos:ConceptScheme ;
         skos:definition "Specifies the available list of enumerations for the road sign types, defined in accordance with ISO 14823"@en ;
       dc:isFormatOf :RoadSignType .

### http://spec.tn-its.eu/owl/tnits-owl:SiteAccessibilityType
:SiteAccessibilityType a owl:Class ;
       rdfs:subClassOf :tnitsCodeList ;
         skos:definition "Specifies the available list of enumerations for types of site accessibility"@en ;
       rdfs:label "SiteAccessibilityType"@en .

### http://spec.tn-its.eu/owl/tnits-owl:SiteAccessibilityTypeCode
:SiteAccessibilityTypeCode a skos:ConceptScheme ;
         skos:definition "Specifies the available list of enumerations for types of site accessibility"@en ;
       dc:isFormatOf :SiteAccessibilityType .

### http://spec.tn-its.eu/owl/tnits-owl:TunnelCategory
:TunnelCategory a owl:Class ;
       rdfs:subClassOf :tnitsCodeList ;
         skos:definition "Specifies the available list of enumerations for the categories of tunnel access"@en ;
       rdfs:label "TunnelCategory"@en .

### http://spec.tn-its.eu/owl/tnits-owl:TunnelCategoryCode
:TunnelCategoryCode a skos:ConceptScheme ;
         skos:definition "Specifies the available list of enumerations for the categories of tunnel access"@en ;
       dc:isFormatOf :TunnelCategory .

### http://spec.tn-its.eu/owl/tnits-owl:UomIdentifier
:UomIdentifier a owl:Class ;
       rdfs:subClassOf :tnitsCodeList ;
         skos:definition "Specifies the available list of preferred enumerations for identifiers for units of measure"@en ;
       rdfs:label "UomIdentifier"@en .

### http://spec.tn-its.eu/owl/tnits-owl:UomIdentifierCode
:UomIdentifierCode a skos:ConceptScheme ;
         skos:definition "Specifies the available list of preferred enumerations for identifiers for units of measure"@en ;
       dc:isFormatOf :UomIdentifier .


### http://spec.tn-its.eu/owl/tnits-owl:AreaCondition
:AreaCondition a owl:Class ;
         skos:definition "Specifies area type condition applicability relating to a road feature  "@en ;
       rdfs:label "AreaCondition"@en .
:AreaCondition rdfs:subClassOf :Condition .

### http://spec.tn-its.eu/owl/tnits-owl#AreaCondition.areaType
:AreaCondition.areaType rdf:type owl:ObjectProperty ;
         skos:definition "Specifies the available list of enumerations for the area type condition for a road feature by reference to an item in an external code list "@en ;
         rdfs:domain :AreaCondition;
         rdfs:range :AreaType;
         rdf:type owl:FunctionalProperty;
         rdfs:label "AreaCondition.areaType"@en .
:AreaCondition rdfs:subClassOf [ rdf:type owl:Restriction ;
         owl:onProperty :AreaCondition.areaType;
         owl:onClass :AreaType;
       owl:qualifiedCardinality "1"^^xsd:nonNegativeInteger ;
         ] .
:AreaCondition rdfs:subClassOf [ rdf:type owl:Restriction ;
         owl:onProperty :AreaCondition.areaType;
         owl:allValuesFrom :AreaType;
         ] .


### http://spec.tn-its.eu/owl/tnits-owl:AreaType
:AreaType a owl:Class ;
       rdfs:subClassOf :tnitsCodeList ;
         skos:definition "Specifies the available list of enumerations for the area type condition for a road feature "@en ;
       rdfs:label "AreaType"@en .

### http://spec.tn-its.eu/owl/tnits-owl:AreaTypeCode
:AreaTypeCode a skos:ConceptScheme ;
         skos:definition "Specifies the available list of enumerations for the area type condition for a road feature "@en ;
       dc:isFormatOf :AreaType .

### http://spec.tn-its.eu/owl/tnits-owl:Condition
:Condition a owl:Class ;
       rdfs:subClassOf :tnitsDataType ;
         skos:definition "Abstract class that specifies a condition for the validity of a certain road feature such as time, weather conditions, vehicle type, vehicle propulsion fuel, vehicle occupancy, vehicle usage, restrictions of the vehicle driver’s licence permissions, vehicle dimensions or weight characteristics."@en ;
       rdfs:label "Condition"@en .

### http://spec.tn-its.eu/owl/tnits-owl#negate
:negate rdf:type owl:DatatypeProperty ;
         skos:definition "If set to true means that the entire condition shall be negated. Note:  A condition stating VehicleType=EmergencyVehicle and negate = true would mean all vehicles except those of type EmergencyVehicle. "@en ;
         rdfs:domain :Condition;
         rdfs:range xsd:boolean;
         rdfs:label "negate"@en .
:Condition rdfs:subClassOf [ rdf:type owl:Restriction ;
         owl:onProperty :negate;
         owl:onDataRange xsd:boolean;
       owl:maxQualifiedCardinality "1"^^xsd:nonNegativeInteger ;
         ] .
:Condition rdfs:subClassOf [ rdf:type owl:Restriction ;
         owl:onProperty :negate;
         owl:allValuesFrom xsd:boolean;
         ] .

:Condition owl:disjointUnionOf ( :TimeCondition :ConditionSet :AreaCondition :VehicleCondition :WeatherCondition :RoadCategoryCondition :LaneCondition  ) ; .

### http://spec.tn-its.eu/owl/tnits-owl:ConditionSet
:ConditionSet a owl:Class ;
         skos:definition "Groups a number of conditions into a condition set"@en ;
       rdfs:label "ConditionSet"@en .
:ConditionSet rdfs:subClassOf :Condition .

### http://spec.tn-its.eu/owl/tnits-owl#conditions
:conditions rdf:type owl:ObjectProperty ;
         skos:definition "Specifies the conditions that are present in the set "@en ;
         rdfs:domain :ConditionSet;
         rdfs:range :Condition;
         rdfs:label "conditions"@en .
:ConditionSet rdfs:subClassOf [ rdf:type owl:Restriction ;
         owl:onProperty :conditions;
         owl:onClass :Condition;
       owl:minQualifiedCardinality "1"^^xsd:nonNegativeInteger ;
         ] .
:ConditionSet rdfs:subClassOf [ rdf:type owl:Restriction ;
         owl:onProperty :conditions;
         owl:allValuesFrom :Condition;
         ] .


### http://spec.tn-its.eu/owl/tnits-owl#operator
:operator rdf:type owl:ObjectProperty ;
         skos:definition "Specifies the operator to be applied between the conditions in the set "@en ;
         rdfs:domain :ConditionSet;
         rdfs:range :ConditionOperator;
         rdf:type owl:FunctionalProperty;
         rdfs:label "operator"@en .
:ConditionSet rdfs:subClassOf [ rdf:type owl:Restriction ;
         owl:onProperty :operator;
         owl:onClass :ConditionOperator;
       owl:qualifiedCardinality "1"^^xsd:nonNegativeInteger ;
         ] .
:ConditionSet rdfs:subClassOf [ rdf:type owl:Restriction ;
         owl:onProperty :operator;
         owl:allValuesFrom :ConditionOperator;
         ] .


### http://spec.tn-its.eu/owl/tnits-owl:LaneCondition
:LaneCondition a owl:Class ;
         skos:definition "Specifies the applicability of a condition to specific lanes "@en ;
       rdfs:label "LaneCondition"@en .
:LaneCondition rdfs:subClassOf :Condition .

### http://spec.tn-its.eu/owl/tnits-owl#startLane
:startLane rdf:type owl:DatatypeProperty ;
         skos:definition "Start lane counted from the right side for which the condition applies. NOTE \"Right side\" is to be interpreted in relation to the direction of the location reference.  Numbering starts from 1.  All lanes should be considered, e.g. including emergency lanes, special purpose lanes, etc. "@en ;
         rdfs:domain :LaneCondition;
         rdfs:range xsd:integer;
         rdf:type owl:FunctionalProperty;
         rdfs:label "startLane"@en .
:LaneCondition rdfs:subClassOf [ rdf:type owl:Restriction ;
         owl:onProperty :startLane;
         owl:onDataRange xsd:integer;
       owl:qualifiedCardinality "1"^^xsd:nonNegativeInteger ;
         ] .
:LaneCondition rdfs:subClassOf [ rdf:type owl:Restriction ;
         owl:onProperty :startLane;
         owl:allValuesFrom xsd:integer;
         ] .


### http://spec.tn-its.eu/owl/tnits-owl#laneExtension
:laneExtension rdf:type owl:DatatypeProperty ;
         skos:definition "Number of lanes including the start lane counted from the right-hand side for which the condition applies. "@en ;
         rdfs:domain :LaneCondition;
         rdfs:range xsd:integer;
         rdf:type owl:FunctionalProperty;
         rdfs:label "laneExtension"@en .
:LaneCondition rdfs:subClassOf [ rdf:type owl:Restriction ;
         owl:onProperty :laneExtension;
         owl:onDataRange xsd:integer;
       owl:qualifiedCardinality "1"^^xsd:nonNegativeInteger ;
         ] .
:LaneCondition rdfs:subClassOf [ rdf:type owl:Restriction ;
         owl:onProperty :laneExtension;
         owl:allValuesFrom xsd:integer;
         ] .


### http://spec.tn-its.eu/owl/tnits-owl:RoadCategory
:RoadCategory a owl:Class ;
       rdfs:subClassOf :tnitsCodeList ;
         skos:definition "Specifies the available list of enumerations for the road category types"@en ;
       rdfs:label "RoadCategory"@en .

### http://spec.tn-its.eu/owl/tnits-owl:RoadCategoryCode
:RoadCategoryCode a skos:ConceptScheme ;
         skos:definition "Specifies the available list of enumerations for the road category types"@en ;
       dc:isFormatOf :RoadCategory .

### http://spec.tn-its.eu/owl/tnits-owl:RoadCategoryCondition
:RoadCategoryCondition a owl:Class ;
         skos:definition "Specifies road category condition applicability relating to a road feature "@en ;
       rdfs:label "RoadCategoryCondition"@en .
:RoadCategoryCondition rdfs:subClassOf :Condition .

### http://spec.tn-its.eu/owl/tnits-owl#RoadCategoryCondition.roadCategory
:RoadCategoryCondition.roadCategory rdf:type owl:ObjectProperty ;
         skos:definition "Specifies the available list of enumerations for the category of road for a road feature by reference to an item in an external code list "@en ;
         rdfs:domain :RoadCategoryCondition;
         rdfs:range :RoadCategory;
         rdf:type owl:FunctionalProperty;
         rdfs:label "RoadCategoryCondition.roadCategory"@en .
:RoadCategoryCondition rdfs:subClassOf [ rdf:type owl:Restriction ;
         owl:onProperty :RoadCategoryCondition.roadCategory;
         owl:onClass :RoadCategory;
       owl:qualifiedCardinality "1"^^xsd:nonNegativeInteger ;
         ] .
:RoadCategoryCondition rdfs:subClassOf [ rdf:type owl:Restriction ;
         owl:onProperty :RoadCategoryCondition.roadCategory;
         owl:allValuesFrom :RoadCategory;
         ] .


### http://spec.tn-its.eu/owl/tnits-owl:TimeCondition
:TimeCondition a owl:Class ;
         skos:definition "Specifies timing applicability relating to a road feature  "@en ;
       rdfs:label "TimeCondition"@en .
:TimeCondition rdfs:subClassOf :Condition .

### http://spec.tn-its.eu/owl/tnits-owl#validityPeriod
:validityPeriod rdf:type owl:ObjectProperty ;
         skos:definition "Specifies the time period for which this time condition applies "@en ;
         rdfs:domain :TimeCondition;
         rdfs:range :Validity;
         rdf:type owl:FunctionalProperty;
         rdfs:label "validityPeriod"@en .
:TimeCondition rdfs:subClassOf [ rdf:type owl:Restriction ;
         owl:onProperty :validityPeriod;
         owl:onClass :Validity;
       owl:qualifiedCardinality "1"^^xsd:nonNegativeInteger ;
         ] .
:TimeCondition rdfs:subClassOf [ rdf:type owl:Restriction ;
         owl:onProperty :validityPeriod;
         owl:allValuesFrom :Validity;
         ] .


### http://spec.tn-its.eu/owl/tnits-owl:VehicleCondition
:VehicleCondition a owl:Class ;
         skos:definition "Specifies vehicle type condition applicability relating to a road feature  "@en ;
       rdfs:label "VehicleCondition"@en .
:VehicleCondition rdfs:subClassOf :Condition .

### http://spec.tn-its.eu/owl/tnits-owl#VehicleCondition.vehicleCharacteristics
:VehicleCondition.vehicleCharacteristics rdf:type owl:ObjectProperty ;
         skos:definition "Specifies the vehicle characteristics that are applicable to the vehicle type condition for a road feature "@en ;
         rdfs:domain :VehicleCondition;
         rdfs:range :VehicleCharacteristics;
         rdf:type owl:FunctionalProperty;
         rdfs:label "VehicleCondition.vehicleCharacteristics"@en .
:VehicleCondition rdfs:subClassOf [ rdf:type owl:Restriction ;
         owl:onProperty :VehicleCondition.vehicleCharacteristics;
         owl:onClass :VehicleCharacteristics;
       owl:qualifiedCardinality "1"^^xsd:nonNegativeInteger ;
         ] .
:VehicleCondition rdfs:subClassOf [ rdf:type owl:Restriction ;
         owl:onProperty :VehicleCondition.vehicleCharacteristics;
         owl:allValuesFrom :VehicleCharacteristics;
         ] .


### http://spec.tn-its.eu/owl/tnits-owl:WeatherCondition
:WeatherCondition a owl:Class ;
         skos:definition "Specifies weather type condition applicability relating to a road feature  "@en ;
       rdfs:label "WeatherCondition"@en .
:WeatherCondition rdfs:subClassOf :Condition .

### http://spec.tn-its.eu/owl/tnits-owl#WeatherCondition.weatherType
:WeatherCondition.weatherType rdf:type owl:ObjectProperty ;
         skos:definition "Specifies the available list of enumerations for the weather type condition for a road feature by reference to an item in an external code list "@en ;
         rdfs:domain :WeatherCondition;
         rdfs:range :WeatherType;
         rdf:type owl:FunctionalProperty;
         rdfs:label "WeatherCondition.weatherType"@en .
:WeatherCondition rdfs:subClassOf [ rdf:type owl:Restriction ;
         owl:onProperty :WeatherCondition.weatherType;
         owl:onClass :WeatherType;
       owl:qualifiedCardinality "1"^^xsd:nonNegativeInteger ;
         ] .
:WeatherCondition rdfs:subClassOf [ rdf:type owl:Restriction ;
         owl:onProperty :WeatherCondition.weatherType;
         owl:allValuesFrom :WeatherType;
         ] .


### http://spec.tn-its.eu/owl/tnits-owl:WeatherType
:WeatherType a owl:Class ;
       rdfs:subClassOf :tnitsCodeList ;
         skos:definition "Types of weather conditions which affect driving conditions."@en ;
       rdfs:label "WeatherType"@en .

### http://spec.tn-its.eu/owl/tnits-owl:WeatherTypeCode
:WeatherTypeCode a skos:ConceptScheme ;
         skos:definition "Types of weather conditions which affect driving conditions."@en ;
       dc:isFormatOf :WeatherType .

### http://spec.tn-its.eu/owl/tnits-owl:ConditionOperator
:ConditionOperator a owl:Class ;
       rdfs:subClassOf :tnitsEnumeration ;
         skos:definition "The logical operator to be used in a comparison operation."@en ;
       rdfs:label "ConditionOperator"@en .

### http://spec.tn-its.eu/owl/tnits-owl:ConditionOperatorCode
:ConditionOperatorCode a skos:ConceptScheme ;
         skos:definition "The logical operator to be used in a comparison operation."@en ;
       dc:isFormatOf :ConditionOperator .

### http://spec.tn-its.eu/owl/tnits-owl:ConditionOperator.OR
:ConditionOperator.OR a :ConditionOperator,skos:Concept ;
         skos:inScheme :ConditionOperatorCode ;
         skos:definition "The OR logical operator – a logical operation to determine if any conditions in a test are TRUE "@en ;
         rdfs:label "OR"@no .

### http://spec.tn-its.eu/owl/tnits-owl:ConditionOperator.XOR
:ConditionOperator.XOR a :ConditionOperator,skos:Concept ;
         skos:inScheme :ConditionOperatorCode ;
         skos:definition "The XOR logical operator - a logical operation that outputs true only when inputs differ (one is true, the other is false). "@en ;
         rdfs:label "XOR"@no .

### http://spec.tn-its.eu/owl/tnits-owl:ConditionOperator.AND
:ConditionOperator.AND a :ConditionOperator,skos:Concept ;
         skos:inScheme :ConditionOperatorCode ;
         skos:definition "The AND logical operator – a logical operation to determine if all conditions in a test are TRUE "@en ;
         rdfs:label "AND"@no .
:ConditionOperator owl:oneOf ( :ConditionOperator.OR :ConditionOperator.XOR :ConditionOperator.AND  ) ; .


### http://spec.tn-its.eu/owl/tnits-owl:FuzzyTimeType
:FuzzyTimeType a owl:Class ;
       rdfs:subClassOf :tnitsCodeList ;
         skos:definition "Specifies the available list of enumerations for the fuzzy time concepts, which provided the definition of start, end or duration time concepts that support the expression of a non-precise or variable qualified concept, resulting in a non-precise, potentially circumstantial defined time period.  Note: Example roads closed at the start of winter in mountainous areas, which is based on actual experienced weather conditions and therefore is not pre-defined.  "@en ;
       rdfs:label "FuzzyTimeType"@en .

### http://spec.tn-its.eu/owl/tnits-owl:FuzzyTimeTypeCode
:FuzzyTimeTypeCode a skos:ConceptScheme ;
         skos:definition "Specifies the available list of enumerations for the fuzzy time concepts, which provided the definition of start, end or duration time concepts that support the expression of a non-precise or variable qualified concept, resulting in a non-precise, potentially circumstantial defined time period.  Note: Example roads closed at the start of winter in mountainous areas, which is based on actual experienced weather conditions and therefore is not pre-defined.  "@en ;
       dc:isFormatOf :FuzzyTimeType .

### http://spec.tn-its.eu/owl/tnits-owl:OverallPeriod
:OverallPeriod a owl:Class ;
       rdfs:subClassOf :tnitsDataType ;
         skos:definition "A continuous or discontinuous period of validity defined by overall bounding start and end times and the possible intersection of valid periods (potentially recurring) with the complement of exception periods (also potentially recurring). [SOURCE: CEN/TS16157-3:2011]"@en ;
       rdfs:label "OverallPeriod"@en .

### http://spec.tn-its.eu/owl/tnits-owl#exceptionPeriod
:exceptionPeriod rdf:type owl:ObjectProperty ;
         skos:definition "A single time period, a recurring time period or a set of different recurring time periods during which validity is false. [SOURCE: CEN/TS16157-3:2011] "@en ;
         rdfs:domain :OverallPeriod;
         rdfs:range :Period;
         rdfs:label "exceptionPeriod"@en .
:OverallPeriod rdfs:subClassOf [ rdf:type owl:Restriction ;
         owl:onProperty :exceptionPeriod;
         owl:allValuesFrom :Period;
         ] .


### http://spec.tn-its.eu/owl/tnits-owl#validPeriod
:validPeriod rdf:type owl:ObjectProperty ;
         skos:definition "A single time period, a recurring time period or a set of different recurring time periods during which validity is true. [SOURCE: CEN/TS16157-3:2011] "@en ;
         rdfs:domain :OverallPeriod;
         rdfs:range :Period;
         rdfs:label "validPeriod"@en .
:OverallPeriod rdfs:subClassOf [ rdf:type owl:Restriction ;
         owl:onProperty :validPeriod;
         owl:allValuesFrom :Period;
         ] .


### http://spec.tn-its.eu/owl/tnits-owl#overallStartTime
:overallStartTime rdf:type owl:DatatypeProperty ;
         skos:definition "Start of bounding period of validity defined by date and time. [SOURCE: CEN/TS16157-3:2011] "@en ;
         rdfs:domain :OverallPeriod;
         rdfs:range xsd:dateTime;
         rdf:type owl:FunctionalProperty;
         rdfs:label "overallStartTime"@en .
:OverallPeriod rdfs:subClassOf [ rdf:type owl:Restriction ;
         owl:onProperty :overallStartTime;
         owl:onDataRange xsd:dateTime;
       owl:qualifiedCardinality "1"^^xsd:nonNegativeInteger ;
         ] .
:OverallPeriod rdfs:subClassOf [ rdf:type owl:Restriction ;
         owl:onProperty :overallStartTime;
         owl:allValuesFrom xsd:dateTime;
         ] .


### http://spec.tn-its.eu/owl/tnits-owl#overallEndTime
:overallEndTime rdf:type owl:DatatypeProperty ;
         skos:definition "End of bounding period of validity defined by date and time. [SOURCE: CEN/TS16157-3:2011] If not present the overall period is considered to continue indefinitely into the future. "@en ;
         rdfs:domain :OverallPeriod;
         rdfs:range xsd:dateTime;
         rdfs:label "overallEndTime"@en .
:OverallPeriod rdfs:subClassOf [ rdf:type owl:Restriction ;
         owl:onProperty :overallEndTime;
         owl:onDataRange xsd:dateTime;
       owl:maxQualifiedCardinality "1"^^xsd:nonNegativeInteger ;
         ] .
:OverallPeriod rdfs:subClassOf [ rdf:type owl:Restriction ;
         owl:onProperty :overallEndTime;
         owl:allValuesFrom xsd:dateTime;
         ] .


### http://spec.tn-its.eu/owl/tnits-owl:Period
:Period a owl:Class ;
       rdfs:subClassOf :tnitsDataType ;
         skos:definition "A continuous time period or a set of discontinuous time periods defined by the intersection of a set of criteria all within an overall delimiting interval.  [SOURCE: CEN/TS16157-3:2011]"@en ;
       rdfs:label "Period"@en .

### http://spec.tn-its.eu/owl/tnits-owl#recurringSpecialDay
:recurringSpecialDay rdf:type owl:ObjectProperty ;
         skos:definition "A recurring period of a special type of day, possibly also a public holiday. Can be country or region specific. [SOURCE: DATEX 3.0 Part 7 (proposed EN 16157-7:2018)] "@en ;
         rdfs:domain :Period;
         rdfs:range :SpecialDay;
         rdfs:label "recurringSpecialDay"@en .
:Period rdfs:subClassOf [ rdf:type owl:Restriction ;
         owl:onProperty :recurringSpecialDay;
         owl:allValuesFrom :SpecialDay;
         ] .


### http://spec.tn-its.eu/owl/tnits-owl#recurringDayWeekMonthPeriod
:recurringDayWeekMonthPeriod rdf:type owl:ObjectProperty ;
         skos:definition "Specification of periods defined by the intersection of days, weeks and months. [SOURCE: CEN/TS16157-3:2011] "@en ;
         rdfs:domain :Period;
         rdfs:range :DayWeekMonth;
         rdfs:label "recurringDayWeekMonthPeriod"@en .
:Period rdfs:subClassOf [ rdf:type owl:Restriction ;
         owl:onProperty :recurringDayWeekMonthPeriod;
         owl:allValuesFrom :DayWeekMonth;
         ] .


### http://spec.tn-its.eu/owl/tnits-owl#recurringFuzzyTimePeriod
:recurringFuzzyTimePeriod rdf:type owl:ObjectProperty ;
         skos:definition "defines a time period whose start, end or duration is based upon a non-precise or variable qualified concept, resulting in a non-precise, potentially circumstantial defined time period"@en ;
         rdfs:domain :Period;
         rdfs:range :FuzzyTimePeriod;
         rdfs:label "recurringFuzzyTimePeriod"@en .
:Period rdfs:subClassOf [ rdf:type owl:Restriction ;
         owl:onProperty :recurringFuzzyTimePeriod;
         owl:allValuesFrom :FuzzyTimePeriod;
         ] .


### http://spec.tn-its.eu/owl/tnits-owl#recurringTimePeriodOfDay
:recurringTimePeriodOfDay rdf:type owl:ObjectProperty ;
         skos:definition "A recurring period of a day. [SOURCE: CEN/TS16157-3:2011] "@en ;
         rdfs:domain :Period;
         rdfs:range :TimePeriodOfDay;
         rdfs:label "recurringTimePeriodOfDay"@en .
:Period rdfs:subClassOf [ rdf:type owl:Restriction ;
         owl:onProperty :recurringTimePeriodOfDay;
         owl:allValuesFrom :TimePeriodOfDay;
         ] .


### http://spec.tn-its.eu/owl/tnits-owl#startOfPeriod
:startOfPeriod rdf:type owl:DatatypeProperty ;
         skos:definition "Start of period. [SOURCE: CEN/TS16157-3:2011]  Specifies the start date and time of this period. If not present, the start of the period is considered to be continuously on-going from an undefined date in the past. "@en ;
         rdfs:domain :Period;
         rdfs:range xsd:dateTime;
         rdfs:label "startOfPeriod"@en .
:Period rdfs:subClassOf [ rdf:type owl:Restriction ;
         owl:onProperty :startOfPeriod;
         owl:onDataRange xsd:dateTime;
       owl:maxQualifiedCardinality "1"^^xsd:nonNegativeInteger ;
         ] .
:Period rdfs:subClassOf [ rdf:type owl:Restriction ;
         owl:onProperty :startOfPeriod;
         owl:allValuesFrom xsd:dateTime;
         ] .


### http://spec.tn-its.eu/owl/tnits-owl#endOfPeriod
:endOfPeriod rdf:type owl:DatatypeProperty ;
         skos:definition "End of a period. [SOURCE: CEN/TS16157-3:2011]  Specifies the end date and time of this period. If not present, the end of the period is considered to be continuously on-going to an undefined date in the future."@en ;
         rdfs:domain :Period;
         rdfs:range xsd:dateTime;
         rdfs:label "endOfPeriod"@en .
:Period rdfs:subClassOf [ rdf:type owl:Restriction ;
         owl:onProperty :endOfPeriod;
         owl:onDataRange xsd:dateTime;
       owl:maxQualifiedCardinality "1"^^xsd:nonNegativeInteger ;
         ] .
:Period rdfs:subClassOf [ rdf:type owl:Restriction ;
         owl:onProperty :endOfPeriod;
         owl:allValuesFrom xsd:dateTime;
         ] .


### http://spec.tn-its.eu/owl/tnits-owl#periodName
:periodName rdf:type owl:DatatypeProperty ;
         skos:definition "The name of the period. [SOURCE: CEN/TS16157-3:2011] "@en ;
         rdfs:domain :Period;
         rdfs:range xsd:string;
         rdfs:label "periodName"@en .
:Period rdfs:subClassOf [ rdf:type owl:Restriction ;
         owl:onProperty :periodName;
         owl:onDataRange xsd:string;
       owl:maxQualifiedCardinality "1"^^xsd:nonNegativeInteger ;
         ] .
:Period rdfs:subClassOf [ rdf:type owl:Restriction ;
         owl:onProperty :periodName;
         owl:allValuesFrom xsd:string;
         ] .


### http://spec.tn-its.eu/owl/tnits-owl:SpecialDay
:SpecialDay a owl:Class ;
       rdfs:subClassOf :tnitsDataType ;
         skos:definition "Specification of a special type of day, possibly also a public holiday. Can be country or region specific. [SOURCE: DATEX 3.0 Part 7 (proposed EN 161577:2018)] "@en ;
       rdfs:label "SpecialDay"@en .

### http://spec.tn-its.eu/owl/tnits-owl#intersectWithApplicableDays
:intersectWithApplicableDays rdf:type owl:DatatypeProperty ;
         skos:definition "When true, the period is the intersection of applicable days and this special day. When false, the period is the union of applicable days and this special day. [SOURCE: DATEX 3.0 Part 7 (proposed EN 16157-7:2018)] "@en ;
         rdfs:domain :SpecialDay;
         rdfs:range xsd:boolean;
         rdf:type owl:FunctionalProperty;
         rdfs:label "intersectWithApplicableDays"@en .
:SpecialDay rdfs:subClassOf [ rdf:type owl:Restriction ;
         owl:onProperty :intersectWithApplicableDays;
         owl:onDataRange xsd:boolean;
       owl:qualifiedCardinality "1"^^xsd:nonNegativeInteger ;
         ] .
:SpecialDay rdfs:subClassOf [ rdf:type owl:Restriction ;
         owl:onProperty :intersectWithApplicableDays;
         owl:allValuesFrom xsd:boolean;
         ] .


### http://spec.tn-its.eu/owl/tnits-owl#SpecialDay.specialDayType
:SpecialDay.specialDayType rdf:type owl:ObjectProperty ;
         skos:definition "Specification of a special day, for example schoolDay, publicHoliday, ... [SOURCE: DATEX 3.0 Part 7 (proposed EN 16157-7:2018)] "@en ;
         rdfs:domain :SpecialDay;
         rdfs:range :SpecialDayType;
         rdf:type owl:FunctionalProperty;
         rdfs:label "SpecialDay.specialDayType"@en .
:SpecialDay rdfs:subClassOf [ rdf:type owl:Restriction ;
         owl:onProperty :SpecialDay.specialDayType;
         owl:onClass :SpecialDayType;
       owl:qualifiedCardinality "1"^^xsd:nonNegativeInteger ;
         ] .
:SpecialDay rdfs:subClassOf [ rdf:type owl:Restriction ;
         owl:onProperty :SpecialDay.specialDayType;
         owl:allValuesFrom :SpecialDayType;
         ] .


### http://spec.tn-its.eu/owl/tnits-owl#publicEvent
:publicEvent rdf:type owl:DatatypeProperty ;
         skos:definition "Type of public event on this special day. [SOURCE: DATEX 3.0 Part 7 (proposed EN 16157-7:2018)] "@en ;
         rdfs:domain :SpecialDay;
         rdfs:range xsd:string;
         rdfs:label "publicEvent"@en .
:SpecialDay rdfs:subClassOf [ rdf:type owl:Restriction ;
         owl:onProperty :publicEvent;
         owl:onDataRange xsd:string;
       owl:maxQualifiedCardinality "1"^^xsd:nonNegativeInteger ;
         ] .
:SpecialDay rdfs:subClassOf [ rdf:type owl:Restriction ;
         owl:onProperty :publicEvent;
         owl:allValuesFrom xsd:string;
         ] .

:SpecialDay owl:disjointUnionOf ( :PublicHoliday  ) ; .

### http://spec.tn-its.eu/owl/tnits-owl:SpecialDayType
:SpecialDayType a owl:Class ;
       rdfs:subClassOf :tnitsCodeList ;
         skos:definition "Specifies the available list of enumerations for the special days"@en ;
       rdfs:label "SpecialDayType"@en .

### http://spec.tn-its.eu/owl/tnits-owl:SpecialDayTypeCode
:SpecialDayTypeCode a skos:ConceptScheme ;
         skos:definition "Specifies the available list of enumerations for the special days"@en ;
       dc:isFormatOf :SpecialDayType .

### http://spec.tn-its.eu/owl/tnits-owl:TimePeriodOfDay
:TimePeriodOfDay a owl:Class ;
       rdfs:subClassOf :tnitsDataType ;
         skos:definition "Specification of a continuous period of time within a 24 hour period. [SOURCE: CEN/TS16157-3:2011] "@en ;
       rdfs:label "TimePeriodOfDay"@en .

### http://spec.tn-its.eu/owl/tnits-owl#startTimeOfPeriod
:startTimeOfPeriod rdf:type owl:ObjectProperty ;
         skos:definition "Start of time period. [SOURCE: CEN/TS16157-3:2011] "@en ;
         rdfs:domain :TimePeriodOfDay;
         rdfs:range :Time;
         rdf:type owl:FunctionalProperty;
         rdfs:label "startTimeOfPeriod"@en .
:TimePeriodOfDay rdfs:subClassOf [ rdf:type owl:Restriction ;
         owl:onProperty :startTimeOfPeriod;
         owl:onClass :Time;
       owl:qualifiedCardinality "1"^^xsd:nonNegativeInteger ;
         ] .
:TimePeriodOfDay rdfs:subClassOf [ rdf:type owl:Restriction ;
         owl:onProperty :startTimeOfPeriod;
         owl:allValuesFrom :Time;
         ] .


### http://spec.tn-its.eu/owl/tnits-owl#endTimeOfPeriod
:endTimeOfPeriod rdf:type owl:ObjectProperty ;
         skos:definition "End of time period. [SOURCE: CEN/TS16157-3:2011] "@en ;
         rdfs:domain :TimePeriodOfDay;
         rdfs:range :Time;
         rdf:type owl:FunctionalProperty;
         rdfs:label "endTimeOfPeriod"@en .
:TimePeriodOfDay rdfs:subClassOf [ rdf:type owl:Restriction ;
         owl:onProperty :endTimeOfPeriod;
         owl:onClass :Time;
       owl:qualifiedCardinality "1"^^xsd:nonNegativeInteger ;
         ] .
:TimePeriodOfDay rdfs:subClassOf [ rdf:type owl:Restriction ;
         owl:onProperty :endTimeOfPeriod;
         owl:allValuesFrom :Time;
         ] .


### http://spec.tn-its.eu/owl/tnits-owl:Validity
:Validity a owl:Class ;
       rdfs:subClassOf :tnitsDataType ;
         skos:definition "Specifies the periods of validity that relate to a road feature  "@en ;
       rdfs:label "Validity"@en .

### http://spec.tn-its.eu/owl/tnits-owl#validityTimeSpecification
:validityTimeSpecification rdf:type owl:ObjectProperty ;
         skos:definition "A specification of periods of validity defined by overall bounding start and end times and the possible intersection of valid periods with exception periods (exception periods overriding valid periods). [SOURCE: CEN/TS161573:2011] "@en ;
         rdfs:domain :Validity;
         rdfs:range :OverallPeriod;
         rdf:type owl:FunctionalProperty;
         rdfs:label "validityTimeSpecification"@en .
:Validity rdfs:subClassOf [ rdf:type owl:Restriction ;
         owl:onProperty :validityTimeSpecification;
         owl:onClass :OverallPeriod;
       owl:qualifiedCardinality "1"^^xsd:nonNegativeInteger ;
         ] .
:Validity rdfs:subClassOf [ rdf:type owl:Restriction ;
         owl:onProperty :validityTimeSpecification;
         owl:allValuesFrom :OverallPeriod;
         ] .


### http://spec.tn-its.eu/owl/tnits-owl:FuzzyTimePeriod
:FuzzyTimePeriod a owl:Class ;
       rdfs:subClassOf :tnitsDataType ;
         skos:definition "Specifies the time period with non-precise characteristics  "@en ;
       rdfs:label "FuzzyTimePeriod"@en .

### http://spec.tn-its.eu/owl/tnits-owl#beginOrDuration
:beginOrDuration rdf:type owl:ObjectProperty ;
         skos:definition "Time period begins with a fuzzy time or the duration is a fuzzy time "@en ;
         rdfs:domain :FuzzyTimePeriod;
         rdfs:range :FuzzyTimeType;
         rdf:type owl:FunctionalProperty;
         rdfs:label "beginOrDuration"@en .
:FuzzyTimePeriod rdfs:subClassOf [ rdf:type owl:Restriction ;
         owl:onProperty :beginOrDuration;
         owl:onClass :FuzzyTimeType;
       owl:qualifiedCardinality "1"^^xsd:nonNegativeInteger ;
         ] .
:FuzzyTimePeriod rdfs:subClassOf [ rdf:type owl:Restriction ;
         owl:onProperty :beginOrDuration;
         owl:allValuesFrom :FuzzyTimeType;
         ] .


### http://spec.tn-its.eu/owl/tnits-owl#endOrDuration
:endOrDuration rdf:type owl:ObjectProperty ;
         skos:definition "time period ends with a fuzzy time or the duration is a fuzzy time."@en ;
         rdfs:domain :FuzzyTimePeriod;
         rdfs:range :FuzzyTimeType;
         rdfs:label "endOrDuration"@en .
:FuzzyTimePeriod rdfs:subClassOf [ rdf:type owl:Restriction ;
         owl:onProperty :endOrDuration;
         owl:onClass :FuzzyTimeType;
       owl:maxQualifiedCardinality "1"^^xsd:nonNegativeInteger ;
         ] .
:FuzzyTimePeriod rdfs:subClassOf [ rdf:type owl:Restriction ;
         owl:onProperty :endOrDuration;
         owl:allValuesFrom :FuzzyTimeType;
         ] .


### http://spec.tn-its.eu/owl/tnits-owl:DayWeekMonth
:DayWeekMonth a owl:Class ;
       rdfs:subClassOf :tnitsDataType ;
         skos:definition "A recurring period defined in terms of days of the week, weeks of the month and months of the year. [SOURCE: CEN/TS16157-3:2011]"@en ;
       rdfs:label "DayWeekMonth"@en .

### http://spec.tn-its.eu/owl/tnits-owl#applicableDay
:applicableDay rdf:type owl:ObjectProperty ;
         skos:definition "Applicable day of the week. \"All days of the week\" is expressed by noninclusion of this attribute. [SOURCE: CEN/TS16157-3:2011]"@en ;
         rdfs:domain :DayWeekMonth;
         rdfs:range :DayOfWeek;
         rdfs:label "applicableDay"@en .
:DayWeekMonth rdfs:subClassOf [ rdf:type owl:Restriction ;
         owl:onProperty :applicableDay;
         owl:onClass :DayOfWeek;
       owl:maxQualifiedCardinality "7"^^xsd:nonNegativeInteger ;
         ] .
:DayWeekMonth rdfs:subClassOf [ rdf:type owl:Restriction ;
         owl:onProperty :applicableDay;
         owl:allValuesFrom :DayOfWeek;
         ] .


### http://spec.tn-its.eu/owl/tnits-owl#applicableWeek
:applicableWeek rdf:type owl:ObjectProperty ;
         skos:definition "Applicable week of the month (1 to 5). \"All weeks of the month\" is expressed by non-inclusion of this attribute.  [SOURCE: CEN/TS16157-3:2011]"@en ;
         rdfs:domain :DayWeekMonth;
         rdfs:range :WeekOfMonth;
         rdfs:label "applicableWeek"@en .
:DayWeekMonth rdfs:subClassOf [ rdf:type owl:Restriction ;
         owl:onProperty :applicableWeek;
         owl:onClass :WeekOfMonth;
       owl:maxQualifiedCardinality "5"^^xsd:nonNegativeInteger ;
         ] .
:DayWeekMonth rdfs:subClassOf [ rdf:type owl:Restriction ;
         owl:onProperty :applicableWeek;
         owl:allValuesFrom :WeekOfMonth;
         ] .


### http://spec.tn-its.eu/owl/tnits-owl#applicableMonth
:applicableMonth rdf:type owl:ObjectProperty ;
         skos:definition "Applicable month of the year.  \"All months of the year\" is expressed by noninclusion of this attribute. [SOURCE: CEN/TS16157-3:2011]"@en ;
         rdfs:domain :DayWeekMonth;
         rdfs:range :MonthOfYear;
         rdfs:label "applicableMonth"@en .
:DayWeekMonth rdfs:subClassOf [ rdf:type owl:Restriction ;
         owl:onProperty :applicableMonth;
         owl:onClass :MonthOfYear;
       owl:maxQualifiedCardinality "12"^^xsd:nonNegativeInteger ;
         ] .
:DayWeekMonth rdfs:subClassOf [ rdf:type owl:Restriction ;
         owl:onProperty :applicableMonth;
         owl:allValuesFrom :MonthOfYear;
         ] .


### http://spec.tn-its.eu/owl/tnits-owl:PublicHoliday
:PublicHoliday a owl:Class ;
         skos:definition "Specification of a specific public holiday in case specialDayType is set to 'publicHoliday'. [SOURCE: DATEX 3.0 Part 7 (proposed EN 16157-7:2018)] "@en ;
       rdfs:label "PublicHoliday"@en .
:PublicHoliday rdfs:subClassOf :SpecialDay .

### http://spec.tn-its.eu/owl/tnits-owl#publicHolidayName
:publicHolidayName rdf:type owl:DatatypeProperty ;
         skos:definition "Specification of a specific public holiday by its name. [SOURCE: DATEX 3.0 Part 7 (proposed EN 16157-7:2018)] "@en ;
         rdfs:domain :PublicHoliday;
         rdfs:range xsd:string;
         rdf:type owl:FunctionalProperty;
         rdfs:label "publicHolidayName"@en .
:PublicHoliday rdfs:subClassOf [ rdf:type owl:Restriction ;
         owl:onProperty :publicHolidayName;
         owl:onDataRange xsd:string;
       owl:qualifiedCardinality "1"^^xsd:nonNegativeInteger ;
         ] .
:PublicHoliday rdfs:subClassOf [ rdf:type owl:Restriction ;
         owl:onProperty :publicHolidayName;
         owl:allValuesFrom xsd:string;
         ] .


### http://spec.tn-its.eu/owl/tnits-owl:DayOfWeek
:DayOfWeek a owl:Class ;
       rdfs:subClassOf :tnitsEnumeration ;
         skos:definition "Applicable day of the week."@en ;
       rdfs:label "DayOfWeek"@en .

### http://spec.tn-its.eu/owl/tnits-owl:DayOfWeekCode
:DayOfWeekCode a skos:ConceptScheme ;
         skos:definition "Applicable day of the week."@en ;
       dc:isFormatOf :DayOfWeek .

### http://spec.tn-its.eu/owl/tnits-owl:DayOfWeek.monday
:DayOfWeek.monday a :DayOfWeek,skos:Concept ;
         skos:inScheme :DayOfWeekCode ;
         rdfs:label "monday"@no .

### http://spec.tn-its.eu/owl/tnits-owl:DayOfWeek.tuesday
:DayOfWeek.tuesday a :DayOfWeek,skos:Concept ;
         skos:inScheme :DayOfWeekCode ;
         rdfs:label "tuesday"@no .

### http://spec.tn-its.eu/owl/tnits-owl:DayOfWeek.wednesday
:DayOfWeek.wednesday a :DayOfWeek,skos:Concept ;
         skos:inScheme :DayOfWeekCode ;
         rdfs:label "wednesday"@no .

### http://spec.tn-its.eu/owl/tnits-owl:DayOfWeek.thursday
:DayOfWeek.thursday a :DayOfWeek,skos:Concept ;
         skos:inScheme :DayOfWeekCode ;
         rdfs:label "thursday"@no .

### http://spec.tn-its.eu/owl/tnits-owl:DayOfWeek.friday
:DayOfWeek.friday a :DayOfWeek,skos:Concept ;
         skos:inScheme :DayOfWeekCode ;
         rdfs:label "friday"@no .

### http://spec.tn-its.eu/owl/tnits-owl:DayOfWeek.saturday
:DayOfWeek.saturday a :DayOfWeek,skos:Concept ;
         skos:inScheme :DayOfWeekCode ;
         rdfs:label "saturday"@no .

### http://spec.tn-its.eu/owl/tnits-owl:DayOfWeek.sunday
:DayOfWeek.sunday a :DayOfWeek,skos:Concept ;
         skos:inScheme :DayOfWeekCode ;
         rdfs:label "sunday"@no .
:DayOfWeek owl:oneOf ( :DayOfWeek.monday :DayOfWeek.tuesday :DayOfWeek.wednesday :DayOfWeek.thursday :DayOfWeek.friday :DayOfWeek.saturday :DayOfWeek.sunday  ) ; .

### http://spec.tn-its.eu/owl/tnits-owl:MonthOfYear
:MonthOfYear a owl:Class ;
       rdfs:subClassOf :tnitsEnumeration ;
         skos:definition "Applicable month of the year."@en ;
       rdfs:label "MonthOfYear"@en .

### http://spec.tn-its.eu/owl/tnits-owl:MonthOfYearCode
:MonthOfYearCode a skos:ConceptScheme ;
         skos:definition "Applicable month of the year."@en ;
       dc:isFormatOf :MonthOfYear .

### http://spec.tn-its.eu/owl/tnits-owl:MonthOfYear.january
:MonthOfYear.january a :MonthOfYear,skos:Concept ;
         skos:inScheme :MonthOfYearCode ;
         rdfs:label "january"@no .

### http://spec.tn-its.eu/owl/tnits-owl:MonthOfYear.february
:MonthOfYear.february a :MonthOfYear,skos:Concept ;
         skos:inScheme :MonthOfYearCode ;
         rdfs:label "february"@no .

### http://spec.tn-its.eu/owl/tnits-owl:MonthOfYear.march
:MonthOfYear.march a :MonthOfYear,skos:Concept ;
         skos:inScheme :MonthOfYearCode ;
         rdfs:label "march"@no .

### http://spec.tn-its.eu/owl/tnits-owl:MonthOfYear.april
:MonthOfYear.april a :MonthOfYear,skos:Concept ;
         skos:inScheme :MonthOfYearCode ;
         rdfs:label "april"@no .

### http://spec.tn-its.eu/owl/tnits-owl:MonthOfYear.may
:MonthOfYear.may a :MonthOfYear,skos:Concept ;
         skos:inScheme :MonthOfYearCode ;
         rdfs:label "may"@no .

### http://spec.tn-its.eu/owl/tnits-owl:MonthOfYear.june
:MonthOfYear.june a :MonthOfYear,skos:Concept ;
         skos:inScheme :MonthOfYearCode ;
         rdfs:label "june"@no .

### http://spec.tn-its.eu/owl/tnits-owl:MonthOfYear.july
:MonthOfYear.july a :MonthOfYear,skos:Concept ;
         skos:inScheme :MonthOfYearCode ;
         rdfs:label "july"@no .

### http://spec.tn-its.eu/owl/tnits-owl:MonthOfYear.august
:MonthOfYear.august a :MonthOfYear,skos:Concept ;
         skos:inScheme :MonthOfYearCode ;
         rdfs:label "august"@no .

### http://spec.tn-its.eu/owl/tnits-owl:MonthOfYear.september
:MonthOfYear.september a :MonthOfYear,skos:Concept ;
         skos:inScheme :MonthOfYearCode ;
         rdfs:label "september"@no .

### http://spec.tn-its.eu/owl/tnits-owl:MonthOfYear.october
:MonthOfYear.october a :MonthOfYear,skos:Concept ;
         skos:inScheme :MonthOfYearCode ;
         rdfs:label "october"@no .

### http://spec.tn-its.eu/owl/tnits-owl:MonthOfYear.november
:MonthOfYear.november a :MonthOfYear,skos:Concept ;
         skos:inScheme :MonthOfYearCode ;
         rdfs:label "november"@no .

### http://spec.tn-its.eu/owl/tnits-owl:MonthOfYear.december
:MonthOfYear.december a :MonthOfYear,skos:Concept ;
         skos:inScheme :MonthOfYearCode ;
         rdfs:label "december"@no .
:MonthOfYear owl:oneOf ( :MonthOfYear.january :MonthOfYear.february :MonthOfYear.march :MonthOfYear.april :MonthOfYear.may :MonthOfYear.june :MonthOfYear.july :MonthOfYear.august :MonthOfYear.september :MonthOfYear.october :MonthOfYear.november :MonthOfYear.december  ) ; .

### http://spec.tn-its.eu/owl/tnits-owl:WeekOfMonth
:WeekOfMonth a owl:Class ;
       rdfs:subClassOf :tnitsEnumeration ;
         skos:definition "Applicable week of the month."@en ;
       rdfs:label "WeekOfMonth"@en .

### http://spec.tn-its.eu/owl/tnits-owl:WeekOfMonthCode
:WeekOfMonthCode a skos:ConceptScheme ;
         skos:definition "Applicable week of the month."@en ;
       dc:isFormatOf :WeekOfMonth .

### http://spec.tn-its.eu/owl/tnits-owl:WeekOfMonth.firstWeekOfMonth
:WeekOfMonth.firstWeekOfMonth a :WeekOfMonth,skos:Concept ;
         skos:inScheme :WeekOfMonthCode ;
         rdfs:label "firstWeekOfMonth"@no .

### http://spec.tn-its.eu/owl/tnits-owl:WeekOfMonth.secondWeekOfMonth
:WeekOfMonth.secondWeekOfMonth a :WeekOfMonth,skos:Concept ;
         skos:inScheme :WeekOfMonthCode ;
         rdfs:label "secondWeekOfMonth"@no .

### http://spec.tn-its.eu/owl/tnits-owl:WeekOfMonth.thirdWeekOfMonth
:WeekOfMonth.thirdWeekOfMonth a :WeekOfMonth,skos:Concept ;
         skos:inScheme :WeekOfMonthCode ;
         rdfs:label "thirdWeekOfMonth"@no .

### http://spec.tn-its.eu/owl/tnits-owl:WeekOfMonth.fourthWeekOfMonth
:WeekOfMonth.fourthWeekOfMonth a :WeekOfMonth,skos:Concept ;
         skos:inScheme :WeekOfMonthCode ;
         rdfs:label "fourthWeekOfMonth"@no .

### http://spec.tn-its.eu/owl/tnits-owl:WeekOfMonth.fifthWeekOfMonth
:WeekOfMonth.fifthWeekOfMonth a :WeekOfMonth,skos:Concept ;
         skos:inScheme :WeekOfMonthCode ;
         rdfs:label "fifthWeekOfMonth"@no .

### http://spec.tn-its.eu/owl/tnits-owl:WeekOfMonth.sixthWeekOfMonth
:WeekOfMonth.sixthWeekOfMonth a :WeekOfMonth,skos:Concept ;
         skos:inScheme :WeekOfMonthCode ;
         rdfs:label "sixthWeekOfMonth"@no .
:WeekOfMonth owl:oneOf ( :WeekOfMonth.firstWeekOfMonth :WeekOfMonth.secondWeekOfMonth :WeekOfMonth.thirdWeekOfMonth :WeekOfMonth.fourthWeekOfMonth :WeekOfMonth.fifthWeekOfMonth :WeekOfMonth.sixthWeekOfMonth  ) ; .


### http://spec.tn-its.eu/owl/tnits-owl:EmissionClassificationEuro
:EmissionClassificationEuro a owl:Class ;
       rdfs:subClassOf :tnitsCodeList ;
         skos:definition "Specifies the available list of enumerations for the minimum Euro emission classification the vehicle(s) have to comply with according to the 1970 Directive 70/220/EEC and its several amendments. Note that vehicleType and fuelType need to be provided in order to make this classification explicit. [SOURCE - DATEX 3.0 Part 7 (proposed EN/16157-7:2018)]"@en ;
       rdfs:label "EmissionClassificationEuro"@en .

### http://spec.tn-its.eu/owl/tnits-owl:EmissionClassificationEuroCode
:EmissionClassificationEuroCode a skos:ConceptScheme ;
         skos:definition "Specifies the available list of enumerations for the minimum Euro emission classification the vehicle(s) have to comply with according to the 1970 Directive 70/220/EEC and its several amendments. Note that vehicleType and fuelType need to be provided in order to make this classification explicit. [SOURCE - DATEX 3.0 Part 7 (proposed EN/16157-7:2018)]"@en ;
       dc:isFormatOf :EmissionClassificationEuro .

### http://spec.tn-its.eu/owl/tnits-owl:Emissions
:Emissions a owl:Class ;
       rdfs:subClassOf :tnitsDataType ;
         skos:definition "Emission characteristics of vehicles. [SOURCE: DATEX 3.0 Part 7 (proposed EN 16157-7:2018)]  "@en ;
       rdfs:label "Emissions"@en .

### http://spec.tn-its.eu/owl/tnits-owl#Emissions.emissionClassificationEuro
:Emissions.emissionClassificationEuro rdf:type owl:ObjectProperty ;
         skos:definition "The minimum Euro emission classification the vehicle(s) have to comply with according to the 1970 Directive 70/220/EEC and its several amendments. Note that vehicleType and fuelType need to be provided in order to make this classification explicit. [SOURCE: DATEX 3.0 Part 7 (proposed EN 161577:2018)] "@en ;
         rdfs:domain :Emissions;
         rdfs:range :EmissionClassificationEuro;
         rdfs:label "Emissions.emissionClassificationEuro"@en .
:Emissions rdfs:subClassOf [ rdf:type owl:Restriction ;
         owl:onProperty :Emissions.emissionClassificationEuro;
         owl:onClass :EmissionClassificationEuro;
       owl:maxQualifiedCardinality "1"^^xsd:nonNegativeInteger ;
         ] .
:Emissions rdfs:subClassOf [ rdf:type owl:Restriction ;
         owl:onProperty :Emissions.emissionClassificationEuro;
         owl:allValuesFrom :EmissionClassificationEuro;
         ] .


### http://spec.tn-its.eu/owl/tnits-owl#emissionClassificationOther
:emissionClassificationOther rdf:type owl:DatatypeProperty ;
         skos:definition "Some other (probably locally defined) value(s) for emission classification. [SOURCE: DATEX 3.0 Part 7 (proposed EN 16157-7:2018)] "@en ;
         rdfs:domain :Emissions;
         rdfs:range xsd:string;
         rdfs:label "emissionClassificationOther"@en .
:Emissions rdfs:subClassOf [ rdf:type owl:Restriction ;
         owl:onProperty :emissionClassificationOther;
         owl:allValuesFrom xsd:string;
         ] .


### http://spec.tn-its.eu/owl/tnits-owl#emissionLevel
:emissionLevel rdf:type owl:ObjectProperty ;
         skos:definition "The low emission level of a vehicle. [SOURCE: DATEX 3.0 Part 7 (proposed EN 16157-7:2018)] "@en ;
         rdfs:domain :Emissions;
         rdfs:range :LowEmissionLevel;
         rdfs:label "emissionLevel"@en .
:Emissions rdfs:subClassOf [ rdf:type owl:Restriction ;
         owl:onProperty :emissionLevel;
         owl:onClass :LowEmissionLevel;
       owl:maxQualifiedCardinality "1"^^xsd:nonNegativeInteger ;
         ] .
:Emissions rdfs:subClassOf [ rdf:type owl:Restriction ;
         owl:onProperty :emissionLevel;
         owl:allValuesFrom :LowEmissionLevel;
         ] .


### http://spec.tn-its.eu/owl/tnits-owl:FuelType
:FuelType a owl:Class ;
       rdfs:subClassOf :tnitsCodeList ;
         skos:definition "Specifies the available list of enumerations for the type of fuel used by the vehicle."@en ;
       rdfs:label "FuelType"@en .

### http://spec.tn-its.eu/owl/tnits-owl:FuelTypeCode
:FuelTypeCode a skos:ConceptScheme ;
         skos:definition "Specifies the available list of enumerations for the type of fuel used by the vehicle."@en ;
       dc:isFormatOf :FuelType .

### http://spec.tn-its.eu/owl/tnits-owl:GrossWeightCharacteristic
:GrossWeightCharacteristic a owl:Class ;
       rdfs:subClassOf :tnitsDataType ;
         skos:definition "Gross weight characteristic of a vehicle. [SOURCE: CEN/TS16157-3:2011] "@en ;
       rdfs:label "GrossWeightCharacteristic"@en .

### http://spec.tn-its.eu/owl/tnits-owl#comparisonOperator
:comparisonOperator rdf:type owl:ObjectProperty ;
         skos:definition "The operator to be used in the vehicle characteristic comparison operation. [SOURCE: CEN/TS16157-3:2011] "@en ;
         rdfs:range :ComparisonOperator;
         rdfs:label "comparisonOperator"@en .
:GrossWeightCharacteristic rdfs:subClassOf [ rdf:type owl:Restriction ;
         owl:onProperty :comparisonOperator;
         owl:onClass :ComparisonOperator;
       owl:qualifiedCardinality "1"^^xsd:nonNegativeInteger ;
         ] .
:GrossWeightCharacteristic rdfs:subClassOf [ rdf:type owl:Restriction ;
         owl:onProperty :comparisonOperator;
         owl:allValuesFrom :ComparisonOperator;
         ] .


### http://spec.tn-its.eu/owl/tnits-owl#grossVehicleWeight
:grossVehicleWeight rdf:type owl:ObjectProperty ;
         skos:definition "The gross weight of the vehicle and its load, including any trailers. [SOURCE: CEN/TS16157-3:2011]"@en ;
         rdfs:domain :GrossWeightCharacteristic;
         rdfs:range :Measure;
         rdf:type owl:FunctionalProperty;
         rdfs:label "grossVehicleWeight"@en .
:GrossWeightCharacteristic rdfs:subClassOf [ rdf:type owl:Restriction ;
         owl:onProperty :grossVehicleWeight;
         owl:onClass :Measure;
       owl:qualifiedCardinality "1"^^xsd:nonNegativeInteger ;
         ] .
:GrossWeightCharacteristic rdfs:subClassOf [ rdf:type owl:Restriction ;
         owl:onProperty :grossVehicleWeight;
         owl:allValuesFrom :Measure;
         ] .


### http://spec.tn-its.eu/owl/tnits-owl#typeOfWeight
:typeOfWeight rdf:type owl:ObjectProperty ;
         skos:definition "The meaning of the weight value. [SOURCE: CEN/TS16157-3:2011]"@en ;
         rdfs:domain :GrossWeightCharacteristic;
         rdfs:range :WeightType;
         rdf:type owl:FunctionalProperty;
         rdfs:label "typeOfWeight"@en .
:GrossWeightCharacteristic rdfs:subClassOf [ rdf:type owl:Restriction ;
         owl:onProperty :typeOfWeight;
         owl:onClass :WeightType;
       owl:qualifiedCardinality "1"^^xsd:nonNegativeInteger ;
         ] .
:GrossWeightCharacteristic rdfs:subClassOf [ rdf:type owl:Restriction ;
         owl:onProperty :typeOfWeight;
         owl:allValuesFrom :WeightType;
         ] .


### http://spec.tn-its.eu/owl/tnits-owl:HeaviestAxleWeightCharacteristic
:HeaviestAxleWeightCharacteristic a owl:Class ;
       rdfs:subClassOf :tnitsDataType ;
         skos:definition "Weight characteristic of the heaviest axle on the vehicle. [SOURCE: CEN/TS16157-3:2011] "@en ;
       rdfs:label "HeaviestAxleWeightCharacteristic"@en .
:HeaviestAxleWeightCharacteristic rdfs:subClassOf [ rdf:type owl:Restriction ;
         owl:onProperty :comparisonOperator;
         owl:onClass :ComparisonOperator;
       owl:qualifiedCardinality "1"^^xsd:nonNegativeInteger ;
         ] .
:HeaviestAxleWeightCharacteristic rdfs:subClassOf [ rdf:type owl:Restriction ;
         owl:onProperty :comparisonOperator;
         owl:allValuesFrom :ComparisonOperator;
         ] .


### http://spec.tn-its.eu/owl/tnits-owl#heaviestAxleWeight
:heaviestAxleWeight rdf:type owl:ObjectProperty ;
         skos:definition "The weight of the heaviest axle on the vehicle. [SOURCE: CEN/TS161573:2011]"@en ;
         rdfs:domain :HeaviestAxleWeightCharacteristic;
         rdfs:range :Measure;
         rdf:type owl:FunctionalProperty;
         rdfs:label "heaviestAxleWeight"@en .
:HeaviestAxleWeightCharacteristic rdfs:subClassOf [ rdf:type owl:Restriction ;
         owl:onProperty :heaviestAxleWeight;
         owl:onClass :Measure;
       owl:qualifiedCardinality "1"^^xsd:nonNegativeInteger ;
         ] .
:HeaviestAxleWeightCharacteristic rdfs:subClassOf [ rdf:type owl:Restriction ;
         owl:onProperty :heaviestAxleWeight;
         owl:allValuesFrom :Measure;
         ] .


### http://spec.tn-its.eu/owl/tnits-owl:HeightCharacteristic
:HeightCharacteristic a owl:Class ;
       rdfs:subClassOf :tnitsDataType ;
         skos:definition "Height characteristic of a vehicle. [SOURCE: CEN/TS16157-3:2011] "@en ;
       rdfs:label "HeightCharacteristic"@en .
:HeightCharacteristic rdfs:subClassOf [ rdf:type owl:Restriction ;
         owl:onProperty :comparisonOperator;
         owl:onClass :ComparisonOperator;
       owl:qualifiedCardinality "1"^^xsd:nonNegativeInteger ;
         ] .
:HeightCharacteristic rdfs:subClassOf [ rdf:type owl:Restriction ;
         owl:onProperty :comparisonOperator;
         owl:allValuesFrom :ComparisonOperator;
         ] .


### http://spec.tn-its.eu/owl/tnits-owl#vehicleHeight
:vehicleHeight rdf:type owl:ObjectProperty ;
         skos:definition "The height of the highest part, excluding antennae, of an individual vehicle above the road surface, in metres. [SOURCE: CEN/TS16157-3:2011]"@en ;
         rdfs:domain :HeightCharacteristic;
         rdfs:range :Measure;
         rdf:type owl:FunctionalProperty;
         rdfs:label "vehicleHeight"@en .
:HeightCharacteristic rdfs:subClassOf [ rdf:type owl:Restriction ;
         owl:onProperty :vehicleHeight;
         owl:onClass :Measure;
       owl:qualifiedCardinality "1"^^xsd:nonNegativeInteger ;
         ] .
:HeightCharacteristic rdfs:subClassOf [ rdf:type owl:Restriction ;
         owl:onProperty :vehicleHeight;
         owl:allValuesFrom :Measure;
         ] .


### http://spec.tn-its.eu/owl/tnits-owl:LengthCharacteristic
:LengthCharacteristic a owl:Class ;
       rdfs:subClassOf :tnitsDataType ;
         skos:definition "Length characteristic of a vehicle. [SOURCE: CEN/TS16157-3:2011] "@en ;
       rdfs:label "LengthCharacteristic"@en .
:LengthCharacteristic rdfs:subClassOf [ rdf:type owl:Restriction ;
         owl:onProperty :comparisonOperator;
         owl:onClass :ComparisonOperator;
       owl:qualifiedCardinality "1"^^xsd:nonNegativeInteger ;
         ] .
:LengthCharacteristic rdfs:subClassOf [ rdf:type owl:Restriction ;
         owl:onProperty :comparisonOperator;
         owl:allValuesFrom :ComparisonOperator;
         ] .


### http://spec.tn-its.eu/owl/tnits-owl#vehicleLength
:vehicleLength rdf:type owl:ObjectProperty ;
         skos:definition "The overall distance between the front and back of an individual vehicle, including the length of any trailers, couplings, etc. [SOURCE: CEN/TS161573:2011] "@en ;
         rdfs:domain :LengthCharacteristic;
         rdfs:range :Measure;
         rdf:type owl:FunctionalProperty;
         rdfs:label "vehicleLength"@en .
:LengthCharacteristic rdfs:subClassOf [ rdf:type owl:Restriction ;
         owl:onProperty :vehicleLength;
         owl:onClass :Measure;
       owl:qualifiedCardinality "1"^^xsd:nonNegativeInteger ;
         ] .
:LengthCharacteristic rdfs:subClassOf [ rdf:type owl:Restriction ;
         owl:onProperty :vehicleLength;
         owl:allValuesFrom :Measure;
         ] .


### http://spec.tn-its.eu/owl/tnits-owl:LoadType
:LoadType a owl:Class ;
       rdfs:subClassOf :tnitsCodeList ;
         skos:definition "Specifies the available list of enumerations for types of vehicle loads"@en ;
       rdfs:label "LoadType"@en .

### http://spec.tn-its.eu/owl/tnits-owl:LoadTypeCode
:LoadTypeCode a skos:ConceptScheme ;
         skos:definition "Specifies the available list of enumerations for types of vehicle loads"@en ;
       dc:isFormatOf :LoadType .

### http://spec.tn-its.eu/owl/tnits-owl:LowEmissionLevel
:LowEmissionLevel a owl:Class ;
       rdfs:subClassOf :tnitsCodeList ;
         skos:definition "Specifies the available list of enumerations for vehicle emission levels"@en ;
       rdfs:label "LowEmissionLevel"@en .

### http://spec.tn-its.eu/owl/tnits-owl:LowEmissionLevelCode
:LowEmissionLevelCode a skos:ConceptScheme ;
         skos:definition "Specifies the available list of enumerations for vehicle emission levels"@en ;
       dc:isFormatOf :LowEmissionLevel .

### http://spec.tn-its.eu/owl/tnits-owl:NumberOfAxlesCharacteristic
:NumberOfAxlesCharacteristic a owl:Class ;
       rdfs:subClassOf :tnitsDataType ;
         skos:definition "Number of axles characteristic of a vehicle. [SOURCE: CEN/TS16157-3:2011] "@en ;
       rdfs:label "NumberOfAxlesCharacteristic"@en .
:NumberOfAxlesCharacteristic rdfs:subClassOf [ rdf:type owl:Restriction ;
         owl:onProperty :comparisonOperator;
         owl:onClass :ComparisonOperator;
       owl:qualifiedCardinality "1"^^xsd:nonNegativeInteger ;
         ] .
:NumberOfAxlesCharacteristic rdfs:subClassOf [ rdf:type owl:Restriction ;
         owl:onProperty :comparisonOperator;
         owl:allValuesFrom :ComparisonOperator;
         ] .


### http://spec.tn-its.eu/owl/tnits-owl#numberOfAxles
:numberOfAxles rdf:type owl:DatatypeProperty ;
         skos:definition "The total number of axles of an individual vehicle.  [SOURCE: CEN/TS161573:2011]"@en ;
         rdfs:domain :NumberOfAxlesCharacteristic;
         rdfs:range xsd:integer;
         rdf:type owl:FunctionalProperty;
         rdfs:label "numberOfAxles"@en .
:NumberOfAxlesCharacteristic rdfs:subClassOf [ rdf:type owl:Restriction ;
         owl:onProperty :numberOfAxles;
         owl:onDataRange xsd:integer;
       owl:qualifiedCardinality "1"^^xsd:nonNegativeInteger ;
         ] .
:NumberOfAxlesCharacteristic rdfs:subClassOf [ rdf:type owl:Restriction ;
         owl:onProperty :numberOfAxles;
         owl:allValuesFrom xsd:integer;
         ] .


### http://spec.tn-its.eu/owl/tnits-owl:VehicleCharacteristics
:VehicleCharacteristics a owl:Class ;
       rdfs:subClassOf :tnitsDataType ;
         skos:definition "A collection of parameters which characterise a vehicle. [SOURCE: DATEX 3.0 Part 7 (proposed EN 16157-7:2018)] "@en ;
       rdfs:label "VehicleCharacteristics"@en .

### http://spec.tn-its.eu/owl/tnits-owl#VehicleCharacteristics.heightCharacteristic
:VehicleCharacteristics.heightCharacteristic rdf:type owl:ObjectProperty ;
         skos:definition "Height characteristic of a vehicle. [SOURCE: CEN/TS16157-3:2011] "@en ;
         rdfs:domain :VehicleCharacteristics;
         rdfs:range :HeightCharacteristic;
         rdfs:label "VehicleCharacteristics.heightCharacteristic"@en .
:VehicleCharacteristics rdfs:subClassOf [ rdf:type owl:Restriction ;
         owl:onProperty :VehicleCharacteristics.heightCharacteristic;
         owl:allValuesFrom :HeightCharacteristic;
         ] .


### http://spec.tn-its.eu/owl/tnits-owl#VehicleCharacteristics.widthCharacteristic
:VehicleCharacteristics.widthCharacteristic rdf:type owl:ObjectProperty ;
         skos:definition "Width characteristic of a vehicle. [SOURCE: CEN/TS16157-3:2011] "@en ;
         rdfs:domain :VehicleCharacteristics;
         rdfs:range :WidthCharacteristic;
         rdfs:label "VehicleCharacteristics.widthCharacteristic"@en .
:VehicleCharacteristics rdfs:subClassOf [ rdf:type owl:Restriction ;
         owl:onProperty :VehicleCharacteristics.widthCharacteristic;
         owl:allValuesFrom :WidthCharacteristic;
         ] .


### http://spec.tn-its.eu/owl/tnits-owl#VehicleCharacteristics.heaviestAxleWeightCharacteristic
:VehicleCharacteristics.heaviestAxleWeightCharacteristic rdf:type owl:ObjectProperty ;
         skos:definition "Weight characteristic of the heaviest axle on the vehicle. [SOURCE: CEN/TS16157-3:2011] "@en ;
         rdfs:domain :VehicleCharacteristics;
         rdfs:range :HeaviestAxleWeightCharacteristic;
         rdfs:label "VehicleCharacteristics.heaviestAxleWeightCharacteristic"@en .
:VehicleCharacteristics rdfs:subClassOf [ rdf:type owl:Restriction ;
         owl:onProperty :VehicleCharacteristics.heaviestAxleWeightCharacteristic;
         owl:allValuesFrom :HeaviestAxleWeightCharacteristic;
         ] .


### http://spec.tn-its.eu/owl/tnits-owl#VehicleCharacteristics.grossWeightCharacteristic
:VehicleCharacteristics.grossWeightCharacteristic rdf:type owl:ObjectProperty ;
         skos:definition "Gross weight characteristic of a vehicle. [SOURCE: CEN/TS16157-3:2011] "@en ;
         rdfs:domain :VehicleCharacteristics;
         rdfs:range :GrossWeightCharacteristic;
         rdfs:label "VehicleCharacteristics.grossWeightCharacteristic"@en .
:VehicleCharacteristics rdfs:subClassOf [ rdf:type owl:Restriction ;
         owl:onProperty :VehicleCharacteristics.grossWeightCharacteristic;
         owl:allValuesFrom :GrossWeightCharacteristic;
         ] .


### http://spec.tn-its.eu/owl/tnits-owl#VehicleCharacteristics.numberOfAxlesCharacteristic
:VehicleCharacteristics.numberOfAxlesCharacteristic rdf:type owl:ObjectProperty ;
         skos:definition "Number of axles characteristic of a vehicle. [SOURCE: CEN/TS16157-3:2011] "@en ;
         rdfs:domain :VehicleCharacteristics;
         rdfs:range :NumberOfAxlesCharacteristic;
         rdfs:label "VehicleCharacteristics.numberOfAxlesCharacteristic"@en .
:VehicleCharacteristics rdfs:subClassOf [ rdf:type owl:Restriction ;
         owl:onProperty :VehicleCharacteristics.numberOfAxlesCharacteristic;
         owl:allValuesFrom :NumberOfAxlesCharacteristic;
         ] .


### http://spec.tn-its.eu/owl/tnits-owl#VehicleCharacteristics.emissions
:VehicleCharacteristics.emissions rdf:type owl:ObjectProperty ;
         skos:definition "Emission characteristics of vehicles. [SOURCE: DATEX 3.0 Part 7 (proposed EN 16157-7:2018)] "@en ;
         rdfs:domain :VehicleCharacteristics;
         rdfs:range :Emissions;
         rdfs:label "VehicleCharacteristics.emissions"@en .
:VehicleCharacteristics rdfs:subClassOf [ rdf:type owl:Restriction ;
         owl:onProperty :VehicleCharacteristics.emissions;
         owl:allValuesFrom :Emissions;
         ] .


### http://spec.tn-its.eu/owl/tnits-owl#VehicleCharacteristics.lengthCharacteristic
:VehicleCharacteristics.lengthCharacteristic rdf:type owl:ObjectProperty ;
         skos:definition "Length characteristic of a vehicle. [SOURCE: CEN/TS16157-3:2011] "@en ;
         rdfs:domain :VehicleCharacteristics;
         rdfs:range :LengthCharacteristic;
         rdfs:label "VehicleCharacteristics.lengthCharacteristic"@en .
:VehicleCharacteristics rdfs:subClassOf [ rdf:type owl:Restriction ;
         owl:onProperty :VehicleCharacteristics.lengthCharacteristic;
         owl:allValuesFrom :LengthCharacteristic;
         ] .


### http://spec.tn-its.eu/owl/tnits-owl#VehicleCharacteristics.fuelType
:VehicleCharacteristics.fuelType rdf:type owl:ObjectProperty ;
         skos:definition "The type of fuel used by the vehicle. [SOURCE: CEN/TS16157-3:2011] "@en ;
         rdfs:domain :VehicleCharacteristics;
         rdfs:range :FuelType;
         rdfs:label "VehicleCharacteristics.fuelType"@en .
:VehicleCharacteristics rdfs:subClassOf [ rdf:type owl:Restriction ;
         owl:onProperty :VehicleCharacteristics.fuelType;
         owl:allValuesFrom :FuelType;
         ] .


### http://spec.tn-its.eu/owl/tnits-owl#VehicleCharacteristics.loadType
:VehicleCharacteristics.loadType rdf:type owl:ObjectProperty ;
         skos:definition "The type of load carried by the vehicle, especially in respect of hazardous loads. [SOURCE: CEN/TS16157-3:2011]"@en ;
         rdfs:domain :VehicleCharacteristics;
         rdfs:range :LoadType;
         rdfs:label "VehicleCharacteristics.loadType"@en .
:VehicleCharacteristics rdfs:subClassOf [ rdf:type owl:Restriction ;
         owl:onProperty :VehicleCharacteristics.loadType;
         owl:onClass :LoadType;
       owl:maxQualifiedCardinality "1"^^xsd:nonNegativeInteger ;
         ] .
:VehicleCharacteristics rdfs:subClassOf [ rdf:type owl:Restriction ;
         owl:onProperty :VehicleCharacteristics.loadType;
         owl:allValuesFrom :LoadType;
         ] .


### http://spec.tn-its.eu/owl/tnits-owl#VehicleCharacteristics.vehicleEquipment
:VehicleCharacteristics.vehicleEquipment rdf:type owl:ObjectProperty ;
         skos:definition "The type of equipment in use or on board the vehicle. [SOURCE: CEN/TS16157-3:2011]"@en ;
         rdfs:domain :VehicleCharacteristics;
         rdfs:range :VehicleEquipment;
         rdfs:label "VehicleCharacteristics.vehicleEquipment"@en .
:VehicleCharacteristics rdfs:subClassOf [ rdf:type owl:Restriction ;
         owl:onProperty :VehicleCharacteristics.vehicleEquipment;
         owl:onClass :VehicleEquipment;
       owl:maxQualifiedCardinality "1"^^xsd:nonNegativeInteger ;
         ] .
:VehicleCharacteristics rdfs:subClassOf [ rdf:type owl:Restriction ;
         owl:onProperty :VehicleCharacteristics.vehicleEquipment;
         owl:allValuesFrom :VehicleEquipment;
         ] .


### http://spec.tn-its.eu/owl/tnits-owl#VehicleCharacteristics.vehicleType
:VehicleCharacteristics.vehicleType rdf:type owl:ObjectProperty ;
         skos:definition "Vehicle type. [SOURCE: CEN/TS16157-3:2011] "@en ;
         rdfs:domain :VehicleCharacteristics;
         rdfs:range :VehicleType;
         rdfs:label "VehicleCharacteristics.vehicleType"@en .
:VehicleCharacteristics rdfs:subClassOf [ rdf:type owl:Restriction ;
         owl:onProperty :VehicleCharacteristics.vehicleType;
         owl:allValuesFrom :VehicleType;
         ] .


### http://spec.tn-its.eu/owl/tnits-owl#VehicleCharacteristics.vehicleUsage
:VehicleCharacteristics.vehicleUsage rdf:type owl:ObjectProperty ;
         skos:definition "The type of usage of the vehicle (i.e. for what purpose is the vehicle being used). [SOURCE: CEN/TS16157-3:2011]"@en ;
         rdfs:domain :VehicleCharacteristics;
         rdfs:range :VehicleUsage;
         rdfs:label "VehicleCharacteristics.vehicleUsage"@en .
:VehicleCharacteristics rdfs:subClassOf [ rdf:type owl:Restriction ;
         owl:onProperty :VehicleCharacteristics.vehicleUsage;
         owl:onClass :VehicleUsage;
       owl:maxQualifiedCardinality "1"^^xsd:nonNegativeInteger ;
         ] .
:VehicleCharacteristics rdfs:subClassOf [ rdf:type owl:Restriction ;
         owl:onProperty :VehicleCharacteristics.vehicleUsage;
         owl:allValuesFrom :VehicleUsage;
         ] .


### http://spec.tn-its.eu/owl/tnits-owl#yearOfFirstRegistration
:yearOfFirstRegistration rdf:type owl:DatatypeProperty ;
         skos:definition "Year of first registration of the vehicle [SOURCE: DATEX 3.0 Part 7 (proposed EN 16157-7:2018)] "@en ;
         rdfs:domain :VehicleCharacteristics;
         rdfs:range xsd:integer;
         rdfs:label "yearOfFirstRegistration"@en .
:VehicleCharacteristics rdfs:subClassOf [ rdf:type owl:Restriction ;
         owl:onProperty :yearOfFirstRegistration;
         owl:onDataRange xsd:integer;
       owl:maxQualifiedCardinality "1"^^xsd:nonNegativeInteger ;
         ] .
:VehicleCharacteristics rdfs:subClassOf [ rdf:type owl:Restriction ;
         owl:onProperty :yearOfFirstRegistration;
         owl:allValuesFrom xsd:integer;
         ] .


### http://spec.tn-its.eu/owl/tnits-owl:VehicleEquipment
:VehicleEquipment a owl:Class ;
       rdfs:subClassOf :tnitsCodeList ;
         skos:definition "Specifies the available list of enumerations for the vehicle equipment types"@en ;
       rdfs:label "VehicleEquipment"@en .

### http://spec.tn-its.eu/owl/tnits-owl:VehicleEquipmentCode
:VehicleEquipmentCode a skos:ConceptScheme ;
         skos:definition "Specifies the available list of enumerations for the vehicle equipment types"@en ;
       dc:isFormatOf :VehicleEquipment .

### http://spec.tn-its.eu/owl/tnits-owl:VehicleType
:VehicleType a owl:Class ;
       rdfs:subClassOf :tnitsCodeList ;
         skos:definition "Specifies the available list of enumerations for types of vehicle."@en ;
       rdfs:label "VehicleType"@en .

### http://spec.tn-its.eu/owl/tnits-owl:VehicleTypeCode
:VehicleTypeCode a skos:ConceptScheme ;
         skos:definition "Specifies the available list of enumerations for types of vehicle."@en ;
       dc:isFormatOf :VehicleType .

### http://spec.tn-its.eu/owl/tnits-owl:VehicleUsage
:VehicleUsage a owl:Class ;
       rdfs:subClassOf :tnitsCodeList ;
         skos:definition "Specifies the available list of enumerations for types of usage of vehicles."@en ;
       rdfs:label "VehicleUsage"@en .

### http://spec.tn-its.eu/owl/tnits-owl:VehicleUsageCode
:VehicleUsageCode a skos:ConceptScheme ;
         skos:definition "Specifies the available list of enumerations for types of usage of vehicles."@en ;
       dc:isFormatOf :VehicleUsage .

### http://spec.tn-its.eu/owl/tnits-owl:WeightType
:WeightType a owl:Class ;
       rdfs:subClassOf :tnitsCodeList ;
         skos:definition "Type of weight - describing the meaning of a vehicle weight value"@en ;
       rdfs:label "WeightType"@en .

### http://spec.tn-its.eu/owl/tnits-owl:WeightTypeCode
:WeightTypeCode a skos:ConceptScheme ;
         skos:definition "Type of weight - describing the meaning of a vehicle weight value"@en ;
       dc:isFormatOf :WeightType .

### http://spec.tn-its.eu/owl/tnits-owl:WidthCharacteristic
:WidthCharacteristic a owl:Class ;
       rdfs:subClassOf :tnitsDataType ;
         skos:definition "Width characteristic of a vehicle. [SOURCE: CEN/TS16157-3:2011] "@en ;
       rdfs:label "WidthCharacteristic"@en .
:WidthCharacteristic rdfs:subClassOf [ rdf:type owl:Restriction ;
         owl:onProperty :comparisonOperator;
         owl:onClass :ComparisonOperator;
       owl:qualifiedCardinality "1"^^xsd:nonNegativeInteger ;
         ] .
:WidthCharacteristic rdfs:subClassOf [ rdf:type owl:Restriction ;
         owl:onProperty :comparisonOperator;
         owl:allValuesFrom :ComparisonOperator;
         ] .


### http://spec.tn-its.eu/owl/tnits-owl#vehicleWidth
:vehicleWidth rdf:type owl:ObjectProperty ;
         skos:definition "The maximum width of an individual vehicle, in metres. [SOURCE: CEN/TS16157-3:2011]"@en ;
         rdfs:domain :WidthCharacteristic;
         rdfs:range :Measure;
         rdf:type owl:FunctionalProperty;
         rdfs:label "vehicleWidth"@en .
:WidthCharacteristic rdfs:subClassOf [ rdf:type owl:Restriction ;
         owl:onProperty :vehicleWidth;
         owl:onClass :Measure;
       owl:qualifiedCardinality "1"^^xsd:nonNegativeInteger ;
         ] .
:WidthCharacteristic rdfs:subClassOf [ rdf:type owl:Restriction ;
         owl:onProperty :vehicleWidth;
         owl:allValuesFrom :Measure;
         ] .


### http://spec.tn-its.eu/owl/tnits-owl:ComparisonOperator
:ComparisonOperator a owl:Class ;
       rdfs:subClassOf :tnitsEnumeration ;
         skos:definition "The logical operator to be used in a comparison operation. "@en ;
       rdfs:label "ComparisonOperator"@en .

### http://spec.tn-its.eu/owl/tnits-owl:ComparisonOperatorCode
:ComparisonOperatorCode a skos:ConceptScheme ;
         skos:definition "The logical operator to be used in a comparison operation. "@en ;
       dc:isFormatOf :ComparisonOperator .

### http://spec.tn-its.eu/owl/tnits-owl:ComparisonOperator.equalTo
:ComparisonOperator.equalTo a :ComparisonOperator,skos:Concept ;
         skos:inScheme :ComparisonOperatorCode ;
         skos:definition "Logical comparison operator of \"equal to\". "@en ;
         rdfs:label "equalTo"@no .

### http://spec.tn-its.eu/owl/tnits-owl:ComparisonOperator.greaterThan
:ComparisonOperator.greaterThan a :ComparisonOperator,skos:Concept ;
         skos:inScheme :ComparisonOperatorCode ;
         skos:definition "Logical comparison operator of \"greater than\". "@en ;
         rdfs:label "greaterThan"@no .

### http://spec.tn-its.eu/owl/tnits-owl:ComparisonOperator.greaterThanOrEqualTo
:ComparisonOperator.greaterThanOrEqualTo a :ComparisonOperator,skos:Concept ;
         skos:inScheme :ComparisonOperatorCode ;
         skos:definition "Logical comparison operator of \"greater than or equal to\". "@en ;
         rdfs:label "greaterThanOrEqualTo"@no .

### http://spec.tn-its.eu/owl/tnits-owl:ComparisonOperator.lessThan
:ComparisonOperator.lessThan a :ComparisonOperator,skos:Concept ;
         skos:inScheme :ComparisonOperatorCode ;
         skos:definition "Logical comparison operator of \"less than\". "@en ;
         rdfs:label "lessThan"@no .

### http://spec.tn-its.eu/owl/tnits-owl:ComparisonOperator.lessThanOrEqualTo
:ComparisonOperator.lessThanOrEqualTo a :ComparisonOperator,skos:Concept ;
         skos:inScheme :ComparisonOperatorCode ;
         skos:definition "Logical comparison operator of \"less than or equal to\". "@en ;
         rdfs:label "lessThanOrEqualTo"@no .
:ComparisonOperator owl:oneOf ( :ComparisonOperator.equalTo :ComparisonOperator.greaterThan :ComparisonOperator.greaterThanOrEqualTo :ComparisonOperator.lessThan :ComparisonOperator.lessThanOrEqualTo  ) ; .


### http://spec.tn-its.eu/owl/tnits-owl:AgoraBinaryVersion
:AgoraBinaryVersion a owl:Class ;
       rdfs:subClassOf :tnitsCodeList ;
         skos:definition "Specifies the available list of enumerations for the version of the AGORA binary specification being used"@en ;
       rdfs:label "AgoraBinaryVersion"@en .

### http://spec.tn-its.eu/owl/tnits-owl:AgoraBinaryVersionCode
:AgoraBinaryVersionCode a skos:ConceptScheme ;
         skos:definition "Specifies the available list of enumerations for the version of the AGORA binary specification being used"@en ;
       dc:isFormatOf :AgoraBinaryVersion .

### http://spec.tn-its.eu/owl/tnits-owl:BinaryLocationReference
:BinaryLocationReference a owl:Class ;
       rdfs:subClassOf :tnitsDataType ;
         skos:definition "OpenLR location reference using binary encoding "@en ;
       rdfs:label "BinaryLocationReference"@en .

### http://spec.tn-its.eu/owl/tnits-owl#BinaryLocationReference.base64String
:BinaryLocationReference.base64String rdf:type owl:DatatypeProperty ;
         skos:definition "The OpenRL binary string encoded using base64"@en ;
         rdfs:domain :BinaryLocationReference;
         rdfs:range xsd:string;
         rdf:type owl:FunctionalProperty;
         rdfs:label "BinaryLocationReference.base64String"@en .
:BinaryLocationReference rdfs:subClassOf [ rdf:type owl:Restriction ;
         owl:onProperty :BinaryLocationReference.base64String;
         owl:onDataRange xsd:string;
       owl:qualifiedCardinality "1"^^xsd:nonNegativeInteger ;
         ] .
:BinaryLocationReference rdfs:subClassOf [ rdf:type owl:Restriction ;
         owl:onProperty :BinaryLocationReference.base64String;
         owl:allValuesFrom xsd:string;
         ] .


### http://spec.tn-its.eu/owl/tnits-owl#BinaryLocationReference.openLRBinaryVersion
:BinaryLocationReference.openLRBinaryVersion rdf:type owl:ObjectProperty ;
         skos:definition "Provides reference to the version of the OpenLR Binary string encoding used by reference to an item in an external code list (see OpenLRBinaryVersion Class)"@en ;
         rdfs:domain :BinaryLocationReference;
         rdfs:range :OpenLRBinaryVersion;
         rdf:type owl:FunctionalProperty;
         rdfs:label "BinaryLocationReference.openLRBinaryVersion"@en .
:BinaryLocationReference rdfs:subClassOf [ rdf:type owl:Restriction ;
         owl:onProperty :BinaryLocationReference.openLRBinaryVersion;
         owl:onClass :OpenLRBinaryVersion;
       owl:qualifiedCardinality "1"^^xsd:nonNegativeInteger ;
         ] .
:BinaryLocationReference rdfs:subClassOf [ rdf:type owl:Restriction ;
         owl:onProperty :BinaryLocationReference.openLRBinaryVersion;
         owl:allValuesFrom :OpenLRBinaryVersion;
         ] .


### http://spec.tn-its.eu/owl/tnits-owl:GeometryLocationReference
:GeometryLocationReference a owl:Class ;
         skos:definition "Class that references location by use of a geometry reference "@en ;
       rdfs:label "GeometryLocationReference"@en .
:GeometryLocationReference rdfs:subClassOf :LocationReference .

### http://spec.tn-its.eu/owl/tnits-owl#encodedGeometry
:encodedGeometry rdf:type owl:ObjectProperty ;
         skos:definition "the geometry in the source road database that was used to encode the location reference of the referenced location "@en ;
         rdfs:domain :GeometryLocationReference;
         rdfs:range <http://www.opengis.net/ont/geosparql#Geometry>;
         rdf:type owl:FunctionalProperty;
         rdfs:label "encodedGeometry"@en .
:GeometryLocationReference rdfs:subClassOf [ rdf:type owl:Restriction ;
         owl:onProperty :encodedGeometry;
         owl:onClass <http://www.opengis.net/ont/geosparql#Geometry>;
       owl:qualifiedCardinality "1"^^xsd:nonNegativeInteger ;
         ] .
:GeometryLocationReference rdfs:subClassOf [ rdf:type owl:Restriction ;
         owl:onProperty :encodedGeometry;
         owl:allValuesFrom <http://www.opengis.net/ont/geosparql#Geometry>;
         ] .


### http://spec.tn-its.eu/owl/tnits-owl:LinkDirectionValue
:LinkDirectionValue a owl:Class ;
       rdfs:subClassOf :tnitsCodeList ;
         skos:definition "-- Definition -- List of values for directions relative to a link"@en ;
       rdfs:label "LinkDirectionValue"@en .

### http://spec.tn-its.eu/owl/tnits-owl:LinkDirectionValueCode
:LinkDirectionValueCode a skos:ConceptScheme ;
         skos:definition "-- Definition -- List of values for directions relative to a link"@en ;
       dc:isFormatOf :LinkDirectionValue .

### http://spec.tn-its.eu/owl/tnits-owl:LinkDirectionValue.bothDirections
:LinkDirectionValue.bothDirections a :LinkDirectionValue,skos:Concept ;
         skos:inScheme :LinkDirectionValueCode ;
         skos:definition "-- Definition -- In both directions. "@en ;
         rdfs:label "bothDirections"@no .

### http://spec.tn-its.eu/owl/tnits-owl:LinkDirectionValue.inDirection
:LinkDirectionValue.inDirection a :LinkDirectionValue,skos:Concept ;
         skos:inScheme :LinkDirectionValueCode ;
         skos:definition "-- Definition -- In direction of the link. "@en ;
         rdfs:label "inDirection"@no .

### http://spec.tn-its.eu/owl/tnits-owl:LinkDirectionValue.inOppositeDirection
:LinkDirectionValue.inOppositeDirection a :LinkDirectionValue,skos:Concept ;
         skos:inScheme :LinkDirectionValueCode ;
         skos:definition "-- Definition -- In the opposite direction of the link. "@en ;
         rdfs:label "inOppositeDirection"@no .

### http://spec.tn-its.eu/owl/tnits-owl:LinkReference
:LinkReference a owl:Class ;
         skos:definition "A specialisation of a network reference to provide a reference to a network link "@en ;
       rdfs:label "LinkReference"@en .
:LinkReference rdfs:subClassOf :NetworkReference .

### http://spec.tn-its.eu/owl/tnits-owl#applicableDirection
:applicableDirection rdf:type owl:ObjectProperty ;
         skos:definition "Indicates the applicable direction "@en ;
         rdfs:domain :LinkReference;
         rdfs:range :LinkDirectionValue;
         rdf:type owl:FunctionalProperty;
         rdfs:label "applicableDirection"@en .
:LinkReference rdfs:subClassOf [ rdf:type owl:Restriction ;
         owl:onProperty :applicableDirection;
         owl:onClass :LinkDirectionValue;
       owl:qualifiedCardinality "1"^^xsd:nonNegativeInteger ;
         ] .
:LinkReference rdfs:subClassOf [ rdf:type owl:Restriction ;
         owl:onProperty :applicableDirection;
         owl:allValuesFrom :LinkDirectionValue;
         ] .

:LinkReference owl:disjointUnionOf ( :SimplePointReference :SimpleLinearReference  ) ; .

### http://spec.tn-its.eu/owl/tnits-owl:LocationByExternalReference
:LocationByExternalReference a owl:Class ;
         skos:definition "A type of precoded location reference that references a location by use of a specified reference  "@en ;
       rdfs:label "LocationByExternalReference"@en .
:LocationByExternalReference rdfs:subClassOf :PreCodedLocationReference .

### http://spec.tn-its.eu/owl/tnits-owl#predefinedLocationReference
:predefinedLocationReference rdf:type owl:ObjectProperty ;
         skos:definition "A location reference to an object that has pre-defined and stored for future reference "@en ;
         rdfs:domain :LocationByExternalReference;
         rdfs:range :PredefinedLocation;
         rdf:type owl:FunctionalProperty;
         rdfs:label "predefinedLocationReference"@en .
:LocationByExternalReference rdfs:subClassOf [ rdf:type owl:Restriction ;
         owl:onProperty :predefinedLocationReference;
         owl:onClass :PredefinedLocation;
       owl:qualifiedCardinality "1"^^xsd:nonNegativeInteger ;
         ] .
:LocationByExternalReference rdfs:subClassOf [ rdf:type owl:Restriction ;
         owl:onProperty :predefinedLocationReference;
         owl:allValuesFrom :PredefinedLocation;
         ] .


### http://spec.tn-its.eu/owl/tnits-owl:NetworkElement
:NetworkElement a owl:Class ;
       rdfs:subClassOf <http://www.roadotl.eu/iso19148/def/LinearElement> ;
       rdfs:subClassOf :tnitsFeature ;
         skos:definition "Base type representing an element in a network. Every element in a network provides some function that is of interest in the network. "@en ;
       rdfs:label "NetworkElement"@en .

### http://spec.tn-its.eu/owl/tnits-owl#id
:id rdf:type owl:ObjectProperty ;
         skos:definition "External identifier of the network element."@en ;
         rdfs:domain :NetworkElement;
         rdfs:range :Identifier;
         rdfs:label "id"@en .
:NetworkElement rdfs:subClassOf [ rdf:type owl:Restriction ;
         owl:onProperty :id;
         owl:onClass :Identifier;
       owl:maxQualifiedCardinality "1"^^xsd:nonNegativeInteger ;
         ] .
:NetworkElement rdfs:subClassOf [ rdf:type owl:Restriction ;
         owl:onProperty :id;
         owl:allValuesFrom :Identifier;
         ] .


### http://spec.tn-its.eu/owl/tnits-owl:NetworkReference
:NetworkReference a owl:Class ;
       owl:equivalentClass <http://www.roadotl.eu/iso19148/def/LinearEventLocation> ;
       rdfs:subClassOf :tnitsDataType ;
         skos:definition "A general class defining a location reference by reference to a Network Reference "@en ;
       rdfs:label "NetworkReference"@en .

### http://spec.tn-its.eu/owl/tnits-owl#element
:element rdf:type owl:ObjectProperty ;
         skos:definition "The referenced network element."@en ;
         owl:equivalentProperty <http://www.roadotl.eu/iso19148/def/hasLinearElement> ;
         rdfs:domain :NetworkReference;
         rdfs:range :NetworkElement;
         rdf:type owl:FunctionalProperty;
         rdfs:label "element"@en .
:NetworkReference rdfs:subClassOf [ rdf:type owl:Restriction ;
         owl:onProperty :element;
         owl:onClass :NetworkElement;
       owl:qualifiedCardinality "1"^^xsd:nonNegativeInteger ;
         ] .
:NetworkReference rdfs:subClassOf [ rdf:type owl:Restriction ;
         owl:onProperty :element;
         owl:allValuesFrom :NetworkElement;
         ] .


### http://spec.tn-its.eu/owl/tnits-owl#overridingLRM
:overridingLRM rdf:type owl:ObjectProperty ;
         skos:definition "linear referencing method overriding default method for the data set"@en ;
         owl:equivalentProperty <http://www.roadotl.eu/iso19148/def/hasOverridingLRM> ;
         rdfs:domain :NetworkReference;
         rdfs:range <http://www.roadotl.eu/iso19148/def/LinearReferencingMethod>;
         rdfs:label "overridingLRM"@en .
:NetworkReference rdfs:subClassOf [ rdf:type owl:Restriction ;
         owl:onProperty :overridingLRM;
         owl:onClass <http://www.roadotl.eu/iso19148/def/LinearReferencingMethod>;
       owl:maxQualifiedCardinality "1"^^xsd:nonNegativeInteger ;
         ] .
:NetworkReference rdfs:subClassOf [ rdf:type owl:Restriction ;
         owl:onProperty :overridingLRM;
         owl:allValuesFrom <http://www.roadotl.eu/iso19148/def/LinearReferencingMethod>;
         ] .

:NetworkReference owl:disjointUnionOf ( :LinkReference  ) ; .

### http://spec.tn-its.eu/owl/tnits-owl:OpenLRBinaryVersion
:OpenLRBinaryVersion a owl:Class ;
       rdfs:subClassOf :tnitsCodeList ;
         skos:definition "Specifies the available list of enumerations for the version of the OpenLR binary specification"@en ;
       rdfs:label "OpenLRBinaryVersion"@en .

### http://spec.tn-its.eu/owl/tnits-owl:OpenLRBinaryVersionCode
:OpenLRBinaryVersionCode a skos:ConceptScheme ;
         skos:definition "Specifies the available list of enumerations for the version of the OpenLR binary specification"@en ;
       dc:isFormatOf :OpenLRBinaryVersion .

### http://spec.tn-its.eu/owl/tnits-owl:PredefinedLocation
:PredefinedLocation a owl:Class ;
       rdfs:subClassOf :tnitsCodeList ;
         skos:definition "Specifies the available list of enumerations for predefined locations "@en ;
       rdfs:label "PredefinedLocation"@en .

### http://spec.tn-its.eu/owl/tnits-owl:PredefinedLocationCode
:PredefinedLocationCode a skos:ConceptScheme ;
         skos:definition "Specifies the available list of enumerations for predefined locations "@en ;
       dc:isFormatOf :PredefinedLocation .

### http://spec.tn-its.eu/owl/tnits-owl:SimpleLinearReference
:SimpleLinearReference a owl:Class ;
       owl:equivalentClass <http://www.roadotl.eu/iso19148/def/LinearFromToLocation> ;
         skos:definition "A network reference that is restricted to part of a linear network element. The part is the part of the network element between fromPosition and toPosition. "@en ;
       rdfs:label "SimpleLinearReference"@en .
:SimpleLinearReference rdfs:subClassOf :LinkReference .
:SimpleLinearReference rdfs:subClassOf [ rdf:type owl:Restriction ;
         owl:onProperty <http://www.roadotl.eu/iso19148/def/fromPosition>;
         owl:onClass <http://www.roadotl.eu/iso19148/def/DistanceExpression>;
       owl:qualifiedCardinality "1"^^xsd:nonNegativeInteger ;
         ] .
:SimpleLinearReference rdfs:subClassOf [ rdf:type owl:Restriction ;
         owl:onProperty <http://www.roadotl.eu/iso19148/def/fromPosition>;
         owl:allValuesFrom <http://www.roadotl.eu/iso19148/def/DistanceExpression>;
         ] .

:SimpleLinearReference rdfs:subClassOf [ rdf:type owl:Restriction ;
         owl:onProperty <http://www.roadotl.eu/iso19148/def/toPosition>;
         owl:onClass <http://www.roadotl.eu/iso19148/def/DistanceExpression>;
       owl:qualifiedCardinality "1"^^xsd:nonNegativeInteger ;
         ] .
:SimpleLinearReference rdfs:subClassOf [ rdf:type owl:Restriction ;
         owl:onProperty <http://www.roadotl.eu/iso19148/def/toPosition>;
         owl:allValuesFrom <http://www.roadotl.eu/iso19148/def/DistanceExpression>;
         ] .


### http://spec.tn-its.eu/owl/tnits-owl:SimplePointReference
:SimplePointReference a owl:Class ;
       owl:equivalentClass <http://www.roadotl.eu/iso19148/def/LinearAtLocation> ;
         skos:definition "A network reference that is restricted to a point on a linear network element. The point is the location on the network element at the position atPosition along the network.  "@en ;
       rdfs:label "SimplePointReference"@en .
:SimplePointReference rdfs:subClassOf :LinkReference .
:SimplePointReference rdfs:subClassOf [ rdf:type owl:Restriction ;
         owl:onProperty <http://www.roadotl.eu/iso19148/def/atPosition>;
         owl:onClass <http://www.roadotl.eu/iso19148/def/DistanceExpression>;
       owl:qualifiedCardinality "1"^^xsd:nonNegativeInteger ;
         ] .
:SimplePointReference rdfs:subClassOf [ rdf:type owl:Restriction ;
         owl:onProperty <http://www.roadotl.eu/iso19148/def/atPosition>;
         owl:allValuesFrom <http://www.roadotl.eu/iso19148/def/DistanceExpression>;
         ] .


### http://spec.tn-its.eu/owl/tnits-owl:DynamicLocationReference
:DynamicLocationReference a owl:Class ;
         skos:definition "Abstract class that specifies all types of dynamic location references in accordance with ISO 19111. "@en ;
       rdfs:label "DynamicLocationReference"@en .
:DynamicLocationReference rdfs:subClassOf :LocationReference .
:DynamicLocationReference owl:disjointUnionOf ( :AgoraLocationReference :OpenLRLocationReference  ) ; .

### http://spec.tn-its.eu/owl/tnits-owl:PreCodedLocationReference
:PreCodedLocationReference a owl:Class ;
         skos:definition "Abstract class that serves as a placeholder for any type of precoded location reference that may be used in TN-ITS NOTE 1 Examples of precoded location references are: linear reference;  address; location code.  NOTE 2 Linear referencing is the preferred location referencing method for data associated with the road network in INSPIRE.   NOTE 3 This kind of location reference is classified as \"PreCoded\" in ISO 17572. "@en ;
       rdfs:label "PreCodedLocationReference"@en .
:PreCodedLocationReference rdfs:subClassOf :LocationReference .
:PreCodedLocationReference owl:disjointUnionOf ( :LinearLocationReference :LocationByExternalReference  ) ; .

### http://spec.tn-its.eu/owl/tnits-owl:AgoraLocationReference
:AgoraLocationReference a owl:Class ;
         skos:definition "A type of dynamic location reference that uses coordinates and core attribution according to ISO 17572-3.  "@en ;
       rdfs:label "AgoraLocationReference"@en .
:AgoraLocationReference rdfs:subClassOf :DynamicLocationReference .

### http://spec.tn-its.eu/owl/tnits-owl#AgoraLocationReference.base64String
:AgoraLocationReference.base64String rdf:type owl:DatatypeProperty ;
         skos:definition "The AGORA binary string encoded using base64 "@en ;
         rdfs:domain :AgoraLocationReference;
         rdfs:range xsd:string;
         rdf:type owl:FunctionalProperty;
         rdfs:label "AgoraLocationReference.base64String"@en .
:AgoraLocationReference rdfs:subClassOf [ rdf:type owl:Restriction ;
         owl:onProperty :AgoraLocationReference.base64String;
         owl:onDataRange xsd:string;
       owl:qualifiedCardinality "1"^^xsd:nonNegativeInteger ;
         ] .
:AgoraLocationReference rdfs:subClassOf [ rdf:type owl:Restriction ;
         owl:onProperty :AgoraLocationReference.base64String;
         owl:allValuesFrom xsd:string;
         ] .


### http://spec.tn-its.eu/owl/tnits-owl#AgoraLocationReference.agoraBinaryVersion
:AgoraLocationReference.agoraBinaryVersion rdf:type owl:ObjectProperty ;
         skos:definition "Provides reference to the version of the AGORA Binary string encoding used by reference to an item in an external code list (see AgoraBinaryVersion Class)"@en ;
         rdfs:domain :AgoraLocationReference;
         rdfs:range :AgoraBinaryVersion;
         rdf:type owl:FunctionalProperty;
         rdfs:label "AgoraLocationReference.agoraBinaryVersion"@en .
:AgoraLocationReference rdfs:subClassOf [ rdf:type owl:Restriction ;
         owl:onProperty :AgoraLocationReference.agoraBinaryVersion;
         owl:onClass :AgoraBinaryVersion;
       owl:qualifiedCardinality "1"^^xsd:nonNegativeInteger ;
         ] .
:AgoraLocationReference rdfs:subClassOf [ rdf:type owl:Restriction ;
         owl:onProperty :AgoraLocationReference.agoraBinaryVersion;
         owl:allValuesFrom :AgoraBinaryVersion;
         ] .


### http://spec.tn-its.eu/owl/tnits-owl:OpenLRLocationReference
:OpenLRLocationReference a owl:Class ;
         skos:definition "A type of dynamic location reference that uses coordinates and core attribution according to the OpenLR specification (see bibliography)  "@en ;
       rdfs:label "OpenLRLocationReference"@en .
:OpenLRLocationReference rdfs:subClassOf :DynamicLocationReference .

### http://spec.tn-its.eu/owl/tnits-owl#OpenLRLocationReference.binaryLocationReference
:OpenLRLocationReference.binaryLocationReference rdf:type owl:ObjectProperty ;
         skos:definition "OpenLR location reference using binary encoding "@en ;
         rdfs:domain :OpenLRLocationReference;
         rdfs:range :BinaryLocationReference;
         rdfs:label "OpenLRLocationReference.binaryLocationReference"@en .
:OpenLRLocationReference rdfs:subClassOf [ rdf:type owl:Restriction ;
         owl:onProperty :OpenLRLocationReference.binaryLocationReference;
         owl:onClass :BinaryLocationReference;
       owl:maxQualifiedCardinality "1"^^xsd:nonNegativeInteger ;
         ] .
:OpenLRLocationReference rdfs:subClassOf [ rdf:type owl:Restriction ;
         owl:onProperty :OpenLRLocationReference.binaryLocationReference;
         owl:allValuesFrom :BinaryLocationReference;
         ] .


### http://spec.tn-its.eu/owl/tnits-owl#OpenLRLocationReference.xMLLocationReference
:OpenLRLocationReference.xMLLocationReference rdf:type owl:ObjectProperty ;
         skos:definition "OpenLR location reference using XML encoding "@en ;
         rdfs:domain :OpenLRLocationReference;
         rdfs:range :XMLLocationReference;
         rdfs:label "OpenLRLocationReference.xMLLocationReference"@en .
:OpenLRLocationReference rdfs:subClassOf [ rdf:type owl:Restriction ;
         owl:onProperty :OpenLRLocationReference.xMLLocationReference;
         owl:onClass :XMLLocationReference;
       owl:maxQualifiedCardinality "1"^^xsd:nonNegativeInteger ;
         ] .
:OpenLRLocationReference rdfs:subClassOf [ rdf:type owl:Restriction ;
         owl:onProperty :OpenLRLocationReference.xMLLocationReference;
         owl:allValuesFrom :XMLLocationReference;
         ] .


### http://spec.tn-its.eu/owl/tnits-owl:LinearLocationReference
:LinearLocationReference a owl:Class ;
         skos:definition "A type of precoded location reference that references a location by use of a specified reference  "@en ;
       rdfs:label "LinearLocationReference"@en .
:LinearLocationReference rdfs:subClassOf :PreCodedLocationReference .

### http://spec.tn-its.eu/owl/tnits-owl#LinearLocationReference.networkReference
:LinearLocationReference.networkReference rdf:type owl:ObjectProperty ;
         skos:definition "A link to a specific network reference "@en ;
         rdfs:domain :LinearLocationReference;
         rdfs:range :NetworkReference;
         rdfs:label "LinearLocationReference.networkReference"@en .
:LinearLocationReference rdfs:subClassOf [ rdf:type owl:Restriction ;
         owl:onProperty :LinearLocationReference.networkReference;
         owl:onClass :NetworkReference;
       owl:minQualifiedCardinality "1"^^xsd:nonNegativeInteger ;
         ] .
:LinearLocationReference rdfs:subClassOf [ rdf:type owl:Restriction ;
         owl:onProperty :LinearLocationReference.networkReference;
         owl:allValuesFrom :NetworkReference;
         ] .


### http://spec.tn-its.eu/owl/tnits-owl#name
:name rdf:type owl:DatatypeProperty ;
         skos:definition "A free text string providing the name for the linear location "@en ;
         rdfs:domain :LinearLocationReference;
         rdfs:range xsd:string;
         rdfs:label "name"@en .
:LinearLocationReference rdfs:subClassOf [ rdf:type owl:Restriction ;
         owl:onProperty :name;
         owl:onDataRange xsd:string;
       owl:maxQualifiedCardinality "1"^^xsd:nonNegativeInteger ;
         ] .
:LinearLocationReference rdfs:subClassOf [ rdf:type owl:Restriction ;
         owl:onProperty :name;
         owl:allValuesFrom xsd:string;
         ] .


### http://spec.tn-its.eu/owl/tnits-owl#description
:description rdf:type owl:DatatypeProperty ;
         skos:definition "A free text string providing a description for the linear location "@en ;
         rdfs:domain :LinearLocationReference;
         rdfs:range xsd:string;
         rdfs:label "description"@en .
:LinearLocationReference rdfs:subClassOf [ rdf:type owl:Restriction ;
         owl:onProperty :description;
         owl:onDataRange xsd:string;
       owl:maxQualifiedCardinality "1"^^xsd:nonNegativeInteger ;
         ] .
:LinearLocationReference rdfs:subClassOf [ rdf:type owl:Restriction ;
         owl:onProperty :description;
         owl:allValuesFrom xsd:string;
         ] .


### http://spec.tn-its.eu/owl/tnits-owl:LocationReference
:LocationReference a owl:Class ;
       rdfs:subClassOf :tnitsDataType ;
         skos:definition "Abstract class that specifies any type of location reference for TN-ITS "@en ;
       rdfs:label "LocationReference"@en .
:LocationReference owl:disjointUnionOf ( :GeometryLocationReference :PreCodedLocationReference :DynamicLocationReference  ) ; .


### http://spec.tn-its.eu/owl/tnits-owl:UpdateInfo
:UpdateInfo a owl:Class ;
       rdfs:subClassOf :tnitsDataType ;
         skos:definition "Characterises the nature of the update for a road feature "@en ;
       rdfs:label "UpdateInfo"@en .

### http://spec.tn-its.eu/owl/tnits-owl#UpdateInfo.type
:UpdateInfo.type rdf:type owl:ObjectProperty ;
         skos:definition "The type of update "@en ;
         rdfs:domain :UpdateInfo;
         rdfs:range :UpdateType;
         rdf:type owl:FunctionalProperty;
         rdfs:label "UpdateInfo.type"@en .
:UpdateInfo rdfs:subClassOf [ rdf:type owl:Restriction ;
         owl:onProperty :UpdateInfo.type;
         owl:onClass :UpdateType;
       owl:qualifiedCardinality "1"^^xsd:nonNegativeInteger ;
         ] .
:UpdateInfo rdfs:subClassOf [ rdf:type owl:Restriction ;
         owl:onProperty :UpdateInfo.type;
         owl:allValuesFrom :UpdateType;
         ] .


### http://spec.tn-its.eu/owl/tnits-owl:UpdateType
:UpdateType a owl:Class ;
       rdfs:subClassOf :tnitsEnumeration ;
         skos:definition "Defines the different update types "@en ;
       rdfs:label "UpdateType"@en .

### http://spec.tn-its.eu/owl/tnits-owl:UpdateTypeCode
:UpdateTypeCode a skos:ConceptScheme ;
         skos:definition "Defines the different update types "@en ;
       dc:isFormatOf :UpdateType .

### http://spec.tn-its.eu/owl/tnits-owl:UpdateType.Add
:UpdateType.Add a :UpdateType,skos:Concept ;
         skos:inScheme :UpdateTypeCode ;
         skos:definition "A new feature is inserted at the referenced location, without affecting any existing attribute feature "@en ;
         rdfs:label "Add"@no .

### http://spec.tn-its.eu/owl/tnits-owl:UpdateType.Modify
:UpdateType.Modify a :UpdateType,skos:Concept ;
         skos:inScheme :UpdateTypeCode ;
         skos:definition "Signals a modification of the attributes of an existing road feature referenced by an object identifier "@en ;
         rdfs:label "Modify"@no .

### http://spec.tn-its.eu/owl/tnits-owl:UpdateType.Remove
:UpdateType.Remove a :UpdateType,skos:Concept ;
         skos:inScheme :UpdateTypeCode ;
         skos:definition "Signals a removal of the existing road feature referenced by an object identifier "@en ;
         rdfs:label "Remove"@no .
:UpdateType owl:oneOf ( :UpdateType.Add :UpdateType.Modify :UpdateType.Remove  ) ; .


### http://spec.tn-its.eu/owl/tnits-owl:FeedbackInformation
:FeedbackInformation a owl:Class ;
       rdfs:subClassOf :tnitsFeature ;
         skos:definition "Represents the information sent back from a downloading client to the provider of road attributes  "@en ;
       rdfs:label "FeedbackInformation"@en .

### http://spec.tn-its.eu/owl/tnits-owl#log
:log rdf:type owl:ObjectProperty ;
         skos:definition "Refers to a log which records all the interesting events during download and integration of road features. "@en ;
         rdfs:domain :FeedbackInformation;
         rdfs:range :FeedbackLog;
         rdf:type owl:FunctionalProperty;
         rdfs:label "log"@en .
:FeedbackInformation rdfs:subClassOf [ rdf:type owl:Restriction ;
         owl:onProperty :log;
         owl:onClass :FeedbackLog;
       owl:qualifiedCardinality "1"^^xsd:nonNegativeInteger ;
         ] .
:FeedbackInformation rdfs:subClassOf [ rdf:type owl:Restriction ;
         owl:onProperty :log;
         owl:allValuesFrom :FeedbackLog;
         ] .


### http://spec.tn-its.eu/owl/tnits-owl#datasetId
:datasetId rdf:type owl:ObjectProperty ;
         skos:definition "The identification of the dataset which is the source of this feedback information. This identifier shall correspond to the metadata element Unique resource identifier in the dataset for which the feedback is created."@en ;
         rdfs:range :Identifier;
         rdfs:label "datasetId"@en .
:FeedbackInformation rdfs:subClassOf [ rdf:type owl:Restriction ;
         owl:onProperty :datasetId;
         owl:onClass :Identifier;
       owl:qualifiedCardinality "1"^^xsd:nonNegativeInteger ;
         ] .
:FeedbackInformation rdfs:subClassOf [ rdf:type owl:Restriction ;
         owl:onProperty :datasetId;
         owl:allValuesFrom :Identifier;
         ] .


### http://spec.tn-its.eu/owl/tnits-owl#processed
:processed rdf:type owl:DatatypeProperty ;
         skos:definition "The declared date and time when the dataset was processed "@en ;
         rdfs:domain :FeedbackInformation;
         rdfs:range xsd:dateTime;
         rdf:type owl:FunctionalProperty;
         rdfs:label "processed"@en .
:FeedbackInformation rdfs:subClassOf [ rdf:type owl:Restriction ;
         owl:onProperty :processed;
         owl:onDataRange xsd:dateTime;
       owl:qualifiedCardinality "1"^^xsd:nonNegativeInteger ;
         ] .
:FeedbackInformation rdfs:subClassOf [ rdf:type owl:Restriction ;
         owl:onProperty :processed;
         owl:allValuesFrom xsd:dateTime;
         ] .


### http://spec.tn-its.eu/owl/tnits-owl:FeedbackLog
:FeedbackLog a owl:Class ;
       rdfs:subClassOf :tnitsFeature ;
         skos:definition "Represents a log which records all events that are reported back from a client as a result of download and integration of data  "@en ;
       rdfs:label "FeedbackLog"@en .

### http://spec.tn-its.eu/owl/tnits-owl#summary
:summary rdf:type owl:ObjectProperty ;
         skos:definition "A result summary "@en ;
         rdfs:domain :FeedbackLog;
         rdfs:range :SummaryInfo;
         rdf:type owl:FunctionalProperty;
         rdfs:label "summary"@en .
:FeedbackLog rdfs:subClassOf [ rdf:type owl:Restriction ;
         owl:onProperty :summary;
         owl:onClass :SummaryInfo;
       owl:qualifiedCardinality "1"^^xsd:nonNegativeInteger ;
         ] .
:FeedbackLog rdfs:subClassOf [ rdf:type owl:Restriction ;
         owl:onProperty :summary;
         owl:allValuesFrom :SummaryInfo;
         ] .


### http://spec.tn-its.eu/owl/tnits-owl#events
:events rdf:type owl:ObjectProperty ;
         skos:definition "The set of Refers to a log which records all the interesting events during download and integration of road features. "@en ;
         rdfs:domain :FeedbackLog;
         rdfs:range :FeedbackLogEvent;
         rdfs:label "events"@en .
:FeedbackLog rdfs:subClassOf [ rdf:type owl:Restriction ;
         owl:onProperty :events;
         owl:allValuesFrom :FeedbackLogEvent;
         ] .


### http://spec.tn-its.eu/owl/tnits-owl:FeedbackLogEvent
:FeedbackLogEvent a owl:Class ;
       rdfs:subClassOf :tnitsFeature ;
         skos:definition "Abstract base class that represents any type of event that may occur during download and integration of data that needs to be reported back to the provider  "@en ;
       rdfs:label "FeedbackLogEvent"@en .
:FeedbackLogEvent owl:disjointUnionOf ( :GeneralFeedbackEvent :FreeTextEvent :RoadFeatureEvent  ) ; .

### http://spec.tn-its.eu/owl/tnits-owl:FreeTextEvent
:FreeTextEvent a owl:Class ;
         skos:definition "Represents one event that is described using free text  "@en ;
       rdfs:label "FreeTextEvent"@en .
:FreeTextEvent rdfs:subClassOf :FeedbackLogEvent .

### http://spec.tn-its.eu/owl/tnits-owl#FreeTextEvent.text
:FreeTextEvent.text rdf:type owl:DatatypeProperty ;
         skos:definition "The text describing the event "@en ;
         rdfs:domain :FreeTextEvent;
         rdfs:range xsd:string;
         rdf:type owl:FunctionalProperty;
         rdfs:label "FreeTextEvent.text"@en .
:FreeTextEvent rdfs:subClassOf [ rdf:type owl:Restriction ;
         owl:onProperty :FreeTextEvent.text;
         owl:onDataRange xsd:string;
       owl:qualifiedCardinality "1"^^xsd:nonNegativeInteger ;
         ] .
:FreeTextEvent rdfs:subClassOf [ rdf:type owl:Restriction ;
         owl:onProperty :FreeTextEvent.text;
         owl:allValuesFrom xsd:string;
         ] .


### http://spec.tn-its.eu/owl/tnits-owl:GeneralFeedbackEvent
:GeneralFeedbackEvent a owl:Class ;
         skos:definition "Represents one event that may occur during download and integration of data that needs to be reported back to the provider  "@en ;
       rdfs:label "GeneralFeedbackEvent"@en .
:GeneralFeedbackEvent rdfs:subClassOf :FeedbackLogEvent .

### http://spec.tn-its.eu/owl/tnits-owl#eventCode
:eventCode rdf:type owl:ObjectProperty ;
         skos:definition "Indicates the type of event that occurred "@en ;
         rdfs:label "eventCode"@en .
:GeneralFeedbackEvent rdfs:subClassOf [ rdf:type owl:Restriction ;
         owl:onProperty :eventCode;
         owl:onClass :GeneralFeedbackEventType;
       owl:qualifiedCardinality "1"^^xsd:nonNegativeInteger ;
         ] .
:GeneralFeedbackEvent rdfs:subClassOf [ rdf:type owl:Restriction ;
         owl:onProperty :eventCode;
         owl:allValuesFrom :GeneralFeedbackEventType;
         ] .


### http://spec.tn-its.eu/owl/tnits-owl:GeneralFeedbackEventType
:GeneralFeedbackEventType a owl:Class ;
       rdfs:subClassOf :tnitsCodeList ;
         skos:definition "Specifies the available list of enumerations for types of general feedback events."@en ;
       rdfs:label "GeneralFeedbackEventType"@en .

### http://spec.tn-its.eu/owl/tnits-owl:GeneralFeedbackEventTypeCode
:GeneralFeedbackEventTypeCode a skos:ConceptScheme ;
         skos:definition "Specifies the available list of enumerations for types of general feedback events."@en ;
       dc:isFormatOf :GeneralFeedbackEventType .

### http://spec.tn-its.eu/owl/tnits-owl:RoadFeatureEvent
:RoadFeatureEvent a owl:Class ;
         skos:definition "Represents one event that may occur during download and integration of data that needs to be reported back to the provider  "@en ;
       rdfs:label "RoadFeatureEvent"@en .
:RoadFeatureEvent rdfs:subClassOf :FeedbackLogEvent .
:RoadFeatureEvent rdfs:subClassOf [ rdf:type owl:Restriction ;
         owl:onProperty :roadFeatureId;
         owl:onClass :Identifier;
       owl:qualifiedCardinality "1"^^xsd:nonNegativeInteger ;
         ] .
:RoadFeatureEvent rdfs:subClassOf [ rdf:type owl:Restriction ;
         owl:onProperty :roadFeatureId;
         owl:allValuesFrom :Identifier;
         ] .


### http://spec.tn-its.eu/owl/tnits-owl#RoadFeatureEvent.roadFeaturePropertyType
:RoadFeatureEvent.roadFeaturePropertyType rdf:type owl:ObjectProperty ;
         skos:definition "The identification of the road feature property type that is concerned by the event. If unset, this event does not concern any road feature property type in particular. "@en ;
         rdfs:domain :RoadFeatureEvent;
         rdfs:range :RoadFeaturePropertyType;
         rdf:type owl:FunctionalProperty;
         rdfs:label "RoadFeatureEvent.roadFeaturePropertyType"@en .
:RoadFeatureEvent rdfs:subClassOf [ rdf:type owl:Restriction ;
         owl:onProperty :RoadFeatureEvent.roadFeaturePropertyType;
         owl:onClass :RoadFeaturePropertyType;
       owl:qualifiedCardinality "1"^^xsd:nonNegativeInteger ;
         ] .
:RoadFeatureEvent rdfs:subClassOf [ rdf:type owl:Restriction ;
         owl:onProperty :RoadFeatureEvent.roadFeaturePropertyType;
         owl:allValuesFrom :RoadFeaturePropertyType;
         ] .

:RoadFeatureEvent rdfs:subClassOf [ rdf:type owl:Restriction ;
         owl:onProperty :eventCode;
         owl:onClass :RoadFeatureEventType;
       owl:qualifiedCardinality "1"^^xsd:nonNegativeInteger ;
         ] .
:RoadFeatureEvent rdfs:subClassOf [ rdf:type owl:Restriction ;
         owl:onProperty :eventCode;
         owl:allValuesFrom :RoadFeatureEventType;
         ] .


### http://spec.tn-its.eu/owl/tnits-owl:RoadFeatureEventType
:RoadFeatureEventType a owl:Class ;
       rdfs:subClassOf :tnitsCodeList ;
         skos:definition "Specifies the available list of enumerations for the types of Road Feature Events"@en ;
       rdfs:label "RoadFeatureEventType"@en .

### http://spec.tn-its.eu/owl/tnits-owl:RoadFeatureEventTypeCode
:RoadFeatureEventTypeCode a skos:ConceptScheme ;
         skos:definition "Specifies the available list of enumerations for the types of Road Feature Events"@en ;
       dc:isFormatOf :RoadFeatureEventType .

### http://spec.tn-its.eu/owl/tnits-owl:SummaryInfo
:SummaryInfo a owl:Class ;
       rdfs:subClassOf :tnitsDataType ;
         skos:definition "Information that summarizes a feedback result "@en ;
       rdfs:label "SummaryInfo"@en .

### http://spec.tn-its.eu/owl/tnits-owl#nrSuccess
:nrSuccess rdf:type owl:DatatypeProperty ;
         skos:definition "Number of successfully decoded and integrated road features. "@en ;
         rdfs:domain :SummaryInfo;
         rdfs:range xsd:integer;
         rdf:type owl:FunctionalProperty;
         rdfs:label "nrSuccess"@en .
:SummaryInfo rdfs:subClassOf [ rdf:type owl:Restriction ;
         owl:onProperty :nrSuccess;
         owl:onDataRange xsd:integer;
       owl:qualifiedCardinality "1"^^xsd:nonNegativeInteger ;
         ] .
:SummaryInfo rdfs:subClassOf [ rdf:type owl:Restriction ;
         owl:onProperty :nrSuccess;
         owl:allValuesFrom xsd:integer;
         ] .


### http://spec.tn-its.eu/owl/tnits-owl#nrFail
:nrFail rdf:type owl:DatatypeProperty ;
         skos:definition "Number of road features for which integration failed. "@en ;
         rdfs:domain :SummaryInfo;
         rdfs:range xsd:integer;
         rdf:type owl:FunctionalProperty;
         rdfs:label "nrFail"@en .
:SummaryInfo rdfs:subClassOf [ rdf:type owl:Restriction ;
         owl:onProperty :nrFail;
         owl:onDataRange xsd:integer;
       owl:qualifiedCardinality "1"^^xsd:nonNegativeInteger ;
         ] .
:SummaryInfo rdfs:subClassOf [ rdf:type owl:Restriction ;
         owl:onProperty :nrFail;
         owl:allValuesFrom xsd:integer;
         ] .



### http://spec.tn-its.eu/owl/tnits-owl:XMLLocationReference
:XMLLocationReference a owl:Class ;
       rdfs:subClassOf :tnitsDataType ;
         skos:definition "A OpenLR location reference encoded using XML according to the OpenLR specification (see bibliography)  "@en ;
       rdfs:label "XMLLocationReference"@en .


### http://spec.tn-its.eu/owl/tnits-owl:DCAT
:DCAT a owl:Class ;
       rdfs:label "DCAT"@en .

### http://spec.tn-its.eu/owl/tnits-owl:Metadata
:Metadata a owl:Class ;
       rdfs:subClassOf :tnitsDataType ;
         skos:definition "Characterises the type of metadata "@en ;
       rdfs:label "Metadata"@en .

### http://spec.tn-its.eu/owl/tnits-owl#ISO19115Metadata
:ISO19115Metadata rdf:type owl:ObjectProperty ;
         rdfs:domain :Metadata;
         rdfs:range <http://def.isotc211.org/iso19115/-1/2014/MetadataInformation#MD_Metadata>;
         rdfs:label "ISO19115Metadata"@en .
:Metadata rdfs:subClassOf [ rdf:type owl:Restriction ;
         owl:onProperty :ISO19115Metadata;
         owl:onClass <http://def.isotc211.org/iso19115/-1/2014/MetadataInformation#MD_Metadata>;
       owl:maxQualifiedCardinality "1"^^xsd:nonNegativeInteger ;
         ] .
:Metadata rdfs:subClassOf [ rdf:type owl:Restriction ;
         owl:onProperty :ISO19115Metadata;
         owl:allValuesFrom <http://def.isotc211.org/iso19115/-1/2014/MetadataInformation#MD_Metadata>;
         ] .

:Metadata rdfs:subClassOf [ rdf:type owl:Restriction ;
         owl:onProperty :datasetId;
         owl:onClass :Identifier;
       owl:qualifiedCardinality "1"^^xsd:nonNegativeInteger ;
         ] .
:Metadata rdfs:subClassOf [ rdf:type owl:Restriction ;
         owl:onProperty :datasetId;
         owl:allValuesFrom :Identifier;
         ] .


### http://spec.tn-its.eu/owl/tnits-owl#datasetCreationTime
:datasetCreationTime rdf:type owl:DatatypeProperty ;
         skos:definition "Indicates when the metadata are created "@en ;
         rdfs:domain :Metadata;
         rdfs:range xsd:dateTime;
         rdf:type owl:FunctionalProperty;
         rdfs:label "datasetCreationTime"@en .
:Metadata rdfs:subClassOf [ rdf:type owl:Restriction ;
         owl:onProperty :datasetCreationTime;
         owl:onDataRange xsd:dateTime;
       owl:qualifiedCardinality "1"^^xsd:nonNegativeInteger ;
         ] .
:Metadata rdfs:subClassOf [ rdf:type owl:Restriction ;
         owl:onProperty :datasetCreationTime;
         owl:allValuesFrom xsd:dateTime;
         ] .

:tnitsFeature owl:disjointUnionOf ( :Dataset :RoadFeature :NetworkElement :FeedbackInformation :FeedbackLog :FeedbackLogEvent     ) ; .
:tnitsEnumeration owl:disjointUnionOf ( :DatasetType :ConditionOperator :DayOfWeek :MonthOfYear :WeekOfMonth :ComparisonOperator :UpdateType     ) ; .
:tnitsDataType owl:disjointUnionOf ( :Identifier :AbstractRoadFeatureProperty :RoadSignContent :Condition :OverallPeriod :Period :SpecialDay :TimePeriodOfDay :Validity :FuzzyTimePeriod :DayWeekMonth :Emissions :GrossWeightCharacteristic :HeaviestAxleWeightCharacteristic :HeightCharacteristic :LengthCharacteristic :NumberOfAxlesCharacteristic :VehicleCharacteristics :WidthCharacteristic :BinaryLocationReference :NetworkReference :LocationReference :UpdateInfo :SummaryInfo :XMLLocationReference :Metadata     ) ; .
