@prefix : <http://spec.tn-its.eu/owl/tnits-owl#> .
@prefix dc: <http://purl.org/dc/elements/1.1/> .
@prefix owl: <http://www.w3.org/2002/07/owl#> .
@prefix rdf: <http://www.w3.org/1999/02/22-rdf-syntax-ns#> .
@prefix xml: <http://www.w3.org/XML/1998/namespace> .
@prefix xsd: <http://www.w3.org/2001/XMLSchema#> .
@prefix rdfs: <http://www.w3.org/2000/01/rdf-schema#> .
@prefix skos: <http://www.w3.org/2004/02/skos/core#> .
@prefix tnits: <http://spec.tn-its.eu/owl/tnits-owl#> .
@prefix dcterms: <http://purl.org/dc/terms/> .
@base <http://spec.tn-its.eu/owl/tnits-owl> .

<http://spec.tn-its.eu/owl/tnits-owl/codes> a owl:Ontology ;
	owl:imports <http://www.w3.org/2004/02/skos/core> ;
	dc:creator "TN-ITS" ;
	dc:date "20211006" ;
	dc:description "Code list values for TN-ITS code lists"@en ;
	dcterms:title "TN-ITS Codes"@en.
    
    

:WeightTypeCode a skos:ConceptScheme ;
    dc:isFormatOf :WeightType ;
    	skos:definition "Type of weight - describing the meaning of a vehicle weight value" .
    
    
:WeightType.actual a :WeightType, skos:Concept  ;
         skos:inScheme :WeightTypeCode ;
         rdfs:label "actual"@en ;
         skos:definition "The weight is the actual weight of a specific vehicle"@en .
         :WeightType.maximumPermitted a :WeightType, skos:Concept  ;
         skos:inScheme :WeightTypeCode ;
         rdfs:label "maximumPermitted"@en ;
         skos:definition "The weight is the maximum permitted weight for a vehicle"@en .
         

:ParkingSiteTypeCode a skos:ConceptScheme ;
    dc:isFormatOf :ParkingSiteType ;
    	skos:definition "Specifies the available list of enumerations for the types of parking sites" .
    
    
:ParkingSiteType.urbanParkingSite a :ParkingSiteType, skos:Concept  ;
         skos:inScheme :ParkingSiteTypeCode ;
         rdfs:label "urbanParkingSite"@en ;
         skos:definition "parking site in an urban context (e.g. parking lot, parking garage, on-street-parking, parkAndRide)"@en .
         :ParkingSiteType.interUrbanParkingSite a :ParkingSiteType, skos:Concept  ;
         skos:inScheme :ParkingSiteTypeCode ;
         rdfs:label "interUrbanParkingSite"@en ;
         skos:definition "A parking site in an interurban context (like nearby motorway, motorway, ferry terminal, airport terminal, on street parking)"@en .
         :ParkingSiteType.specialLocationParkingSite a :ParkingSiteType, skos:Concept  ;
         skos:inScheme :ParkingSiteTypeCode ;
         rdfs:label "specialLocationParkingSite"@en ;
         skos:definition "A parking site which is located at a special location, often associated with some building"@en .
         

:WeatherTypeCode a skos:ConceptScheme ;
    dc:isFormatOf :WeatherType ;
    	skos:definition "Types of weather conditions which affect driving conditions." .
    
    
:WeatherType.fog a :WeatherType, skos:Concept  ;
         skos:inScheme :WeatherTypeCode ;
         rdfs:label "fog"@en ;
         skos:definition "Fog, with reduced visibility"@en .
         :WeatherType.ice a :WeatherType, skos:Concept  ;
         skos:inScheme :WeatherTypeCode ;
         rdfs:label "ice"@en ;
         skos:definition "Increased skid risk due to ice (of any kind)"@en .
         :WeatherType.rain a :WeatherType, skos:Concept  ;
         skos:inScheme :WeatherTypeCode ;
         rdfs:label "rain"@en ;
         skos:definition "Rain, with reduced visibility, and increased skid risk"@en .
         :WeatherType.airPollution a :WeatherType, skos:Concept  ;
         skos:inScheme :WeatherTypeCode ;
         rdfs:label "airPollution"@en ;
         skos:definition "Air pollution"@en .
         :WeatherType.snow a :WeatherType, skos:Concept  ;
         skos:inScheme :WeatherTypeCode ;
         rdfs:label "snow"@en ;
         skos:definition "Snow, with reduced visibility, and increased skid risk"@en .
         :WeatherType.wind a :WeatherType, skos:Concept  ;
         skos:inScheme :WeatherTypeCode ;
         rdfs:label "wind"@en ;
         skos:definition "Wind conditions on the road"@en .
         :WeatherType.wet a :WeatherType, skos:Concept  ;
         skos:inScheme :WeatherTypeCode ;
         rdfs:label "wet"@en ;
         skos:definition "Road surface is wet"@en .
         

:AreaTypeCode a skos:ConceptScheme ;
    dc:isFormatOf :AreaType ;
    	skos:definition "Specifies the available list of enumerations for the area type condition for a road feature " .
    
    
:AreaType.inNationalPark a :AreaType, skos:Concept  ;
         skos:inScheme :AreaTypeCode ;
         rdfs:label "inNationalPark"@en ;
         skos:definition "Within the boundary of a recognised national park"@en .
         :AreaType.insideCities a :AreaType, skos:Concept  ;
         skos:inScheme :AreaTypeCode ;
         rdfs:label "insideCities"@en ;
         skos:definition "Within the notional or actual boundary of a city"@en .
         :AreaType.nearRailroadCrossing a :AreaType, skos:Concept  ;
         skos:inScheme :AreaTypeCode ;
         rdfs:label "nearRailroadCrossing"@en ;
         skos:definition "In close proximity to a railway level crossing"@en .
         :AreaType.nearSchool a :AreaType, skos:Concept  ;
         skos:inScheme :AreaTypeCode ;
         rdfs:label "nearSchool"@en ;
         skos:definition "In close proximity to a school"@en .
         :AreaType.outsideCities a :AreaType, skos:Concept  ;
         skos:inScheme :AreaTypeCode ;
         rdfs:label "outsideCities"@en ;
         skos:definition "Outside the notional or actual boundary of a city"@en .
         :AreaType.trafficCalmingArea a :AreaType, skos:Concept  ;
         skos:inScheme :AreaTypeCode ;
         rdfs:label "trafficCalmingArea"@en ;
         skos:definition "In a zone which is subject to traffic calming measures"@en .
         

:RoadSignTypeCode a skos:ConceptScheme ;
    dc:isFormatOf :RoadSignType ;
    	skos:definition "Specifies the available list of enumerations for the road sign types, defined in accordance with ISO 14823" .
    
    
:RoadSignType.11_111 a :RoadSignType, skos:Concept  ;
         skos:inScheme :RoadSignTypeCode ;
         rdfs:label "11_111"@en ;
         skos:definition "Intersection where the priority is prescribed by the general priority rule (Crossroads)"@en .
         :RoadSignType.11_112 a :RoadSignType, skos:Concept  ;
         skos:inScheme :RoadSignTypeCode ;
         rdfs:label "11_112"@en ;
         skos:definition "Intersection where the priority is prescribed by the general priority rule (Side road right)"@en .
         :RoadSignType.11_113 a :RoadSignType, skos:Concept  ;
         skos:inScheme :RoadSignTypeCode ;
         rdfs:label "11_113"@en ;
         skos:definition "Intersection where the priority is prescribed by the general priority rule (Side road left)"@en .
         :RoadSignType.11_115 a :RoadSignType, skos:Concept  ;
         skos:inScheme :RoadSignTypeCode ;
         rdfs:label "11_115"@en ;
         skos:definition "Intersection where the priority is prescribed by the general priority rule (Forked Intersection)"@en .
         :RoadSignType.11_116 a :RoadSignType, skos:Concept  ;
         skos:inScheme :RoadSignTypeCode ;
         rdfs:label "11_116"@en ;
         skos:definition "Intersection where the priority is prescribed by the general priority rule (T junction)"@en .
         :RoadSignType.11_117 a :RoadSignType, skos:Concept  ;
         skos:inScheme :RoadSignTypeCode ;
         rdfs:label "11_117"@en ;
         skos:definition "Intersection where the priority is prescribed by the general priority rule (Y intersection)"@en .
         :RoadSignType.11_118 a :RoadSignType, skos:Concept  ;
         skos:inScheme :RoadSignTypeCode ;
         rdfs:label "11_118"@en ;
         skos:definition "Intersection where the priority is prescribed by the general priority rule (Staggered intersection)"@en .
         :RoadSignType.11_132 a :RoadSignType, skos:Concept  ;
         skos:inScheme :RoadSignTypeCode ;
         rdfs:label "11_132"@en ;
         skos:definition "Intersection with a road the users of which must give way"@en .
         :RoadSignType.11_133 a :RoadSignType, skos:Concept  ;
         skos:inScheme :RoadSignTypeCode ;
         rdfs:label "11_133"@en ;
         skos:definition "Intersection with a road the users of which must give way  T-shaped crossing left "@en .
         :RoadSignType.11_134 a :RoadSignType, skos:Concept  ;
         skos:inScheme :RoadSignTypeCode ;
         rdfs:label "11_134"@en ;
         skos:definition "Intersection with a road the users of which must give way  T-shaped crossing righ "@en .
         :RoadSignType.11_135 a :RoadSignType, skos:Concept  ;
         skos:inScheme :RoadSignTypeCode ;
         rdfs:label "11_135"@en ;
         skos:definition "Intersection with a road the users of which must give way T-shaped crossing of folk type Lower left"@en .
         :RoadSignType.11_136 a :RoadSignType, skos:Concept  ;
         skos:inScheme :RoadSignTypeCode ;
         rdfs:label "11_136"@en ;
         skos:definition "Intersection with a road the users of which must give way T-shaped crossing of folk type Lower right"@en .
         :RoadSignType.11_148 a :RoadSignType, skos:Concept  ;
         skos:inScheme :RoadSignTypeCode ;
         rdfs:label "11_148"@en ;
         skos:definition "Warning of roundabout (Clockwise)   "@en .
         :RoadSignType.11_149 a :RoadSignType, skos:Concept  ;
         skos:inScheme :RoadSignTypeCode ;
         rdfs:label "11_149"@en ;
         skos:definition "Warning of roundabout (Anti-clockwise)   "@en .
         :RoadSignType.11_161 a :RoadSignType, skos:Concept  ;
         skos:inScheme :RoadSignTypeCode ;
         rdfs:label "11_161"@en ;
         skos:definition "Right bend"@en .
         :RoadSignType.11_162 a :RoadSignType, skos:Concept  ;
         skos:inScheme :RoadSignTypeCode ;
         rdfs:label "11_162"@en ;
         skos:definition "Left Bend"@en .
         :RoadSignType.11_174 a :RoadSignType, skos:Concept  ;
         skos:inScheme :RoadSignTypeCode ;
         rdfs:label "11_174"@en ;
         skos:definition "Right turn"@en .
         :RoadSignType.11_175 a :RoadSignType, skos:Concept  ;
         skos:inScheme :RoadSignTypeCode ;
         rdfs:label "11_175"@en ;
         skos:definition "Left turn "@en .
         :RoadSignType.11_187 a :RoadSignType, skos:Concept  ;
         skos:inScheme :RoadSignTypeCode ;
         rdfs:label "11_187"@en ;
         skos:definition "Reverse curve (Right and left)"@en .
         :RoadSignType.11_188 a :RoadSignType, skos:Concept  ;
         skos:inScheme :RoadSignTypeCode ;
         rdfs:label "11_188"@en ;
         skos:definition "Reverse curve (Left and right)"@en .
         :RoadSignType.11_211 a :RoadSignType, skos:Concept  ;
         skos:inScheme :RoadSignTypeCode ;
         rdfs:label "11_211"@en ;
         skos:definition "Double bend, right"@en .
         :RoadSignType.11_212 a :RoadSignType, skos:Concept  ;
         skos:inScheme :RoadSignTypeCode ;
         rdfs:label "11_212"@en ;
         skos:definition "Double bend, left"@en .
         :RoadSignType.11_224 a :RoadSignType, skos:Concept  ;
         skos:inScheme :RoadSignTypeCode ;
         rdfs:label "11_224"@en ;
         skos:definition "Winding road (First to the right)"@en .
         :RoadSignType.11_225 a :RoadSignType, skos:Concept  ;
         skos:inScheme :RoadSignTypeCode ;
         rdfs:label "11_225"@en ;
         skos:definition "Winding road (First to the left)"@en .
         :RoadSignType.11_236 a :RoadSignType, skos:Concept  ;
         skos:inScheme :RoadSignTypeCode ;
         rdfs:label "11_236"@en ;
         skos:definition "Level crossing with gate"@en .
         :RoadSignType.11_237 a :RoadSignType, skos:Concept  ;
         skos:inScheme :RoadSignTypeCode ;
         rdfs:label "11_237"@en ;
         skos:definition "Other level-crossing"@en .
         :RoadSignType.11_238 a :RoadSignType, skos:Concept  ;
         skos:inScheme :RoadSignTypeCode ;
         rdfs:label "11_238"@en ;
         skos:definition "Intersection with a tramway line"@en .
         :RoadSignType.11_239 a :RoadSignType, skos:Concept  ;
         skos:inScheme :RoadSignTypeCode ;
         rdfs:label "11_239"@en ;
         skos:definition "Children"@en .
         :RoadSignType.11_241 a :RoadSignType, skos:Concept  ;
         skos:inScheme :RoadSignTypeCode ;
         rdfs:label "11_241"@en ;
         skos:definition "Pedestrian crossing(right) "@en .
         :RoadSignType.11_242 a :RoadSignType, skos:Concept  ;
         skos:inScheme :RoadSignTypeCode ;
         rdfs:label "11_242"@en ;
         skos:definition "Elderly or disabled pedestrians likely to cross ahead"@en .
         :RoadSignType.11_244 a :RoadSignType, skos:Concept  ;
         skos:inScheme :RoadSignTypeCode ;
         rdfs:label "11_244"@en ;
         skos:definition "Children(left)"@en .
         :RoadSignType.11_245 a :RoadSignType, skos:Concept  ;
         skos:inScheme :RoadSignTypeCode ;
         rdfs:label "11_245"@en ;
         skos:definition "Pedestrians (left)"@en .
         :RoadSignType.11_246 a :RoadSignType, skos:Concept  ;
         skos:inScheme :RoadSignTypeCode ;
         rdfs:label "11_246"@en ;
         skos:definition "Pedestrian crossing (left)"@en .
         :RoadSignType.11_247 a :RoadSignType, skos:Concept  ;
         skos:inScheme :RoadSignTypeCode ;
         rdfs:label "11_247"@en ;
         skos:definition "Pedestrian crossing"@en .
         :RoadSignType.11_253 a :RoadSignType, skos:Concept  ;
         skos:inScheme :RoadSignTypeCode ;
         rdfs:label "11_253"@en ;
         skos:definition "Light signals"@en .
         :RoadSignType.11_254 a :RoadSignType, skos:Concept  ;
         skos:inScheme :RoadSignTypeCode ;
         rdfs:label "11_254"@en ;
         skos:definition "Slippery Road"@en .
         :RoadSignType.11_255 a :RoadSignType, skos:Concept  ;
         skos:inScheme :RoadSignTypeCode ;
         rdfs:label "11_255"@en ;
         skos:definition "Falling rocks"@en .
         :RoadSignType.11_256 a :RoadSignType, skos:Concept  ;
         skos:inScheme :RoadSignTypeCode ;
         rdfs:label "11_256"@en ;
         skos:definition "Loose gravel"@en .
         :RoadSignType.11_257 a :RoadSignType, skos:Concept  ;
         skos:inScheme :RoadSignTypeCode ;
         rdfs:label "11_257"@en ;
         skos:definition "Dangerous shoulder"@en .
         :RoadSignType.11_258 a :RoadSignType, skos:Concept  ;
         skos:inScheme :RoadSignTypeCode ;
         rdfs:label "11_258"@en ;
         skos:definition "Falling rocks(right)"@en .
         :RoadSignType.11_268 a :RoadSignType, skos:Concept  ;
         skos:inScheme :RoadSignTypeCode ;
         rdfs:label "11_268"@en ;
         skos:definition "Uneven road"@en .
         :RoadSignType.11_269 a :RoadSignType, skos:Concept  ;
         skos:inScheme :RoadSignTypeCode ;
         rdfs:label "11_269"@en ;
         skos:definition "Uneven road(hump)"@en .
         :RoadSignType.11_271 a :RoadSignType, skos:Concept  ;
         skos:inScheme :RoadSignTypeCode ;
         rdfs:label "11_271"@en ;
         skos:definition "Uneven road(dip)"@en .
         :RoadSignType.11_283 a :RoadSignType, skos:Concept  ;
         skos:inScheme :RoadSignTypeCode ;
         rdfs:label "11_283"@en ;
         skos:definition "Traffic merging from the right"@en .
         :RoadSignType.11_285 a :RoadSignType, skos:Concept  ;
         skos:inScheme :RoadSignTypeCode ;
         rdfs:label "11_285"@en ;
         skos:definition "Traffic merging from left ahead"@en .
         :RoadSignType.11_296 a :RoadSignType, skos:Concept  ;
         skos:inScheme :RoadSignTypeCode ;
         rdfs:label "11_296"@en ;
         skos:definition "Carriageway narrows from the right"@en .
         :RoadSignType.11_297 a :RoadSignType, skos:Concept  ;
         skos:inScheme :RoadSignTypeCode ;
         rdfs:label "11_297"@en ;
         skos:definition "Carriageway narrows from the left"@en .
         :RoadSignType.11_319 a :RoadSignType, skos:Concept  ;
         skos:inScheme :RoadSignTypeCode ;
         rdfs:label "11_319"@en ;
         skos:definition "Carriageway narrows"@en .
         :RoadSignType.11_332 a :RoadSignType, skos:Concept  ;
         skos:inScheme :RoadSignTypeCode ;
         rdfs:label "11_332"@en ;
         skos:definition "Two-way traffic "@en .
         :RoadSignType.11_346 a :RoadSignType, skos:Concept  ;
         skos:inScheme :RoadSignTypeCode ;
         rdfs:label "11_346"@en ;
         skos:definition "Steep ascent"@en .
         :RoadSignType.11_347 a :RoadSignType, skos:Concept  ;
         skos:inScheme :RoadSignTypeCode ;
         rdfs:label "11_347"@en ;
         skos:definition "Dangerous descent"@en .
         :RoadSignType.11_348 a :RoadSignType, skos:Concept  ;
         skos:inScheme :RoadSignTypeCode ;
         rdfs:label "11_348"@en ;
         skos:definition "Road works"@en .
         :RoadSignType.11_361 a :RoadSignType, skos:Concept  ;
         skos:inScheme :RoadSignTypeCode ;
         rdfs:label "11_361"@en ;
         skos:definition "Cross-wind"@en .
         :RoadSignType.11_362 a :RoadSignType, skos:Concept  ;
         skos:inScheme :RoadSignTypeCode ;
         rdfs:label "11_362"@en ;
         skos:definition "Airfiled"@en .
         :RoadSignType.11_363 a :RoadSignType, skos:Concept  ;
         skos:inScheme :RoadSignTypeCode ;
         rdfs:label "11_363"@en ;
         skos:definition "Cattle or other animals crossing"@en .
         :RoadSignType.11_364 a :RoadSignType, skos:Concept  ;
         skos:inScheme :RoadSignTypeCode ;
         rdfs:label "11_364"@en ;
         skos:definition "Cattle or other animals crossing"@en .
         :RoadSignType.11_365 a :RoadSignType, skos:Concept  ;
         skos:inScheme :RoadSignTypeCode ;
         rdfs:label "11_365"@en ;
         skos:definition "Cross-wind(left)"@en .
         :RoadSignType.11_366 a :RoadSignType, skos:Concept  ;
         skos:inScheme :RoadSignTypeCode ;
         rdfs:label "11_366"@en ;
         skos:definition "Airfiled(left)"@en .
         :RoadSignType.11_367 a :RoadSignType, skos:Concept  ;
         skos:inScheme :RoadSignTypeCode ;
         rdfs:label "11_367"@en ;
         skos:definition "Cattle or other animals crossing(left)"@en .
         :RoadSignType.11_368 a :RoadSignType, skos:Concept  ;
         skos:inScheme :RoadSignTypeCode ;
         rdfs:label "11_368"@en ;
         skos:definition "Cattle or other animals crossing(left)"@en .
         :RoadSignType.11_378 a :RoadSignType, skos:Concept  ;
         skos:inScheme :RoadSignTypeCode ;
         rdfs:label "11_378"@en ;
         skos:definition "Swing bridge"@en .
         :RoadSignType.11_379 a :RoadSignType, skos:Concept  ;
         skos:inScheme :RoadSignTypeCode ;
         rdfs:label "11_379"@en ;
         skos:definition "Road leads on to quar or river"@en .
         :RoadSignType.11_381 a :RoadSignType, skos:Concept  ;
         skos:inScheme :RoadSignTypeCode ;
         rdfs:label "11_381"@en ;
         skos:definition "Cyclist entering or crossing"@en .
         :RoadSignType.11_382 a :RoadSignType, skos:Concept  ;
         skos:inScheme :RoadSignTypeCode ;
         rdfs:label "11_382"@en ;
         skos:definition "Cyclist entering or crossing, left"@en .
         :RoadSignType.11_395 a :RoadSignType, skos:Concept  ;
         skos:inScheme :RoadSignTypeCode ;
         rdfs:label "11_395"@en ;
         skos:definition "Give way "@en .
         :RoadSignType.11_396 a :RoadSignType, skos:Concept  ;
         skos:inScheme :RoadSignTypeCode ;
         rdfs:label "11_396"@en ;
         skos:definition "Distance to 'Give Way' line ahead"@en .
         :RoadSignType.11_398 a :RoadSignType, skos:Concept  ;
         skos:inScheme :RoadSignTypeCode ;
         rdfs:label "11_398"@en ;
         skos:definition "Attention wrong way driver"@en .
         :RoadSignType.11_411 a :RoadSignType, skos:Concept  ;
         skos:inScheme :RoadSignTypeCode ;
         rdfs:label "11_411"@en ;
         skos:definition "Signs to be placed in the immediate vicinity of level-crossings(vertical)"@en .
         :RoadSignType.11_412 a :RoadSignType, skos:Concept  ;
         skos:inScheme :RoadSignTypeCode ;
         rdfs:label "11_412"@en ;
         skos:definition "Signs to be placed in the immediate vicinity of level-crossings (horizontal)"@en .
         :RoadSignType.11_413 a :RoadSignType, skos:Concept  ;
         skos:inScheme :RoadSignTypeCode ;
         rdfs:label "11_413"@en ;
         skos:definition "Signs to be placed in the immediate vicinity of level-crossings Two or more tracks (vertical)"@en .
         :RoadSignType.11_414 a :RoadSignType, skos:Concept  ;
         skos:inScheme :RoadSignTypeCode ;
         rdfs:label "11_414"@en ;
         skos:definition "Signs to be placed in the immediate vicinity of level-crossings  Two or more Tracks (horizontal)"@en .
         :RoadSignType.11_998 a :RoadSignType, skos:Concept  ;
         skos:inScheme :RoadSignTypeCode ;
         rdfs:label "11_998"@en ;
         skos:definition "Caution"@en .
         :RoadSignType.11_999 a :RoadSignType, skos:Concept  ;
         skos:inScheme :RoadSignTypeCode ;
         rdfs:label "11_999"@en ;
         skos:definition "Other danger"@en .
         :RoadSignType.12_111 a :RoadSignType, skos:Concept  ;
         skos:inScheme :RoadSignTypeCode ;
         rdfs:label "12_111"@en ;
         skos:definition "Priority for oncoming traffic "@en .
         :RoadSignType.12_112 a :RoadSignType, skos:Concept  ;
         skos:inScheme :RoadSignTypeCode ;
         rdfs:label "12_112"@en ;
         skos:definition "STOP"@en .
         :RoadSignType.12_113 a :RoadSignType, skos:Concept  ;
         skos:inScheme :RoadSignTypeCode ;
         rdfs:label "12_113"@en ;
         skos:definition "Compulsory stopping XXm ahead"@en .
         :RoadSignType.12_114 a :RoadSignType, skos:Concept  ;
         skos:inScheme :RoadSignTypeCode ;
         rdfs:label "12_114"@en ;
         skos:definition "Assigned lane for light vehicles or motor cycles"@en .
         :RoadSignType.12_115 a :RoadSignType, skos:Concept  ;
         skos:inScheme :RoadSignTypeCode ;
         rdfs:label "12_115"@en ;
         skos:definition "Assigned lane for trucks"@en .
         :RoadSignType.12_116 a :RoadSignType, skos:Concept  ;
         skos:inScheme :RoadSignTypeCode ;
         rdfs:label "12_116"@en ;
         skos:definition "Assigned lane on motorway for trailers"@en .
         :RoadSignType.12_117 a :RoadSignType, skos:Concept  ;
         skos:inScheme :RoadSignTypeCode ;
         rdfs:label "12_117"@en ;
         skos:definition "Give way"@en .
         :RoadSignType.12_127 a :RoadSignType, skos:Concept  ;
         skos:inScheme :RoadSignTypeCode ;
         rdfs:label "12_127"@en ;
         skos:definition "Assigned lane for trailers"@en .
         :RoadSignType.12_128 a :RoadSignType, skos:Concept  ;
         skos:inScheme :RoadSignTypeCode ;
         rdfs:label "12_128"@en ;
         skos:definition "With-flow bus lane which pedal cycles may also use"@en .
         :RoadSignType.12_129 a :RoadSignType, skos:Concept  ;
         skos:inScheme :RoadSignTypeCode ;
         rdfs:label "12_129"@en ;
         skos:definition "Exclusive lane for route bus"@en .
         :RoadSignType.12_131 a :RoadSignType, skos:Concept  ;
         skos:inScheme :RoadSignTypeCode ;
         rdfs:label "12_131"@en ;
         skos:definition "Buses and pedal cycles only"@en .
         :RoadSignType.12_132 a :RoadSignType, skos:Concept  ;
         skos:inScheme :RoadSignTypeCode ;
         rdfs:label "12_132"@en ;
         skos:definition "Priority lane for route bus"@en .
         :RoadSignType.12_133 a :RoadSignType, skos:Concept  ;
         skos:inScheme :RoadSignTypeCode ;
         rdfs:label "12_133"@en ;
         skos:definition "Vehicles under XXt are permitted "@en .
         :RoadSignType.12_134 a :RoadSignType, skos:Concept  ;
         skos:inScheme :RoadSignTypeCode ;
         rdfs:label "12_134"@en ;
         skos:definition "High occupancy vehicle lane"@en .
         :RoadSignType.12_154 a :RoadSignType, skos:Concept  ;
         skos:inScheme :RoadSignTypeCode ;
         rdfs:label "12_154"@en ;
         skos:definition "Centre line"@en .
         :RoadSignType.12_155 a :RoadSignType, skos:Concept  ;
         skos:inScheme :RoadSignTypeCode ;
         rdfs:label "12_155"@en ;
         skos:definition "Turning restriction on a multi-lane approach to an intersection"@en .
         :RoadSignType.12_156 a :RoadSignType, skos:Concept  ;
         skos:inScheme :RoadSignTypeCode ;
         rdfs:label "12_156"@en ;
         skos:definition "Stop line"@en .
         :RoadSignType.12_157 a :RoadSignType, skos:Concept  ;
         skos:inScheme :RoadSignTypeCode ;
         rdfs:label "12_157"@en ;
         skos:definition "Two-step right turn for mopeds"@en .
         :RoadSignType.12_158 a :RoadSignType, skos:Concept  ;
         skos:inScheme :RoadSignTypeCode ;
         rdfs:label "12_158"@en ;
         skos:definition "Do not make two-step right turn "@en .
         :RoadSignType.12_176 a :RoadSignType, skos:Concept  ;
         skos:inScheme :RoadSignTypeCode ;
         rdfs:label "12_176"@en ;
         skos:definition "Slow down"@en .
         :RoadSignType.12_177 a :RoadSignType, skos:Concept  ;
         skos:inScheme :RoadSignTypeCode ;
         rdfs:label "12_177"@en ;
         skos:definition "Yield right of way "@en .
         :RoadSignType.12_178 a :RoadSignType, skos:Concept  ;
         skos:inScheme :RoadSignTypeCode ;
         rdfs:label "12_178"@en ;
         skos:definition "Priority road"@en .
         :RoadSignType.12_411 a :RoadSignType, skos:Concept  ;
         skos:inScheme :RoadSignTypeCode ;
         rdfs:label "12_411"@en ;
         skos:definition "No entry for all vehicles, mopeds, cycles, pedestrians"@en .
         :RoadSignType.12_412 a :RoadSignType, skos:Concept  ;
         skos:inScheme :RoadSignTypeCode ;
         rdfs:label "12_412"@en ;
         skos:definition "No entry"@en .
         :RoadSignType.12_413 a :RoadSignType, skos:Concept  ;
         skos:inScheme :RoadSignTypeCode ;
         rdfs:label "12_413"@en ;
         skos:definition "No entry into the designated direction"@en .
         :RoadSignType.12_414 a :RoadSignType, skos:Concept  ;
         skos:inScheme :RoadSignTypeCode ;
         rdfs:label "12_414"@en ;
         skos:definition "No vehicles crossing (except for vehicles turning left to enter or exit a facility off the road) "@en .
         :RoadSignType.12_415 a :RoadSignType, skos:Concept  ;
         skos:inScheme :RoadSignTypeCode ;
         rdfs:label "12_415"@en ;
         skos:definition "Closed to all vehicles in both directions"@en .
         :RoadSignType.12_416 a :RoadSignType, skos:Concept  ;
         skos:inScheme :RoadSignTypeCode ;
         rdfs:label "12_416"@en ;
         skos:definition "No entry for for any power driven vehicle except two wheeled motor cycles without a side-car"@en .
         :RoadSignType.12_417 a :RoadSignType, skos:Concept  ;
         skos:inScheme :RoadSignTypeCode ;
         rdfs:label "12_417"@en ;
         skos:definition "No entry for motor cycles"@en .
         :RoadSignType.12_418 a :RoadSignType, skos:Concept  ;
         skos:inScheme :RoadSignTypeCode ;
         rdfs:label "12_418"@en ;
         skos:definition "No entry for cycles"@en .
         :RoadSignType.12_419 a :RoadSignType, skos:Concept  ;
         skos:inScheme :RoadSignTypeCode ;
         rdfs:label "12_419"@en ;
         skos:definition "No entry for mopeds"@en .
         :RoadSignType.12_421 a :RoadSignType, skos:Concept  ;
         skos:inScheme :RoadSignTypeCode ;
         rdfs:label "12_421"@en ;
         skos:definition "No entry for goods vehicles"@en .
         :RoadSignType.12_422 a :RoadSignType, skos:Concept  ;
         skos:inScheme :RoadSignTypeCode ;
         rdfs:label "12_422"@en ;
         skos:definition "No entry for any power driven vehicle drawing a trailer include a semi-trailer or a single axle trailer "@en .
         :RoadSignType.12_423 a :RoadSignType, skos:Concept  ;
         skos:inScheme :RoadSignTypeCode ;
         rdfs:label "12_423"@en ;
         skos:definition "No entry for pedestrians"@en .
         :RoadSignType.12_424 a :RoadSignType, skos:Concept  ;
         skos:inScheme :RoadSignTypeCode ;
         rdfs:label "12_424"@en ;
         skos:definition "No entry for animal-drawn vehicles"@en .
         :RoadSignType.12_425 a :RoadSignType, skos:Concept  ;
         skos:inScheme :RoadSignTypeCode ;
         rdfs:label "12_425"@en ;
         skos:definition "No entry for handcarts."@en .
         :RoadSignType.12_426 a :RoadSignType, skos:Concept  ;
         skos:inScheme :RoadSignTypeCode ;
         rdfs:label "12_426"@en ;
         skos:definition "No entry for power driven agricultural vehicles"@en .
         :RoadSignType.12_427 a :RoadSignType, skos:Concept  ;
         skos:inScheme :RoadSignTypeCode ;
         rdfs:label "12_427"@en ;
         skos:definition "No buses"@en .
         :RoadSignType.12_429 a :RoadSignType, skos:Concept  ;
         skos:inScheme :RoadSignTypeCode ;
         rdfs:label "12_429"@en ;
         skos:definition "No entry for any power driven vehicle drawing a trailer other than a semi-trailer or a single axle trailer"@en .
         :RoadSignType.12_431 a :RoadSignType, skos:Concept  ;
         skos:inScheme :RoadSignTypeCode ;
         rdfs:label "12_431"@en ;
         skos:definition "No ridden or accompanied horses"@en .
         :RoadSignType.12_433 a :RoadSignType, skos:Concept  ;
         skos:inScheme :RoadSignTypeCode ;
         rdfs:label "12_433"@en ;
         skos:definition "No vehicles that cannot exceed 25 km/h"@en .
         :RoadSignType.12_434 a :RoadSignType, skos:Concept  ;
         skos:inScheme :RoadSignTypeCode ;
         rdfs:label "12_434"@en ;
         skos:definition "No entry for any power-driven vehicle drawing a trailer"@en .
         :RoadSignType.12_451 a :RoadSignType, skos:Concept  ;
         skos:inScheme :RoadSignTypeCode ;
         rdfs:label "12_451"@en ;
         skos:definition "No entry for power driven vehicles"@en .
         :RoadSignType.12_452 a :RoadSignType, skos:Concept  ;
         skos:inScheme :RoadSignTypeCode ;
         rdfs:label "12_452"@en ;
         skos:definition "No entry for power driven vehicles or animal-drawn vehicles "@en .
         :RoadSignType.12_453 a :RoadSignType, skos:Concept  ;
         skos:inScheme :RoadSignTypeCode ;
         rdfs:label "12_453"@en ;
         skos:definition "No entry for goods vehicles and buses"@en .
         :RoadSignType.12_454 a :RoadSignType, skos:Concept  ;
         skos:inScheme :RoadSignTypeCode ;
         rdfs:label "12_454"@en ;
         skos:definition "No entry for bicycles, mopeds and disabled drivers vehicles"@en .
         :RoadSignType.12_455 a :RoadSignType, skos:Concept  ;
         skos:inScheme :RoadSignTypeCode ;
         rdfs:label "12_455"@en ;
         skos:definition "No entry for vehicles that are not able or aloud to go faster than 25 km/h, no microcars, bikes, mopeds and disabled drivers vehicles."@en .
         :RoadSignType.12_475 a :RoadSignType, skos:Concept  ;
         skos:inScheme :RoadSignTypeCode ;
         rdfs:label "12_475"@en ;
         skos:definition "No entry for vehicles carrying more than a certain quantity of explosives or readily inflammable substances"@en .
         :RoadSignType.12_476 a :RoadSignType, skos:Concept  ;
         skos:inScheme :RoadSignTypeCode ;
         rdfs:label "12_476"@en ;
         skos:definition "No entry for  vehicles carrying dangerous goods for which special sign plating is required"@en .
         :RoadSignType.12_477 a :RoadSignType, skos:Concept  ;
         skos:inScheme :RoadSignTypeCode ;
         rdfs:label "12_477"@en ;
         skos:definition "No entry for vehicles carrying more than a certain quantity of substances liable to cause water pollution"@en .
         :RoadSignType.12_499 a :RoadSignType, skos:Concept  ;
         skos:inScheme :RoadSignTypeCode ;
         rdfs:label "12_499"@en ;
         skos:definition "No entry for vehicles having an overall width exceeding X metres"@en .
         :RoadSignType.12_511 a :RoadSignType, skos:Concept  ;
         skos:inScheme :RoadSignTypeCode ;
         rdfs:label "12_511"@en ;
         skos:definition "No entry for vehicles having an overall height exceeding X metres"@en .
         :RoadSignType.12_512 a :RoadSignType, skos:Concept  ;
         skos:inScheme :RoadSignTypeCode ;
         rdfs:label "12_512"@en ;
         skos:definition "No entry for vehicles exceeding XX t laden mass"@en .
         :RoadSignType.12_513 a :RoadSignType, skos:Concept  ;
         skos:inScheme :RoadSignTypeCode ;
         rdfs:label "12_513"@en ;
         skos:definition "No entry for vehicles having a mass exceeding XX t on one axle "@en .
         :RoadSignType.12_514 a :RoadSignType, skos:Concept  ;
         skos:inScheme :RoadSignTypeCode ;
         rdfs:label "12_514"@en ;
         skos:definition "No entry for vehicles or combinations of vehicles exceeding XXm in length"@en .
         :RoadSignType.12_515 a :RoadSignType, skos:Concept  ;
         skos:inScheme :RoadSignTypeCode ;
         rdfs:label "12_515"@en ;
         skos:definition "Driving of vehicles less than XX m apart prohibited"@en .
         :RoadSignType.12_527 a :RoadSignType, skos:Concept  ;
         skos:inScheme :RoadSignTypeCode ;
         rdfs:label "12_527"@en ;
         skos:definition "No left turns"@en .
         :RoadSignType.12_528 a :RoadSignType, skos:Concept  ;
         skos:inScheme :RoadSignTypeCode ;
         rdfs:label "12_528"@en ;
         skos:definition "No right turns"@en .
         :RoadSignType.12_529 a :RoadSignType, skos:Concept  ;
         skos:inScheme :RoadSignTypeCode ;
         rdfs:label "12_529"@en ;
         skos:definition "No U-turns"@en .
         :RoadSignType.12_542 a :RoadSignType, skos:Concept  ;
         skos:inScheme :RoadSignTypeCode ;
         rdfs:label "12_542"@en ;
         skos:definition "Overtaking prohibited "@en .
         :RoadSignType.12_543 a :RoadSignType, skos:Concept  ;
         skos:inScheme :RoadSignTypeCode ;
         rdfs:label "12_543"@en ;
         skos:definition "End of overtaking prohibited"@en .
         :RoadSignType.12_544 a :RoadSignType, skos:Concept  ;
         skos:inScheme :RoadSignTypeCode ;
         rdfs:label "12_544"@en ;
         skos:definition "Overtaking by goods vehicles prohibited "@en .
         :RoadSignType.12_545 a :RoadSignType, skos:Concept  ;
         skos:inScheme :RoadSignTypeCode ;
         rdfs:label "12_545"@en ;
         skos:definition "End of overtaking by goods vehicles prohibited "@en .
         :RoadSignType.12_557 a :RoadSignType, skos:Concept  ;
         skos:inScheme :RoadSignTypeCode ;
         rdfs:label "12_557"@en ;
         skos:definition "Maximum speed limited to the figure indicated"@en .
         :RoadSignType.12_558 a :RoadSignType, skos:Concept  ;
         skos:inScheme :RoadSignTypeCode ;
         rdfs:label "12_558"@en ;
         skos:definition "Use of audible warning devices prohibited"@en .
         :RoadSignType.12_561 a :RoadSignType, skos:Concept  ;
         skos:inScheme :RoadSignTypeCode ;
         rdfs:label "12_561"@en ;
         skos:definition "Passing without stopping prohibited (Customs) "@en .
         :RoadSignType.12_562 a :RoadSignType, skos:Concept  ;
         skos:inScheme :RoadSignTypeCode ;
         rdfs:label "12_562"@en ;
         skos:definition "Stop for (Military police check)"@en .
         :RoadSignType.12_563 a :RoadSignType, skos:Concept  ;
         skos:inScheme :RoadSignTypeCode ;
         rdfs:label "12_563"@en ;
         skos:definition "Stop for (Police check) ) "@en .
         :RoadSignType.12_564 a :RoadSignType, skos:Concept  ;
         skos:inScheme :RoadSignTypeCode ;
         rdfs:label "12_564"@en ;
         skos:definition "Stop for (Toll gate)"@en .
         :RoadSignType.12_565 a :RoadSignType, skos:Concept  ;
         skos:inScheme :RoadSignTypeCode ;
         rdfs:label "12_565"@en ;
         skos:definition "Pedestrians crossover prohibited "@en .
         :RoadSignType.12_577 a :RoadSignType, skos:Concept  ;
         skos:inScheme :RoadSignTypeCode ;
         rdfs:label "12_577"@en ;
         skos:definition "Parking prohibited "@en .
         :RoadSignType.12_578 a :RoadSignType, skos:Concept  ;
         skos:inScheme :RoadSignTypeCode ;
         rdfs:label "12_578"@en ;
         skos:definition "Standing and parking prohibited"@en .
         :RoadSignType.12_579 a :RoadSignType, skos:Concept  ;
         skos:inScheme :RoadSignTypeCode ;
         rdfs:label "12_579"@en ;
         skos:definition "Alternate parking(1st to 15th days) "@en .
         :RoadSignType.12_581 a :RoadSignType, skos:Concept  ;
         skos:inScheme :RoadSignTypeCode ;
         rdfs:label "12_581"@en ;
         skos:definition "Alternate parking (16th to 31st days)"@en .
         :RoadSignType.12_592 a :RoadSignType, skos:Concept  ;
         skos:inScheme :RoadSignTypeCode ;
         rdfs:label "12_592"@en ;
         skos:definition "Emergency parking only"@en .
         :RoadSignType.12_593 a :RoadSignType, skos:Concept  ;
         skos:inScheme :RoadSignTypeCode ;
         rdfs:label "12_593"@en ;
         skos:definition "Entrance to a controlled parking zone"@en .
         :RoadSignType.12_594 a :RoadSignType, skos:Concept  ;
         skos:inScheme :RoadSignTypeCode ;
         rdfs:label "12_594"@en ;
         skos:definition "Limited duration no parking zone "@en .
         :RoadSignType.12_711 a :RoadSignType, skos:Concept  ;
         skos:inScheme :RoadSignTypeCode ;
         rdfs:label "12_711"@en ;
         skos:definition "Direction to be followed (Left)"@en .
         :RoadSignType.12_712 a :RoadSignType, skos:Concept  ;
         skos:inScheme :RoadSignTypeCode ;
         rdfs:label "12_712"@en ;
         skos:definition "Direction to be followed (Right)"@en .
         :RoadSignType.12_713 a :RoadSignType, skos:Concept  ;
         skos:inScheme :RoadSignTypeCode ;
         rdfs:label "12_713"@en ;
         skos:definition "Direction to be followed  (straight ahead)"@en .
         :RoadSignType.12_714 a :RoadSignType, skos:Concept  ;
         skos:inScheme :RoadSignTypeCode ;
         rdfs:label "12_714"@en ;
         skos:definition "Direction to be followed (Right turn)"@en .
         :RoadSignType.12_715 a :RoadSignType, skos:Concept  ;
         skos:inScheme :RoadSignTypeCode ;
         rdfs:label "12_715"@en ;
         skos:definition "Direction to be followed (Left turn) "@en .
         :RoadSignType.12_716 a :RoadSignType, skos:Concept  ;
         skos:inScheme :RoadSignTypeCode ;
         rdfs:label "12_716"@en ;
         skos:definition "Direction to be followed (Right, straight)"@en .
         :RoadSignType.12_717 a :RoadSignType, skos:Concept  ;
         skos:inScheme :RoadSignTypeCode ;
         rdfs:label "12_717"@en ;
         skos:definition "Direction to be followed (Left, straight) "@en .
         :RoadSignType.12_718 a :RoadSignType, skos:Concept  ;
         skos:inScheme :RoadSignTypeCode ;
         rdfs:label "12_718"@en ;
         skos:definition "Pass this side  (right side)"@en .
         :RoadSignType.12_719 a :RoadSignType, skos:Concept  ;
         skos:inScheme :RoadSignTypeCode ;
         rdfs:label "12_719"@en ;
         skos:definition "Pass this side  left side"@en .
         :RoadSignType.12_721 a :RoadSignType, skos:Concept  ;
         skos:inScheme :RoadSignTypeCode ;
         rdfs:label "12_721"@en ;
         skos:definition "Pass this side (Right turn, left turn) "@en .
         :RoadSignType.12_723 a :RoadSignType, skos:Concept  ;
         skos:inScheme :RoadSignTypeCode ;
         rdfs:label "12_723"@en ;
         skos:definition "Pass this side  (both sides)"@en .
         :RoadSignType.12_724 a :RoadSignType, skos:Concept  ;
         skos:inScheme :RoadSignTypeCode ;
         rdfs:label "12_724"@en ;
         skos:definition "Compulsory direction for vehicles carrying dangerous goods"@en .
         :RoadSignType.12_743 a :RoadSignType, skos:Concept  ;
         skos:inScheme :RoadSignTypeCode ;
         rdfs:label "12_743"@en ;
         skos:definition "Direction to be followed (Two-way traffic) "@en .
         :RoadSignType.12_744 a :RoadSignType, skos:Concept  ;
         skos:inScheme :RoadSignTypeCode ;
         rdfs:label "12_744"@en ;
         skos:definition "Direction to be followed (One-way street)"@en .
         :RoadSignType.12_745 a :RoadSignType, skos:Concept  ;
         skos:inScheme :RoadSignTypeCode ;
         rdfs:label "12_745"@en ;
         skos:definition "Direction to be followed (Left) (One-way road) "@en .
         :RoadSignType.12_746 a :RoadSignType, skos:Concept  ;
         skos:inScheme :RoadSignTypeCode ;
         rdfs:label "12_746"@en ;
         skos:definition "Compulsory roundabout (Clockwise)"@en .
         :RoadSignType.12_747 a :RoadSignType, skos:Concept  ;
         skos:inScheme :RoadSignTypeCode ;
         rdfs:label "12_747"@en ;
         skos:definition "Compulsory roundabout "@en .
         :RoadSignType.12_748 a :RoadSignType, skos:Concept  ;
         skos:inScheme :RoadSignTypeCode ;
         rdfs:label "12_748"@en ;
         skos:definition "Road for motor vehicles only"@en .
         :RoadSignType.12_749 a :RoadSignType, skos:Concept  ;
         skos:inScheme :RoadSignTypeCode ;
         rdfs:label "12_749"@en ;
         skos:definition "Compulsary cycle track"@en .
         :RoadSignType.12_751 a :RoadSignType, skos:Concept  ;
         skos:inScheme :RoadSignTypeCode ;
         rdfs:label "12_751"@en ;
         skos:definition "Abreast riding permitted "@en .
         :RoadSignType.12_752 a :RoadSignType, skos:Concept  ;
         skos:inScheme :RoadSignTypeCode ;
         rdfs:label "12_752"@en ;
         skos:definition "Bicycle crossing zone "@en .
         :RoadSignType.12_753 a :RoadSignType, skos:Concept  ;
         skos:inScheme :RoadSignTypeCode ;
         rdfs:label "12_753"@en ;
         skos:definition "Compulsary footpath"@en .
         :RoadSignType.12_754 a :RoadSignType, skos:Concept  ;
         skos:inScheme :RoadSignTypeCode ;
         rdfs:label "12_754"@en ;
         skos:definition "Compulsay track for riders on horseback"@en .
         :RoadSignType.12_772 a :RoadSignType, skos:Concept  ;
         skos:inScheme :RoadSignTypeCode ;
         rdfs:label "12_772"@en ;
         skos:definition "Pedestrian and bicycle crossing zone"@en .
         :RoadSignType.12_773 a :RoadSignType, skos:Concept  ;
         skos:inScheme :RoadSignTypeCode ;
         rdfs:label "12_773"@en ;
         skos:definition "Compulsary cycle track and Compulsary footpath"@en .
         :RoadSignType.12_795 a :RoadSignType, skos:Concept  ;
         skos:inScheme :RoadSignTypeCode ;
         rdfs:label "12_795"@en ;
         skos:definition "Compulsory minimum speed"@en .
         :RoadSignType.12_796 a :RoadSignType, skos:Concept  ;
         skos:inScheme :RoadSignTypeCode ;
         rdfs:label "12_796"@en ;
         skos:definition "Snow chains compulsory"@en .
         :RoadSignType.12_851 a :RoadSignType, skos:Concept  ;
         skos:inScheme :RoadSignTypeCode ;
         rdfs:label "12_851"@en ;
         skos:definition "End of priority"@en .
         :RoadSignType.12_852 a :RoadSignType, skos:Concept  ;
         skos:inScheme :RoadSignTypeCode ;
         rdfs:label "12_852"@en ;
         skos:definition "Distance plate indicating end of priority"@en .
         :RoadSignType.12_853 a :RoadSignType, skos:Concept  ;
         skos:inScheme :RoadSignTypeCode ;
         rdfs:label "12_853"@en ;
         skos:definition "Priority for oncoming trafic"@en .
         :RoadSignType.12_861 a :RoadSignType, skos:Concept  ;
         skos:inScheme :RoadSignTypeCode ;
         rdfs:label "12_861"@en ;
         skos:definition "End of all local prohibition imposed on moving vehicles "@en .
         :RoadSignType.12_862 a :RoadSignType, skos:Concept  ;
         skos:inScheme :RoadSignTypeCode ;
         rdfs:label "12_862"@en ;
         skos:definition "End of prohibition of overtaking"@en .
         :RoadSignType.12_863 a :RoadSignType, skos:Concept  ;
         skos:inScheme :RoadSignTypeCode ;
         rdfs:label "12_863"@en ;
         skos:definition "End of prohibition of overtaking for goods vehicles "@en .
         :RoadSignType.12_864 a :RoadSignType, skos:Concept  ;
         skos:inScheme :RoadSignTypeCode ;
         rdfs:label "12_864"@en ;
         skos:definition "End of speed limit"@en .
         :RoadSignType.12_865 a :RoadSignType, skos:Concept  ;
         skos:inScheme :RoadSignTypeCode ;
         rdfs:label "12_865"@en ;
         skos:definition "End of compulsory minimum speed "@en .
         :RoadSignType.12_871 a :RoadSignType, skos:Concept  ;
         skos:inScheme :RoadSignTypeCode ;
         rdfs:label "12_871"@en ;
         skos:definition "Driving on tram track permitted"@en .
         :RoadSignType.12_872 a :RoadSignType, skos:Concept  ;
         skos:inScheme :RoadSignTypeCode ;
         rdfs:label "12_872"@en ;
         skos:definition "Stopping permitted "@en .
         :RoadSignType.13_111 a :RoadSignType, skos:Concept  ;
         skos:inScheme :RoadSignTypeCode ;
         rdfs:label "13_111"@en ;
         skos:definition "Advance direction signs "@en .
         :RoadSignType.13_112 a :RoadSignType, skos:Concept  ;
         skos:inScheme :RoadSignTypeCode ;
         rdfs:label "13_112"@en ;
         skos:definition "Advance sign showing the direction of places "@en .
         :RoadSignType.13_121 a :RoadSignType, skos:Concept  ;
         skos:inScheme :RoadSignTypeCode ;
         rdfs:label "13_121"@en ;
         skos:definition "Advance direction signs(root to be followe) "@en .
         :RoadSignType.13_133 a :RoadSignType, skos:Concept  ;
         skos:inScheme :RoadSignTypeCode ;
         rdfs:label "13_133"@en ;
         skos:definition "Advance direction signs showing the common road name "@en .
         :RoadSignType.13_168 a :RoadSignType, skos:Concept  ;
         skos:inScheme :RoadSignTypeCode ;
         rdfs:label "13_168"@en ;
         skos:definition "Motorway"@en .
         :RoadSignType.13_169 a :RoadSignType, skos:Concept  ;
         skos:inScheme :RoadSignTypeCode ;
         rdfs:label "13_169"@en ;
         skos:definition "Advance signs showing the morotway with place name"@en .
         :RoadSignType.13_171 a :RoadSignType, skos:Concept  ;
         skos:inScheme :RoadSignTypeCode ;
         rdfs:label "13_171"@en ;
         skos:definition "Advance direction signs showing the exit of motorway with road number"@en .
         :RoadSignType.13_172 a :RoadSignType, skos:Concept  ;
         skos:inScheme :RoadSignTypeCode ;
         rdfs:label "13_172"@en ;
         skos:definition "Advance direction signs showing the exit of motorway"@en .
         :RoadSignType.13_173 a :RoadSignType, skos:Concept  ;
         skos:inScheme :RoadSignTypeCode ;
         rdfs:label "13_173"@en ;
         skos:definition "Advance signs showing the service area on motorway"@en .
         :RoadSignType.13_174 a :RoadSignType, skos:Concept  ;
         skos:inScheme :RoadSignTypeCode ;
         rdfs:label "13_174"@en ;
         skos:definition "End of motorway"@en .
         :RoadSignType.13_184 a :RoadSignType, skos:Concept  ;
         skos:inScheme :RoadSignTypeCode ;
         rdfs:label "13_184"@en ;
         skos:definition "Multiple destinations and distances"@en .
         :RoadSignType.13_185 a :RoadSignType, skos:Concept  ;
         skos:inScheme :RoadSignTypeCode ;
         rdfs:label "13_185"@en ;
         skos:definition "Sign showing the direction of places"@en .
         :RoadSignType.13_186 a :RoadSignType, skos:Concept  ;
         skos:inScheme :RoadSignTypeCode ;
         rdfs:label "13_186"@en ;
         skos:definition "Sign showing the direction of places with road number"@en .
         :RoadSignType.13_187 a :RoadSignType, skos:Concept  ;
         skos:inScheme :RoadSignTypeCode ;
         rdfs:label "13_187"@en ;
         skos:definition "Sign showing the direction of places on the following road "@en .
         :RoadSignType.13_188 a :RoadSignType, skos:Concept  ;
         skos:inScheme :RoadSignTypeCode ;
         rdfs:label "13_188"@en ;
         skos:definition "Sign showing the direction of places with junction layout"@en .
         :RoadSignType.13_189 a :RoadSignType, skos:Concept  ;
         skos:inScheme :RoadSignTypeCode ;
         rdfs:label "13_189"@en ;
         skos:definition "Sign showing the direction of places with common road names"@en .
         :RoadSignType.13_222 a :RoadSignType, skos:Concept  ;
         skos:inScheme :RoadSignTypeCode ;
         rdfs:label "13_222"@en ;
         skos:definition "Direction signs showing the entrance of motorway"@en .
         :RoadSignType.13_223 a :RoadSignType, skos:Concept  ;
         skos:inScheme :RoadSignTypeCode ;
         rdfs:label "13_223"@en ;
         skos:definition "Direction signs showing the exit of motorway with the place name"@en .
         :RoadSignType.13_224 a :RoadSignType, skos:Concept  ;
         skos:inScheme :RoadSignTypeCode ;
         rdfs:label "13_224"@en ;
         skos:definition " Direction signs showing the exit of motorway"@en .
         :RoadSignType.13_225 a :RoadSignType, skos:Concept  ;
         skos:inScheme :RoadSignTypeCode ;
         rdfs:label "13_225"@en ;
         skos:definition " Lane for the place on the motorway "@en .
         :RoadSignType.13_226 a :RoadSignType, skos:Concept  ;
         skos:inScheme :RoadSignTypeCode ;
         rdfs:label "13_226"@en ;
         skos:definition " Service area on motorway"@en .
         :RoadSignType.13_326 a :RoadSignType, skos:Concept  ;
         skos:inScheme :RoadSignTypeCode ;
         rdfs:label "13_326"@en ;
         skos:definition "National/State motorway number"@en .
         :RoadSignType.13_327 a :RoadSignType, skos:Concept  ;
         skos:inScheme :RoadSignTypeCode ;
         rdfs:label "13_327"@en ;
         skos:definition "Local motorway number"@en .
         :RoadSignType.13_525 a :RoadSignType, skos:Concept  ;
         skos:inScheme :RoadSignTypeCode ;
         rdfs:label "13_525"@en ;
         skos:definition "No through road(front)"@en .
         :RoadSignType.13_526 a :RoadSignType, skos:Concept  ;
         skos:inScheme :RoadSignTypeCode ;
         rdfs:label "13_526"@en ;
         skos:definition "No through road(right)"@en .
         :RoadSignType.13_538 a :RoadSignType, skos:Concept  ;
         skos:inScheme :RoadSignTypeCode ;
         rdfs:label "13_538"@en ;
         skos:definition "Vehicles from opposite direction must give priority"@en .
         :RoadSignType.13_539 a :RoadSignType, skos:Concept  ;
         skos:inScheme :RoadSignTypeCode ;
         rdfs:label "13_539"@en ;
         skos:definition "Access permitted"@en .
         :RoadSignType.13_611 a :RoadSignType, skos:Concept  ;
         skos:inScheme :RoadSignTypeCode ;
         rdfs:label "13_611"@en ;
         skos:definition " Number and direction of traffic lanes"@en .
         :RoadSignType.13_612 a :RoadSignType, skos:Concept  ;
         skos:inScheme :RoadSignTypeCode ;
         rdfs:label "13_612"@en ;
         skos:definition "Lane ends "@en .
         :RoadSignType.13_613 a :RoadSignType, skos:Concept  ;
         skos:inScheme :RoadSignTypeCode ;
         rdfs:label "13_613"@en ;
         skos:definition "Lane divergence"@en .
         :RoadSignType.13_614 a :RoadSignType, skos:Concept  ;
         skos:inScheme :RoadSignTypeCode ;
         rdfs:label "13_614"@en ;
         skos:definition "Trucks prohibited from this lane "@en .
         :RoadSignType.13_615 a :RoadSignType, skos:Concept  ;
         skos:inScheme :RoadSignTypeCode ;
         rdfs:label "13_615"@en ;
         skos:definition "Trucks prohibited from main lanes"@en .
         :RoadSignType.13_616 a :RoadSignType, skos:Concept  ;
         skos:inScheme :RoadSignTypeCode ;
         rdfs:label "13_616"@en ;
         skos:definition "Trucks prohibited from diverging lane"@en .
         :RoadSignType.13_617 a :RoadSignType, skos:Concept  ;
         skos:inScheme :RoadSignTypeCode ;
         rdfs:label "13_617"@en ;
         skos:definition "Advance direction sign for route to be followed"@en .
         :RoadSignType.13_618 a :RoadSignType, skos:Concept  ;
         skos:inScheme :RoadSignTypeCode ;
         rdfs:label "13_618"@en ;
         skos:definition "Detour"@en .
         :RoadSignType.13_619 a :RoadSignType, skos:Concept  ;
         skos:inScheme :RoadSignTypeCode ;
         rdfs:label "13_619"@en ;
         skos:definition "Crawler lane"@en .
         :RoadSignType.13_621 a :RoadSignType, skos:Concept  ;
         skos:inScheme :RoadSignTypeCode ;
         rdfs:label "13_621"@en ;
         skos:definition "Escape lane (Right type 1) "@en .
         :RoadSignType.13_622 a :RoadSignType, skos:Concept  ;
         skos:inScheme :RoadSignTypeCode ;
         rdfs:label "13_622"@en ;
         skos:definition "Escape lane"@en .
         :RoadSignType.13_623 a :RoadSignType, skos:Concept  ;
         skos:inScheme :RoadSignTypeCode ;
         rdfs:label "13_623"@en ;
         skos:definition "One-way street"@en .
         :RoadSignType.13_624 a :RoadSignType, skos:Concept  ;
         skos:inScheme :RoadSignTypeCode ;
         rdfs:label "13_624"@en ;
         skos:definition "Lane convergence"@en .
         :RoadSignType.13_643 a :RoadSignType, skos:Concept  ;
         skos:inScheme :RoadSignTypeCode ;
         rdfs:label "13_643"@en ;
         skos:definition "Directional flows"@en .
         :RoadSignType.13_644 a :RoadSignType, skos:Concept  ;
         skos:inScheme :RoadSignTypeCode ;
         rdfs:label "13_644"@en ;
         skos:definition "Directional flows and lane convergence"@en .
         :RoadSignType.12_645 a :RoadSignType, skos:Concept  ;
         skos:inScheme :RoadSignTypeCode ;
         rdfs:label "12_645"@en ;
         skos:definition "Rush hour lane open 3/1"@en .
         :RoadSignType.12_646 a :RoadSignType, skos:Concept  ;
         skos:inScheme :RoadSignTypeCode ;
         rdfs:label "12_646"@en ;
         skos:definition "End of rush hour lane"@en .
         :RoadSignType.12_647 a :RoadSignType, skos:Concept  ;
         skos:inScheme :RoadSignTypeCode ;
         rdfs:label "12_647"@en ;
         skos:definition "End of rush hour lane 3/1"@en .
         :RoadSignType.12_648 a :RoadSignType, skos:Concept  ;
         skos:inScheme :RoadSignTypeCode ;
         rdfs:label "12_648"@en ;
         skos:definition "Clear rush hour lane"@en .
         :RoadSignType.12_649 a :RoadSignType, skos:Concept  ;
         skos:inScheme :RoadSignTypeCode ;
         rdfs:label "12_649"@en ;
         skos:definition "Clear rush hour lane 3/1"@en .
         :RoadSignType.13_651 a :RoadSignType, skos:Concept  ;
         skos:inScheme :RoadSignTypeCode ;
         rdfs:label "13_651"@en ;
         skos:definition " Closure of a traffic lane, two lanes to one (right lane ends)"@en .
         :RoadSignType.13_652 a :RoadSignType, skos:Concept  ;
         skos:inScheme :RoadSignTypeCode ;
         rdfs:label "13_652"@en ;
         skos:definition "Closure of a traffic lane, three lanes to two (right lane ends)"@en .
         :RoadSignType.13_653 a :RoadSignType, skos:Concept  ;
         skos:inScheme :RoadSignTypeCode ;
         rdfs:label "13_653"@en ;
         skos:definition "Lane convergence, four lanes to three (right lane ends)"@en .
         :RoadSignType.13_654 a :RoadSignType, skos:Concept  ;
         skos:inScheme :RoadSignTypeCode ;
         rdfs:label "13_654"@en ;
         skos:definition "Closure of a traffic lane, two lanes to one (left lane ends)"@en .
         :RoadSignType.13_655 a :RoadSignType, skos:Concept  ;
         skos:inScheme :RoadSignTypeCode ;
         rdfs:label "13_655"@en ;
         skos:definition "Closure of a traffic lane, three lanes to two (left lane ends)"@en .
         :RoadSignType.13_656 a :RoadSignType, skos:Concept  ;
         skos:inScheme :RoadSignTypeCode ;
         rdfs:label "13_656"@en ;
         skos:definition "Closure of a traffic lane, four lanes to three  (left lane ends)"@en .
         :RoadSignType.13_657 a :RoadSignType, skos:Concept  ;
         skos:inScheme :RoadSignTypeCode ;
         rdfs:label "13_657"@en ;
         skos:definition "Left lane shift onto oncoming lane"@en .
         :RoadSignType.13_658 a :RoadSignType, skos:Concept  ;
         skos:inScheme :RoadSignTypeCode ;
         rdfs:label "13_658"@en ;
         skos:definition "Two lane right shift onto hard shoulder"@en .
         :RoadSignType.13_768 a :RoadSignType, skos:Concept  ;
         skos:inScheme :RoadSignTypeCode ;
         rdfs:label "13_768"@en ;
         skos:definition "Lane closed"@en .
         :RoadSignType.13_769 a :RoadSignType, skos:Concept  ;
         skos:inScheme :RoadSignTypeCode ;
         rdfs:label "13_769"@en ;
         skos:definition "Lane free"@en .
         :RoadSignType.13_771 a :RoadSignType, skos:Concept  ;
         skos:inScheme :RoadSignTypeCode ;
         rdfs:label "13_771"@en ;
         skos:definition "Clear lane to left"@en .
         :RoadSignType.13_772 a :RoadSignType, skos:Concept  ;
         skos:inScheme :RoadSignTypeCode ;
         rdfs:label "13_772"@en ;
         skos:definition "Clear lane to right"@en .
         :RoadSignType.13_773 a :RoadSignType, skos:Concept  ;
         skos:inScheme :RoadSignTypeCode ;
         rdfs:label "13_773"@en ;
         skos:definition "End of all restrictions by electronic signs"@en .
         :RoadSignType.13_781 a :RoadSignType, skos:Concept  ;
         skos:inScheme :RoadSignTypeCode ;
         rdfs:label "13_781"@en ;
         skos:definition "compulsory minimum speed applying to different lanes"@en .
         :RoadSignType.13_782 a :RoadSignType, skos:Concept  ;
         skos:inScheme :RoadSignTypeCode ;
         rdfs:label "13_782"@en ;
         skos:definition "compulsory minimum speed applying to one lane"@en .
         :RoadSignType.13_783 a :RoadSignType, skos:Concept  ;
         skos:inScheme :RoadSignTypeCode ;
         rdfs:label "13_783"@en ;
         skos:definition "speed limits applying to different lanes"@en .
         :RoadSignType.13_784 a :RoadSignType, skos:Concept  ;
         skos:inScheme :RoadSignTypeCode ;
         rdfs:label "13_784"@en ;
         skos:definition "lanes reserved for buses"@en .
         :RoadSignType.13_785 a :RoadSignType, skos:Concept  ;
         skos:inScheme :RoadSignTypeCode ;
         rdfs:label "13_785"@en ;
         skos:definition "One-way"@en .
         :RoadSignType.13_786 a :RoadSignType, skos:Concept  ;
         skos:inScheme :RoadSignTypeCode ;
         rdfs:label "13_786"@en ;
         skos:definition "Preselection sign"@en .
         :RoadSignType.13_811 a :RoadSignType, skos:Concept  ;
         skos:inScheme :RoadSignTypeCode ;
         rdfs:label "13_811"@en ;
         skos:definition "Road for motor vehicles"@en .
         :RoadSignType.13_812 a :RoadSignType, skos:Concept  ;
         skos:inScheme :RoadSignTypeCode ;
         rdfs:label "13_812"@en ;
         skos:definition "End of road for motor vehicles"@en .
         :RoadSignType.13_813 a :RoadSignType, skos:Concept  ;
         skos:inScheme :RoadSignTypeCode ;
         rdfs:label "13_813"@en ;
         skos:definition "Tunnel"@en .
         :RoadSignType.13_814 a :RoadSignType, skos:Concept  ;
         skos:inScheme :RoadSignTypeCode ;
         rdfs:label "13_814"@en ;
         skos:definition "End of tunnel"@en .
         :RoadSignType.13_815 a :RoadSignType, skos:Concept  ;
         skos:inScheme :RoadSignTypeCode ;
         rdfs:label "13_815"@en ;
         skos:definition "Pedestrian crossing"@en .
         :RoadSignType.13_821 a :RoadSignType, skos:Concept  ;
         skos:inScheme :RoadSignTypeCode ;
         rdfs:label "13_821"@en ;
         skos:definition "Safety evacuation area "@en .
         :RoadSignType.13_822 a :RoadSignType, skos:Concept  ;
         skos:inScheme :RoadSignTypeCode ;
         rdfs:label "13_822"@en ;
         skos:definition "Emergency exit "@en .
         :RoadSignType.13_823 a :RoadSignType, skos:Concept  ;
         skos:inScheme :RoadSignTypeCode ;
         rdfs:label "13_823"@en ;
         skos:definition "Fire extinguisher "@en .
         :RoadSignType.13_824 a :RoadSignType, skos:Concept  ;
         skos:inScheme :RoadSignTypeCode ;
         rdfs:label "13_824"@en ;
         skos:definition "Emergency roadside telephone"@en .
         :RoadSignType.13_825 a :RoadSignType, skos:Concept  ;
         skos:inScheme :RoadSignTypeCode ;
         rdfs:label "13_825"@en ;
         skos:definition "Emergency call button"@en .
         :RoadSignType.13_826 a :RoadSignType, skos:Concept  ;
         skos:inScheme :RoadSignTypeCode ;
         rdfs:label "13_826"@en ;
         skos:definition "Emergency stopping place"@en .
         :RoadSignType.13_827 a :RoadSignType, skos:Concept  ;
         skos:inScheme :RoadSignTypeCode ;
         rdfs:label "13_827"@en ;
         skos:definition "Waiting area for slower traffic "@en .
         :RoadSignType.13_828 a :RoadSignType, skos:Concept  ;
         skos:inScheme :RoadSignTypeCode ;
         rdfs:label "13_828"@en ;
         skos:definition "Safety zone"@en .
         :RoadSignType.13_829 a :RoadSignType, skos:Concept  ;
         skos:inScheme :RoadSignTypeCode ;
         rdfs:label "13_829"@en ;
         skos:definition "Hospital"@en .
         :RoadSignType.13_831 a :RoadSignType, skos:Concept  ;
         skos:inScheme :RoadSignTypeCode ;
         rdfs:label "13_831"@en ;
         skos:definition "Toll gate"@en .
         :RoadSignType.13_832 a :RoadSignType, skos:Concept  ;
         skos:inScheme :RoadSignTypeCode ;
         rdfs:label "13_832"@en ;
         skos:definition "Toll zone"@en .
         :RoadSignType.13_833 a :RoadSignType, skos:Concept  ;
         skos:inScheme :RoadSignTypeCode ;
         rdfs:label "13_833"@en ;
         skos:definition "Automatic toll gate "@en .
         :RoadSignType.13_834 a :RoadSignType, skos:Concept  ;
         skos:inScheme :RoadSignTypeCode ;
         rdfs:label "13_834"@en ;
         skos:definition "Manual toll gate "@en .
         :RoadSignType.13_835 a :RoadSignType, skos:Concept  ;
         skos:inScheme :RoadSignTypeCode ;
         rdfs:label "13_835"@en ;
         skos:definition "Bicycle"@en .
         :RoadSignType.13_836 a :RoadSignType, skos:Concept  ;
         skos:inScheme :RoadSignTypeCode ;
         rdfs:label "13_836"@en ;
         skos:definition "Aircraft/ Airport"@en .
         :RoadSignType.13_837 a :RoadSignType, skos:Concept  ;
         skos:inScheme :RoadSignTypeCode ;
         rdfs:label "13_837"@en ;
         skos:definition "Departures "@en .
         :RoadSignType.13_838 a :RoadSignType, skos:Concept  ;
         skos:inScheme :RoadSignTypeCode ;
         rdfs:label "13_838"@en ;
         skos:definition "Arrivals"@en .
         :RoadSignType.13_839 a :RoadSignType, skos:Concept  ;
         skos:inScheme :RoadSignTypeCode ;
         rdfs:label "13_839"@en ;
         skos:definition "Helicopter/ Heliport"@en .
         :RoadSignType.13_841 a :RoadSignType, skos:Concept  ;
         skos:inScheme :RoadSignTypeCode ;
         rdfs:label "13_841"@en ;
         skos:definition "Railway/ Railway station"@en .
         :RoadSignType.13_842 a :RoadSignType, skos:Concept  ;
         skos:inScheme :RoadSignTypeCode ;
         rdfs:label "13_842"@en ;
         skos:definition "Rent a car"@en .
         :RoadSignType.13_843 a :RoadSignType, skos:Concept  ;
         skos:inScheme :RoadSignTypeCode ;
         rdfs:label "13_843"@en ;
         skos:definition "Taxi stop"@en .
         :RoadSignType.13_844 a :RoadSignType, skos:Concept  ;
         skos:inScheme :RoadSignTypeCode ;
         rdfs:label "13_844"@en ;
         skos:definition "Bus stop "@en .
         :RoadSignType.13_845 a :RoadSignType, skos:Concept  ;
         skos:inScheme :RoadSignTypeCode ;
         rdfs:label "13_845"@en ;
         skos:definition "Tramway stop "@en .
         :RoadSignType.13_846 a :RoadSignType, skos:Concept  ;
         skos:inScheme :RoadSignTypeCode ;
         rdfs:label "13_846"@en ;
         skos:definition "Road open or closed "@en .
         :RoadSignType.13_847 a :RoadSignType, skos:Concept  ;
         skos:inScheme :RoadSignTypeCode ;
         rdfs:label "13_847"@en ;
         skos:definition "Parking space for vehicles with permission "@en .
         :RoadSignType.13_851 a :RoadSignType, skos:Concept  ;
         skos:inScheme :RoadSignTypeCode ;
         rdfs:label "13_851"@en ;
         skos:definition "Parking"@en .
         :RoadSignType.13_852 a :RoadSignType, skos:Concept  ;
         skos:inScheme :RoadSignTypeCode ;
         rdfs:label "13_852"@en ;
         skos:definition "Parking (Machine-charged) "@en .
         :RoadSignType.13_853 a :RoadSignType, skos:Concept  ;
         skos:inScheme :RoadSignTypeCode ;
         rdfs:label "13_853"@en ;
         skos:definition "Park-and-ride point"@en .
         :RoadSignType.13_854 a :RoadSignType, skos:Concept  ;
         skos:inScheme :RoadSignTypeCode ;
         rdfs:label "13_854"@en ;
         skos:definition "Car ferry"@en .
         :RoadSignType.13_855 a :RoadSignType, skos:Concept  ;
         skos:inScheme :RoadSignTypeCode ;
         rdfs:label "13_855"@en ;
         skos:definition "Car train "@en .
         :RoadSignType.13_861 a :RoadSignType, skos:Concept  ;
         skos:inScheme :RoadSignTypeCode ;
         rdfs:label "13_861"@en ;
         skos:definition "Beginning of a built-up area"@en .
         :RoadSignType.13_862 a :RoadSignType, skos:Concept  ;
         skos:inScheme :RoadSignTypeCode ;
         rdfs:label "13_862"@en ;
         skos:definition "End of a built-up area"@en .
         :RoadSignType.13_863 a :RoadSignType, skos:Concept  ;
         skos:inScheme :RoadSignTypeCode ;
         rdfs:label "13_863"@en ;
         skos:definition "Zone in which parking is prohibited"@en .
         :RoadSignType.13_864 a :RoadSignType, skos:Concept  ;
         skos:inScheme :RoadSignTypeCode ;
         rdfs:label "13_864"@en ;
         skos:definition "Zone in which parking is prohibited at certain times"@en .
         :RoadSignType.13_865 a :RoadSignType, skos:Concept  ;
         skos:inScheme :RoadSignTypeCode ;
         rdfs:label "13_865"@en ;
         skos:definition "Parking zone"@en .
         :RoadSignType.13_866 a :RoadSignType, skos:Concept  ;
         skos:inScheme :RoadSignTypeCode ;
         rdfs:label "13_866"@en ;
         skos:definition "Maximum speed zone"@en .
         :RoadSignType.13_867 a :RoadSignType, skos:Concept  ;
         skos:inScheme :RoadSignTypeCode ;
         rdfs:label "13_867"@en ;
         skos:definition "End of zone in which parking is prohibited"@en .
         :RoadSignType.13_868 a :RoadSignType, skos:Concept  ;
         skos:inScheme :RoadSignTypeCode ;
         rdfs:label "13_868"@en ;
         skos:definition "End of zone in which parking is prohibited at certain times"@en .
         :RoadSignType.13_869 a :RoadSignType, skos:Concept  ;
         skos:inScheme :RoadSignTypeCode ;
         rdfs:label "13_869"@en ;
         skos:definition "End of parking zone"@en .
         :RoadSignType.13_871 a :RoadSignType, skos:Concept  ;
         skos:inScheme :RoadSignTypeCode ;
         rdfs:label "13_871"@en ;
         skos:definition "End of maximum speed zone"@en .
         :RoadSignType.13_872 a :RoadSignType, skos:Concept  ;
         skos:inScheme :RoadSignTypeCode ;
         rdfs:label "13_872"@en ;
         skos:definition "Residential area"@en .
         :RoadSignType.13_873 a :RoadSignType, skos:Concept  ;
         skos:inScheme :RoadSignTypeCode ;
         rdfs:label "13_873"@en ;
         skos:definition "End of residential area"@en .
         :RoadSignType.13_881 a :RoadSignType, skos:Concept  ;
         skos:inScheme :RoadSignTypeCode ;
         rdfs:label "13_881"@en ;
         skos:definition " Direction of an airfield"@en .
         :RoadSignType.13_882 a :RoadSignType, skos:Concept  ;
         skos:inScheme :RoadSignTypeCode ;
         rdfs:label "13_882"@en ;
         skos:definition "Direction of a camping site."@en .
         :RoadSignType.13_883 a :RoadSignType, skos:Concept  ;
         skos:inScheme :RoadSignTypeCode ;
         rdfs:label "13_883"@en ;
         skos:definition " Direction of a youth hostel"@en .
         :RoadSignType.13_884 a :RoadSignType, skos:Concept  ;
         skos:inScheme :RoadSignTypeCode ;
         rdfs:label "13_884"@en ;
         skos:definition "Direction of public transport"@en .
         :RoadSignType.13_885 a :RoadSignType, skos:Concept  ;
         skos:inScheme :RoadSignTypeCode ;
         rdfs:label "13_885"@en ;
         skos:definition "Confirmatory signs"@en .
         :RoadSignType.13_886 a :RoadSignType, skos:Concept  ;
         skos:inScheme :RoadSignTypeCode ;
         rdfs:label "13_886"@en ;
         skos:definition "Chains or snow tyres recommended"@en .
         :RoadSignType.13_887 a :RoadSignType, skos:Concept  ;
         skos:inScheme :RoadSignTypeCode ;
         rdfs:label "13_887"@en ;
         skos:definition "Advisory speed\""@en .
         :RoadSignType.13_889 a :RoadSignType, skos:Concept  ;
         skos:inScheme :RoadSignTypeCode ;
         rdfs:label "13_889"@en ;
         skos:definition "Advised itinerary for heavy vehicles"@en .
         :RoadSignType.13_891 a :RoadSignType, skos:Concept  ;
         skos:inScheme :RoadSignTypeCode ;
         rdfs:label "13_891"@en ;
         skos:definition " Pedestrian  underpass."@en .
         :RoadSignType.13_892 a :RoadSignType, skos:Concept  ;
         skos:inScheme :RoadSignTypeCode ;
         rdfs:label "13_892"@en ;
         skos:definition "Pedestrian overpass"@en .
         :RoadSignType.13_893 a :RoadSignType, skos:Concept  ;
         skos:inScheme :RoadSignTypeCode ;
         rdfs:label "13_893"@en ;
         skos:definition " Exit from a motorway"@en .
         :RoadSignType.13_894 a :RoadSignType, skos:Concept  ;
         skos:inScheme :RoadSignTypeCode ;
         rdfs:label "13_894"@en ;
         skos:definition "Direction and distance of the nearest emergency exits"@en .
         :RoadSignType.21_111 a :RoadSignType, skos:Concept  ;
         skos:inScheme :RoadSignTypeCode ;
         rdfs:label "21_111"@en ;
         skos:definition "Tourist information"@en .
         :RoadSignType.21_112 a :RoadSignType, skos:Concept  ;
         skos:inScheme :RoadSignTypeCode ;
         rdfs:label "21_112"@en ;
         skos:definition "Police"@en .
         :RoadSignType.21_113 a :RoadSignType, skos:Concept  ;
         skos:inScheme :RoadSignTypeCode ;
         rdfs:label "21_113"@en ;
         skos:definition "Facilities for wheelchair user"@en .
         :RoadSignType.21_114 a :RoadSignType, skos:Concept  ;
         skos:inScheme :RoadSignTypeCode ;
         rdfs:label "21_114"@en ;
         skos:definition "Telephone"@en .
         :RoadSignType.21_115 a :RoadSignType, skos:Concept  ;
         skos:inScheme :RoadSignTypeCode ;
         rdfs:label "21_115"@en ;
         skos:definition "First-aid station"@en .
         :RoadSignType.21_125 a :RoadSignType, skos:Concept  ;
         skos:inScheme :RoadSignTypeCode ;
         rdfs:label "21_125"@en ;
         skos:definition "Maintenance service"@en .
         :RoadSignType.21_126 a :RoadSignType, skos:Concept  ;
         skos:inScheme :RoadSignTypeCode ;
         rdfs:label "21_126"@en ;
         skos:definition "Breakdown service"@en .
         :RoadSignType.21_128 a :RoadSignType, skos:Concept  ;
         skos:inScheme :RoadSignTypeCode ;
         rdfs:label "21_128"@en ;
         skos:definition "Filling station"@en .
         :RoadSignType.21_129 a :RoadSignType, skos:Concept  ;
         skos:inScheme :RoadSignTypeCode ;
         rdfs:label "21_129"@en ;
         skos:definition "Filling station (+GPL)"@en .
         :RoadSignType.21_145 a :RoadSignType, skos:Concept  ;
         skos:inScheme :RoadSignTypeCode ;
         rdfs:label "21_145"@en ;
         skos:definition "Washroom/Restroom"@en .
         :RoadSignType.21_146 a :RoadSignType, skos:Concept  ;
         skos:inScheme :RoadSignTypeCode ;
         rdfs:label "21_146"@en ;
         skos:definition "Restroom for wheelchair user"@en .
         :RoadSignType.21_161 a :RoadSignType, skos:Concept  ;
         skos:inScheme :RoadSignTypeCode ;
         rdfs:label "21_161"@en ;
         skos:definition "Restaurant"@en .
         :RoadSignType.21_162 a :RoadSignType, skos:Concept  ;
         skos:inScheme :RoadSignTypeCode ;
         rdfs:label "21_162"@en ;
         skos:definition "Refreshment stand/ Caféteria"@en .
         :RoadSignType.21_163 a :RoadSignType, skos:Concept  ;
         skos:inScheme :RoadSignTypeCode ;
         rdfs:label "21_163"@en ;
         skos:definition "Service area"@en .
         :RoadSignType.21_164 a :RoadSignType, skos:Concept  ;
         skos:inScheme :RoadSignTypeCode ;
         rdfs:label "21_164"@en ;
         skos:definition "Postal office"@en .
         :RoadSignType.21_181 a :RoadSignType, skos:Concept  ;
         skos:inScheme :RoadSignTypeCode ;
         rdfs:label "21_181"@en ;
         skos:definition "Hotel or Motel"@en .
         :RoadSignType.21_183 a :RoadSignType, skos:Concept  ;
         skos:inScheme :RoadSignTypeCode ;
         rdfs:label "21_183"@en ;
         skos:definition "Youth hostel"@en .
         :RoadSignType.21_185 a :RoadSignType, skos:Concept  ;
         skos:inScheme :RoadSignTypeCode ;
         rdfs:label "21_185"@en ;
         skos:definition "Camping site"@en .
         :RoadSignType.21_186 a :RoadSignType, skos:Concept  ;
         skos:inScheme :RoadSignTypeCode ;
         rdfs:label "21_186"@en ;
         skos:definition "Caravan site"@en .
         :RoadSignType.21_187 a :RoadSignType, skos:Concept  ;
         skos:inScheme :RoadSignTypeCode ;
         rdfs:label "21_187"@en ;
         skos:definition "Camping and caravan site"@en .
         :RoadSignType.21_188 a :RoadSignType, skos:Concept  ;
         skos:inScheme :RoadSignTypeCode ;
         rdfs:label "21_188"@en ;
         skos:definition "Recreational vehicle sanitary station"@en .
         :RoadSignType.21_189 a :RoadSignType, skos:Concept  ;
         skos:inScheme :RoadSignTypeCode ;
         rdfs:label "21_189"@en ;
         skos:definition "Picnic site"@en .
         :RoadSignType.21_191 a :RoadSignType, skos:Concept  ;
         skos:inScheme :RoadSignTypeCode ;
         rdfs:label "21_191"@en ;
         skos:definition "Amusement park"@en .
         :RoadSignType.21_192 a :RoadSignType, skos:Concept  ;
         skos:inScheme :RoadSignTypeCode ;
         rdfs:label "21_192"@en ;
         skos:definition "Starting-point for walks"@en .
         :RoadSignType.21_193 a :RoadSignType, skos:Concept  ;
         skos:inScheme :RoadSignTypeCode ;
         rdfs:label "21_193"@en ;
         skos:definition "Jogging course"@en .
         :RoadSignType.21_194 a :RoadSignType, skos:Concept  ;
         skos:inScheme :RoadSignTypeCode ;
         rdfs:label "21_194"@en ;
         skos:definition "Skiing site"@en .
         :RoadSignType.21_195 a :RoadSignType, skos:Concept  ;
         skos:inScheme :RoadSignTypeCode ;
         rdfs:label "21_195"@en ;
         skos:definition "Ski lift"@en .
         :RoadSignType.21_196 a :RoadSignType, skos:Concept  ;
         skos:inScheme :RoadSignTypeCode ;
         rdfs:label "21_196"@en ;
         skos:definition "Cable car"@en .
         :RoadSignType.21_198 a :RoadSignType, skos:Concept  ;
         skos:inScheme :RoadSignTypeCode ;
         rdfs:label "21_198"@en ;
         skos:definition "Canoeing site"@en .
         :RoadSignType.21_199 a :RoadSignType, skos:Concept  ;
         skos:inScheme :RoadSignTypeCode ;
         rdfs:label "21_199"@en ;
         skos:definition "Cultural assets"@en .
         :RoadSignType.21_211 a :RoadSignType, skos:Concept  ;
         skos:inScheme :RoadSignTypeCode ;
         rdfs:label "21_211"@en ;
         skos:definition "Natural assets"@en .
         :RoadSignType.21_212 a :RoadSignType, skos:Concept  ;
         skos:inScheme :RoadSignTypeCode ;
         rdfs:label "21_212"@en ;
         skos:definition "Museum"@en .
         :RoadSignType.21_213 a :RoadSignType, skos:Concept  ;
         skos:inScheme :RoadSignTypeCode ;
         rdfs:label "21_213"@en ;
         skos:definition "View point"@en .
         :RoadSignType.21_214 a :RoadSignType, skos:Concept  ;
         skos:inScheme :RoadSignTypeCode ;
         rdfs:label "21_214"@en ;
         skos:definition "Park"@en .
         :RoadSignType.31_111 a :RoadSignType, skos:Concept  ;
         skos:inScheme :RoadSignTypeCode ;
         rdfs:label "31_111"@en ;
         skos:definition "Rainfall"@en .
         :RoadSignType.31_112 a :RoadSignType, skos:Concept  ;
         skos:inScheme :RoadSignTypeCode ;
         rdfs:label "31_112"@en ;
         skos:definition "Slippery due to snow / ice"@en .
         :RoadSignType.31_114 a :RoadSignType, skos:Concept  ;
         skos:inScheme :RoadSignTypeCode ;
         rdfs:label "31_114"@en ;
         skos:definition "Poor visibility through snow, rain or fog"@en .
         :RoadSignType.31_113 a :RoadSignType, skos:Concept  ;
         skos:inScheme :RoadSignTypeCode ;
         rdfs:label "31_113"@en ;
         skos:definition "Fog"@en .
         :RoadSignType.31_359 a :RoadSignType, skos:Concept  ;
         skos:inScheme :RoadSignTypeCode ;
         rdfs:label "31_359"@en ;
         skos:definition "Strong side-wind"@en .
         :RoadSignType.31_361 a :RoadSignType, skos:Concept  ;
         skos:inScheme :RoadSignTypeCode ;
         rdfs:label "31_361"@en ;
         skos:definition "Flood"@en .
         :RoadSignType.32_111 a :RoadSignType, skos:Concept  ;
         skos:inScheme :RoadSignTypeCode ;
         rdfs:label "32_111"@en ;
         skos:definition "Traffic congestion"@en .
         :RoadSignType.32_112 a :RoadSignType, skos:Concept  ;
         skos:inScheme :RoadSignTypeCode ;
         rdfs:label "32_112"@en ;
         skos:definition "Accident"@en .
         :RoadSignType.32_113 a :RoadSignType, skos:Concept  ;
         skos:inScheme :RoadSignTypeCode ;
         rdfs:label "32_113"@en ;
         skos:definition "Vehicle on fire"@en .
         :RoadSignType.32_114 a :RoadSignType, skos:Concept  ;
         skos:inScheme :RoadSignTypeCode ;
         rdfs:label "32_114"@en ;
         skos:definition "Shed loads"@en .
         :RoadSignType.32_115 a :RoadSignType, skos:Concept  ;
         skos:inScheme :RoadSignTypeCode ;
         rdfs:label "32_115"@en ;
         skos:definition "Slow moving maintenance vehicle"@en .
         :RoadSignType.32_116 a :RoadSignType, skos:Concept  ;
         skos:inScheme :RoadSignTypeCode ;
         rdfs:label "32_116"@en ;
         skos:definition "Breakdown vehicle"@en .
         

:ChargingPointUsageTypeCode a skos:ConceptScheme ;
    dc:isFormatOf :ChargingPointUsageType ;
    	skos:definition "Specifies the available list of enumerations for the use of electric charging point " .
    
    
:ChargingPointUsageType.electricVehicle a :ChargingPointUsageType, skos:Concept  ;
         skos:inScheme :ChargingPointUsageTypeCode ;
         rdfs:label "electricVehicle"@en ;
         skos:definition "Electric vehicle"@en .
         :ChargingPointUsageType.motorhomeOrCaravanSupply a :ChargingPointUsageType, skos:Concept  ;
         skos:inScheme :ChargingPointUsageTypeCode ;
         rdfs:label "motorhomeOrCaravanSupply"@en ;
         skos:definition "Supplies for charging motorhomes or caravans"@en .
         :ChargingPointUsageType.electricBikeOrMotorcycle a :ChargingPointUsageType, skos:Concept  ;
         skos:inScheme :ChargingPointUsageTypeCode ;
         rdfs:label "electricBikeOrMotorcycle"@en ;
         skos:definition "Supplies for charging electric bikes or motorcycles"@en .
         :ChargingPointUsageType.lorryPowerConsumption a :ChargingPointUsageType, skos:Concept  ;
         skos:inScheme :ChargingPointUsageTypeCode ;
         rdfs:label "lorryPowerConsumption"@en ;
         skos:definition "Lorry power consumption"@en .
         :ChargingPointUsageType.electricalDevices a :ChargingPointUsageType, skos:Concept  ;
         skos:inScheme :ChargingPointUsageTypeCode ;
         rdfs:label "electricalDevices"@en ;
         skos:definition "Supplies for charging electrical devices"@en .
         :ChargingPointUsageType.other a :ChargingPointUsageType, skos:Concept  ;
         skos:inScheme :ChargingPointUsageTypeCode ;
         rdfs:label "other"@en ;
         skos:definition "Other"@en .
         

:OpenLRBinaryVersionCode a skos:ConceptScheme ;
    dc:isFormatOf :OpenLRBinaryVersion ;
    	skos:definition "Specifies the available list of enumerations for the version of the OpenLR binary specification" .
    
    
:OpenLRBinaryVersion.v2_4 a :OpenLRBinaryVersion, skos:Concept  ;
         skos:inScheme :OpenLRBinaryVersionCode ;
         rdfs:label "v2_4"@en ;
         skos:definition "Version 2.4"@en .
         

:EmissionClassificationEuroCode a skos:ConceptScheme ;
    dc:isFormatOf :EmissionClassificationEuro ;
    	skos:definition "Specifies the available list of enumerations for the minimum Euro emission classification the vehicle(s) have to comply with according to the 1970 Directive 70/220/EEC and its several amendments. Note that vehicleType and fuelType need to be provided in order to make this classification explicit. [SOURCE - DATEX 3.0 Part 7 (proposed EN/16157-7:2018)]" .
    
    
:EmissionClassificationEuro.euro5 a :EmissionClassificationEuro, skos:Concept  ;
         skos:inScheme :EmissionClassificationEuroCode ;
         rdfs:label "euro5"@en ;
         skos:definition "Euro 5"@en .
         :EmissionClassificationEuro.euro5a a :EmissionClassificationEuro, skos:Concept  ;
         skos:inScheme :EmissionClassificationEuroCode ;
         rdfs:label "euro5a"@en ;
         skos:definition "Euro 5a"@en .
         :EmissionClassificationEuro.euro5b a :EmissionClassificationEuro, skos:Concept  ;
         skos:inScheme :EmissionClassificationEuroCode ;
         rdfs:label "euro5b"@en ;
         skos:definition "Euro 5b"@en .
         :EmissionClassificationEuro.euro6 a :EmissionClassificationEuro, skos:Concept  ;
         skos:inScheme :EmissionClassificationEuroCode ;
         rdfs:label "euro6"@en ;
         skos:definition "Euro 6"@en .
         :EmissionClassificationEuro.euro6a a :EmissionClassificationEuro, skos:Concept  ;
         skos:inScheme :EmissionClassificationEuroCode ;
         rdfs:label "euro6a"@en ;
         skos:definition "Euro 6a"@en .
         :EmissionClassificationEuro.euro6b a :EmissionClassificationEuro, skos:Concept  ;
         skos:inScheme :EmissionClassificationEuroCode ;
         rdfs:label "euro6b"@en ;
         skos:definition "Euro 6b"@en .
         :EmissionClassificationEuro.euro6c a :EmissionClassificationEuro, skos:Concept  ;
         skos:inScheme :EmissionClassificationEuroCode ;
         rdfs:label "euro6c"@en ;
         skos:definition "Euro 6c"@en .
         :EmissionClassificationEuro.euroV a :EmissionClassificationEuro, skos:Concept  ;
         skos:inScheme :EmissionClassificationEuroCode ;
         rdfs:label "euroV"@en ;
         skos:definition "Euro V"@en .
         :EmissionClassificationEuro.euroVI a :EmissionClassificationEuro, skos:Concept  ;
         skos:inScheme :EmissionClassificationEuroCode ;
         rdfs:label "euroVI"@en ;
         skos:definition "Euro VI"@en .
         :EmissionClassificationEuro.other a :EmissionClassificationEuro, skos:Concept  ;
         skos:inScheme :EmissionClassificationEuroCode ;
         rdfs:label "other"@en ;
         skos:definition "Other Euro classifications"@en .
         

:LowEmissionLevelCode a skos:ConceptScheme ;
    dc:isFormatOf :LowEmissionLevel ;
    	skos:definition "Specifies the available list of enumerations for vehicle emission levels" .
    
    
:LowEmissionLevel.lowLevelEmission a :LowEmissionLevel, skos:Concept  ;
         skos:inScheme :LowEmissionLevelCode ;
         rdfs:label "lowLevelEmission"@en ;
         skos:definition "Vehicles with low emission levels."@en .
         :LowEmissionLevel.freeOfEmission a :LowEmissionLevel, skos:Concept  ;
         skos:inScheme :LowEmissionLevelCode ;
         rdfs:label "freeOfEmission"@en ;
         skos:definition "Only vehicles that do not produce emissions (e.g. electric driven). Hybrid driven cars are allowed, when they switch to emission free mode within the considered situation."@en .
         

:RoadFeatureEventTypeCode a skos:ConceptScheme ;
    dc:isFormatOf :RoadFeatureEventType ;
    	skos:definition "Specifies the available list of enumerations for the types of Road Feature Events" .
    
    
:RoadFeatureEventType.decodeLocationError a :RoadFeatureEventType, skos:Concept  ;
         skos:inScheme :RoadFeatureEventTypeCode ;
         rdfs:label "decodeLocationError"@en ;
         skos:definition "An error occured when trying to decode the location for the given safety feature"@en .
         :RoadFeatureEventType.decodeLocationErrorGeometryMismatch a :RoadFeatureEventType, skos:Concept  ;
         skos:inScheme :RoadFeatureEventTypeCode ;
         rdfs:label "decodeLocationErrorGeometryMismatch"@en ;
         skos:definition "An error occured when trying to decode the location for the given safety feature due to geometry mismatch"@en .
         :RoadFeatureEventType.decodeLocationRoadDescriptorMismatch a :RoadFeatureEventType, skos:Concept  ;
         skos:inScheme :RoadFeatureEventTypeCode ;
         rdfs:label "decodeLocationRoadDescriptorMismatch"@en ;
         skos:definition "An error occured when trying to decode the location for the given safety feature due to road descriptor mismatch"@en .
         :RoadFeatureEventType.illegalPropertyValue a :RoadFeatureEventType, skos:Concept  ;
         skos:inScheme :RoadFeatureEventTypeCode ;
         rdfs:label "illegalPropertyValue"@en ;
         skos:definition "An error occured due to an illegal properfty value for the given safety feature"@en .
         :RoadFeatureEventType.success a :RoadFeatureEventType, skos:Concept  ;
         skos:inScheme :RoadFeatureEventTypeCode ;
         rdfs:label "success"@en ;
         skos:definition "The safty feature was successfully integrated on the receiver side"@en .
         

:RoadFeaturePropertyTypeCode a skos:ConceptScheme ;
    dc:isFormatOf :RoadFeaturePropertyType ;
    	skos:definition "Specifies the available list of enumerations for the various types of road features" .
    
    
:RoadFeaturePropertyType.maximumSpeedLimit a :RoadFeaturePropertyType, skos:Concept  ;
         skos:inScheme :RoadFeaturePropertyTypeCode ;
         rdfs:label "maximumSpeedLimit"@en ;
         skos:definition "Specifies the maximum speed limit, aligned with the concept of maximum speed limit of the Vienna Convention on Road Signs, 1968, where this concept is defined as the maximum speed in the unit of measurement most commonly used to express the speed of vehicles in the country concerned"@en .
         :RoadFeaturePropertyType.compulsoryMinimumSpeed a :RoadFeaturePropertyType, skos:Concept  ;
         skos:inScheme :RoadFeaturePropertyTypeCode ;
         rdfs:label "compulsoryMinimumSpeed"@en ;
         skos:definition "Specifies the compulsory minimum speed, aligned with the concept of compulsort minimum speed of the Vienna Convention on Road Signs, 1968, where this concept is defined as that vehicles using the road at the entrance to which it (the sign) is placed shall travel at not less than the speed specified ... shown on the sign shall express this speed in the unit of measurement most commonly used to express the speed of vehicles in the country concerned. "@en .
         :RoadFeaturePropertyType.advisorySpeed a :RoadFeaturePropertyType, skos:Concept  ;
         skos:inScheme :RoadFeaturePropertyTypeCode ;
         rdfs:label "advisorySpeed"@en ;
         skos:definition " \"ADVISORY SPEED\" shall be used to show the speed at which it is advisable to drive if circumstances permit and if the driver is not required to comply with a lower limit specific to his category of vehicle. [SOURCE: Vienna Convention on Road Signs, 1968]"@en .
         :RoadFeaturePropertyType.maximumWeightPerSingleAxle a :RoadFeaturePropertyType, skos:Concept  ;
         skos:inScheme :RoadFeaturePropertyTypeCode ;
         rdfs:label "maximumWeightPerSingleAxle"@en ;
         skos:definition "The maximum weight per single axle allowed"@en .
         :RoadFeaturePropertyType.maximumHeight a :RoadFeaturePropertyType, skos:Concept  ;
         skos:inScheme :RoadFeaturePropertyTypeCode ;
         rdfs:label "maximumHeight"@en ;
         skos:definition "The maximum height allowed"@en .
         :RoadFeaturePropertyType.maximumWidth a :RoadFeaturePropertyType, skos:Concept  ;
         skos:inScheme :RoadFeaturePropertyTypeCode ;
         rdfs:label "maximumWidth"@en ;
         skos:definition "The maximum width allowed"@en .
         :RoadFeaturePropertyType.maximumLadenWeight a :RoadFeaturePropertyType, skos:Concept  ;
         skos:inScheme :RoadFeaturePropertyTypeCode ;
         rdfs:label "maximumLadenWeight"@en ;
         skos:definition "The maximum laden weight allowed"@en .
         :RoadFeaturePropertyType.maximumLength a :RoadFeaturePropertyType, skos:Concept  ;
         skos:inScheme :RoadFeaturePropertyTypeCode ;
         rdfs:label "maximumLength"@en ;
         skos:definition "The maximum length allowed"@en .
         :RoadFeaturePropertyType.maximumDistanceBetweenVehicles a :RoadFeaturePropertyType, skos:Concept  ;
         skos:inScheme :RoadFeaturePropertyTypeCode ;
         rdfs:label "maximumDistanceBetweenVehicles"@en ;
         skos:definition "The maximum distance between vehicles allowed"@en .
         :RoadFeaturePropertyType.roadSignType a :RoadFeaturePropertyType, skos:Concept  ;
         skos:inScheme :RoadFeaturePropertyTypeCode ;
         rdfs:label "roadSignType"@en ;
         skos:definition "The type of road sign according to separate codelist (see RoadSignType)"@en .
         :RoadFeaturePropertyType.controlled a :RoadFeaturePropertyType, skos:Concept  ;
         skos:inScheme :RoadFeaturePropertyTypeCode ;
         rdfs:label "controlled"@en ;
         skos:definition "Property for pedestrian crossing indicating with a boolean value whether the crossing is controlled by traffic signals or not"@en .
         :RoadFeaturePropertyType.tunnelCategory a :RoadFeaturePropertyType, skos:Concept  ;
         skos:inScheme :RoadFeaturePropertyTypeCode ;
         rdfs:label "tunnelCategory"@en ;
         skos:definition "The used Tunnel Categories are based on the European Agreement Concerning the International Carriage of Dangerous Goods by Road (ADR). If tunnel restrictions on the passage of vehicles carrying dangerous goods are in place, the competent authority shall assign the road tunnel to one or more of the tunnel categories A, B, C, D, E and shall indicate the restriction by means of a road sign and signals as follows:  Tunnel Category A: no sign Tunnel Category B: sign and signal with additional panel bearing a letter B Tunnel Category C: sign and signal with additional panel bearing a letter C Tunnel Category D: sign and signal with additional panel bearing a letter D Tunnel Category E: sign and signal with additional panel bearing a letter E  The European Agreement concerning the International Carriage of Dangerous Goods by Road provides more information about the types of dangerous goods that can be transported through different categories of tunnel "@en .
         :RoadFeaturePropertyType.paymentMethod a :RoadFeaturePropertyType, skos:Concept  ;
         skos:inScheme :RoadFeaturePropertyTypeCode ;
         rdfs:label "paymentMethod"@en ;
         skos:definition "The payment method depends on the toll collection method or system in place. For road users it is of interest what kind of payment method is required or accepted"@en .
         :RoadFeaturePropertyType.fixedCharge a :RoadFeaturePropertyType, skos:Concept  ;
         skos:inScheme :RoadFeaturePropertyTypeCode ;
         rdfs:label "fixedCharge"@en ;
         skos:definition "A fixed charge or pricing assessed for the toll road"@en .
         :RoadFeaturePropertyType.parkingSite a :RoadFeaturePropertyType, skos:Concept  ;
         skos:inScheme :RoadFeaturePropertyTypeCode ;
         rdfs:label "parkingSite"@en ;
         skos:definition "A record containing static details of a parking site. Must be specialised as an 'Urban-' or 'InterUrbanParkingSite' or a 'SpecialLocationParkingSite'. UrbanParkingSite = parking site in an urban context (e.g. parking lot, parking garage, on-street-parking, parkAndRide) InterUrbanParking = A parking site in an interurban context (like nearby motorway, motorway, ferry terminal, airport terminal, on street parking) SpecialLocationParkingSites = A parking site which is located at a special location, often associated with some building."@en .
         :RoadFeaturePropertyType.siteAccessability a :RoadFeaturePropertyType, skos:Concept  ;
         skos:inScheme :RoadFeaturePropertyTypeCode ;
         rdfs:label "siteAccessability"@en ;
         skos:definition "Type of accessability to site (e.g. ChargingPoint, RefillPointGas)"@en .
         :RoadFeaturePropertyType.chargingPointUsageType a :RoadFeaturePropertyType, skos:Concept  ;
         skos:inScheme :RoadFeaturePropertyTypeCode ;
         rdfs:label "chargingPointUsageType"@en ;
         skos:definition "Specifies usage of the charging point"@en .
         :RoadFeaturePropertyType.gasType a :RoadFeaturePropertyType, skos:Concept  ;
         skos:inScheme :RoadFeaturePropertyTypeCode ;
         rdfs:label "gasType"@en ;
         skos:definition "Type of fuel used by a vehicle; proposed enumerations are taken from the Del. Reg: Compressed natural gas (CNG); liquefied natural gas (LNG); liquefied petroleum gas (LPG)"@en .
         :RoadFeaturePropertyType.iFOPTobjectKey a :RoadFeaturePropertyType, skos:Concept  ;
         skos:inScheme :RoadFeaturePropertyTypeCode ;
         rdfs:label "iFOPTobjectKey"@en ;
         skos:definition "When referencing public transport stops and stopping points use the European Standard IFOPT (CEN, EN 28701:2012). The syntax of a IFOPT referencing key is: country_code:region:stop_number:stop_area:stop_point (e.g. de:9162:1 for Stop Karlsplatz in Munich)"@en .
         :RoadFeaturePropertyType.vMSUnitIdentifier a :RoadFeaturePropertyType, skos:Concept  ;
         skos:inScheme :RoadFeaturePropertyTypeCode ;
         rdfs:label "vMSUnitIdentifier"@en ;
         skos:definition "Specifies a data provider unique value for the identifier for a specific variable message sign unit"@en .
         :RoadFeaturePropertyType.trafficSignalIdentifier a :RoadFeaturePropertyType, skos:Concept  ;
         skos:inScheme :RoadFeaturePropertyTypeCode ;
         rdfs:label "trafficSignalIdentifier"@en ;
         skos:definition "Specifies a data provider unique value for the identifier for a specific traffic signal site"@en .
         

:RoadCategoryCode a skos:ConceptScheme ;
    dc:isFormatOf :RoadCategory ;
    	skos:definition "Specifies the available list of enumerations for the road category types" .
    
    
:RoadCategory.motorway a :RoadCategory, skos:Concept  ;
         skos:inScheme :RoadCategoryCode ;
         rdfs:label "motorway"@en ;
         skos:definition "Indicating the presence of a motorway. NOTE: the Vienna Convention 1968 indicates a motorway as meet the following: (j) \"Motorway\" means a road specially designed and built for motor traffic, which does not serve properties bordering on it, and which:  (i) Is provided, except at special points or temporarily, with separate carriageways for the two directions of traffic, separated from each other either by a dividing strip not intended for traffic or, exceptionally, by other means;   (ii) Does not cross at level with any road, railway or tramway track, or footpath; and   (iii) Is specially signposted as a motorway;"@en .
         :RoadCategory.roadWithDualCarriageway a :RoadCategory, skos:Concept  ;
         skos:inScheme :RoadCategoryCode ;
         rdfs:label "roadWithDualCarriageway"@en ;
         skos:definition "Road with more than one divided carriageway"@en .
         :RoadCategory.roadWithSingleCarriageway a :RoadCategory, skos:Concept  ;
         skos:inScheme :RoadCategoryCode ;
         rdfs:label "roadWithSingleCarriageway"@en ;
         skos:definition "Road with only one carriageway. NOTE: May be with traffic in one direction or two."@en .
         :RoadCategory.urbanRoad a :RoadCategory, skos:Concept  ;
         skos:inScheme :RoadCategoryCode ;
         rdfs:label "urbanRoad"@en ;
         skos:definition "Road in an urban environment"@en .
         :RoadCategory.residentialAreaRoad a :RoadCategory, skos:Concept  ;
         skos:inScheme :RoadCategoryCode ;
         rdfs:label "residentialAreaRoad"@en ;
         skos:definition "Road in a residential zone"@en .
         :RoadCategory.otherRoad a :RoadCategory, skos:Concept  ;
         skos:inScheme :RoadCategoryCode ;
         rdfs:label "otherRoad"@en ;
         skos:definition "Road of a category other than the above"@en .
         

:RoadFeatureTypeCode a skos:ConceptScheme ;
    dc:isFormatOf :RoadFeatureType ;
    	skos:definition "Specifies the available list of enumerations for the various types of road features" .
    
    
:RoadFeatureType.pedestrianCrossing a :RoadFeatureType, skos:Concept  ;
         skos:inScheme :RoadFeatureTypeCode ;
         rdfs:label "pedestrianCrossing"@en ;
         skos:definition "A specified part of a road where pedestrians have right of way to cross"@en .
         :RoadFeatureType.restrictionForVehicles a :RoadFeatureType, skos:Concept  ;
         skos:inScheme :RoadFeatureTypeCode ;
         rdfs:label "restrictionForVehicles"@en ;
         skos:definition "Restriction for vehicles regarding weight, height or length"@en .
         :RoadFeatureType.speedLimit a :RoadFeatureType, skos:Concept  ;
         skos:inScheme :RoadFeatureTypeCode ;
         rdfs:label "speedLimit"@en ;
         skos:definition "Location of a speed restricted zone which defines a speed limit characteristic (e.g. maximum, compulsory minimum, advisory [maximum]) providing context for vehicles travelling on a particular stretch of road "@en .
         :RoadFeatureType.startOfSpeedLimit a :RoadFeatureType, skos:Concept  ;
         skos:inScheme :RoadFeatureTypeCode ;
         rdfs:label "startOfSpeedLimit"@en ;
         skos:definition "Location of the start of a speed restricted zone which defines a speed limit characteristic (e.g. maximum, compulsory minimum, advisory [maximum]) providing context for vehicles travelling on a particular stretch of road"@en .
         :RoadFeatureType.endOfSpeedLimit a :RoadFeatureType, skos:Concept  ;
         skos:inScheme :RoadFeatureTypeCode ;
         rdfs:label "endOfSpeedLimit"@en ;
         skos:definition "Location of the end of a speed restricted zone which defines a speed limit characteristic (e.g. maximum, compulsory minimum, advisory [maximum]) providing context for vehicles travelling on a particular stretch of road"@en .
         :RoadFeatureType.prohibitionOfOvertaking a :RoadFeatureType, skos:Concept  ;
         skos:inScheme :RoadFeatureTypeCode ;
         rdfs:label "prohibitionOfOvertaking"@en ;
         skos:definition "Indicating a zone where overtaking of other vehicles is prohibited.  NOTE: Overtaking is normally interpreted as crossing the central dividing line of a single carriageway two-way road, to facilitate the overtaking of another slower-moving vehicle, but can also involve other forms of restriction such as lorries being limited to use of specified slower lanes, and not being permitted to move to other lanes."@en .
         :RoadFeatureType.startOfProhibitionOfOvertaking a :RoadFeatureType, skos:Concept  ;
         skos:inScheme :RoadFeatureTypeCode ;
         rdfs:label "startOfProhibitionOfOvertaking"@en ;
         skos:definition "Indicating the start of a zone which is subject to a prohibition of overtaking."@en .
         :RoadFeatureType.useOfAudibleWarningDevicesProhibited a :RoadFeatureType, skos:Concept  ;
         skos:inScheme :RoadFeatureTypeCode ;
         rdfs:label "useOfAudibleWarningDevicesProhibited"@en ;
         skos:definition "Indicating a zone which is subject to a prohibition on the use of audible warning devices.  NOTE: Audible warning devices include vehicle horns."@en .
         :RoadFeatureType.startOfUseOfAudibleWarningDevicesProhibited a :RoadFeatureType, skos:Concept  ;
         skos:inScheme :RoadFeatureTypeCode ;
         rdfs:label "startOfUseOfAudibleWarningDevicesProhibited"@en ;
         skos:definition "The start of a zone which is subject to a prohibition on the use of audible warning devices."@en .
         :RoadFeatureType.endOfProhibitionOrRestriction a :RoadFeatureType, skos:Concept  ;
         skos:inScheme :RoadFeatureTypeCode ;
         rdfs:label "endOfProhibitionOrRestriction"@en ;
         skos:definition "A zone which is the end of prohibition or restriction.  NOTE: This is considered to apply to any single or multiple prohibitions or restrictions. In the case where the end of prohibitions or restrictions coincide, this location reference is used to indicate the end of at least one prohibition or restriction."@en .
         :RoadFeatureType.prohibitedTurn a :RoadFeatureType, skos:Concept  ;
         skos:inScheme :RoadFeatureTypeCode ;
         rdfs:label "prohibitedTurn"@en ;
         skos:definition "Indicating a prohibited turning motion and a junction of roads.  NOTE: Turn restrictions types come in many forms and can be dependent of the type of vehicle; its usage; its load; vehicle occupancy; the capabilities permitted under the licence of the vehicle driver’s driver licence permissions; vehicle physical characteristics; propulsion type; the restrictions may also be time and day dependent, weather dependent, etc."@en .
         :RoadFeatureType.passingWithoutStoppingProhibited a :RoadFeatureType, skos:Concept  ;
         skos:inScheme :RoadFeatureTypeCode ;
         rdfs:label "passingWithoutStoppingProhibited"@en ;
         skos:definition "Indicating a zone which is subject to a prohibition of continuing without coming to a stop.  Note: this may be in common use at toll plazas, police and other checkpoints, custom checkpoints, etc"@en .
         :RoadFeatureType.motorway a :RoadFeatureType, skos:Concept  ;
         skos:inScheme :RoadFeatureTypeCode ;
         rdfs:label "motorway"@en ;
         skos:definition "Indicating the presence of a motorway.  NOTE: the Vienna Convention 1968 indicates a motorway as meet the following:   (j) \"Motorway\" means a road specially designed and built for motor traffic, which does not serve properties bordering on it, and which:         (i) Is provided, except at special points or temporarily, with separate carriageways for the two directions of traffic, separated from each other either by a dividing strip not intended for traffic or, exceptionally, by other means;        (ii) Does not cross at level with any road, railway or tramway track, or footpath; and       (iii) Is specially signposted as a motorway;"@en .
         :RoadFeatureType.startOfMotorway a :RoadFeatureType, skos:Concept  ;
         skos:inScheme :RoadFeatureTypeCode ;
         rdfs:label "startOfMotorway"@en ;
         skos:definition "indicating the start of a motorway."@en .
         :RoadFeatureType.endOfMotorway a :RoadFeatureType, skos:Concept  ;
         skos:inScheme :RoadFeatureTypeCode ;
         rdfs:label "endOfMotorway"@en ;
         skos:definition "indicating the end of a motorway"@en .
         :RoadFeatureType.noEntry a :RoadFeatureType, skos:Concept  ;
         skos:inScheme :RoadFeatureTypeCode ;
         rdfs:label "noEntry"@en ;
         skos:definition "indicating no entry to a section of road.  NOTE: No entry restrictions may be qualified by a range of conditions, including but not limited to: time/day/date; vehicle type; vehicle usage, etc"@en .
         :RoadFeatureType.closedToAllVehiclesInBothDirections a :RoadFeatureType, skos:Concept  ;
         skos:inScheme :RoadFeatureTypeCode ;
         rdfs:label "closedToAllVehiclesInBothDirections"@en ;
         skos:definition "indicating a section of road is closed to all vehicles in both directions of travel."@en .
         :RoadFeatureType.directionToBeFollowed a :RoadFeatureType, skos:Concept  ;
         skos:inScheme :RoadFeatureTypeCode ;
         rdfs:label "directionToBeFollowed"@en ;
         skos:definition "indicating a mandatory route or turn to be followed."@en .
         :RoadFeatureType.snowChainsCompulsory a :RoadFeatureType, skos:Concept  ;
         skos:inScheme :RoadFeatureTypeCode ;
         rdfs:label "snowChainsCompulsory"@en ;
         skos:definition "indicating a zone where the use of snow chains or equivalent winter equipment is mandatory."@en .
         :RoadFeatureType.compulsoryDirectionForVehicleCarryingDangerousGoods a :RoadFeatureType, skos:Concept  ;
         skos:inScheme :RoadFeatureTypeCode ;
         rdfs:label "compulsoryDirectionForVehicleCarryingDangerousGoods"@en ;
         skos:definition "indicating a mandatory route or turn to be followed for vehicles carrying Dangerous Goods.  Note: See European Agreement Concerning the International Carriage of Dangerous Goods by Road (ADR) in Europe."@en .
         :RoadFeatureType.roadForMotorVehicles a :RoadFeatureType, skos:Concept  ;
         skos:inScheme :RoadFeatureTypeCode ;
         rdfs:label "roadForMotorVehicles"@en ;
         skos:definition "indicating a zone which is a road intended for use by motor vehicles."@en .
         :RoadFeatureType.startOfRoadForMotorVehicles a :RoadFeatureType, skos:Concept  ;
         skos:inScheme :RoadFeatureTypeCode ;
         rdfs:label "startOfRoadForMotorVehicles"@en ;
         skos:definition "indicating the start of a zone which is a road intended for use by motor vehicles"@en .
         :RoadFeatureType.endOfRoadForMotorVehicles a :RoadFeatureType, skos:Concept  ;
         skos:inScheme :RoadFeatureTypeCode ;
         rdfs:label "endOfRoadForMotorVehicles"@en ;
         skos:definition "indicating the end of a zone which is a road intended for use by motor vehicles"@en .
         :RoadFeatureType.builtUpArea a :RoadFeatureType, skos:Concept  ;
         skos:inScheme :RoadFeatureTypeCode ;
         rdfs:label "builtUpArea"@en ;
         skos:definition "indicating a zone which is of an urban developed nature.  NOTE: This form of safety feature may be further characterised, or provide reference to common regulations and restrictions that are applicable in a built-up area.  NOTE: Taking into account e.g. the UK Highway Code, a built-up area is a settled area in which the speed limit of a road is automatically 30 mph (48 km/h). These roads are known as 'restricted roads' and are identified by the presence of street lights.  That means that there is a traffic regulation existing that assigns automatically a speed limit to a specific road (by law)."@en .
         :RoadFeatureType.startOfBuiltUpArea a :RoadFeatureType, skos:Concept  ;
         skos:inScheme :RoadFeatureTypeCode ;
         rdfs:label "startOfBuiltUpArea"@en ;
         skos:definition "indicating the start of a zone which is of an urban developed nature."@en .
         :RoadFeatureType.endOfBuiltUpArea a :RoadFeatureType, skos:Concept  ;
         skos:inScheme :RoadFeatureTypeCode ;
         rdfs:label "endOfBuiltUpArea"@en ;
         skos:definition "indicating the end of a zone which is of an urban developed nature."@en .
         :RoadFeatureType.residentialArea a :RoadFeatureType, skos:Concept  ;
         skos:inScheme :RoadFeatureTypeCode ;
         rdfs:label "residentialArea"@en ;
         skos:definition "indicating a zone which is of a residential housing nature.  NOTE: This form of safety feature may be further characterised, or provide reference to common regulations and restrictions that are applicable in a residential area.  A residential area is a road or a zone where most of the buildings are houses and is mostly a traffic-calmed sector, where automatically specific traffic regulations apply, like speed limits."@en .
         :RoadFeatureType.startOfResidentialArea a :RoadFeatureType, skos:Concept  ;
         skos:inScheme :RoadFeatureTypeCode ;
         rdfs:label "startOfResidentialArea"@en ;
         skos:definition "indicating the start of a zone which is of a residential housing nature"@en .
         :RoadFeatureType.endOfResidentialArea a :RoadFeatureType, skos:Concept  ;
         skos:inScheme :RoadFeatureTypeCode ;
         rdfs:label "endOfResidentialArea"@en ;
         skos:definition "indicating the end of a zone which is of a residential housing nature."@en .
         :RoadFeatureType.roadSign a :RoadFeatureType, skos:Concept  ;
         skos:inScheme :RoadFeatureTypeCode ;
         rdfs:label "roadSign"@en ;
         skos:definition "indicating the presence of a road sign "@en .
         :RoadFeatureType.tollStation a :RoadFeatureType, skos:Concept  ;
         skos:inScheme :RoadFeatureTypeCode ;
         rdfs:label "tollStation"@en ;
         skos:definition "Toll or road usage fee collection point known as toll booths, toll houses, plazas, stations or gates"@en .
         :RoadFeatureType.tollRoad a :RoadFeatureType, skos:Concept  ;
         skos:inScheme :RoadFeatureTypeCode ;
         rdfs:label "tollRoad"@en ;
         skos:definition "Public or private roadway for which a road-usage fee or toll is assessed for passage. There are various fee charging concepts and toll collection methods available"@en .
         :RoadFeatureType.parkingSite a :RoadFeatureType, skos:Concept  ;
         skos:inScheme :RoadFeatureTypeCode ;
         rdfs:label "parkingSite"@en ;
         skos:definition "named according to DATEX II Package ParkingSite"@en .
         :RoadFeatureType.chargingPoint a :RoadFeatureType, skos:Concept  ;
         skos:inScheme :RoadFeatureTypeCode ;
         rdfs:label "chargingPoint"@en ;
         skos:definition "Electric vehicle charging point, also called EV charging station (element in an infrastructure that supplies electric energy for the recharging of electric vehicles)."@en .
         :RoadFeatureType.refillPointGas a :RoadFeatureType, skos:Concept  ;
         skos:inScheme :RoadFeatureTypeCode ;
         rdfs:label "refillPointGas"@en ;
         skos:definition "Refill point for gas is an element in an infrastructure that supplies different kind of gas fuels for recharging for natural gas vehicles"@en .
         :RoadFeatureType.publicTransportStop a :RoadFeatureType, skos:Concept  ;
         skos:inScheme :RoadFeatureTypeCode ;
         rdfs:label "publicTransportStop"@en ;
         skos:definition "Public transport stop"@en .
         :RoadFeatureType.transferNodeStopPoint a :RoadFeatureType, skos:Concept  ;
         skos:inScheme :RoadFeatureTypeCode ;
         rdfs:label "transferNodeStopPoint"@en ;
         skos:definition "Stop point at a transfer node, e.g. Airport, Railway station, where people or goods may change mode of transport (ISO 19147)"@en .
         

:SiteAccessibilityTypeCode a skos:ConceptScheme ;
    dc:isFormatOf :SiteAccessibilityType ;
    	skos:definition "Specifies the available list of enumerations for types of site accessibility" .
    
    
:SiteAccessibilityType.publicAccessible a :SiteAccessibilityType, skos:Concept  ;
         skos:inScheme :SiteAccessibilityTypeCode ;
         rdfs:label "publicAccessible"@en ;
         skos:definition "Public accessible"@en .
         :SiteAccessibilityType.restrictedAccess a :SiteAccessibilityType, skos:Concept  ;
         skos:inScheme :SiteAccessibilityTypeCode ;
         rdfs:label "restrictedAccess"@en ;
         skos:definition "RestrictedAccess"@en .
         :SiteAccessibilityType.unspecified a :SiteAccessibilityType, skos:Concept  ;
         skos:inScheme :SiteAccessibilityTypeCode ;
         rdfs:label "unspecified"@en ;
         skos:definition "Unspecified"@en .
         

:LoadTypeCode a skos:ConceptScheme ;
    dc:isFormatOf :LoadType ;
    	skos:definition "Specifies the available list of enumerations for types of vehicle loads" .
    
    
:LoadType.abnormalLoad a :LoadType, skos:Concept  ;
         skos:inScheme :LoadTypeCode ;
         rdfs:label "abnormalLoad"@en ;
         skos:definition "A load that exceeds normal vehicle dimensions in terms of height, length, width, gross vehicle weight or axle weight or any combination of these. Generally termed an \"abnormal load\"."@en .
         :LoadType.ammunition a :LoadType, skos:Concept  ;
         skos:inScheme :LoadTypeCode ;
         rdfs:label "ammunition"@en ;
         skos:definition "Ammunition. "@en .
         :LoadType.chemicals a :LoadType, skos:Concept  ;
         skos:inScheme :LoadTypeCode ;
         rdfs:label "chemicals"@en ;
         skos:definition "Chemicals of unspecified type. "@en .
         :LoadType.combustibleMaterials a :LoadType, skos:Concept  ;
         skos:inScheme :LoadTypeCode ;
         rdfs:label "combustibleMaterials"@en ;
         skos:definition "Combustible materials of unspecified type. "@en .
         :LoadType.corrosiveMaterials a :LoadType, skos:Concept  ;
         skos:inScheme :LoadTypeCode ;
         rdfs:label "corrosiveMaterials"@en ;
         skos:definition "Corrosive materials of unspecified type. "@en .
         :LoadType.debris a :LoadType, skos:Concept  ;
         skos:inScheme :LoadTypeCode ;
         rdfs:label "debris"@en ;
         skos:definition "Debris of unspecified type. "@en .
         :LoadType.empty a :LoadType, skos:Concept  ;
         skos:inScheme :LoadTypeCode ;
         rdfs:label "empty"@en ;
         skos:definition "No load"@en .
         :LoadType.explosiveMaterials a :LoadType, skos:Concept  ;
         skos:inScheme :LoadTypeCode ;
         rdfs:label "explosiveMaterials"@en ;
         skos:definition "Explosive materials of unspecified type. "@en .
         :LoadType.extraHighLoad a :LoadType, skos:Concept  ;
         skos:inScheme :LoadTypeCode ;
         rdfs:label "extraHighLoad"@en ;
         skos:definition "A load of exceptional height. "@en .
         :LoadType.extraLongLoad a :LoadType, skos:Concept  ;
         skos:inScheme :LoadTypeCode ;
         rdfs:label "extraLongLoad"@en ;
         skos:definition "A load of exceptional length. "@en .
         :LoadType.extraWideLoad a :LoadType, skos:Concept  ;
         skos:inScheme :LoadTypeCode ;
         rdfs:label "extraWideLoad"@en ;
         skos:definition "A load of exceptional width. "@en .
         :LoadType.fuel a :LoadType, skos:Concept  ;
         skos:inScheme :LoadTypeCode ;
         rdfs:label "fuel"@en ;
         skos:definition "Fuel of unspecified type. "@en .
         :LoadType.glass a :LoadType, skos:Concept  ;
         skos:inScheme :LoadTypeCode ;
         rdfs:label "glass"@en ;
         skos:definition "Glass. "@en .
         :LoadType.goods a :LoadType, skos:Concept  ;
         skos:inScheme :LoadTypeCode ;
         rdfs:label "goods"@en ;
         skos:definition "Any goods of a commercial nature. "@en .
         :LoadType.hazardousMaterials a :LoadType, skos:Concept  ;
         skos:inScheme :LoadTypeCode ;
         rdfs:label "hazardousMaterials"@en ;
         skos:definition "Materials classed as being of a hazardous nature. "@en .
         :LoadType.liquid a :LoadType, skos:Concept  ;
         skos:inScheme :LoadTypeCode ;
         rdfs:label "liquid"@en ;
         skos:definition "Liquid of an unspecified nature. "@en .
         :LoadType.livestock a :LoadType, skos:Concept  ;
         skos:inScheme :LoadTypeCode ;
         rdfs:label "livestock"@en ;
         skos:definition "Livestock. "@en .
         :LoadType.materials a :LoadType, skos:Concept  ;
         skos:inScheme :LoadTypeCode ;
         rdfs:label "materials"@en ;
         skos:definition "General materials of unspecified type. "@en .
         :LoadType.materialsDangerousForPeople a :LoadType, skos:Concept  ;
         skos:inScheme :LoadTypeCode ;
         rdfs:label "materialsDangerousForPeople"@en ;
         skos:definition "Materials classed as being of a danger to people or animals."@en .
         :LoadType.materialsDangerousForTheEnvironment a :LoadType, skos:Concept  ;
         skos:inScheme :LoadTypeCode ;
         rdfs:label "materialsDangerousForTheEnvironment"@en ;
         skos:definition "Materials classed as being potentially dangerous to the environment. "@en .
         :LoadType.materialsDangerousForWater a :LoadType, skos:Concept  ;
         skos:inScheme :LoadTypeCode ;
         rdfs:label "materialsDangerousForWater"@en ;
         skos:definition "Materials classed as being dangerous when exposed to water (e.g. materials which may react exothermically with water). "@en .
         :LoadType.oil a :LoadType, skos:Concept  ;
         skos:inScheme :LoadTypeCode ;
         rdfs:label "oil"@en ;
         skos:definition "Oil. "@en .
         :LoadType.ordinary a :LoadType, skos:Concept  ;
         skos:inScheme :LoadTypeCode ;
         rdfs:label "ordinary"@en ;
         skos:definition "Materials that present limited environmental or health risk. Non-combustible, non-toxic, non-corrosive. "@en .
         :LoadType.perishableProducts a :LoadType, skos:Concept  ;
         skos:inScheme :LoadTypeCode ;
         rdfs:label "perishableProducts"@en ;
         skos:definition "Products or produce that will significantly degrade in quality or freshness over a short period of time. "@en .
         :LoadType.petrol a :LoadType, skos:Concept  ;
         skos:inScheme :LoadTypeCode ;
         rdfs:label "petrol"@en ;
         skos:definition "Petrol or petroleum. "@en .
         :LoadType.pharmaceuticalMaterials a :LoadType, skos:Concept  ;
         skos:inScheme :LoadTypeCode ;
         rdfs:label "pharmaceuticalMaterials"@en ;
         skos:definition "Pharmaceutical materials. "@en .
         :LoadType.radioactiveMaterials a :LoadType, skos:Concept  ;
         skos:inScheme :LoadTypeCode ;
         rdfs:label "radioactiveMaterials"@en ;
         skos:definition "Materials that emit significant quantities of electromagnetic radiation that may present a risk to people, animals or the environment"@en .
         :LoadType.refrigeratedGoods a :LoadType, skos:Concept  ;
         skos:inScheme :LoadTypeCode ;
         rdfs:label "refrigeratedGoods"@en ;
         skos:definition "Refrigerated goods."@en .
         :LoadType.refuse a :LoadType, skos:Concept  ;
         skos:inScheme :LoadTypeCode ;
         rdfs:label "refuse"@en ;
         skos:definition "Refuse."@en .
         :LoadType.toxicMaterials a :LoadType, skos:Concept  ;
         skos:inScheme :LoadTypeCode ;
         rdfs:label "toxicMaterials"@en ;
         skos:definition "Materials of a toxic nature which may damage the environment or endanger public health."@en .
         :LoadType.vehicles a :LoadType, skos:Concept  ;
         skos:inScheme :LoadTypeCode ;
         rdfs:label "vehicles"@en ;
         skos:definition "Vehicles of any type which are being transported."@en .
         :LoadType.other a :LoadType, skos:Concept  ;
         skos:inScheme :LoadTypeCode ;
         rdfs:label "other"@en ;
         skos:definition "Other than as defined in this enumeration."@en .
         

:VehicleEquipmentCode a skos:ConceptScheme ;
    dc:isFormatOf :VehicleEquipment ;
    	skos:definition "Specifies the available list of enumerations for the vehicle equipment types" .
    
    
:VehicleEquipment.notUsingSnowChains a :VehicleEquipment, skos:Concept  ;
         skos:inScheme :VehicleEquipmentCode ;
         rdfs:label "notUsingSnowChains"@en ;
         skos:definition "Vehicle not using snow chains."@en .
         :VehicleEquipment.notUsingSnowChainsOrTyres a :VehicleEquipment, skos:Concept  ;
         skos:inScheme :VehicleEquipmentCode ;
         rdfs:label "notUsingSnowChainsOrTyres"@en ;
         skos:definition "Vehicle not using either snow tyres or snow chains"@en .
         :VehicleEquipment.snowChainsInUse a :VehicleEquipment, skos:Concept  ;
         skos:inScheme :VehicleEquipmentCode ;
         rdfs:label "snowChainsInUse"@en ;
         skos:definition "Vehicle using snow chains. "@en .
         :VehicleEquipment.snowTyresInUse a :VehicleEquipment, skos:Concept  ;
         skos:inScheme :VehicleEquipmentCode ;
         rdfs:label "snowTyresInUse"@en ;
         skos:definition "Vehicle using snow tyres or snow chains. "@en .
         :VehicleEquipment.snowChainsOrTyresInUse a :VehicleEquipment, skos:Concept  ;
         skos:inScheme :VehicleEquipmentCode ;
         rdfs:label "snowChainsOrTyresInUse"@en ;
         skos:definition "Vehicle using snow tyres. "@en .
         :VehicleEquipment.withoutSnowTyresOrChainsOnBoard a :VehicleEquipment, skos:Concept  ;
         skos:inScheme :VehicleEquipmentCode ;
         rdfs:label "withoutSnowTyresOrChainsOnBoard"@en ;
         skos:definition "Vehicle which is not carrying on board snow tyres orchains"@en .
         

:VehicleTypeCode a skos:ConceptScheme ;
    dc:isFormatOf :VehicleType ;
    	skos:definition "Specifies the available list of enumerations for types of vehicle." .
    
    
:VehicleType.anyVehicle a :VehicleType, skos:Concept  ;
         skos:inScheme :VehicleTypeCode ;
         rdfs:label "anyVehicle"@en ;
         skos:definition "Vehicle of any type."@en .
         :VehicleType.articulatedVehicle a :VehicleType, skos:Concept  ;
         skos:inScheme :VehicleTypeCode ;
         rdfs:label "articulatedVehicle"@en ;
         skos:definition "Transport vehicle with articulation between component carriage parts of the vehicle"@en .
         :VehicleType.bicycle a :VehicleType, skos:Concept  ;
         skos:inScheme :VehicleTypeCode ;
         rdfs:label "bicycle"@en ;
         skos:definition "Pedal-driven two-wheeled vehicle"@en .
         :VehicleType.moped a :VehicleType, skos:Concept  ;
         skos:inScheme :VehicleTypeCode ;
         rdfs:label "moped"@en ;
         skos:definition "Moped (a two wheeled motor vehicle characterized by a small engine typically less than 50cc and by normally having pedals). "@en .
         :VehicleType.motorcycle a :VehicleType, skos:Concept  ;
         skos:inScheme :VehicleTypeCode ;
         rdfs:label "motorcycle"@en ;
         skos:definition "Two-wheeled motor vehicle without pedal propulsion"@en .
         :VehicleType.motorscooter a :VehicleType, skos:Concept  ;
         skos:inScheme :VehicleTypeCode ;
         rdfs:label "motorscooter"@en ;
         skos:definition "Motorscooter (a two wheeled motor vehicle characterized by a step-through frame and small diameter wheels). "@en .
         :VehicleType.motorcycleWithSideCar a :VehicleType, skos:Concept  ;
         skos:inScheme :VehicleTypeCode ;
         rdfs:label "motorcycleWithSideCar"@en ;
         skos:definition "Three wheeled vehicle comprising a motorcycle with an attached side car. "@en .
         :VehicleType.car a :VehicleType, skos:Concept  ;
         skos:inScheme :VehicleTypeCode ;
         rdfs:label "car"@en ;
         skos:definition "Small, often privately owned, typically four wheel vehicle for transport of persons and limited goods."@en .
         :VehicleType.largeCar a :VehicleType, skos:Concept  ;
         skos:inScheme :VehicleTypeCode ;
         rdfs:label "largeCar"@en ;
         skos:definition "See car, typically greater than 4.5 metres in length"@en .
         :VehicleType.passengerCar a :VehicleType, skos:Concept  ;
         skos:inScheme :VehicleTypeCode ;
         rdfs:label "passengerCar"@en ;
         skos:definition "See car"@en .
         :VehicleType.smallCar a :VehicleType, skos:Concept  ;
         skos:inScheme :VehicleTypeCode ;
         rdfs:label "smallCar"@en ;
         skos:definition "See car, typically greater than 3.75 metres in length"@en .
         :VehicleType.caravan a :VehicleType, skos:Concept  ;
         skos:inScheme :VehicleTypeCode ;
         rdfs:label "caravan"@en ;
         skos:definition "Non-motorised trailer for towing, intended for human occupancy "@en .
         :VehicleType.carOrLightVehicle a :VehicleType, skos:Concept  ;
         skos:inScheme :VehicleTypeCode ;
         rdfs:label "carOrLightVehicle"@en ;
         skos:definition "Car or light vehicle. "@en .
         :VehicleType.carWithCaravan a :VehicleType, skos:Concept  ;
         skos:inScheme :VehicleTypeCode ;
         rdfs:label "carWithCaravan"@en ;
         skos:definition "Car towing a caravan. "@en .
         :VehicleType.carWithTrailer a :VehicleType, skos:Concept  ;
         skos:inScheme :VehicleTypeCode ;
         rdfs:label "carWithTrailer"@en ;
         skos:definition "Car towing a trailer"@en .
         :VehicleType.bus a :VehicleType, skos:Concept  ;
         skos:inScheme :VehicleTypeCode ;
         rdfs:label "bus"@en ;
         skos:definition "Vehicle for mass road transport"@en .
         :VehicleType.articulatedBus a :VehicleType, skos:Concept  ;
         skos:inScheme :VehicleTypeCode ;
         rdfs:label "articulatedBus"@en ;
         skos:definition "Articulated vehicle. "@en .
         :VehicleType.fourWheelDrive a :VehicleType, skos:Concept  ;
         skos:inScheme :VehicleTypeCode ;
         rdfs:label "fourWheelDrive"@en ;
         skos:definition "Four wheel drive vehicle. "@en .
         :VehicleType.highSidedVehicle a :VehicleType, skos:Concept  ;
         skos:inScheme :VehicleTypeCode ;
         rdfs:label "highSidedVehicle"@en ;
         skos:definition "High sided vehicle. "@en .
         :VehicleType.heavyGoodsVehicle a :VehicleType, skos:Concept  ;
         skos:inScheme :VehicleTypeCode ;
         rdfs:label "heavyGoodsVehicle"@en ;
         skos:definition "Large road vehicle, typically over 2 tonnes gross weight, primarily intended for the transport of goods"@en .
         :VehicleType.heavyGoodsVehicleWithTrailer a :VehicleType, skos:Concept  ;
         skos:inScheme :VehicleTypeCode ;
         rdfs:label "heavyGoodsVehicleWithTrailer"@en ;
         skos:definition "Large road vehicle, typically over 2 tonnes gross weight, primarily intended for the transport of goods with attached towed trailer"@en .
         :VehicleType.heavyDutyTransporter a :VehicleType, skos:Concept  ;
         skos:inScheme :VehicleTypeCode ;
         rdfs:label "heavyDutyTransporter"@en ;
         skos:definition "Large road vehicle, primarily intended for the transport of other vehicles"@en .
         :VehicleType.heavyVehicle a :VehicleType, skos:Concept  ;
         skos:inScheme :VehicleTypeCode ;
         rdfs:label "heavyVehicle"@en ;
         skos:definition "See Heavy Goods Vehicle"@en .
         :VehicleType.lightCommercialVehicle a :VehicleType, skos:Concept  ;
         skos:inScheme :VehicleTypeCode ;
         rdfs:label "lightCommercialVehicle"@en ;
         skos:definition "Road vehicle, typically under 2 tonnes gross weight, primarily intended for the transport of goods"@en .
         :VehicleType.largeGoodsVehicle a :VehicleType, skos:Concept  ;
         skos:inScheme :VehicleTypeCode ;
         rdfs:label "largeGoodsVehicle"@en ;
         skos:definition "See Heavy Goods Vehicle"@en .
         :VehicleType.lightCommercialVehicleWithTrailer a :VehicleType, skos:Concept  ;
         skos:inScheme :VehicleTypeCode ;
         rdfs:label "lightCommercialVehicleWithTrailer"@en ;
         skos:definition "Road vehicle, typically under 2 tonnes gross weight, primarily intended for the transport of goods, with attached towed trailer"@en .
         :VehicleType.longHeavyLorry a :VehicleType, skos:Concept  ;
         skos:inScheme :VehicleTypeCode ;
         rdfs:label "longHeavyLorry"@en ;
         skos:definition "See Heavy Goods Vehicle"@en .
         :VehicleType.lorry a :VehicleType, skos:Concept  ;
         skos:inScheme :VehicleTypeCode ;
         rdfs:label "lorry"@en ;
         skos:definition "Lorry of any type. "@en .
         :VehicleType.van a :VehicleType, skos:Concept  ;
         skos:inScheme :VehicleTypeCode ;
         rdfs:label "van"@en ;
         skos:definition "See light commercial vehicle"@en .
         :VehicleType.minibus a :VehicleType, skos:Concept  ;
         skos:inScheme :VehicleTypeCode ;
         rdfs:label "minibus"@en ;
         skos:definition "Road vehicle, typically under 2 tonnes gross weight, primarily intended for the transport of peoeple"@en .
         :VehicleType.motorhome a :VehicleType, skos:Concept  ;
         skos:inScheme :VehicleTypeCode ;
         rdfs:label "motorhome"@en ;
         skos:definition "Motorised vehicle, intended for human occupancy "@en .
         :VehicleType.agriculturalVehicle a :VehicleType, skos:Concept  ;
         skos:inScheme :VehicleTypeCode ;
         rdfs:label "agriculturalVehicle"@en ;
         skos:definition "Vehicle normally used for agricultural purposes, e.g. tractor, combined harvester etc. "@en .
         :VehicleType.constructionOrMaintenanceVehicle a :VehicleType, skos:Concept  ;
         skos:inScheme :VehicleTypeCode ;
         rdfs:label "constructionOrMaintenanceVehicle"@en ;
         skos:definition "Vehicle normally used for construction or maintenance purposes, e.g. digger, excavator, bulldozer, lorry mounted crane etc."@en .
         :VehicleType.tanker a :VehicleType, skos:Concept  ;
         skos:inScheme :VehicleTypeCode ;
         rdfs:label "tanker"@en ;
         skos:definition "Vehicle with large tank for carrying bulk liquids. "@en .
         :VehicleType.twoWheeledVehicle a :VehicleType, skos:Concept  ;
         skos:inScheme :VehicleTypeCode ;
         rdfs:label "twoWheeledVehicle"@en ;
         skos:definition "Two wheeled vehicle of unspecified type. "@en .
         :VehicleType.threeWheeledVehicle a :VehicleType, skos:Concept  ;
         skos:inScheme :VehicleTypeCode ;
         rdfs:label "threeWheeledVehicle"@en ;
         skos:definition "Three wheeled vehicle of unspecified type. "@en .
         :VehicleType.vehicleWithCaravan a :VehicleType, skos:Concept  ;
         skos:inScheme :VehicleTypeCode ;
         rdfs:label "vehicleWithCaravan"@en ;
         skos:definition "Vehicle (of unspecified type) towing a caravan. "@en .
         :VehicleType.vehicleWithCatalyticConverter a :VehicleType, skos:Concept  ;
         skos:inScheme :VehicleTypeCode ;
         rdfs:label "vehicleWithCatalyticConverter"@en ;
         skos:definition "Vehicle with catalytic converter. "@en .
         :VehicleType.vehicleWithoutCatalyticConverter a :VehicleType, skos:Concept  ;
         skos:inScheme :VehicleTypeCode ;
         rdfs:label "vehicleWithoutCatalyticConverter"@en ;
         skos:definition "Vehicle without catalytic converter. "@en .
         :VehicleType.vehicleWithTrailer a :VehicleType, skos:Concept  ;
         skos:inScheme :VehicleTypeCode ;
         rdfs:label "vehicleWithTrailer"@en ;
         skos:definition "Vehicle (of unspecified type) towing a trailer. "@en .
         :VehicleType.withEvenNumberedRegistrationPlates a :VehicleType, skos:Concept  ;
         skos:inScheme :VehicleTypeCode ;
         rdfs:label "withEvenNumberedRegistrationPlates"@en ;
         skos:definition "Vehicle with even numbered registration plate. "@en .
         :VehicleType.withOddNumberedRegistrationPlates a :VehicleType, skos:Concept  ;
         skos:inScheme :VehicleTypeCode ;
         rdfs:label "withOddNumberedRegistrationPlates"@en ;
         skos:definition "Vehicle with odd numbered registration plate. "@en .
         :VehicleType.metro a :VehicleType, skos:Concept  ;
         skos:inScheme :VehicleTypeCode ;
         rdfs:label "metro"@en ;
         skos:definition "Train-like transport vehicle limited to a rail network within a limited area; at surface, below surface or above surface"@en .
         :VehicleType.lightRail a :VehicleType, skos:Concept  ;
         skos:inScheme :VehicleTypeCode ;
         rdfs:label "lightRail"@en ;
         skos:definition "Train-like transport vehicle limited to a rail network within a limited area; does not include heavy rail lines"@en .
         :VehicleType.trailer a :VehicleType, skos:Concept  ;
         skos:inScheme :VehicleTypeCode ;
         rdfs:label "trailer"@en ;
         skos:definition "Non-motorised vehicle, intended to be towed"@en .
         :VehicleType.tram a :VehicleType, skos:Concept  ;
         skos:inScheme :VehicleTypeCode ;
         rdfs:label "tram"@en ;
         skos:definition "Train-like mass transport vehicle, running on rails, typically partially or wholly on the road network"@en .
         :VehicleType.trolleyBus a :VehicleType, skos:Concept  ;
         skos:inScheme :VehicleTypeCode ;
         rdfs:label "trolleyBus"@en ;
         skos:definition "Bus-like mass transport vehicle hocked up to an electrical network for power supply"@en .
         :VehicleType.articulatedTrolleyBus a :VehicleType, skos:Concept  ;
         skos:inScheme :VehicleTypeCode ;
         rdfs:label "articulatedTrolleyBus"@en ;
         skos:definition "Bus-like mass transport vehicle hocked up to an electrical network for power supply, with articulation between component carriage parts of the vehicle"@en .
         :VehicleType.unknown a :VehicleType, skos:Concept  ;
         skos:inScheme :VehicleTypeCode ;
         rdfs:label "unknown"@en ;
         skos:definition "Unknown vehicle type"@en .
         :VehicleType.other a :VehicleType, skos:Concept  ;
         skos:inScheme :VehicleTypeCode ;
         rdfs:label "other"@en ;
         skos:definition "Other than as defined in this enumeration. "@en .
         

:GasTypeCode a skos:ConceptScheme ;
    dc:isFormatOf :GasType ;
    	skos:definition "Specifies the available list of enumerations for types of propellant gas." .
    
    
:GasType.all a :GasType, skos:Concept  ;
         skos:inScheme :GasTypeCode ;
         rdfs:label "all"@en ;
         skos:definition "All"@en .
         :GasType.cNG a :GasType, skos:Concept  ;
         skos:inScheme :GasTypeCode ;
         rdfs:label "cNG"@en ;
         skos:definition "Compressed natural gas"@en .
         :GasType.lPG a :GasType, skos:Concept  ;
         skos:inScheme :GasTypeCode ;
         rdfs:label "lPG"@en ;
         skos:definition "Liquified petroleum gas"@en .
         :GasType.lNG a :GasType, skos:Concept  ;
         skos:inScheme :GasTypeCode ;
         rdfs:label "lNG"@en ;
         skos:definition "Liquified natural gas"@en .
         :GasType.other a :GasType, skos:Concept  ;
         skos:inScheme :GasTypeCode ;
         rdfs:label "other"@en ;
         skos:definition "Other"@en .
         :GasType.unknown a :GasType, skos:Concept  ;
         skos:inScheme :GasTypeCode ;
         rdfs:label "unknown"@en ;
         skos:definition "Unknown"@en .
         

:AgoraBinaryVersionCode a skos:ConceptScheme ;
    dc:isFormatOf :AgoraBinaryVersion ;
    	skos:definition "Specifies the available list of enumerations for the version of the AGORA binary specification being used" .
    
    
:AgoraBinaryVersion.v1_0 a :AgoraBinaryVersion, skos:Concept  ;
         skos:inScheme :AgoraBinaryVersionCode ;
         rdfs:label "v1_0"@en ;
         skos:definition "Version 1.0"@en .
         :AgoraBinaryVersion.v1_3 a :AgoraBinaryVersion, skos:Concept  ;
         skos:inScheme :AgoraBinaryVersionCode ;
         rdfs:label "v1_3"@en ;
         skos:definition "Version 1.3"@en .
         :AgoraBinaryVersion.v2_4 a :AgoraBinaryVersion, skos:Concept  ;
         skos:inScheme :AgoraBinaryVersionCode ;
         rdfs:label "v2_4"@en ;
         skos:definition "Version 1.0"@en .
         :AgoraBinaryVersion.v2_5 a :AgoraBinaryVersion, skos:Concept  ;
         skos:inScheme :AgoraBinaryVersionCode ;
         rdfs:label "v2_5"@en ;
         skos:definition "Version 2.5"@en .
         :AgoraBinaryVersion.v3_0 a :AgoraBinaryVersion, skos:Concept  ;
         skos:inScheme :AgoraBinaryVersionCode ;
         rdfs:label "v3_0"@en ;
         skos:definition "Version 3.0"@en .
         

:FuzzyTimeTypeCode a skos:ConceptScheme ;
    dc:isFormatOf :FuzzyTimeType ;
    	skos:definition "Specifies the available list of enumerations for the fuzzy time concepts, which provided the definition of start, end or duration time concepts that support the expression of a non-precise or variable qualified concept, resulting in a non-precise, potentially circumstantial defined time period.

Note: Example roads closed at the start of winter in mountainous areas, which is based on actual experienced weather conditions and therefore is not pre-defined.

" .
    
    
:FuzzyTimeType.external a :FuzzyTimeType, skos:Concept  ;
         skos:inScheme :FuzzyTimeTypeCode ;
         rdfs:label "external"@en ;
         skos:definition "Starting period controlled by external device "@en .
         :FuzzyTimeType.dawn a :FuzzyTimeType, skos:Concept  ;
         skos:inScheme :FuzzyTimeTypeCode ;
         rdfs:label "dawn"@en ;
         skos:definition "Starts at dawn"@en .
         :FuzzyTimeType.dusk a :FuzzyTimeType, skos:Concept  ;
         skos:inScheme :FuzzyTimeTypeCode ;
         rdfs:label "dusk"@en ;
         skos:definition "Starts at dusk"@en .
         :FuzzyTimeType.school a :FuzzyTimeType, skos:Concept  ;
         skos:inScheme :FuzzyTimeTypeCode ;
         rdfs:label "school"@en ;
         skos:definition "Starts at any school period (date and hour)"@en .
         :FuzzyTimeType.holiday a :FuzzyTimeType, skos:Concept  ;
         skos:inScheme :FuzzyTimeTypeCode ;
         rdfs:label "holiday"@en ;
         skos:definition "Starts at any holiday"@en .
         :FuzzyTimeType.winter a :FuzzyTimeType, skos:Concept  ;
         skos:inScheme :FuzzyTimeTypeCode ;
         rdfs:label "winter"@en ;
         skos:definition "Beginning of winter"@en .
         :FuzzyTimeType.spring a :FuzzyTimeType, skos:Concept  ;
         skos:inScheme :FuzzyTimeTypeCode ;
         rdfs:label "spring"@en ;
         skos:definition "Beginning of spring"@en .
         :FuzzyTimeType.summer a :FuzzyTimeType, skos:Concept  ;
         skos:inScheme :FuzzyTimeTypeCode ;
         rdfs:label "summer"@en ;
         skos:definition "Beginning of summer"@en .
         :FuzzyTimeType.autumn a :FuzzyTimeType, skos:Concept  ;
         skos:inScheme :FuzzyTimeTypeCode ;
         rdfs:label "autumn"@en ;
         skos:definition "Beginning of autumn"@en .
         :FuzzyTimeType.highTide a :FuzzyTimeType, skos:Concept  ;
         skos:inScheme :FuzzyTimeTypeCode ;
         rdfs:label "highTide"@en ;
         skos:definition "Beginning of high tide"@en .
         :FuzzyTimeType.lowTide a :FuzzyTimeType, skos:Concept  ;
         skos:inScheme :FuzzyTimeTypeCode ;
         rdfs:label "lowTide"@en ;
         skos:definition "Beginning of low tide"@en .
         :FuzzyTimeType.highWater a :FuzzyTimeType, skos:Concept  ;
         skos:inScheme :FuzzyTimeTypeCode ;
         rdfs:label "highWater"@en ;
         skos:definition "Beginning of high water"@en .
         :FuzzyTimeType.lowWater a :FuzzyTimeType, skos:Concept  ;
         skos:inScheme :FuzzyTimeTypeCode ;
         rdfs:label "lowWater"@en ;
         skos:definition "Beginning of low water"@en .
         :FuzzyTimeType.wetSeason a :FuzzyTimeType, skos:Concept  ;
         skos:inScheme :FuzzyTimeTypeCode ;
         rdfs:label "wetSeason"@en ;
         skos:definition "Beginning of wet season"@en .
         :FuzzyTimeType.drySeason a :FuzzyTimeType, skos:Concept  ;
         skos:inScheme :FuzzyTimeTypeCode ;
         rdfs:label "drySeason"@en ;
         skos:definition "Beginning of dry season"@en .
         :FuzzyTimeType.peakHours a :FuzzyTimeType, skos:Concept  ;
         skos:inScheme :FuzzyTimeTypeCode ;
         rdfs:label "peakHours"@en ;
         skos:definition "Start of peak hours, peak hours include rush hour and activity/ scheduled event based times. These would vary by location and by season"@en .
         :FuzzyTimeType.offPeakHours a :FuzzyTimeType, skos:Concept  ;
         skos:inScheme :FuzzyTimeTypeCode ;
         rdfs:label "offPeakHours"@en ;
         skos:definition "start of off-peak hours"@en .
         :FuzzyTimeType.day a :FuzzyTimeType, skos:Concept  ;
         skos:inScheme :FuzzyTimeTypeCode ;
         rdfs:label "day"@en ;
         skos:definition "Start of day"@en .
         :FuzzyTimeType.night a :FuzzyTimeType, skos:Concept  ;
         skos:inScheme :FuzzyTimeTypeCode ;
         rdfs:label "night"@en ;
         skos:definition "Start of night"@en .
         

:VehicleUsageCode a skos:ConceptScheme ;
    dc:isFormatOf :VehicleUsage ;
    	skos:definition "Specifies the available list of enumerations for types of usage of vehicles." .
    
    
:VehicleUsage.agricultural a :VehicleUsage, skos:Concept  ;
         skos:inScheme :VehicleUsageCode ;
         rdfs:label "agricultural"@en ;
         skos:definition "Vehicle used for agricultural purposes. "@en .
         :VehicleUsage.carSharing a :VehicleUsage, skos:Concept  ;
         skos:inScheme :VehicleUsageCode ;
         rdfs:label "carSharing"@en ;
         skos:definition "Vehicles operated by a car-sharing company."@en .
         :VehicleUsage.cityLogistics a :VehicleUsage, skos:Concept  ;
         skos:inScheme :VehicleUsageCode ;
         rdfs:label "cityLogistics"@en ;
         skos:definition "Vehicles that are used to deliver goods in a city area."@en .
         :VehicleUsage.commercial a :VehicleUsage, skos:Concept  ;
         skos:inScheme :VehicleUsageCode ;
         rdfs:label "commercial"@en ;
         skos:definition "Vehicle which is limited to non-private usage or public transport usage.   "@en .
         :VehicleUsage.emergencyServices a :VehicleUsage, skos:Concept  ;
         skos:inScheme :VehicleUsageCode ;
         rdfs:label "emergencyServices"@en ;
         skos:definition "Vehicle used by the emergency services. "@en .
         :VehicleUsage.military a :VehicleUsage, skos:Concept  ;
         skos:inScheme :VehicleUsageCode ;
         rdfs:label "military"@en ;
         skos:definition "Vehicle used by the military. "@en .
         :VehicleUsage.nonCommercial a :VehicleUsage, skos:Concept  ;
         skos:inScheme :VehicleUsageCode ;
         rdfs:label "nonCommercial"@en ;
         skos:definition "Vehicle used for non-commercial or private purposes.    "@en .
         :VehicleUsage.patrol a :VehicleUsage, skos:Concept  ;
         skos:inScheme :VehicleUsageCode ;
         rdfs:label "patrol"@en ;
         skos:definition "Vehicle used as part of a patrol service, e.g. road operator or automobile association patrol vehicle.   "@en .
         :VehicleUsage.recoveryServices a :VehicleUsage, skos:Concept  ;
         skos:inScheme :VehicleUsageCode ;
         rdfs:label "recoveryServices"@en ;
         skos:definition "Vehicle used to provide a recovery service. "@en .
         :VehicleUsage.roadMaintenanceOrConstruction a :VehicleUsage, skos:Concept  ;
         skos:inScheme :VehicleUsageCode ;
         rdfs:label "roadMaintenanceOrConstruction"@en ;
         skos:definition "Vehicle used for road maintenance or construction work purposes. "@en .
         :VehicleUsage.roadOperator a :VehicleUsage, skos:Concept  ;
         skos:inScheme :VehicleUsageCode ;
         rdfs:label "roadOperator"@en ;
         skos:definition "Vehicle used by the road operator. "@en .
         :VehicleUsage.taxi a :VehicleUsage, skos:Concept  ;
         skos:inScheme :VehicleUsageCode ;
         rdfs:label "taxi"@en ;
         skos:definition "Vehicle used to provide an authorised taxi service."@en .
         

:TunnelCategoryCode a skos:ConceptScheme ;
    dc:isFormatOf :TunnelCategory ;
    	skos:definition "Specifies the available list of enumerations for the categories of tunnel access" .
    
    
:TunnelCategory.a a :TunnelCategory, skos:Concept  ;
         skos:inScheme :TunnelCategoryCode ;
         rdfs:label "a"@en ;
         skos:definition "No sign"@en .
         :TunnelCategory.b a :TunnelCategory, skos:Concept  ;
         skos:inScheme :TunnelCategoryCode ;
         rdfs:label "b"@en ;
         skos:definition "Sign with an additional panel bearing a letter B"@en .
         :TunnelCategory.c a :TunnelCategory, skos:Concept  ;
         skos:inScheme :TunnelCategoryCode ;
         rdfs:label "c"@en ;
         skos:definition "Sign with an additional panel bearing a letter C"@en .
         :TunnelCategory.d a :TunnelCategory, skos:Concept  ;
         skos:inScheme :TunnelCategoryCode ;
         rdfs:label "d"@en ;
         skos:definition "Sign with an additional panel bearing a letter D"@en .
         :TunnelCategory.e a :TunnelCategory, skos:Concept  ;
         skos:inScheme :TunnelCategoryCode ;
         rdfs:label "e"@en ;
         skos:definition "Sign with an additional panel bearing a letter E"@en .
         

:UomIdentifierCode a skos:ConceptScheme ;
    dc:isFormatOf :UomIdentifier ;
    	skos:definition "Specifies the available list of preferred enumerations for identifiers for units of measure" .
    
    
:UomIdentifier.kph a :UomIdentifier, skos:Concept  ;
         skos:inScheme :UomIdentifierCode ;
         rdfs:label "kph"@en ;
         skos:definition "Kilometres per hour"@en .
         :UomIdentifier.mph a :UomIdentifier, skos:Concept  ;
         skos:inScheme :UomIdentifierCode ;
         rdfs:label "mph"@en ;
         skos:definition "Miles per hour"@en .
         :UomIdentifier.m a :UomIdentifier, skos:Concept  ;
         skos:inScheme :UomIdentifierCode ;
         rdfs:label "m"@en ;
         skos:definition "Metres"@en .
         :UomIdentifier.yd a :UomIdentifier, skos:Concept  ;
         skos:inScheme :UomIdentifierCode ;
         rdfs:label "yd"@en ;
         skos:definition "Yards"@en .
         :UomIdentifier.mi a :UomIdentifier, skos:Concept  ;
         skos:inScheme :UomIdentifierCode ;
         rdfs:label "mi"@en ;
         skos:definition "Miles"@en .
         :UomIdentifier.km a :UomIdentifier, skos:Concept  ;
         skos:inScheme :UomIdentifierCode ;
         rdfs:label "km"@en ;
         skos:definition "Kilometres"@en .
         :UomIdentifier.ftin a :UomIdentifier, skos:Concept  ;
         skos:inScheme :UomIdentifierCode ;
         rdfs:label "ftin"@en ;
         skos:definition "Feet and inches  Note: To enable this to be coded into a single value the following convention shall be followed.  The feet value is encoded as an integer value and the is suffixed by the inches value which is given as a two digit decimal value, where leading zeros are maintained [e.g. .00, .01, .02, .03, .04, .05, .06, .07, .08, .09, .10, .11, .12].  The value .99 shall indicate the no inches value is provided. "@en .
         :UomIdentifier.t a :UomIdentifier, skos:Concept  ;
         skos:inScheme :UomIdentifierCode ;
         rdfs:label "t"@en ;
         skos:definition "Tonnes"@en .
         :UomIdentifier.kg a :UomIdentifier, skos:Concept  ;
         skos:inScheme :UomIdentifierCode ;
         rdfs:label "kg"@en ;
         skos:definition "Kilogrammes"@en .
         

:NatureOfDistanceMeasureCode a skos:ConceptScheme ;
    dc:isFormatOf :NatureOfDistanceMeasure ;
    	skos:definition "Specifies the available list of enumerations for contexts of forms of interpreting distance measures" .
    
    
:NatureOfDistanceMeasure.advanceWarning a :NatureOfDistanceMeasure, skos:Concept  ;
         skos:inScheme :NatureOfDistanceMeasureCode ;
         rdfs:label "advanceWarning"@en ;
         skos:definition "Advance warning notification of a feature with a specified distance to the feature (e.g. Railway crossing in 200 metres) "@en .
         :NatureOfDistanceMeasure.featureContinuity a :NatureOfDistanceMeasure, skos:Concept  ;
         skos:inScheme :NatureOfDistanceMeasureCode ;
         rdfs:label "featureContinuity"@en ;
         skos:definition "Notification that the effect of the Feature continues for the specified distance (e.g. for the next X km)."@en .
         

:RoadFeatureSourceCode a skos:ConceptScheme ;
    dc:isFormatOf :RoadFeatureSource ;
    	skos:definition "Specifies the available list of enumerations for the various types source concerning road features" .
    
    
:RoadFeatureSource.fixedPlateRoadSign a :RoadFeatureSource, skos:Concept  ;
         skos:inScheme :RoadFeatureSourceCode ;
         rdfs:label "fixedPlateRoadSign"@en ;
         skos:definition "Fixed (permanent, often metal) road sign, with road signs as recognised under the Vienna Convention on Road Signs and Signals, 1968"@en .
         :RoadFeatureSource.variableMessageSign a :RoadFeatureSource, skos:Concept  ;
         skos:inScheme :RoadFeatureSourceCode ;
         rdfs:label "variableMessageSign"@en ;
         skos:definition "Road sign displayed on a variable message sign or other dynamic display equipment, with road signs as recognised under the Vienna Convention on Road Signs and Signals, 1968"@en .
         :RoadFeatureSource.temporaryRoadSign a :RoadFeatureSource, skos:Concept  ;
         skos:inScheme :RoadFeatureSourceCode ;
         rdfs:label "temporaryRoadSign"@en ;
         skos:definition "Temporary (non-permanent) road sign, as recognised under the Vienna Convention on Road Signs and Signals, 1968"@en .
         :RoadFeatureSource.regulation a :RoadFeatureSource, skos:Concept  ;
         skos:inScheme :RoadFeatureSourceCode ;
         rdfs:label "regulation"@en ;
         skos:definition "Road traffic regulation"@en .
         :RoadFeatureSource.otherRoadFeature a :RoadFeatureSource, skos:Concept  ;
         skos:inScheme :RoadFeatureSourceCode ;
         rdfs:label "otherRoadFeature"@en ;
         skos:definition "Other road feature, not covered by the other enumerations"@en .
         

:GeneralFeedbackEventTypeCode a skos:ConceptScheme ;
    dc:isFormatOf :GeneralFeedbackEventType ;
    	skos:definition "Specifies the available list of enumerations for types of general feedback events." .
    
    
:GeneralFeedbackEventType.schemaVersionMismatch a :GeneralFeedbackEventType, skos:Concept  ;
         skos:inScheme :GeneralFeedbackEventTypeCode ;
         rdfs:label "schemaVersionMismatch"@en ;
         skos:definition "There is a mismatch in schema version between the exchanged dataset and what is supported by the receiver"@en .
         

:FuelTypeCode a skos:ConceptScheme ;
    dc:isFormatOf :FuelType ;
    	skos:definition "Specifies the available list of enumerations for the type of fuel used by the vehicle." .
    
    
:FuelType.all a :FuelType, skos:Concept  ;
         skos:inScheme :FuelTypeCode ;
         rdfs:label "all"@en ;
         skos:definition "All fuel types"@en .
         :FuelType.battery a :FuelType, skos:Concept  ;
         skos:inScheme :FuelTypeCode ;
         rdfs:label "battery"@en ;
         skos:definition "Battery"@en .
         :FuelType.biodiesel a :FuelType, skos:Concept  ;
         skos:inScheme :FuelTypeCode ;
         rdfs:label "biodiesel"@en ;
         skos:definition "Biodiesel"@en .
         :FuelType.diesel a :FuelType, skos:Concept  ;
         skos:inScheme :FuelTypeCode ;
         rdfs:label "diesel"@en ;
         skos:definition "Diesel"@en .
         :FuelType.dieselBatteryHybrid a :FuelType, skos:Concept  ;
         skos:inScheme :FuelTypeCode ;
         rdfs:label "dieselBatteryHybrid"@en ;
         skos:definition "Diesel and battery hybrid"@en .
         :FuelType.ethanol a :FuelType, skos:Concept  ;
         skos:inScheme :FuelTypeCode ;
         rdfs:label "ethanol"@en ;
         skos:definition "Ethanol"@en .
         :FuelType.hydrogen a :FuelType, skos:Concept  ;
         skos:inScheme :FuelTypeCode ;
         rdfs:label "hydrogen"@en ;
         skos:definition "Hydrogen"@en .
         :FuelType.liquidGas a :FuelType, skos:Concept  ;
         skos:inScheme :FuelTypeCode ;
         rdfs:label "liquidGas"@en ;
         skos:definition "Liquid gas of any type including LPG. "@en .
         :FuelType.lpg a :FuelType, skos:Concept  ;
         skos:inScheme :FuelTypeCode ;
         rdfs:label "lpg"@en ;
         skos:definition "Liquid petroleum gas"@en .
         :FuelType.methane a :FuelType, skos:Concept  ;
         skos:inScheme :FuelTypeCode ;
         rdfs:label "methane"@en ;
         skos:definition "Methane gas"@en .
         :FuelType.petrol a :FuelType, skos:Concept  ;
         skos:inScheme :FuelTypeCode ;
         rdfs:label "petrol"@en ;
         skos:definition "Petrol"@en .
         :FuelType.petrol95Octane a :FuelType, skos:Concept  ;
         skos:inScheme :FuelTypeCode ;
         rdfs:label "petrol95Octane"@en ;
         skos:definition "Petrol (95 Octane)"@en .
         :FuelType.petrol98Octane a :FuelType, skos:Concept  ;
         skos:inScheme :FuelTypeCode ;
         rdfs:label "petrol98Octane"@en ;
         skos:definition "Petrol (98 Octane)"@en .
         :FuelType.petrolBatteryHybrid a :FuelType, skos:Concept  ;
         skos:inScheme :FuelTypeCode ;
         rdfs:label "petrolBatteryHybrid"@en ;
         skos:definition "Petrol and battery hybrid"@en .
         :FuelType.petrolLeaded a :FuelType, skos:Concept  ;
         skos:inScheme :FuelTypeCode ;
         rdfs:label "petrolLeaded"@en ;
         skos:definition "Leaded petrol"@en .
         :FuelType.petrolUnleaded a :FuelType, skos:Concept  ;
         skos:inScheme :FuelTypeCode ;
         rdfs:label "petrolUnleaded"@en ;
         skos:definition "Unleaded petrol"@en .
         :FuelType.unknown a :FuelType, skos:Concept  ;
         skos:inScheme :FuelTypeCode ;
         rdfs:label "unknown"@en ;
         skos:definition "Unknown"@en .
         :FuelType.other a :FuelType, skos:Concept  ;
         skos:inScheme :FuelTypeCode ;
         rdfs:label "other"@en ;
         skos:definition "Other forms of fuel, not otherwise listed"@en .
         

:SpecialDayTypeCode a skos:ConceptScheme ;
    dc:isFormatOf :SpecialDayType ;
    	skos:definition "Specifies the available list of enumerations for the special days" .
    
    
:SpecialDayType.dayBeforePublicHoliday a :SpecialDayType, skos:Concept  ;
         skos:inScheme :SpecialDayTypeCode ;
         rdfs:label "dayBeforePublicHoliday"@en ;
         skos:definition "The day before a declared Public Holiday"@en .
         :SpecialDayType.publicHoliday a :SpecialDayType, skos:Concept  ;
         skos:inScheme :SpecialDayTypeCode ;
         rdfs:label "publicHoliday"@en ;
         skos:definition "The day of a declared Public Holiday, which may be national, or regional."@en .
         :SpecialDayType.dayFollowingPublicHoliday a :SpecialDayType, skos:Concept  ;
         skos:inScheme :SpecialDayTypeCode ;
         rdfs:label "dayFollowingPublicHoliday"@en ;
         skos:definition "The day following a declared Public Holiday"@en .
         :SpecialDayType.longWeekendDay a :SpecialDayType, skos:Concept  ;
         skos:inScheme :SpecialDayTypeCode ;
         rdfs:label "longWeekendDay"@en ;
         skos:definition "       "@en .
         :SpecialDayType.inLieuOfPublicHoliday a :SpecialDayType, skos:Concept  ;
         skos:inScheme :SpecialDayTypeCode ;
         rdfs:label "inLieuOfPublicHoliday"@en ;
         skos:definition "       "@en .
         :SpecialDayType.schoolDay a :SpecialDayType, skos:Concept  ;
         skos:inScheme :SpecialDayTypeCode ;
         rdfs:label "schoolDay"@en ;
         skos:definition "In the locale a day when schools are open and operating"@en .
         :SpecialDayType.schoolHolidays a :SpecialDayType, skos:Concept  ;
         skos:inScheme :SpecialDayTypeCode ;
         rdfs:label "schoolHolidays"@en ;
         skos:definition "In the locale a day when schools are not open and operating"@en .
         :SpecialDayType.publicEventDay a :SpecialDayType, skos:Concept  ;
         skos:inScheme :SpecialDayTypeCode ;
         rdfs:label "publicEventDay"@en ;
         skos:definition "The day of a declared Public Event, which may be national, or regional.  Note: For example, the day of a Royal Wedding."@en .
         :SpecialDayType.other a :SpecialDayType, skos:Concept  ;
         skos:inScheme :SpecialDayTypeCode ;
         rdfs:label "other"@en ;
         skos:definition "Other than as defined in this enumeration."@en .
         

:PaymentMethodCode a skos:ConceptScheme ;
    dc:isFormatOf :PaymentMethod ;
    	skos:definition "Specifies the available list of enumerations for the methods of payment" .
    
    
:PaymentMethod.cash a :PaymentMethod, skos:Concept  ;
         skos:inScheme :PaymentMethodCode ;
         rdfs:label "cash"@en ;
         skos:definition "Payment using cash"@en .
         :PaymentMethod.creditCard a :PaymentMethod, skos:Concept  ;
         skos:inScheme :PaymentMethodCode ;
         rdfs:label "creditCard"@en ;
         skos:definition "Payment using credit card"@en .
         :PaymentMethod.tollStickers a :PaymentMethod, skos:Concept  ;
         skos:inScheme :PaymentMethodCode ;
         rdfs:label "tollStickers"@en ;
         skos:definition "Payment using (pre-paid) toll stickers"@en .
         :PaymentMethod.electronicTollPayment a :PaymentMethod, skos:Concept  ;
         skos:inScheme :PaymentMethodCode ;
         rdfs:label "electronicTollPayment"@en ;
         skos:definition "Payment using some electronic form"@en .
         


